<?xml version="1.0"?>
<rdf:RDF xmlns="https://ega.industry.com/ontologies/core/ucfurnace#"
     xml:base="https://ega.industry.com/ontologies/core/ucfurnace"
     xmlns:owl="http://www.w3.org/2002/07/owl#"
     xmlns:rdf="http://www.w3.org/1999/02/22-rdf-syntax-ns#"
     xmlns:xml="http://www.w3.org/XML/1998/namespace"
     xmlns:xsd="http://www.w3.org/2001/XMLSchema#"
     xmlns:core="https://saref.etsi.org/core/"
     xmlns:data="https://ega.industry.com/ontologies/core/data/"
     xmlns:qudt="http://qudt.org/schema/qudt/"
     xmlns:rdfs="http://www.w3.org/2000/01/rdf-schema#"
     xmlns:skos="http://www.w3.org/2004/02/skos/core#"
     xmlns:swrl="http://www.w3.org/2003/11/swrl#"
     xmlns:vann="http://purl.org/vocab/vann/"
     xmlns:asset="https://ega.industry.com/ontologies/core/asset/"
     xmlns:swrla="http://swrl.stanford.edu/ontologies/3.3/swrla.owl#"
     xmlns:swrlb="http://www.w3.org/2003/11/swrlb#"
     xmlns:terms="http://purl.org/dc/terms/"
     xmlns:process="https://ega.industry.com/ontologies/core/process/">
    <owl:Ontology rdf:about="https://ega.industry.com/ontologies/core/ucfurnace"/>
    


    <!-- 
    ///////////////////////////////////////////////////////////////////////////////////////
    //
    // Annotation properties
    //
    ///////////////////////////////////////////////////////////////////////////////////////
     -->

    


    <!-- http://purl.org/dc/terms/contributor -->

    <owl:AnnotationProperty rdf:about="http://purl.org/dc/terms/contributor"/>
    


    <!-- http://purl.org/dc/terms/created -->

    <owl:AnnotationProperty rdf:about="http://purl.org/dc/terms/created"/>
    


    <!-- http://purl.org/dc/terms/creator -->

    <owl:AnnotationProperty rdf:about="http://purl.org/dc/terms/creator"/>
    


    <!-- http://purl.org/dc/terms/description -->

    <owl:AnnotationProperty rdf:about="http://purl.org/dc/terms/description"/>
    


    <!-- http://purl.org/dc/terms/issued -->

    <owl:AnnotationProperty rdf:about="http://purl.org/dc/terms/issued"/>
    


    <!-- http://purl.org/dc/terms/license -->

    <owl:AnnotationProperty rdf:about="http://purl.org/dc/terms/license"/>
    


    <!-- http://purl.org/dc/terms/modified -->

    <owl:AnnotationProperty rdf:about="http://purl.org/dc/terms/modified"/>
    


    <!-- http://purl.org/dc/terms/publisher -->

    <owl:AnnotationProperty rdf:about="http://purl.org/dc/terms/publisher"/>
    


    <!-- http://purl.org/dc/terms/source -->

    <owl:AnnotationProperty rdf:about="http://purl.org/dc/terms/source"/>
    


    <!-- http://purl.org/dc/terms/title -->

    <owl:AnnotationProperty rdf:about="http://purl.org/dc/terms/title"/>
    


    <!-- http://purl.org/vocab/vann/preferredNamespacePrefix -->

    <owl:AnnotationProperty rdf:about="http://purl.org/vocab/vann/preferredNamespacePrefix"/>
    


    <!-- http://purl.org/vocab/vann/preferredNamespaceUri -->

    <owl:AnnotationProperty rdf:about="http://purl.org/vocab/vann/preferredNamespaceUri"/>
    


    <!-- http://qudt.org/schema/qudt/dbpediaMatch -->

    <owl:AnnotationProperty rdf:about="http://qudt.org/schema/qudt/dbpediaMatch"/>
    


    <!-- http://qudt.org/schema/qudt/expression -->

    <owl:AnnotationProperty rdf:about="http://qudt.org/schema/qudt/expression"/>
    


    <!-- http://qudt.org/schema/qudt/informativeReference -->

    <owl:AnnotationProperty rdf:about="http://qudt.org/schema/qudt/informativeReference"/>
    


    <!-- http://qudt.org/schema/qudt/omUnit -->

    <owl:AnnotationProperty rdf:about="http://qudt.org/schema/qudt/omUnit"/>
    


    <!-- http://qudt.org/schema/qudt/symbol -->

    <owl:AnnotationProperty rdf:about="http://qudt.org/schema/qudt/symbol"/>
    


    <!-- http://swrl.stanford.edu/ontologies/3.3/swrla.owl#isRuleEnabled -->

    <owl:AnnotationProperty rdf:about="http://swrl.stanford.edu/ontologies/3.3/swrla.owl#isRuleEnabled"/>
    


    <!-- http://www.w3.org/2002/07/owl#minQualifiedCardinality -->

    <owl:AnnotationProperty rdf:about="http://www.w3.org/2002/07/owl#minQualifiedCardinality"/>
    


    <!-- http://www.w3.org/2004/02/skos/core#example -->

    <owl:AnnotationProperty rdf:about="http://www.w3.org/2004/02/skos/core#example"/>
    


    <!-- http://www.w3.org/2004/02/skos/core#historyNote -->

    <owl:AnnotationProperty rdf:about="http://www.w3.org/2004/02/skos/core#historyNote"/>
    


    <!-- http://www.w3.org/2004/02/skos/core#note -->

    <owl:AnnotationProperty rdf:about="http://www.w3.org/2004/02/skos/core#note"/>
    


    <!-- 
    ///////////////////////////////////////////////////////////////////////////////////////
    //
    // Datatypes
    //
    ///////////////////////////////////////////////////////////////////////////////////////
     -->

    


    <!-- http://qudt.org/schema/qudt/LatexString -->

    <rdfs:Datatype rdf:about="http://qudt.org/schema/qudt/LatexString"/>
    


    <!-- http://www.w3.org/1999/02/22-rdf-syntax-ns#HTML -->

    <rdfs:Datatype rdf:about="http://www.w3.org/1999/02/22-rdf-syntax-ns#HTML"/>
    


    <!-- http://www.w3.org/2001/XMLSchema#date -->

    <rdfs:Datatype rdf:about="http://www.w3.org/2001/XMLSchema#date"/>
    


    <!-- 
    ///////////////////////////////////////////////////////////////////////////////////////
    //
    // Object Properties
    //
    ///////////////////////////////////////////////////////////////////////////////////////
     -->

    


    <!-- http://www.w3.org/2002/07/owl#topObjectProperty -->

    <owl:ObjectProperty rdf:about="http://www.w3.org/2002/07/owl#topObjectProperty">
        <rdf:type rdf:resource="http://www.w3.org/2002/07/owl#SymmetricProperty"/>
        <rdf:type rdf:resource="http://www.w3.org/2002/07/owl#TransitiveProperty"/>
        <rdf:type rdf:resource="http://www.w3.org/2002/07/owl#ReflexiveProperty"/>
    </owl:ObjectProperty>
    


    <!-- http://www.w3.org/2004/02/skos/core#broader -->

    <owl:ObjectProperty rdf:about="http://www.w3.org/2004/02/skos/core#broader">
        <owl:inverseOf rdf:resource="http://www.w3.org/2004/02/skos/core#narrower"/>
    </owl:ObjectProperty>
    


    <!-- http://www.w3.org/2004/02/skos/core#narrower -->

    <owl:ObjectProperty rdf:about="http://www.w3.org/2004/02/skos/core#narrower"/>
    


    <!-- https://ega.industry.com/ontologies/core/asset/contains -->

    <owl:ObjectProperty rdf:about="https://ega.industry.com/ontologies/core/asset/contains">
        <rdfs:domain rdf:resource="https://ega.industry.com/ontologies/core/asset/Tank"/>
        <rdfs:range rdf:resource="https://ega.industry.com/ontologies/core/asset/RawMaterialBatch"/>
        <rdfs:comment>Indicates that a production equipment, Device temporarily contains material during processing</rdfs:comment>
        <rdfs:label>contains</rdfs:label>
    </owl:ObjectProperty>
    


    <!-- https://ega.industry.com/ontologies/core/asset/feeds -->

    <owl:ObjectProperty rdf:about="https://ega.industry.com/ontologies/core/asset/feeds">
        <owl:inverseOf rdf:resource="https://ega.industry.com/ontologies/core/asset/isFedBy"/>
        <rdfs:domain>
            <owl:Class>
                <owl:unionOf rdf:parseType="Collection">
                    <rdf:Description rdf:about="https://ega.industry.com/ontologies/core/asset/Furnace"/>
                    <rdf:Description rdf:about="https://ega.industry.com/ontologies/core/asset/IndustrySystem"/>
                </owl:unionOf>
            </owl:Class>
        </rdfs:domain>
        <rdfs:range>
            <owl:Class>
                <owl:unionOf rdf:parseType="Collection">
                    <rdf:Description rdf:about="https://ega.industry.com/ontologies/core/asset/Furnace"/>
                    <rdf:Description rdf:about="https://ega.industry.com/ontologies/core/asset/IndustrySystem"/>
                </owl:unionOf>
            </owl:Class>
        </rdfs:range>
        <rdfs:comment xml:lang="en">A system or sub-system feeds a Feature of Interest (Device)</rdfs:comment>
    </owl:ObjectProperty>
    


    <!-- https://ega.industry.com/ontologies/core/asset/hasOpenReason -->

    <owl:ObjectProperty rdf:about="https://ega.industry.com/ontologies/core/asset/hasOpenReason">
        <owl:inverseOf rdf:resource="https://ega.industry.com/ontologies/core/asset/isOpenReasonOf"/>
        <rdf:type rdf:resource="http://www.w3.org/2002/07/owl#FunctionalProperty"/>
        <rdfs:domain rdf:resource="https://ega.industry.com/ontologies/core/asset/OpenCloseState"/>
        <rdfs:range rdf:resource="https://ega.industry.com/ontologies/core/asset/OpenReason"/>
        <rdfs:comment>Links a StateValue to a Reason ex: Open Door for a reason Sampling duringa Process etc...</rdfs:comment>
        <rdfs:label>has open reason</rdfs:label>
    </owl:ObjectProperty>
    


    <!-- https://ega.industry.com/ontologies/core/asset/hasProcess -->

    <owl:ObjectProperty rdf:about="https://ega.industry.com/ontologies/core/asset/hasProcess">
        <rdfs:domain rdf:resource="https://ega.industry.com/ontologies/core/asset/Furnace"/>
        <rdfs:range rdf:resource="https://ega.industry.com/ontologies/core/process/Process"/>
        <rdfs:comment xml:lang="en">Links a Furnace to process</rdfs:comment>
        <rdfs:label>has process</rdfs:label>
    </owl:ObjectProperty>
    


    <!-- https://ega.industry.com/ontologies/core/asset/isFedBy -->

    <owl:ObjectProperty rdf:about="https://ega.industry.com/ontologies/core/asset/isFedBy">
        <rdfs:comment>Inverse of feeds</rdfs:comment>
        <rdfs:label>is fed by</rdfs:label>
    </owl:ObjectProperty>
    


    <!-- https://ega.industry.com/ontologies/core/asset/isOpenReasonOf -->

    <owl:ObjectProperty rdf:about="https://ega.industry.com/ontologies/core/asset/isOpenReasonOf">
        <rdfs:comment>Inverse Of has reason</rdfs:comment>
        <rdfs:label>is open reason of</rdfs:label>
    </owl:ObjectProperty>
    


    <!-- https://ega.industry.com/ontologies/core/asset/isPartOf -->

    <owl:ObjectProperty rdf:about="https://ega.industry.com/ontologies/core/asset/isPartOf">
        <owl:inverseOf rdf:resource="https://saref.etsi.org/core/consistsOf"/>
        <rdfs:label>is part of</rdfs:label>
        <skos:note>Inverse of cosistis of</skos:note>
    </owl:ObjectProperty>
    


    <!-- https://ega.industry.com/ontologies/core/data/hasSpecificState -->

    <owl:ObjectProperty rdf:about="https://ega.industry.com/ontologies/core/data/hasSpecificState">
        <rdfs:domain rdf:resource="https://ega.industry.com/ontologies/core/data/EventFunction"/>
        <rdfs:range rdf:resource="https://saref.etsi.org/core/State"/>
        <rdfs:comment>A relationship associated with an event function to notify that a state  had certains state value</rdfs:comment>
        <rdfs:label>has specific state</rdfs:label>
    </owl:ObjectProperty>
    


    <!-- https://ega.industry.com/ontologies/core/data/hasThresholdPropertyValue -->

    <owl:ObjectProperty rdf:about="https://ega.industry.com/ontologies/core/data/hasThresholdPropertyValue">
        <rdfs:domain rdf:resource="https://ega.industry.com/ontologies/core/data/EventFunction"/>
        <rdfs:range rdf:resource="https://saref.etsi.org/core/PropertyValue"/>
        <rdfs:comment xml:lang="en">A relationship associated with an event function to notify that a certain threshold measurement has been exceeded</rdfs:comment>
        <rdfs:label>has threshold property value</rdfs:label>
    </owl:ObjectProperty>
    


    <!-- https://ega.industry.com/ontologies/core/process/hasCondition -->

    <owl:ObjectProperty rdf:about="https://ega.industry.com/ontologies/core/process/hasCondition">
        <rdfs:domain rdf:resource="https://ega.industry.com/ontologies/core/process/Step"/>
        <rdfs:range rdf:resource="https://ega.industry.com/ontologies/core/process/Condition"/>
        <rdfs:label>has condition</rdfs:label>
    </owl:ObjectProperty>
    


    <!-- https://ega.industry.com/ontologies/core/process/hasCurrentStep -->

    <owl:ObjectProperty rdf:about="https://ega.industry.com/ontologies/core/process/hasCurrentStep">
        <rdf:type rdf:resource="http://www.w3.org/2002/07/owl#FunctionalProperty"/>
        <rdfs:domain rdf:resource="https://ega.industry.com/ontologies/core/process/SubProcess"/>
        <rdfs:range rdf:resource="https://ega.industry.com/ontologies/core/process/Step"/>
        <rdfs:label>has current step</rdfs:label>
    </owl:ObjectProperty>
    


    <!-- https://ega.industry.com/ontologies/core/process/hasCurrentSubProcess -->

    <owl:ObjectProperty rdf:about="https://ega.industry.com/ontologies/core/process/hasCurrentSubProcess">
        <rdf:type rdf:resource="http://www.w3.org/2002/07/owl#FunctionalProperty"/>
        <rdfs:domain rdf:resource="https://ega.industry.com/ontologies/core/process/Process"/>
        <rdfs:range rdf:resource="https://ega.industry.com/ontologies/core/process/SubProcess"/>
        <rdfs:label>has current subprocess</rdfs:label>
    </owl:ObjectProperty>
    


    <!-- https://ega.industry.com/ontologies/core/process/hasEndStep -->

    <owl:ObjectProperty rdf:about="https://ega.industry.com/ontologies/core/process/hasEndStep">
        <rdfs:domain rdf:resource="https://ega.industry.com/ontologies/core/process/SubProcess"/>
        <rdfs:range rdf:resource="https://ega.industry.com/ontologies/core/process/Step"/>
        <rdfs:label>has end step</rdfs:label>
    </owl:ObjectProperty>
    


    <!-- https://ega.industry.com/ontologies/core/process/hasNextStep -->

    <owl:ObjectProperty rdf:about="https://ega.industry.com/ontologies/core/process/hasNextStep">
        <owl:inverseOf rdf:resource="https://ega.industry.com/ontologies/core/process/hasPreviousStep"/>
        <rdfs:domain rdf:resource="https://ega.industry.com/ontologies/core/process/Step"/>
        <rdfs:range rdf:resource="https://ega.industry.com/ontologies/core/process/Step"/>
        <rdfs:comment>connects a step to its successor step</rdfs:comment>
        <rdfs:label>has next step</rdfs:label>
    </owl:ObjectProperty>
    


    <!-- https://ega.industry.com/ontologies/core/process/hasNextSubProcess -->

    <owl:ObjectProperty rdf:about="https://ega.industry.com/ontologies/core/process/hasNextSubProcess">
        <owl:inverseOf rdf:resource="https://ega.industry.com/ontologies/core/process/hasPreviousSubProcess"/>
        <rdfs:domain rdf:resource="https://ega.industry.com/ontologies/core/process/SubProcess"/>
        <rdfs:range rdf:resource="https://ega.industry.com/ontologies/core/process/SubProcess"/>
        <rdfs:comment>Links a Subprocess to its next process</rdfs:comment>
        <rdfs:label>has next subprocess</rdfs:label>
    </owl:ObjectProperty>
    


    <!-- https://ega.industry.com/ontologies/core/process/hasNextSubProcessOnFailure -->

    <owl:ObjectProperty rdf:about="https://ega.industry.com/ontologies/core/process/hasNextSubProcessOnFailure">
        <rdfs:domain rdf:resource="https://ega.industry.com/ontologies/core/process/ConditionalSubProcess"/>
        <rdfs:range rdf:resource="https://ega.industry.com/ontologies/core/process/SubProcess"/>
        <rdfs:label>has next subprocess onfailure</rdfs:label>
    </owl:ObjectProperty>
    


    <!-- https://ega.industry.com/ontologies/core/process/hasNextSubProcessOnSuccess -->

    <owl:ObjectProperty rdf:about="https://ega.industry.com/ontologies/core/process/hasNextSubProcessOnSuccess">
        <rdfs:domain rdf:resource="https://ega.industry.com/ontologies/core/process/ConditionalSubProcess"/>
        <rdfs:range rdf:resource="https://ega.industry.com/ontologies/core/process/SubProcess"/>
        <rdfs:label>has next subprocess onsuccess</rdfs:label>
    </owl:ObjectProperty>
    


    <!-- https://ega.industry.com/ontologies/core/process/hasPreviousStep -->

    <owl:ObjectProperty rdf:about="https://ega.industry.com/ontologies/core/process/hasPreviousStep">
        <rdfs:subPropertyOf rdf:resource="http://www.w3.org/2002/07/owl#topObjectProperty"/>
        <rdfs:domain rdf:resource="https://ega.industry.com/ontologies/core/process/Step"/>
        <rdfs:range rdf:resource="https://ega.industry.com/ontologies/core/process/Step"/>
        <rdfs:comment>connects a step to its predecessor</rdfs:comment>
        <rdfs:label>has previous step</rdfs:label>
    </owl:ObjectProperty>
    


    <!-- https://ega.industry.com/ontologies/core/process/hasPreviousSubProcess -->

    <owl:ObjectProperty rdf:about="https://ega.industry.com/ontologies/core/process/hasPreviousSubProcess">
        <rdfs:comment>Links a SubProcess to previous Subprocess, it&apos;is inverse of &apos;has next subprocess&apos;</rdfs:comment>
        <rdfs:label>has previous subprocess</rdfs:label>
    </owl:ObjectProperty>
    


    <!-- https://ega.industry.com/ontologies/core/process/hasStartStep -->

    <owl:ObjectProperty rdf:about="https://ega.industry.com/ontologies/core/process/hasStartStep">
        <rdfs:domain rdf:resource="https://ega.industry.com/ontologies/core/process/SubProcess"/>
        <rdfs:range rdf:resource="https://ega.industry.com/ontologies/core/process/Step"/>
        <rdfs:comment>Links a Subprocess to  its initial step of subprocess</rdfs:comment>
        <rdfs:label>has start step</rdfs:label>
    </owl:ObjectProperty>
    


    <!-- https://ega.industry.com/ontologies/core/process/hasStep -->

    <owl:ObjectProperty rdf:about="https://ega.industry.com/ontologies/core/process/hasStep">
        <owl:inverseOf rdf:resource="https://ega.industry.com/ontologies/core/process/isStepOf"/>
        <rdfs:domain rdf:resource="https://ega.industry.com/ontologies/core/process/SubProcess"/>
        <rdfs:range rdf:resource="https://ega.industry.com/ontologies/core/process/Step"/>
        <rdfs:comment>Links a SubProcess to Step</rdfs:comment>
        <rdfs:label>has step</rdfs:label>
    </owl:ObjectProperty>
    


    <!-- https://ega.industry.com/ontologies/core/process/hasStepType -->

    <owl:ObjectProperty rdf:about="https://ega.industry.com/ontologies/core/process/hasStepType">
        <rdfs:domain rdf:resource="https://ega.industry.com/ontologies/core/process/Step"/>
        <rdfs:range rdf:resource="https://ega.industry.com/ontologies/core/process/StepType"/>
        <rdfs:comment>Links a Step to StepType.</rdfs:comment>
        <rdfs:label>has step type</rdfs:label>
    </owl:ObjectProperty>
    


    <!-- https://ega.industry.com/ontologies/core/process/hasSubProcess -->

    <owl:ObjectProperty rdf:about="https://ega.industry.com/ontologies/core/process/hasSubProcess">
        <rdfs:domain rdf:resource="https://ega.industry.com/ontologies/core/process/Process"/>
        <rdfs:range rdf:resource="https://ega.industry.com/ontologies/core/process/SubProcess"/>
        <rdfs:comment>Links a Process to SubProcecess</rdfs:comment>
        <rdfs:label>has subprocess</rdfs:label>
    </owl:ObjectProperty>
    


    <!-- https://ega.industry.com/ontologies/core/process/isStepOf -->

    <owl:ObjectProperty rdf:about="https://ega.industry.com/ontologies/core/process/isStepOf">
        <rdfs:comment>Links a Step to SubProcess, Inverse of &apos;has step&apos;</rdfs:comment>
        <rdfs:label>is step of</rdfs:label>
    </owl:ObjectProperty>
    


    <!-- https://ega.industry.com/ontologies/core/process/isTriggeredBy -->

    <owl:ObjectProperty rdf:about="https://ega.industry.com/ontologies/core/process/isTriggeredBy">
        <owl:inverseOf rdf:resource="https://ega.industry.com/ontologies/core/process/triggers"/>
        <rdfs:domain rdf:resource="https://ega.industry.com/ontologies/core/process/Condition"/>
        <rdfs:range rdf:resource="https://ega.industry.com/ontologies/core/data/EventFunction"/>
        <rdfs:label>is triggered by</rdfs:label>
    </owl:ObjectProperty>
    


    <!-- https://ega.industry.com/ontologies/core/process/pathDependsOnStep -->

    <owl:ObjectProperty rdf:about="https://ega.industry.com/ontologies/core/process/pathDependsOnStep">
        <rdfs:domain rdf:resource="https://ega.industry.com/ontologies/core/process/ConditionalSubProcess"/>
        <rdfs:range rdf:resource="https://ega.industry.com/ontologies/core/process/IterativeStep"/>
        <rdfs:label>path depends</rdfs:label>
    </owl:ObjectProperty>
    


    <!-- https://ega.industry.com/ontologies/core/process/triggers -->

    <owl:ObjectProperty rdf:about="https://ega.industry.com/ontologies/core/process/triggers">
        <rdfs:comment xml:lang="en">Inverse Of IsTriggeredBy, Links a EventFunction to Condition</rdfs:comment>
    </owl:ObjectProperty>
    


    <!-- https://ega.industry.com/ontologies/core/process/useAsset -->

    <owl:ObjectProperty rdf:about="https://ega.industry.com/ontologies/core/process/useAsset">
        <rdfs:domain rdf:resource="https://ega.industry.com/ontologies/core/process/Step"/>
        <rdfs:range>
            <owl:Class>
                <owl:unionOf rdf:parseType="Collection">
                    <rdf:Description rdf:about="https://ega.industry.com/ontologies/core/asset/IndustrySystem"/>
                    <rdf:Description rdf:about="https://saref.etsi.org/core/Device"/>
                </owl:unionOf>
            </owl:Class>
        </rdfs:range>
        <rdfs:comment xml:lang="en">Links a Process Step to a Asset Element</rdfs:comment>
        <rdfs:label xml:lang="en">use asset</rdfs:label>
    </owl:ObjectProperty>
    


    <!-- https://saref.etsi.org/core/accomplishes -->

    <owl:ObjectProperty rdf:about="https://saref.etsi.org/core/accomplishes">
        <owl:inverseOf rdf:resource="https://saref.etsi.org/core/isAccomplishedBy"/>
        <rdfs:range rdf:resource="https://saref.etsi.org/core/Task"/>
        <rdfs:comment xml:lang="en">Links a certain entity (e.g., a device) to the task it accomplishes.</rdfs:comment>
        <rdfs:label xml:lang="en">accomplishes</rdfs:label>
    </owl:ObjectProperty>
    


    <!-- https://saref.etsi.org/core/consistsOf -->

    <owl:ObjectProperty rdf:about="https://saref.etsi.org/core/consistsOf">
        <owl:propertyChainAxiom rdf:parseType="Collection">
            <rdf:Description rdf:about="https://saref.etsi.org/core/consistsOf"/>
            <rdf:Description rdf:about="https://saref.etsi.org/core/hasFeatureKind"/>
        </owl:propertyChainAxiom>
        <owl:propertyChainAxiom rdf:parseType="Collection">
            <rdf:Description rdf:about="https://saref.etsi.org/core/consistsOf"/>
            <rdf:Description rdf:about="https://saref.etsi.org/core/hasPropertyKind"/>
        </owl:propertyChainAxiom>
        <owl:propertyChainAxiom rdf:parseType="Collection">
            <rdf:Description rdf:about="https://saref.etsi.org/core/consistsOf"/>
            <rdf:Description rdf:about="https://saref.etsi.org/core/hasStateKind"/>
        </owl:propertyChainAxiom>
        <owl:propertyChainAxiom rdf:parseType="Collection">
            <rdf:Description rdf:about="https://saref.etsi.org/core/consistsOf"/>
            <rdf:Description rdf:about="https://saref.etsi.org/core/isValueOfProperty"/>
        </owl:propertyChainAxiom>
        <owl:propertyChainAxiom rdf:parseType="Collection">
            <rdf:Description rdf:about="https://saref.etsi.org/core/consistsOf"/>
            <rdf:Description rdf:about="https://saref.etsi.org/core/isValueOfState"/>
        </owl:propertyChainAxiom>
        <rdfs:comment xml:lang="en">A relationship indicating a composite entity that consists of other entities (e.g., a temperature/humidity sensor that consists of a temperature sensor and a humidity sensor)</rdfs:comment>
        <rdfs:label xml:lang="en">consists of</rdfs:label>
        <skos:historyNote xml:lang="en">V3.2.1: Add local restrictions on consistsOf on feature of interest</skos:historyNote>
        <skos:note xml:lang="en">A feature kind (respectively a feature of interest) may consist of (OP saref:consistsOf) other feature kinds (respectively feature kinds or features of interest ).</skos:note>
        <skos:note xml:lang="en">The OP saref:consistsOf can link a composite property, property of interest, or property value to its individual components.</skos:note>
    </owl:ObjectProperty>
    


    <!-- https://saref.etsi.org/core/consumes -->

    <owl:ObjectProperty rdf:about="https://saref.etsi.org/core/consumes">
        <owl:inverseOf rdf:resource="https://saref.etsi.org/core/isConsumedBy"/>
        <rdfs:domain>
            <owl:Class>
                <owl:unionOf rdf:parseType="Collection">
                    <rdf:Description rdf:about="https://saref.etsi.org/core/Device"/>
                    <rdf:Description rdf:about="https://saref.etsi.org/core/DeviceKind"/>
                    <rdf:Description rdf:about="https://saref.etsi.org/core/FeatureKind"/>
                    <rdf:Description rdf:about="https://saref.etsi.org/core/FeatureOfInterest"/>
                </owl:unionOf>
            </owl:Class>
        </rdfs:domain>
        <rdfs:range rdf:resource="https://saref.etsi.org/core/Commodity"/>
        <rdfs:comment xml:lang="en">Links a feature kind, feature of interest, or device, to the commodity it consumes</rdfs:comment>
        <rdfs:label xml:lang="en">consumes</rdfs:label>
        <skos:historyNote xml:lang="en">V3.2.1: Introduced saref:consumes, saref:isConsumedBy, saref:produces, saref:isProducedBy, saref:stores, saref:isStoredBy.</skos:historyNote>
    </owl:ObjectProperty>
    


    <!-- https://saref.etsi.org/core/controls -->

    <owl:ObjectProperty rdf:about="https://saref.etsi.org/core/controls">
        <rdfs:subPropertyOf rdf:resource="https://saref.etsi.org/core/targets"/>
        <owl:inverseOf rdf:resource="https://saref.etsi.org/core/isControlledBy"/>
        <rdfs:domain>
            <owl:Class>
                <owl:unionOf rdf:parseType="Collection">
                    <rdf:Description rdf:about="https://saref.etsi.org/core/Actuation"/>
                    <rdf:Description rdf:about="https://saref.etsi.org/core/Actuator"/>
                    <rdf:Description rdf:about="https://saref.etsi.org/core/Command"/>
                    <rdf:Description rdf:about="https://saref.etsi.org/core/CommandOfInterest"/>
                    <rdf:Description rdf:about="https://saref.etsi.org/core/DeviceKind"/>
                    <rdf:Description rdf:about="https://saref.etsi.org/core/Function"/>
                    <rdf:Description rdf:about="https://saref.etsi.org/core/FunctionOfInterest"/>
                </owl:unionOf>
            </owl:Class>
        </rdfs:domain>
        <rdfs:comment xml:lang="en">Links a device, function, command, or procedure execution, to the feature, property, or state, it controls.</rdfs:comment>
        <rdfs:label xml:lang="en">controls</rdfs:label>
        <skos:historyNote xml:lang="en">V3.2.1: Introduced property saref:controls, as sub-property of saref:targets. and generalization of saref:controlsProperty.</skos:historyNote>
    </owl:ObjectProperty>
    


    <!-- https://saref.etsi.org/core/hasApplicableTime -->

    <owl:ObjectProperty rdf:about="https://saref.etsi.org/core/hasApplicableTime">
        <rdfs:range>
            <owl:Class>
                <owl:unionOf rdf:parseType="Collection">
                    <rdf:Description rdf:about="http://www.w3.org/2006/time#TemporalEntity"/>
                    <rdf:Description rdf:about="http://www.w3.org/2006/time#TemporalPosition"/>
                </owl:unionOf>
            </owl:Class>
        </rdfs:range>
        <rdfs:comment xml:lang="en">Links an entity (e.g., a profile) to an instant or interval or other compound temporal entity expressed using OWL Time, which bounds temporally the applicable context of that entity.</rdfs:comment>
        <rdfs:label xml:lang="en">has applicable time</rdfs:label>
    </owl:ObjectProperty>
    


    <!-- https://saref.etsi.org/core/hasCommand -->

    <owl:ObjectProperty rdf:about="https://saref.etsi.org/core/hasCommand">
        <owl:inverseOf rdf:resource="https://saref.etsi.org/core/isCommandOf"/>
        <rdfs:domain>
            <owl:Class>
                <owl:unionOf rdf:parseType="Collection">
                    <rdf:Description rdf:about="https://saref.etsi.org/core/Function"/>
                    <rdf:Description rdf:about="https://saref.etsi.org/core/FunctionOfInterest"/>
                </owl:unionOf>
            </owl:Class>
        </rdfs:domain>
        <rdfs:range rdf:resource="https://saref.etsi.org/core/Command"/>
        <owl:propertyChainAxiom rdf:parseType="Collection">
            <rdf:Description rdf:about="https://saref.etsi.org/core/hasCommandOfInterest"/>
            <rdf:Description rdf:about="https://saref.etsi.org/core/hasCommandKind"/>
        </owl:propertyChainAxiom>
        <owl:propertyChainAxiom rdf:parseType="Collection">
            <rdf:Description rdf:about="https://saref.etsi.org/core/hasFeatureKind"/>
            <rdf:Description rdf:about="https://saref.etsi.org/core/hasMandatoryCommand"/>
        </owl:propertyChainAxiom>
        <rdfs:comment xml:lang="en">Links a function or function of interest and the command it supports.</rdfs:comment>
        <rdfs:label xml:lang="en">has command</rdfs:label>
        <skos:historyNote xml:lang="en">V3.2.1: Domain of saref:hasCommand is relaxed to saref:Function or saref:FunctionOfInterest.</skos:historyNote>
    </owl:ObjectProperty>
    


    <!-- https://saref.etsi.org/core/hasCommandKind -->

    <owl:ObjectProperty rdf:about="https://saref.etsi.org/core/hasCommandKind">
        <rdfs:domain rdf:resource="https://saref.etsi.org/core/CommandOfInterest"/>
        <rdfs:range rdf:resource="https://saref.etsi.org/core/Command"/>
        <owl:propertyChainAxiom rdf:parseType="Collection">
            <rdf:Description rdf:about="https://saref.etsi.org/core/hasCommandKind"/>
            <rdf:Description rdf:about="http://www.w3.org/2004/02/skos/core#broader"/>
        </owl:propertyChainAxiom>
        <rdfs:comment xml:lang="en">links a command of interest to its kind, a command.</rdfs:comment>
        <rdfs:label xml:lang="en">has command kind</rdfs:label>
    </owl:ObjectProperty>
    


    <!-- https://saref.etsi.org/core/hasCommandOfInterest -->

    <owl:ObjectProperty rdf:about="https://saref.etsi.org/core/hasCommandOfInterest">
        <owl:inverseOf rdf:resource="https://saref.etsi.org/core/isCommandOfInterestOf"/>
        <rdfs:domain rdf:resource="https://saref.etsi.org/core/FunctionOfInterest"/>
        <rdfs:range rdf:resource="https://saref.etsi.org/core/CommandOfInterest"/>
        <rdfs:comment xml:lang="en">Links a function of interest to one of its commands of interest.</rdfs:comment>
        <rdfs:label xml:lang="en">has command of interest</rdfs:label>
    </owl:ObjectProperty>
    


    <!-- https://saref.etsi.org/core/hasDeviceKind -->

    <owl:ObjectProperty rdf:about="https://saref.etsi.org/core/hasDeviceKind">
        <rdfs:subPropertyOf rdf:resource="https://saref.etsi.org/core/hasFeatureKind"/>
        <rdfs:domain rdf:resource="https://saref.etsi.org/core/Device"/>
        <rdfs:range rdf:resource="https://saref.etsi.org/core/DeviceKind"/>
        <rdfs:comment xml:lang="en">Links a device to its kind, a device kind. Kinds of devices describe models of devices, with common properties and common states having the same value, targeting the same properties and states, common functions, and common services.</rdfs:comment>
        <rdfs:label xml:lang="en">has device kind</rdfs:label>
    </owl:ObjectProperty>
    


    <!-- https://saref.etsi.org/core/hasFeatureKind -->

    <owl:ObjectProperty rdf:about="https://saref.etsi.org/core/hasFeatureKind">
        <rdfs:domain rdf:resource="https://saref.etsi.org/core/FeatureOfInterest"/>
        <rdfs:range rdf:resource="https://saref.etsi.org/core/FeatureKind"/>
        <owl:propertyChainAxiom rdf:parseType="Collection">
            <rdf:Description rdf:about="https://saref.etsi.org/core/hasFeatureKind"/>
            <rdf:Description rdf:about="http://www.w3.org/2004/02/skos/core#broader"/>
        </owl:propertyChainAxiom>
        <rdfs:comment xml:lang="en">links a feature of interest to its kind, a feature kind</rdfs:comment>
        <rdfs:label xml:lang="en">has feature kind</rdfs:label>
        <skos:historyNote xml:lang="en">V3.2.1: Introduce hasClassKind for Class is Feature, Device, Property, State, Function, Command.</skos:historyNote>
    </owl:ObjectProperty>
    


    <!-- https://saref.etsi.org/core/hasFunction -->

    <owl:ObjectProperty rdf:about="https://saref.etsi.org/core/hasFunction">
        <owl:inverseOf rdf:resource="https://saref.etsi.org/core/isFunctionOf"/>
        <rdfs:domain>
            <owl:Class>
                <owl:unionOf rdf:parseType="Collection">
                    <rdf:Description rdf:about="https://saref.etsi.org/core/FeatureKind"/>
                    <rdf:Description rdf:about="https://saref.etsi.org/core/FeatureOfInterest"/>
                </owl:unionOf>
            </owl:Class>
        </rdfs:domain>
        <rdfs:range rdf:resource="https://saref.etsi.org/core/Function"/>
        <owl:propertyChainAxiom rdf:parseType="Collection">
            <rdf:Description rdf:about="http://www.w3.org/2004/02/skos/core#broader"/>
            <rdf:Description rdf:about="https://saref.etsi.org/core/hasFunction"/>
        </owl:propertyChainAxiom>
        <owl:propertyChainAxiom rdf:parseType="Collection">
            <rdf:Description rdf:about="https://saref.etsi.org/core/hasDeviceKind"/>
            <rdf:Description rdf:about="https://saref.etsi.org/core/hasFunction"/>
        </owl:propertyChainAxiom>
        <owl:propertyChainAxiom rdf:parseType="Collection">
            <rdf:Description rdf:about="https://saref.etsi.org/core/hasFunctionOfInterest"/>
            <rdf:Description rdf:about="https://saref.etsi.org/core/hasFunctionKind"/>
        </owl:propertyChainAxiom>
        <rdfs:comment>A relationship identifying the function of a device</rdfs:comment>
        <rdfs:comment xml:lang="en">Links a feature kind or a device to one of its functions.</rdfs:comment>
        <rdfs:label xml:lang="en">has function</rdfs:label>
        <skos:historyNote xml:lang="en">V3.2.1: Domain of saref:hasFunction is relaxed.</skos:historyNote>
    </owl:ObjectProperty>
    


    <!-- https://saref.etsi.org/core/hasFunctionKind -->

    <owl:ObjectProperty rdf:about="https://saref.etsi.org/core/hasFunctionKind">
        <rdfs:domain rdf:resource="https://saref.etsi.org/core/FunctionOfInterest"/>
        <rdfs:range rdf:resource="https://saref.etsi.org/core/Function"/>
        <owl:propertyChainAxiom rdf:parseType="Collection">
            <rdf:Description rdf:about="https://saref.etsi.org/core/hasFunctionKind"/>
            <rdf:Description rdf:about="http://www.w3.org/2004/02/skos/core#broader"/>
        </owl:propertyChainAxiom>
        <rdfs:comment xml:lang="en">links a function of interest to its kind, a function</rdfs:comment>
        <rdfs:label xml:lang="en">has function kind</rdfs:label>
    </owl:ObjectProperty>
    


    <!-- https://saref.etsi.org/core/hasFunctionOfInterest -->

    <owl:ObjectProperty rdf:about="https://saref.etsi.org/core/hasFunctionOfInterest">
        <owl:inverseOf rdf:resource="https://saref.etsi.org/core/isFunctionOfInterestOf"/>
        <rdfs:domain rdf:resource="https://saref.etsi.org/core/Device"/>
        <rdfs:range rdf:resource="https://saref.etsi.org/core/FunctionOfInterest"/>
        <rdfs:comment xml:lang="en">Links a device to one of its functions of interest.</rdfs:comment>
        <rdfs:label xml:lang="en">has function of interest</rdfs:label>
    </owl:ObjectProperty>
    


    <!-- https://saref.etsi.org/core/hasInput -->

    <owl:ObjectProperty rdf:about="https://saref.etsi.org/core/hasInput">
        <rdfs:domain>
            <owl:Class>
                <owl:unionOf rdf:parseType="Collection">
                    <rdf:Description rdf:about="https://saref.etsi.org/core/Command"/>
                    <rdf:Description rdf:about="https://saref.etsi.org/core/CommandOfInterest"/>
                    <rdf:Description rdf:about="https://saref.etsi.org/core/Operation"/>
                    <rdf:Description rdf:about="https://saref.etsi.org/core/ProcedureExecution"/>
                </owl:unionOf>
            </owl:Class>
        </rdfs:domain>
        <rdfs:comment xml:lang="en">Links a command, operation, or procedure execution, to its inputs.</rdfs:comment>
        <rdfs:label xml:lang="en">has input</rdfs:label>
        <skos:example xml:lang="en">Different complementary commands can be defined for controlling a light. Turn on or off the light based on a desired state, toggle the light status of a specific light, set the luminosity level with a transition time, set the default transition time, start comfort.</skos:example>
        <skos:historyNote xml:lang="en">V3.2.1: Introduced saref:hasInput and saref:hasOutput.</skos:historyNote>
    </owl:ObjectProperty>
    


    <!-- https://saref.etsi.org/core/hasMandatoryCommand -->

    <owl:ObjectProperty rdf:about="https://saref.etsi.org/core/hasMandatoryCommand">
        <rdfs:subPropertyOf rdf:resource="https://saref.etsi.org/core/hasCommand"/>
        <rdfs:domain rdf:resource="https://saref.etsi.org/core/Function"/>
        <owl:propertyChainAxiom rdf:parseType="Collection">
            <rdf:Description rdf:about="http://www.w3.org/2004/02/skos/core#broader"/>
            <rdf:Description rdf:about="https://saref.etsi.org/core/hasMandatoryCommand"/>
        </owl:propertyChainAxiom>
        <rdfs:comment xml:lang="en">Links a function and one of its mandatory commands</rdfs:comment>
        <rdfs:label xml:lang="en">has mandatory command</rdfs:label>
        <skos:historyNote xml:lang="en">V3.2.1: Introduced mandatory and optional commands.</skos:historyNote>
    </owl:ObjectProperty>
    


    <!-- https://saref.etsi.org/core/hasOperation -->

    <owl:ObjectProperty rdf:about="https://saref.etsi.org/core/hasOperation">
        <owl:inverseOf rdf:resource="https://saref.etsi.org/core/isOperationOf"/>
        <rdfs:domain rdf:resource="https://saref.etsi.org/core/Service"/>
        <rdfs:range rdf:resource="https://saref.etsi.org/core/Operation"/>
        <rdfs:comment xml:lang="en">Links a service to one of its operations.</rdfs:comment>
        <rdfs:label xml:lang="en">has operation</rdfs:label>
    </owl:ObjectProperty>
    


    <!-- https://saref.etsi.org/core/hasOptionalCommand -->

    <owl:ObjectProperty rdf:about="https://saref.etsi.org/core/hasOptionalCommand">
        <rdfs:subPropertyOf rdf:resource="https://saref.etsi.org/core/hasCommand"/>
        <rdfs:domain rdf:resource="https://saref.etsi.org/core/Function"/>
        <rdfs:comment xml:lang="en">Links a function and one of its optional commands</rdfs:comment>
        <rdfs:label xml:lang="en">has optional command</rdfs:label>
    </owl:ObjectProperty>
    


    <!-- https://saref.etsi.org/core/hasOutput -->

    <owl:ObjectProperty rdf:about="https://saref.etsi.org/core/hasOutput">
        <rdfs:domain>
            <owl:Class>
                <owl:unionOf rdf:parseType="Collection">
                    <rdf:Description rdf:about="https://saref.etsi.org/core/Command"/>
                    <rdf:Description rdf:about="https://saref.etsi.org/core/CommandOfInterest"/>
                    <rdf:Description rdf:about="https://saref.etsi.org/core/Operation"/>
                </owl:unionOf>
            </owl:Class>
        </rdfs:domain>
        <rdfs:comment xml:lang="en">Links a command or operation to its outputs.</rdfs:comment>
        <rdfs:label xml:lang="en">has output</rdfs:label>
        <skos:example xml:lang="en">Different complementary commands can be defined for observing a smart home. Observe the temperature once will output the indoor temperature property; observe status of the entry door will output an open/close state.</skos:example>
    </owl:ObjectProperty>
    


    <!-- https://saref.etsi.org/core/hasPhenomenonTime -->

    <owl:ObjectProperty rdf:about="https://saref.etsi.org/core/hasPhenomenonTime">
        <rdfs:range rdf:resource="http://www.w3.org/2006/time#TemporalEntity"/>
        <rdfs:comment xml:lang="en">Links a procedure execution to the time that the result applies. It may be an interval or an instant, or some other compound temporal entity expressed using OWL Time.</rdfs:comment>
        <rdfs:label xml:lang="en">has phenomenon time</rdfs:label>
        <skos:historyNote xml:lang="en">V3.2.1: Introduced saref:hasPhenomenonTime as part of general will to make SAREF and SOSA/SSN converge.</skos:historyNote>
    </owl:ObjectProperty>
    


    <!-- https://saref.etsi.org/core/hasProfile -->

    <owl:ObjectProperty rdf:about="https://saref.etsi.org/core/hasProfile">
        <owl:inverseOf rdf:resource="https://saref.etsi.org/core/isProfileOf"/>
        <rdfs:domain>
            <owl:Class>
                <owl:unionOf rdf:parseType="Collection">
                    <rdf:Description rdf:about="https://saref.etsi.org/core/Device"/>
                    <rdf:Description rdf:about="https://saref.etsi.org/core/DeviceKind"/>
                </owl:unionOf>
            </owl:Class>
        </rdfs:domain>
        <rdfs:range rdf:resource="https://saref.etsi.org/core/Profile"/>
        <rdfs:comment xml:lang="en">Links a device to its profile. Its inverse is saref:isProfileOf. The device should be linked to a certain commodity using OP saref:consumes, saref:produces, or saref:stores, and optionally to some property or state using OP saref:targets or its sub-properties.</rdfs:comment>
        <rdfs:label xml:lang="en">has profile</rdfs:label>
        <skos:historyNote xml:lang="en">V3.2.1: Relaxed domain of saref:hasProfile to saref:FeatureKind or saref:Device</skos:historyNote>
    </owl:ObjectProperty>
    


    <!-- https://saref.etsi.org/core/hasProperty -->

    <owl:ObjectProperty rdf:about="https://saref.etsi.org/core/hasProperty">
        <owl:inverseOf rdf:resource="https://saref.etsi.org/core/isPropertyOf"/>
        <rdfs:domain>
            <owl:Class>
                <owl:unionOf rdf:parseType="Collection">
                    <rdf:Description rdf:about="https://saref.etsi.org/core/FeatureKind"/>
                    <rdf:Description rdf:about="https://saref.etsi.org/core/FeatureOfInterest"/>
                </owl:unionOf>
            </owl:Class>
        </rdfs:domain>
        <rdfs:range rdf:resource="https://saref.etsi.org/core/Property"/>
        <owl:propertyChainAxiom rdf:parseType="Collection">
            <rdf:Description rdf:about="http://www.w3.org/2004/02/skos/core#broader"/>
            <rdf:Description rdf:about="https://saref.etsi.org/core/hasProperty"/>
        </owl:propertyChainAxiom>
        <owl:propertyChainAxiom rdf:parseType="Collection">
            <rdf:Description rdf:about="https://saref.etsi.org/core/hasFeatureKind"/>
            <rdf:Description rdf:about="https://saref.etsi.org/core/hasProperty"/>
        </owl:propertyChainAxiom>
        <owl:propertyChainAxiom rdf:parseType="Collection">
            <rdf:Description rdf:about="https://saref.etsi.org/core/hasProperty"/>
            <rdf:Description rdf:about="https://saref.etsi.org/core/consistsOf"/>
        </owl:propertyChainAxiom>
        <owl:propertyChainAxiom rdf:parseType="Collection">
            <rdf:Description rdf:about="https://saref.etsi.org/core/hasPropertyOfInterest"/>
            <rdf:Description rdf:about="https://saref.etsi.org/core/hasPropertyKind"/>
        </owl:propertyChainAxiom>
        <rdfs:comment xml:lang="en">Links a feature kind or a feature of interest to one of its properties.</rdfs:comment>
        <rdfs:label xml:lang="en">has property</rdfs:label>
        <skos:historyNote xml:lang="en">V3.2.1: applicability of saref:hasProperty is relaxed to also saref:FeatureKind</skos:historyNote>
    </owl:ObjectProperty>
    


    <!-- https://saref.etsi.org/core/hasPropertyKind -->

    <owl:ObjectProperty rdf:about="https://saref.etsi.org/core/hasPropertyKind">
        <rdfs:domain rdf:resource="https://saref.etsi.org/core/PropertyOfInterest"/>
        <rdfs:range rdf:resource="https://saref.etsi.org/core/Property"/>
        <owl:propertyChainAxiom rdf:parseType="Collection">
            <rdf:Description rdf:about="https://saref.etsi.org/core/hasPropertyKind"/>
            <rdf:Description rdf:about="http://www.w3.org/2004/02/skos/core#broader"/>
        </owl:propertyChainAxiom>
        <rdfs:comment xml:lang="en">links a property of interest to its kind, a property.</rdfs:comment>
        <rdfs:label xml:lang="en">has property kind</rdfs:label>
    </owl:ObjectProperty>
    


    <!-- https://saref.etsi.org/core/hasPropertyOfInterest -->

    <owl:ObjectProperty rdf:about="https://saref.etsi.org/core/hasPropertyOfInterest">
        <owl:inverseOf rdf:resource="https://saref.etsi.org/core/isPropertyOfInterestOf"/>
        <rdfs:domain rdf:resource="https://saref.etsi.org/core/FeatureOfInterest"/>
        <rdfs:range rdf:resource="https://saref.etsi.org/core/PropertyOfInterest"/>
        <rdfs:comment xml:lang="en">Links a feature of interest to one of its properties of interest.</rdfs:comment>
        <rdfs:label xml:lang="en">has property of interest</rdfs:label>
        <skos:historyNote xml:lang="en">V3.2.1: Introduced saref:hasPropertyOfInterest and saref:isPropertyOfInterestOf. Cannot use saref:hasProperty due to the combination of cardinality restrictions and sub-property chain axioms makes the ontology exist the OWL 2 DL prodile.</skos:historyNote>
    </owl:ObjectProperty>
    


    <!-- https://saref.etsi.org/core/hasPropertyValue -->

    <owl:ObjectProperty rdf:about="https://saref.etsi.org/core/hasPropertyValue">
        <rdfs:domain>
            <owl:Class>
                <owl:unionOf rdf:parseType="Collection">
                    <rdf:Description rdf:about="https://saref.etsi.org/core/FeatureKind"/>
                    <rdf:Description rdf:about="https://saref.etsi.org/core/FeatureOfInterest"/>
                    <rdf:Description rdf:about="https://saref.etsi.org/core/PropertyOfInterest"/>
                </owl:unionOf>
            </owl:Class>
        </rdfs:domain>
        <rdfs:range rdf:resource="https://saref.etsi.org/core/PropertyValue"/>
        <owl:propertyChainAxiom rdf:parseType="Collection">
            <rdf:Description rdf:about="http://www.w3.org/2004/02/skos/core#broader"/>
            <rdf:Description rdf:about="https://saref.etsi.org/core/hasPropertyValue"/>
        </owl:propertyChainAxiom>
        <rdfs:comment xml:lang="en">Links a feature kind, a feature of interest, or a property of interest, to a property value.</rdfs:comment>
        <rdfs:label xml:lang="en">has property value</rdfs:label>
        <skos:historyNote xml:lang="en">V3.2.1: Introduced saref:hasPropertyValue.</skos:historyNote>
    </owl:ObjectProperty>
    


    <!-- https://saref.etsi.org/core/hasResult -->

    <owl:ObjectProperty rdf:about="https://saref.etsi.org/core/hasResult">
        <rdfs:domain rdf:resource="https://saref.etsi.org/core/ProcedureExecution"/>
        <rdfs:comment xml:lang="en">Links a procedure execution (e.g., an observation) to its result (e.g., a property value).</rdfs:comment>
        <rdfs:label xml:lang="en">has result</rdfs:label>
        <skos:historyNote xml:lang="en">V3.2.1: Introduced saref:hasResult as part of general will to make SAREF and SOSA/SSN converge.</skos:historyNote>
    </owl:ObjectProperty>
    


    <!-- https://saref.etsi.org/core/hasState -->

    <owl:ObjectProperty rdf:about="https://saref.etsi.org/core/hasState">
        <owl:inverseOf rdf:resource="https://saref.etsi.org/core/isStateOf"/>
        <rdfs:domain>
            <owl:Class>
                <owl:unionOf rdf:parseType="Collection">
                    <rdf:Description rdf:about="https://saref.etsi.org/core/FeatureKind"/>
                    <rdf:Description rdf:about="https://saref.etsi.org/core/FeatureOfInterest"/>
                    <rdf:Description rdf:about="https://saref.etsi.org/core/StateOfInterest"/>
                </owl:unionOf>
            </owl:Class>
        </rdfs:domain>
        <rdfs:range rdf:resource="https://saref.etsi.org/core/State"/>
        <owl:propertyChainAxiom rdf:parseType="Collection">
            <rdf:Description rdf:about="http://www.w3.org/2004/02/skos/core#broader"/>
            <rdf:Description rdf:about="https://saref.etsi.org/core/hasState"/>
        </owl:propertyChainAxiom>
        <owl:propertyChainAxiom rdf:parseType="Collection">
            <rdf:Description rdf:about="https://saref.etsi.org/core/hasFeatureKind"/>
            <rdf:Description rdf:about="https://saref.etsi.org/core/hasState"/>
        </owl:propertyChainAxiom>
        <owl:propertyChainAxiom rdf:parseType="Collection">
            <rdf:Description rdf:about="https://saref.etsi.org/core/hasStateOfInterest"/>
            <rdf:Description rdf:about="https://saref.etsi.org/core/hasStateKind"/>
        </owl:propertyChainAxiom>
        <rdfs:comment>A relationship for identifying the state of a production equipment</rdfs:comment>
        <rdfs:comment xml:lang="en">Links a feature kind or a feature of interest to one of its states.</rdfs:comment>
        <rdfs:label xml:lang="en">has state</rdfs:label>
        <skos:historyNote xml:lang="en">V3.2.1: Relaxed domain of saref:hasState.</skos:historyNote>
    </owl:ObjectProperty>
    


    <!-- https://saref.etsi.org/core/hasStateKind -->

    <owl:ObjectProperty rdf:about="https://saref.etsi.org/core/hasStateKind">
        <rdfs:domain rdf:resource="https://saref.etsi.org/core/StateOfInterest"/>
        <rdfs:range rdf:resource="https://saref.etsi.org/core/State"/>
        <owl:propertyChainAxiom rdf:parseType="Collection">
            <rdf:Description rdf:about="https://saref.etsi.org/core/hasStateKind"/>
            <rdf:Description rdf:about="http://www.w3.org/2004/02/skos/core#broader"/>
        </owl:propertyChainAxiom>
        <rdfs:comment xml:lang="en">links a state of interest to its kind, a state</rdfs:comment>
        <rdfs:label xml:lang="en">has state kind</rdfs:label>
    </owl:ObjectProperty>
    


    <!-- https://saref.etsi.org/core/hasStateOfInterest -->

    <owl:ObjectProperty rdf:about="https://saref.etsi.org/core/hasStateOfInterest">
        <owl:inverseOf rdf:resource="https://saref.etsi.org/core/isStateOfInterestOf"/>
        <rdfs:domain rdf:resource="https://saref.etsi.org/core/FeatureOfInterest"/>
        <rdfs:range rdf:resource="https://saref.etsi.org/core/StateOfInterest"/>
        <rdfs:comment xml:lang="en">Links a feature of interest to one of its states of interest.</rdfs:comment>
        <rdfs:label xml:lang="en">has state of interest</rdfs:label>
        <skos:historyNote xml:lang="en">V3.2.1: Introduced saref:hasStateOfInterest and saref:isStateOfInterestOf, parallel to saref:hasPropertyOfInterest and saref:isPropertyOfInterestOf.</skos:historyNote>
    </owl:ObjectProperty>
    


    <!-- https://saref.etsi.org/core/hasStateValue -->

    <owl:ObjectProperty rdf:about="https://saref.etsi.org/core/hasStateValue">
        <rdfs:domain>
            <owl:Class>
                <owl:unionOf rdf:parseType="Collection">
                    <rdf:Description rdf:about="https://saref.etsi.org/core/FeatureKind"/>
                    <rdf:Description rdf:about="https://saref.etsi.org/core/FeatureOfInterest"/>
                    <rdf:Description rdf:about="https://saref.etsi.org/core/StateOfInterest"/>
                </owl:unionOf>
            </owl:Class>
        </rdfs:domain>
        <rdfs:range rdf:resource="https://saref.etsi.org/core/StateValue"/>
        <owl:propertyChainAxiom rdf:parseType="Collection">
            <rdf:Description rdf:about="http://www.w3.org/2004/02/skos/core#broader"/>
            <rdf:Description rdf:about="https://saref.etsi.org/core/hasStateValue"/>
        </owl:propertyChainAxiom>
        <rdfs:comment xml:lang="en">Links a feature kind, a feature of interest, or a state of interest, to a state value.</rdfs:comment>
        <rdfs:label xml:lang="en">has state value</rdfs:label>
        <skos:historyNote xml:lang="en">V4.1.1: Introduced saref:hasStateValue.</skos:historyNote>
    </owl:ObjectProperty>
    


    <!-- https://saref.etsi.org/core/isAccomplishedBy -->

    <owl:ObjectProperty rdf:about="https://saref.etsi.org/core/isAccomplishedBy">
        <rdfs:domain rdf:resource="https://saref.etsi.org/core/Task"/>
        <rdfs:comment xml:lang="en">A relationship identifying an entity (e.g., a device) that can accomplish a task.</rdfs:comment>
        <rdfs:label xml:lang="en">is accomplished by</rdfs:label>
    </owl:ObjectProperty>
    


    <!-- https://saref.etsi.org/core/isCommandOf -->

    <owl:ObjectProperty rdf:about="https://saref.etsi.org/core/isCommandOf">
        <rdfs:domain rdf:resource="https://saref.etsi.org/core/Command"/>
        <rdfs:range>
            <owl:Class>
                <owl:unionOf rdf:parseType="Collection">
                    <rdf:Description rdf:about="https://saref.etsi.org/core/Function"/>
                    <rdf:Description rdf:about="https://saref.etsi.org/core/FunctionOfInterest"/>
                </owl:unionOf>
            </owl:Class>
        </rdfs:range>
        <rdfs:comment xml:lang="en">Links a command and a function or function of interest that supports it.</rdfs:comment>
        <rdfs:label xml:lang="en">is command of</rdfs:label>
    </owl:ObjectProperty>
    


    <!-- https://saref.etsi.org/core/isCommandOfInterestOf -->

    <owl:ObjectProperty rdf:about="https://saref.etsi.org/core/isCommandOfInterestOf">
        <rdf:type rdf:resource="http://www.w3.org/2002/07/owl#FunctionalProperty"/>
        <rdfs:domain rdf:resource="https://saref.etsi.org/core/CommandOfInterest"/>
        <rdfs:range rdf:resource="https://saref.etsi.org/core/FunctionOfInterest"/>
        <rdfs:comment xml:lang="en">Links a command of interest to the function of interest it is a command of.</rdfs:comment>
        <rdfs:label xml:lang="en">is command of interest of</rdfs:label>
    </owl:ObjectProperty>
    


    <!-- https://saref.etsi.org/core/isConsumedBy -->

    <owl:ObjectProperty rdf:about="https://saref.etsi.org/core/isConsumedBy">
        <rdfs:domain rdf:resource="https://saref.etsi.org/core/Commodity"/>
        <rdfs:range>
            <owl:Class>
                <owl:unionOf rdf:parseType="Collection">
                    <rdf:Description rdf:about="https://saref.etsi.org/core/Device"/>
                    <rdf:Description rdf:about="https://saref.etsi.org/core/DeviceKind"/>
                    <rdf:Description rdf:about="https://saref.etsi.org/core/FeatureKind"/>
                    <rdf:Description rdf:about="https://saref.etsi.org/core/FeatureOfInterest"/>
                </owl:unionOf>
            </owl:Class>
        </rdfs:range>
        <rdfs:comment xml:lang="en">Links a commodity to the feature kind, feature of interest, or device, that consumes it</rdfs:comment>
        <rdfs:label xml:lang="en">is consumed by</rdfs:label>
    </owl:ObjectProperty>
    


    <!-- https://saref.etsi.org/core/isControlledBy -->

    <owl:ObjectProperty rdf:about="https://saref.etsi.org/core/isControlledBy">
        <rdfs:subPropertyOf rdf:resource="https://saref.etsi.org/core/isTargetOf"/>
        <rdfs:comment xml:lang="en">Links a feature, property, or state, to the device, function, command, or procedure execution, that controls it.</rdfs:comment>
        <rdfs:label xml:lang="en">is controlled by</rdfs:label>
        <skos:historyNote xml:lang="en">V3.2.1: Introduced property saref:isControlledBy.</skos:historyNote>
    </owl:ObjectProperty>
    


    <!-- https://saref.etsi.org/core/isExecutionOf -->

    <owl:ObjectProperty rdf:about="https://saref.etsi.org/core/isExecutionOf">
        <rdfs:domain rdf:resource="https://saref.etsi.org/core/ProcedureExecution"/>
        <rdfs:range>
            <owl:Class>
                <owl:unionOf rdf:parseType="Collection">
                    <rdf:Description rdf:about="https://saref.etsi.org/core/Command"/>
                    <rdf:Description rdf:about="https://saref.etsi.org/core/CommandOfInterest"/>
                    <rdf:Description rdf:about="https://saref.etsi.org/core/Operation"/>
                </owl:unionOf>
            </owl:Class>
        </rdfs:range>
        <owl:propertyChainAxiom rdf:parseType="Collection">
            <rdf:Description rdf:about="https://saref.etsi.org/core/isExecutionOf"/>
            <rdf:Description rdf:about="http://www.w3.org/2004/02/skos/core#broader"/>
        </owl:propertyChainAxiom>
        <owl:propertyChainAxiom rdf:parseType="Collection">
            <rdf:Description rdf:about="https://saref.etsi.org/core/isExecutionOf"/>
            <rdf:Description rdf:about="https://saref.etsi.org/core/hasCommandKind"/>
        </owl:propertyChainAxiom>
        <rdfs:comment xml:lang="en">Links a command execution to the command or command of interest that was executed. Also liks an operation execution to the operation that was executed</rdfs:comment>
        <rdfs:label xml:lang="en">is execution of</rdfs:label>
    </owl:ObjectProperty>
    


    <!-- https://saref.etsi.org/core/isFunctionOf -->

    <owl:ObjectProperty rdf:about="https://saref.etsi.org/core/isFunctionOf">
        <rdfs:domain rdf:resource="https://saref.etsi.org/core/Function"/>
        <rdfs:range>
            <owl:Class>
                <owl:unionOf rdf:parseType="Collection">
                    <rdf:Description rdf:about="https://saref.etsi.org/core/FeatureKind"/>
                    <rdf:Description rdf:about="https://saref.etsi.org/core/FeatureOfInterest"/>
                </owl:unionOf>
            </owl:Class>
        </rdfs:range>
        <rdfs:comment xml:lang="en">Links a function to the feature kind or device it is a function of.</rdfs:comment>
        <rdfs:label xml:lang="en">is function of</rdfs:label>
        <skos:historyNote xml:lang="en">V3.2.1: Introduced saref:isFunctionOf.</skos:historyNote>
    </owl:ObjectProperty>
    


    <!-- https://saref.etsi.org/core/isFunctionOfInterestOf -->

    <owl:ObjectProperty rdf:about="https://saref.etsi.org/core/isFunctionOfInterestOf">
        <rdf:type rdf:resource="http://www.w3.org/2002/07/owl#FunctionalProperty"/>
        <rdfs:domain rdf:resource="https://saref.etsi.org/core/FunctionOfInterest"/>
        <rdfs:range rdf:resource="https://saref.etsi.org/core/Device"/>
        <rdfs:comment xml:lang="en">Links a function of interest to the device it is a function of.</rdfs:comment>
        <rdfs:label xml:lang="en">is function of interest of</rdfs:label>
    </owl:ObjectProperty>
    


    <!-- https://saref.etsi.org/core/isMeasuredIn -->

    <owl:ObjectProperty rdf:about="https://saref.etsi.org/core/isMeasuredIn">
        <rdfs:range rdf:resource="https://saref.etsi.org/core/UnitOfMeasure"/>
        <rdfs:comment xml:lang="en">A relationship identifying the unit of measure used for a certain entity.</rdfs:comment>
        <rdfs:label xml:lang="en">is measured in</rdfs:label>
        <skos:historyNote xml:lang="en">V3.2.1: Relaxed domain of saref:isMeasuredIn so it can apply to saref:PropertyValue as well as saref:Measurement. The new range will be enforced in the next major revision of SAREF.</skos:historyNote>
    </owl:ObjectProperty>
    


    <!-- https://saref.etsi.org/core/isObservedBy -->

    <owl:ObjectProperty rdf:about="https://saref.etsi.org/core/isObservedBy">
        <rdfs:subPropertyOf rdf:resource="https://saref.etsi.org/core/isTargetOf"/>
        <owl:inverseOf rdf:resource="https://saref.etsi.org/core/observes"/>
        <rdfs:comment xml:lang="en">Links a feature, property, or state, to the device, function, command, or procedure execution, that observes it.</rdfs:comment>
        <rdfs:label xml:lang="en">is observed by</rdfs:label>
    </owl:ObjectProperty>
    


    <!-- https://saref.etsi.org/core/isOfferedBy -->

    <owl:ObjectProperty rdf:about="https://saref.etsi.org/core/isOfferedBy">
        <owl:inverseOf rdf:resource="https://saref.etsi.org/core/offers"/>
        <rdf:type rdf:resource="http://www.w3.org/2002/07/owl#FunctionalProperty"/>
        <rdfs:domain rdf:resource="https://saref.etsi.org/core/Service"/>
        <rdfs:range rdf:resource="https://saref.etsi.org/core/Device"/>
        <rdfs:comment xml:lang="en">Links a service to the device that exposes it to a network</rdfs:comment>
        <rdfs:label xml:lang="en">is offered by</rdfs:label>
        <skos:historyNote xml:lang="en">V3.2.1: Clarified definition of saref:isOfferedBy.</skos:historyNote>
    </owl:ObjectProperty>
    


    <!-- https://saref.etsi.org/core/isOperationOf -->

    <owl:ObjectProperty rdf:about="https://saref.etsi.org/core/isOperationOf">
        <rdf:type rdf:resource="http://www.w3.org/2002/07/owl#FunctionalProperty"/>
        <rdfs:domain rdf:resource="https://saref.etsi.org/core/Operation"/>
        <rdfs:range rdf:resource="https://saref.etsi.org/core/Service"/>
        <rdfs:comment xml:lang="en">Links an operation to the service it belongs to.</rdfs:comment>
        <rdfs:label xml:lang="en">is operation of</rdfs:label>
    </owl:ObjectProperty>
    


    <!-- https://saref.etsi.org/core/isProducedBy -->

    <owl:ObjectProperty rdf:about="https://saref.etsi.org/core/isProducedBy">
        <owl:inverseOf rdf:resource="https://saref.etsi.org/core/produces"/>
        <rdfs:domain rdf:resource="https://saref.etsi.org/core/Commodity"/>
        <rdfs:range>
            <owl:Class>
                <owl:unionOf rdf:parseType="Collection">
                    <rdf:Description rdf:about="https://saref.etsi.org/core/Device"/>
                    <rdf:Description rdf:about="https://saref.etsi.org/core/DeviceKind"/>
                    <rdf:Description rdf:about="https://saref.etsi.org/core/FeatureKind"/>
                    <rdf:Description rdf:about="https://saref.etsi.org/core/FeatureOfInterest"/>
                </owl:unionOf>
            </owl:Class>
        </rdfs:range>
        <rdfs:comment xml:lang="en">Links a commodity to the feature kind, feature of interest, or device, that produces it</rdfs:comment>
        <rdfs:label xml:lang="en">is produced by</rdfs:label>
    </owl:ObjectProperty>
    


    <!-- https://saref.etsi.org/core/isProfileOf -->

    <owl:ObjectProperty rdf:about="https://saref.etsi.org/core/isProfileOf">
        <rdfs:domain rdf:resource="https://saref.etsi.org/core/Profile"/>
        <rdfs:range>
            <owl:Class>
                <owl:unionOf rdf:parseType="Collection">
                    <rdf:Description rdf:about="https://saref.etsi.org/core/Device"/>
                    <rdf:Description rdf:about="https://saref.etsi.org/core/DeviceKind"/>
                </owl:unionOf>
            </owl:Class>
        </rdfs:range>
        <rdfs:comment xml:lang="en">Links a profile to the device it describes. The device should be linked to a certain commodity using OP saref:consumes, saref:produces, or saref:stores, and optionally to some property or state using OP saref:targets or its sub-properties.</rdfs:comment>
        <rdfs:label xml:lang="en">is profile of</rdfs:label>
    </owl:ObjectProperty>
    


    <!-- https://saref.etsi.org/core/isPropertyOf -->

    <owl:ObjectProperty rdf:about="https://saref.etsi.org/core/isPropertyOf">
        <rdfs:domain rdf:resource="https://saref.etsi.org/core/Property"/>
        <rdfs:range>
            <owl:Class>
                <owl:unionOf rdf:parseType="Collection">
                    <rdf:Description rdf:about="https://saref.etsi.org/core/FeatureKind"/>
                    <rdf:Description rdf:about="https://saref.etsi.org/core/FeatureOfInterest"/>
                </owl:unionOf>
            </owl:Class>
        </rdfs:range>
        <rdfs:comment xml:lang="en">Links a property to the feature kind or feature of interest it is a property of.</rdfs:comment>
        <rdfs:label xml:lang="en">is property of</rdfs:label>
    </owl:ObjectProperty>
    


    <!-- https://saref.etsi.org/core/isPropertyOfInterestOf -->

    <owl:ObjectProperty rdf:about="https://saref.etsi.org/core/isPropertyOfInterestOf">
        <rdf:type rdf:resource="http://www.w3.org/2002/07/owl#FunctionalProperty"/>
        <rdfs:domain rdf:resource="https://saref.etsi.org/core/PropertyOfInterest"/>
        <rdfs:range rdf:resource="https://saref.etsi.org/core/FeatureOfInterest"/>
        <rdfs:comment xml:lang="en">Links a property of interest to the feature of interest it is a property of.</rdfs:comment>
        <rdfs:label xml:lang="en">is property of interest of</rdfs:label>
    </owl:ObjectProperty>
    


    <!-- https://saref.etsi.org/core/isStateOf -->

    <owl:ObjectProperty rdf:about="https://saref.etsi.org/core/isStateOf">
        <rdfs:domain rdf:resource="https://saref.etsi.org/core/State"/>
        <rdfs:range>
            <owl:Class>
                <owl:unionOf rdf:parseType="Collection">
                    <rdf:Description rdf:about="https://saref.etsi.org/core/FeatureKind"/>
                    <rdf:Description rdf:about="https://saref.etsi.org/core/FeatureOfInterest"/>
                </owl:unionOf>
            </owl:Class>
        </rdfs:range>
        <rdfs:comment xml:lang="en">Links a state to the feature kind or feature of interest it is a state of.</rdfs:comment>
        <rdfs:label xml:lang="en">is state of</rdfs:label>
        <skos:historyNote xml:lang="en">V3.2.1: Introduced saref:isStateOf.</skos:historyNote>
    </owl:ObjectProperty>
    


    <!-- https://saref.etsi.org/core/isStateOfInterestOf -->

    <owl:ObjectProperty rdf:about="https://saref.etsi.org/core/isStateOfInterestOf">
        <rdf:type rdf:resource="http://www.w3.org/2002/07/owl#FunctionalProperty"/>
        <rdfs:domain rdf:resource="https://saref.etsi.org/core/StateOfInterest"/>
        <rdfs:range rdf:resource="https://saref.etsi.org/core/FeatureOfInterest"/>
        <rdfs:comment xml:lang="en">Links a state of interest to the feature of interest it is a state of.</rdfs:comment>
        <rdfs:label xml:lang="en">is state of interest of</rdfs:label>
    </owl:ObjectProperty>
    


    <!-- https://saref.etsi.org/core/isStoredBy -->

    <owl:ObjectProperty rdf:about="https://saref.etsi.org/core/isStoredBy">
        <owl:inverseOf rdf:resource="https://saref.etsi.org/core/stores"/>
        <rdfs:domain rdf:resource="https://saref.etsi.org/core/Commodity"/>
        <rdfs:range>
            <owl:Class>
                <owl:unionOf rdf:parseType="Collection">
                    <rdf:Description rdf:about="https://saref.etsi.org/core/Device"/>
                    <rdf:Description rdf:about="https://saref.etsi.org/core/DeviceKind"/>
                    <rdf:Description rdf:about="https://saref.etsi.org/core/FeatureKind"/>
                    <rdf:Description rdf:about="https://saref.etsi.org/core/FeatureOfInterest"/>
                </owl:unionOf>
            </owl:Class>
        </rdfs:range>
        <rdfs:comment xml:lang="en">Links a commodity to the feature kind, feature of interest, or device, that stores it</rdfs:comment>
        <rdfs:label xml:lang="en">is stored by</rdfs:label>
    </owl:ObjectProperty>
    


    <!-- https://saref.etsi.org/core/isTargetOf -->

    <owl:ObjectProperty rdf:about="https://saref.etsi.org/core/isTargetOf">
        <owl:inverseOf rdf:resource="https://saref.etsi.org/core/targets"/>
        <rdfs:domain>
            <owl:Class>
                <owl:unionOf rdf:parseType="Collection">
                    <rdf:Description rdf:about="https://saref.etsi.org/core/FeatureKind"/>
                    <rdf:Description rdf:about="https://saref.etsi.org/core/FeatureOfInterest"/>
                    <rdf:Description rdf:about="https://saref.etsi.org/core/Property"/>
                    <rdf:Description rdf:about="https://saref.etsi.org/core/PropertyOfInterest"/>
                    <rdf:Description rdf:about="https://saref.etsi.org/core/State"/>
                    <rdf:Description rdf:about="https://saref.etsi.org/core/StateOfInterest"/>
                </owl:unionOf>
            </owl:Class>
        </rdfs:domain>
        <rdfs:range>
            <owl:Class>
                <owl:unionOf rdf:parseType="Collection">
                    <rdf:Description rdf:about="https://saref.etsi.org/core/Command"/>
                    <rdf:Description rdf:about="https://saref.etsi.org/core/CommandOfInterest"/>
                    <rdf:Description rdf:about="https://saref.etsi.org/core/Device"/>
                    <rdf:Description rdf:about="https://saref.etsi.org/core/DeviceKind"/>
                    <rdf:Description rdf:about="https://saref.etsi.org/core/Function"/>
                    <rdf:Description rdf:about="https://saref.etsi.org/core/FunctionOfInterest"/>
                    <rdf:Description rdf:about="https://saref.etsi.org/core/ProcedureExecution"/>
                </owl:unionOf>
            </owl:Class>
        </rdfs:range>
        <rdfs:comment xml:lang="en">Links a feature, property, or state, to the device, function, command, or procedure execution, that targets it.</rdfs:comment>
        <rdfs:label xml:lang="en">is target of</rdfs:label>
        <skos:historyNote xml:lang="en">V3.2.1: Introduced property saref:isActedUponBy.</skos:historyNote>
        <skos:historyNote xml:lang="en">V4.1.1: Renamed property saref:isActedUponBy into saref:isTargetOf.</skos:historyNote>
    </owl:ObjectProperty>
    


    <!-- https://saref.etsi.org/core/isValueOfProperty -->

    <owl:ObjectProperty rdf:about="https://saref.etsi.org/core/isValueOfProperty">
        <rdfs:domain rdf:resource="https://saref.etsi.org/core/PropertyValue"/>
        <rdfs:range>
            <owl:Class>
                <owl:unionOf rdf:parseType="Collection">
                    <rdf:Description rdf:about="https://saref.etsi.org/core/FeatureKind"/>
                    <rdf:Description rdf:about="https://saref.etsi.org/core/FeatureOfInterest"/>
                    <rdf:Description rdf:about="https://saref.etsi.org/core/Property"/>
                    <rdf:Description rdf:about="https://saref.etsi.org/core/PropertyOfInterest"/>
                </owl:unionOf>
            </owl:Class>
        </rdfs:range>
        <owl:propertyChainAxiom rdf:parseType="Collection">
            <rdf:Description rdf:about="https://saref.etsi.org/core/isValueOfProperty"/>
            <rdf:Description rdf:about="https://saref.etsi.org/core/hasPropertyKind"/>
        </owl:propertyChainAxiom>
        <rdfs:comment xml:lang="en">Links a property value to the property or property of interest it is a value of.</rdfs:comment>
        <rdfs:label xml:lang="en">is value of property</rdfs:label>
        <skos:historyNote xml:lang="en">V3.2.1: Introduced saref:isValueOfProperty.</skos:historyNote>
    </owl:ObjectProperty>
    


    <!-- https://saref.etsi.org/core/isValueOfState -->

    <owl:ObjectProperty rdf:about="https://saref.etsi.org/core/isValueOfState">
        <rdfs:domain rdf:resource="https://saref.etsi.org/core/StateValue"/>
        <rdfs:range>
            <owl:Class>
                <owl:unionOf rdf:parseType="Collection">
                    <rdf:Description rdf:about="https://saref.etsi.org/core/FeatureKind"/>
                    <rdf:Description rdf:about="https://saref.etsi.org/core/FeatureOfInterest"/>
                    <rdf:Description rdf:about="https://saref.etsi.org/core/StateOfInterest"/>
                </owl:unionOf>
            </owl:Class>
        </rdfs:range>
        <owl:propertyChainAxiom rdf:parseType="Collection">
            <rdf:Description rdf:about="https://saref.etsi.org/core/isValueOfState"/>
            <rdf:Description rdf:about="https://saref.etsi.org/core/hasStateKind"/>
        </owl:propertyChainAxiom>
        <rdfs:comment xml:lang="en">Links a state value to the state or state of interest it is a value of.</rdfs:comment>
        <rdfs:label xml:lang="en">is value of state</rdfs:label>
        <skos:historyNote xml:lang="en">V4.1.1: Introduced saref:isValueOfState.</skos:historyNote>
    </owl:ObjectProperty>
    


    <!-- https://saref.etsi.org/core/madeBy -->

    <owl:ObjectProperty rdf:about="https://saref.etsi.org/core/madeBy">
        <owl:inverseOf rdf:resource="https://saref.etsi.org/core/madeExecution"/>
        <rdfs:domain rdf:resource="https://saref.etsi.org/core/ProcedureExecution"/>
        <rdfs:range rdf:resource="https://saref.etsi.org/core/FeatureOfInterest"/>
        <rdfs:comment xml:lang="en">Links a procedure execution to the entity (e.g., device) that made it.</rdfs:comment>
        <rdfs:label xml:lang="en">made by</rdfs:label>
        <skos:historyNote xml:lang="en">V3.2.1: Introduce saref:madeBy (resp. saref:madeExecution) as generalization of saref:measurementMadeBy (resp. saref:makesMeasurement).</skos:historyNote>
    </owl:ObjectProperty>
    


    <!-- https://saref.etsi.org/core/madeExecution -->

    <owl:ObjectProperty rdf:about="https://saref.etsi.org/core/madeExecution">
        <rdfs:domain rdf:resource="https://saref.etsi.org/core/FeatureOfInterest"/>
        <rdfs:range rdf:resource="https://saref.etsi.org/core/ProcedureExecution"/>
        <rdfs:comment xml:lang="en">Links an entity (e.g., device) to the procedure execution it made.</rdfs:comment>
        <rdfs:label xml:lang="en">made execution</rdfs:label>
    </owl:ObjectProperty>
    


    <!-- https://saref.etsi.org/core/makesMeasurement -->

    <owl:ObjectProperty rdf:about="https://saref.etsi.org/core/makesMeasurement">
        <rdfs:comment>A relation between a device and the measurements it makes. Such measurement will link together the value of the measurement, its unit of measure and the property to which it relates.</rdfs:comment>
        <rdfs:label xml:lang="en">makes measurement</rdfs:label>
    </owl:ObjectProperty>
    


    <!-- https://saref.etsi.org/core/measuresProperty -->

    <owl:ObjectProperty rdf:about="https://saref.etsi.org/core/measuresProperty">
        <rdfs:comment>A relationship specifying the property that can be measured by a certain device</rdfs:comment>
        <rdfs:label xml:lang="en">measures property</rdfs:label>
    </owl:ObjectProperty>
    


    <!-- https://saref.etsi.org/core/observes -->

    <owl:ObjectProperty rdf:about="https://saref.etsi.org/core/observes">
        <rdfs:subPropertyOf rdf:resource="https://saref.etsi.org/core/targets"/>
        <rdfs:domain>
            <owl:Class>
                <owl:unionOf rdf:parseType="Collection">
                    <rdf:Description rdf:about="https://saref.etsi.org/core/Command"/>
                    <rdf:Description rdf:about="https://saref.etsi.org/core/CommandOfInterest"/>
                    <rdf:Description rdf:about="https://saref.etsi.org/core/DeviceKind"/>
                    <rdf:Description rdf:about="https://saref.etsi.org/core/Function"/>
                    <rdf:Description rdf:about="https://saref.etsi.org/core/FunctionOfInterest"/>
                    <rdf:Description rdf:about="https://saref.etsi.org/core/Observation"/>
                    <rdf:Description rdf:about="https://saref.etsi.org/core/Sensor"/>
                </owl:unionOf>
            </owl:Class>
        </rdfs:domain>
        <rdfs:comment xml:lang="en">Links a device, function, command, or procedure execution, to the feature, property, or state, it observes.</rdfs:comment>
        <rdfs:label xml:lang="en">observes</rdfs:label>
        <skos:historyNote xml:lang="en">V3.2.1: Introduced property saref:observes, as sub-property of saref:targets. and generalization of measures.</skos:historyNote>
    </owl:ObjectProperty>
    


    <!-- https://saref.etsi.org/core/offers -->

    <owl:ObjectProperty rdf:about="https://saref.etsi.org/core/offers">
        <rdfs:domain rdf:resource="https://saref.etsi.org/core/Device"/>
        <rdfs:range rdf:resource="https://saref.etsi.org/core/Service"/>
        <rdfs:comment xml:lang="en">Links a device to a service it exposes to a network.</rdfs:comment>
        <rdfs:label xml:lang="en">offers</rdfs:label>
        <skos:historyNote xml:lang="en">V3.2.1: Clarified definition of saref:offers.</skos:historyNote>
    </owl:ObjectProperty>
    


    <!-- https://saref.etsi.org/core/produces -->

    <owl:ObjectProperty rdf:about="https://saref.etsi.org/core/produces">
        <rdfs:domain>
            <owl:Class>
                <owl:unionOf rdf:parseType="Collection">
                    <rdf:Description rdf:about="https://saref.etsi.org/core/Device"/>
                    <rdf:Description rdf:about="https://saref.etsi.org/core/DeviceKind"/>
                    <rdf:Description rdf:about="https://saref.etsi.org/core/FeatureKind"/>
                    <rdf:Description rdf:about="https://saref.etsi.org/core/FeatureOfInterest"/>
                </owl:unionOf>
            </owl:Class>
        </rdfs:domain>
        <rdfs:range rdf:resource="https://saref.etsi.org/core/Commodity"/>
        <rdfs:comment xml:lang="en">Links a feature kind, feature of interest, or device, to the commodity it produces</rdfs:comment>
        <rdfs:label xml:lang="en">produces</rdfs:label>
    </owl:ObjectProperty>
    


    <!-- https://saref.etsi.org/core/profileHasPrice -->

    <owl:ObjectProperty rdf:about="https://saref.etsi.org/core/profileHasPrice">
        <rdfs:domain rdf:resource="https://saref.etsi.org/core/Profile"/>
        <rdfs:range rdf:resource="https://saref.etsi.org/core/PropertyValue"/>
        <rdfs:comment xml:lang="en">Links a profile to the money earned (negative values) or paid (positive values) for the use (production or consumption) of the commodity by the device</rdfs:comment>
        <rdfs:label xml:lang="en">has price</rdfs:label>
    </owl:ObjectProperty>
    


    <!-- https://saref.etsi.org/core/represents -->

    <owl:ObjectProperty rdf:about="https://saref.etsi.org/core/represents">
        <rdfs:domain>
            <owl:Class>
                <owl:unionOf rdf:parseType="Collection">
                    <rdf:Description rdf:about="https://saref.etsi.org/core/Operation"/>
                    <rdf:Description rdf:about="https://saref.etsi.org/core/Service"/>
                </owl:unionOf>
            </owl:Class>
        </rdfs:domain>
        <rdfs:range>
            <owl:Class>
                <owl:unionOf rdf:parseType="Collection">
                    <rdf:Description rdf:about="https://saref.etsi.org/core/Command"/>
                    <rdf:Description rdf:about="https://saref.etsi.org/core/CommandOfInterest"/>
                    <rdf:Description rdf:about="https://saref.etsi.org/core/Function"/>
                    <rdf:Description rdf:about="https://saref.etsi.org/core/FunctionOfInterest"/>
                </owl:unionOf>
            </owl:Class>
        </rdfs:range>
        <rdfs:comment xml:lang="en">Links a service to some function or function of interest it exposes to the network. Also links an operation to some command or command of interest it exposes to the network.</rdfs:comment>
        <rdfs:label xml:lang="en">represents</rdfs:label>
        <skos:historyNote xml:lang="en">V3.2.1: Relaxed domain and range of saref:represents.</skos:historyNote>
    </owl:ObjectProperty>
    


    <!-- https://saref.etsi.org/core/stores -->

    <owl:ObjectProperty rdf:about="https://saref.etsi.org/core/stores">
        <rdfs:domain>
            <owl:Class>
                <owl:unionOf rdf:parseType="Collection">
                    <rdf:Description rdf:about="https://saref.etsi.org/core/Device"/>
                    <rdf:Description rdf:about="https://saref.etsi.org/core/DeviceKind"/>
                    <rdf:Description rdf:about="https://saref.etsi.org/core/FeatureKind"/>
                    <rdf:Description rdf:about="https://saref.etsi.org/core/FeatureOfInterest"/>
                </owl:unionOf>
            </owl:Class>
        </rdfs:domain>
        <rdfs:range rdf:resource="https://saref.etsi.org/core/Commodity"/>
        <rdfs:comment xml:lang="en">Links a feature kind, feature of interest, or device, to the commodity it stores</rdfs:comment>
        <rdfs:label xml:lang="en">stores</rdfs:label>
    </owl:ObjectProperty>
    


    <!-- https://saref.etsi.org/core/targets -->

    <owl:ObjectProperty rdf:about="https://saref.etsi.org/core/targets">
        <rdfs:domain>
            <owl:Class>
                <owl:unionOf rdf:parseType="Collection">
                    <rdf:Description rdf:about="https://saref.etsi.org/core/Command"/>
                    <rdf:Description rdf:about="https://saref.etsi.org/core/CommandOfInterest"/>
                    <rdf:Description rdf:about="https://saref.etsi.org/core/Device"/>
                    <rdf:Description rdf:about="https://saref.etsi.org/core/DeviceKind"/>
                    <rdf:Description rdf:about="https://saref.etsi.org/core/Function"/>
                    <rdf:Description rdf:about="https://saref.etsi.org/core/FunctionOfInterest"/>
                    <rdf:Description rdf:about="https://saref.etsi.org/core/ProcedureExecution"/>
                </owl:unionOf>
            </owl:Class>
        </rdfs:domain>
        <rdfs:range>
            <owl:Class>
                <owl:unionOf rdf:parseType="Collection">
                    <rdf:Description rdf:about="https://saref.etsi.org/core/FeatureKind"/>
                    <rdf:Description rdf:about="https://saref.etsi.org/core/FeatureOfInterest"/>
                    <rdf:Description rdf:about="https://saref.etsi.org/core/Property"/>
                    <rdf:Description rdf:about="https://saref.etsi.org/core/PropertyOfInterest"/>
                    <rdf:Description rdf:about="https://saref.etsi.org/core/State"/>
                    <rdf:Description rdf:about="https://saref.etsi.org/core/StateOfInterest"/>
                </owl:unionOf>
            </owl:Class>
        </rdfs:range>
        <rdfs:comment xml:lang="en">Links a device, function, command, or procedure execution, to the feature, property, or state, it targets.</rdfs:comment>
        <rdfs:label xml:lang="en">targets</rdfs:label>
        <skos:historyNote xml:lang="en">V3.2.1: saref:actsUpon now holds not only between a command and a state. It generalizes observes, observes, controls. Domain and range are unions of several classes.</skos:historyNote>
        <skos:historyNote xml:lang="en">V4.1.1: saref:actsUpon is renamed saref:targets.</skos:historyNote>
    </owl:ObjectProperty>
    


    <!-- https://saref.etsi.org/core/whenPropertyValue -->

    <owl:ObjectProperty rdf:about="https://saref.etsi.org/core/whenPropertyValue">
        <rdfs:domain rdf:resource="https://saref.etsi.org/core/Profile"/>
        <rdfs:range rdf:resource="https://saref.etsi.org/core/PropertyValue"/>
        <rdfs:comment xml:lang="en">Links a profile to a property value that contributes to restricting its applicable context.</rdfs:comment>
        <rdfs:label xml:lang="en">when property value</rdfs:label>
    </owl:ObjectProperty>
    


    <!-- https://saref.etsi.org/core/whenState -->

    <owl:ObjectProperty rdf:about="https://saref.etsi.org/core/whenState">
        <rdfs:domain rdf:resource="https://saref.etsi.org/core/Profile"/>
        <rdfs:range rdf:resource="https://saref.etsi.org/core/State"/>
        <rdfs:comment xml:lang="en">Links a profile to a state that contributes to restricting its applicable context.</rdfs:comment>
        <rdfs:label xml:lang="en">when state</rdfs:label>
    </owl:ObjectProperty>
    


    <!-- https://saref.etsi.org/saref4inma/belongsToCategory -->

    <owl:ObjectProperty rdf:about="https://saref.etsi.org/saref4inma/belongsToCategory">
        <owl:inverseOf rdf:resource="https://saref.etsi.org/saref4inma/isCategoryOf"/>
        <rdfs:comment>Link between an entity and its category</rdfs:comment>
        <rdfs:label xml:lang="en">belongs to category</rdfs:label>
    </owl:ObjectProperty>
    


    <!-- https://saref.etsi.org/saref4inma/consistsOfBatch -->

    <owl:ObjectProperty rdf:about="https://saref.etsi.org/saref4inma/consistsOfBatch">
        <rdfs:comment>A relation to express that a batch can recursively consists of other batches</rdfs:comment>
        <rdfs:label xml:lang="en">consists of batch</rdfs:label>
    </owl:ObjectProperty>
    


    <!-- https://saref.etsi.org/saref4inma/consistsOfItem -->

    <owl:ObjectProperty rdf:about="https://saref.etsi.org/saref4inma/consistsOfItem">
        <rdfs:comment>A relation to express that an item can recursively consists of other Items</rdfs:comment>
        <rdfs:label xml:lang="en">consists of item</rdfs:label>
    </owl:ObjectProperty>
    


    <!-- https://saref.etsi.org/saref4inma/creates -->

    <owl:ObjectProperty rdf:about="https://saref.etsi.org/saref4inma/creates">
        <owl:inverseOf rdf:resource="https://saref.etsi.org/saref4inma/isCreatedIn"/>
        <rdfs:comment>A relation between a production process (e.g., Batch) that creates one or more tangible objects (e.g., Items)</rdfs:comment>
        <rdfs:label xml:lang="en">creates</rdfs:label>
    </owl:ObjectProperty>
    


    <!-- https://saref.etsi.org/saref4inma/hasFeatureOfInterest -->

    <owl:ObjectProperty rdf:about="https://saref.etsi.org/saref4inma/hasFeatureOfInterest">
        <owl:inverseOf rdf:resource="https://saref.etsi.org/saref4inma/isFeatureOfInterestOf"/>
        <rdfs:comment>Relationship between a feature of interest and equipment</rdfs:comment>
        <rdfs:label xml:lang="en">has feature of interest</rdfs:label>
    </owl:ObjectProperty>
    


    <!-- https://saref.etsi.org/saref4inma/hasGTIN12ID -->

    <owl:ObjectProperty rdf:about="https://saref.etsi.org/saref4inma/hasGTIN12ID">
        <rdfs:subPropertyOf rdf:resource="https://saref.etsi.org/saref4inma/hasIdentifier"/>
        <rdfs:range rdf:resource="https://saref.etsi.org/saref4inma/GTIN12ID"/>
        <rdfs:comment>A relationship determining the  GTIN-12 identifier</rdfs:comment>
        <rdfs:label xml:lang="en">has GTIN12ID </rdfs:label>
    </owl:ObjectProperty>
    


    <!-- https://saref.etsi.org/saref4inma/hasGTIN13ID -->

    <owl:ObjectProperty rdf:about="https://saref.etsi.org/saref4inma/hasGTIN13ID">
        <rdfs:subPropertyOf rdf:resource="https://saref.etsi.org/saref4inma/hasIdentifier"/>
        <rdfs:range rdf:resource="https://saref.etsi.org/saref4inma/GTIN13ID"/>
        <rdfs:comment>A relationship determining the  GTIN-13 identifier</rdfs:comment>
        <rdfs:label xml:lang="en">has GTIN13ID</rdfs:label>
    </owl:ObjectProperty>
    


    <!-- https://saref.etsi.org/saref4inma/hasGTIN14ID -->

    <owl:ObjectProperty rdf:about="https://saref.etsi.org/saref4inma/hasGTIN14ID">
        <rdfs:subPropertyOf rdf:resource="https://saref.etsi.org/saref4inma/hasIdentifier"/>
        <rdfs:range rdf:resource="https://saref.etsi.org/saref4inma/GTIN14ID"/>
        <rdfs:comment>A relationship determining the  GTIN-14 identifier</rdfs:comment>
        <rdfs:label xml:lang="en">has GTIN14ID</rdfs:label>
    </owl:ObjectProperty>
    


    <!-- https://saref.etsi.org/saref4inma/hasGTIN8ID -->

    <owl:ObjectProperty rdf:about="https://saref.etsi.org/saref4inma/hasGTIN8ID">
        <rdfs:subPropertyOf rdf:resource="https://saref.etsi.org/saref4inma/hasIdentifier"/>
        <rdfs:range rdf:resource="https://saref.etsi.org/saref4inma/GTIN8ID"/>
        <rdfs:comment>A relationship determining the  GTIN-8 identifier</rdfs:comment>
        <rdfs:label xml:lang="en">has GTIN8ID</rdfs:label>
    </owl:ObjectProperty>
    


    <!-- https://saref.etsi.org/saref4inma/hasIRDI -->

    <owl:ObjectProperty rdf:about="https://saref.etsi.org/saref4inma/hasIRDI">
        <rdfs:subPropertyOf rdf:resource="https://saref.etsi.org/saref4inma/hasIdentifier"/>
        <rdfs:range rdf:resource="https://saref.etsi.org/saref4inma/IRDI"/>
        <rdfs:comment>A relationship determining the  International Registration Data Identifier (IRDI)</rdfs:comment>
        <rdfs:label xml:lang="en">has IRDI</rdfs:label>
    </owl:ObjectProperty>
    


    <!-- https://saref.etsi.org/saref4inma/hasIdentifier -->

    <owl:ObjectProperty rdf:about="https://saref.etsi.org/saref4inma/hasIdentifier">
        <rdfs:range rdf:resource="https://saref.etsi.org/saref4inma/ID"/>
        <rdfs:comment>link between an entity and its unique identifier</rdfs:comment>
        <rdfs:label xml:lang="en">has identifier</rdfs:label>
    </owl:ObjectProperty>
    


    <!-- https://saref.etsi.org/saref4inma/hasSize -->

    <owl:ObjectProperty rdf:about="https://saref.etsi.org/saref4inma/hasSize">
        <rdfs:comment>A relationship to count the amount of certain objects in a collection (e.g., size of a material batch)</rdfs:comment>
        <rdfs:label xml:lang="en">has size</rdfs:label>
    </owl:ObjectProperty>
    


    <!-- https://saref.etsi.org/saref4inma/hasUUID -->

    <owl:ObjectProperty rdf:about="https://saref.etsi.org/saref4inma/hasUUID">
        <rdfs:subPropertyOf rdf:resource="https://saref.etsi.org/saref4inma/hasIdentifier"/>
        <rdfs:range rdf:resource="https://saref.etsi.org/saref4inma/UUID"/>
        <rdfs:comment>A relationship determining the Universally Unique Identifier (UUID)</rdfs:comment>
        <rdfs:label xml:lang="en">has UUID</rdfs:label>
    </owl:ObjectProperty>
    


    <!-- https://saref.etsi.org/saref4inma/hasUpdate -->

    <owl:ObjectProperty rdf:about="https://saref.etsi.org/saref4inma/hasUpdate">
        <rdfs:comment>The newer version of a ItemCategory.</rdfs:comment>
        <rdfs:label xml:lang="en">has update</rdfs:label>
    </owl:ObjectProperty>
    


    <!-- https://saref.etsi.org/saref4inma/isCategoryOf -->

    <owl:ObjectProperty rdf:about="https://saref.etsi.org/saref4inma/isCategoryOf">
        <rdfs:comment>Link between a category and its associated entity</rdfs:comment>
        <rdfs:label xml:lang="en">is category of</rdfs:label>
    </owl:ObjectProperty>
    


    <!-- https://saref.etsi.org/saref4inma/isCreatedIn -->

    <owl:ObjectProperty rdf:about="https://saref.etsi.org/saref4inma/isCreatedIn">
        <rdfs:comment>An Item is created in an ItemBatch.</rdfs:comment>
        <rdfs:label xml:lang="en">is created in</rdfs:label>
    </owl:ObjectProperty>
    


    <!-- https://saref.etsi.org/saref4inma/isFeatureOfInterestOf -->

    <owl:ObjectProperty rdf:about="https://saref.etsi.org/saref4inma/isFeatureOfInterestOf">
        <rdfs:comment>Relationship between a feature of interest and equipment</rdfs:comment>
        <rdfs:label xml:lang="en">is feature of interest of</rdfs:label>
    </owl:ObjectProperty>
    


    <!-- https://saref.etsi.org/saref4inma/isProducedBy -->

    <owl:ObjectProperty rdf:about="https://saref.etsi.org/saref4inma/isProducedBy">
        <owl:inverseOf rdf:resource="https://saref.etsi.org/saref4inma/produces"/>
        <rdfs:comment>Items are produced using certain types of ProductionEquipmentCategories, for example: welding machines or laser cutting machines.</rdfs:comment>
        <rdfs:label xml:lang="en">is produced by</rdfs:label>
    </owl:ObjectProperty>
    


    <!-- https://saref.etsi.org/saref4inma/needsEquipment -->

    <owl:ObjectProperty rdf:about="https://saref.etsi.org/saref4inma/needsEquipment">
        <rdfs:comment>A relationship indicating that an entity needs a particular equipment to be produced</rdfs:comment>
        <rdfs:label xml:lang="en">needs equipment</rdfs:label>
    </owl:ObjectProperty>
    


    <!-- https://saref.etsi.org/saref4inma/produces -->

    <owl:ObjectProperty rdf:about="https://saref.etsi.org/saref4inma/produces">
        <rdfs:comment>ProductionEquipmentCategory, such as welding machines or laser cutting machines, produce certain categories of items (inverse of s4inma:isProducedBy)</rdfs:comment>
        <rdfs:label xml:lang="en">produces</rdfs:label>
    </owl:ObjectProperty>
    


    <!-- 
    ///////////////////////////////////////////////////////////////////////////////////////
    //
    // Data properties
    //
    ///////////////////////////////////////////////////////////////////////////////////////
     -->

    


    <!-- https://ega.industry.com/ontologies/core/data/hasSymbol -->

    <owl:DatatypeProperty rdf:about="https://ega.industry.com/ontologies/core/data/hasSymbol">
        <rdfs:domain rdf:resource="https://saref.etsi.org/core/UnitOfMeasure"/>
        <rdfs:range rdf:resource="http://www.w3.org/2001/XMLSchema#string"/>
        <rdfs:comment xml:lang="en">Represents the symbol of unit of measure ex: Temperature unit in C or Pressure  in B (Bar)</rdfs:comment>
        <rdfs:label>has symbol</rdfs:label>
    </owl:DatatypeProperty>
    


    <!-- https://ega.industry.com/ontologies/core/data/hasTag -->

    <owl:DatatypeProperty rdf:about="https://ega.industry.com/ontologies/core/data/hasTag">
        <rdfs:range rdf:resource="http://www.w3.org/2001/XMLSchema#string"/>
        <rdfs:label>has tag</rdfs:label>
    </owl:DatatypeProperty>
    


    <!-- https://ega.industry.com/ontologies/core/process/conditionAchieved -->

    <owl:DatatypeProperty rdf:about="https://ega.industry.com/ontologies/core/process/conditionAchieved">
        <rdfs:domain rdf:resource="https://ega.industry.com/ontologies/core/process/Condition"/>
        <rdfs:range rdf:resource="http://www.w3.org/2001/XMLSchema#boolean"/>
        <rdfs:label>condition achieved</rdfs:label>
    </owl:DatatypeProperty>
    


    <!-- https://ega.industry.com/ontologies/core/process/hasAlloyCode -->

    <owl:DatatypeProperty rdf:about="https://ega.industry.com/ontologies/core/process/hasAlloyCode">
        <rdfs:domain rdf:resource="https://ega.industry.com/ontologies/core/process/Process"/>
        <rdfs:range rdf:resource="http://www.w3.org/2001/XMLSchema#integer"/>
        <rdfs:label>has alloy code</rdfs:label>
    </owl:DatatypeProperty>
    


    <!-- https://ega.industry.com/ontologies/core/process/hasAlloyCodeId -->

    <owl:DatatypeProperty rdf:about="https://ega.industry.com/ontologies/core/process/hasAlloyCodeId">
        <rdfs:domain rdf:resource="https://ega.industry.com/ontologies/core/process/Process"/>
        <rdfs:range rdf:resource="http://www.w3.org/2001/XMLSchema#integer"/>
        <rdfs:label>has alloy code id</rdfs:label>
    </owl:DatatypeProperty>
    


    <!-- https://ega.industry.com/ontologies/core/process/hasBatchId -->

    <owl:DatatypeProperty rdf:about="https://ega.industry.com/ontologies/core/process/hasBatchId">
        <rdfs:domain rdf:resource="https://ega.industry.com/ontologies/core/process/Process"/>
        <rdfs:range rdf:resource="http://www.w3.org/2001/XMLSchema#integer"/>
        <rdfs:label>has batch id</rdfs:label>
    </owl:DatatypeProperty>
    


    <!-- https://ega.industry.com/ontologies/core/process/hasBatchNo -->

    <owl:DatatypeProperty rdf:about="https://ega.industry.com/ontologies/core/process/hasBatchNo">
        <rdfs:domain rdf:resource="https://ega.industry.com/ontologies/core/process/Process"/>
        <rdfs:range rdf:resource="http://www.w3.org/2001/XMLSchema#string"/>
        <rdfs:label>has batch no</rdfs:label>
    </owl:DatatypeProperty>
    


    <!-- https://ega.industry.com/ontologies/core/process/hasEndTimestamp -->

    <owl:DatatypeProperty rdf:about="https://ega.industry.com/ontologies/core/process/hasEndTimestamp">
        <rdfs:domain>
            <owl:Class>
                <owl:unionOf rdf:parseType="Collection">
                    <rdf:Description rdf:about="https://ega.industry.com/ontologies/core/process/Process"/>
                    <rdf:Description rdf:about="https://ega.industry.com/ontologies/core/process/Step"/>
                    <rdf:Description rdf:about="https://ega.industry.com/ontologies/core/process/SubProcess"/>
                </owl:unionOf>
            </owl:Class>
        </rdfs:domain>
        <rdfs:range rdf:resource="http://www.w3.org/2001/XMLSchema#dateTime"/>
        <rdfs:label>has end timestamp</rdfs:label>
    </owl:DatatypeProperty>
    


    <!-- https://ega.industry.com/ontologies/core/process/hasStartTimestamp -->

    <owl:DatatypeProperty rdf:about="https://ega.industry.com/ontologies/core/process/hasStartTimestamp">
        <rdfs:domain>
            <owl:Class>
                <owl:unionOf rdf:parseType="Collection">
                    <rdf:Description rdf:about="https://ega.industry.com/ontologies/core/process/Process"/>
                    <rdf:Description rdf:about="https://ega.industry.com/ontologies/core/process/Step"/>
                    <rdf:Description rdf:about="https://ega.industry.com/ontologies/core/process/SubProcess"/>
                </owl:unionOf>
            </owl:Class>
        </rdfs:domain>
        <rdfs:range rdf:resource="http://www.w3.org/2001/XMLSchema#dateTime"/>
        <rdfs:label>has start timestamp</rdfs:label>
    </owl:DatatypeProperty>
    


    <!-- https://ega.industry.com/ontologies/core/process/hasStepId -->

    <owl:DatatypeProperty rdf:about="https://ega.industry.com/ontologies/core/process/hasStepId">
        <rdfs:domain rdf:resource="https://ega.industry.com/ontologies/core/process/Step"/>
        <rdfs:range rdf:resource="http://www.w3.org/2001/XMLSchema#integer"/>
        <rdfs:label>has step id</rdfs:label>
    </owl:DatatypeProperty>
    


    <!-- https://ega.industry.com/ontologies/core/process/hasSubProcessId -->

    <owl:DatatypeProperty rdf:about="https://ega.industry.com/ontologies/core/process/hasSubProcessId">
        <rdfs:domain rdf:resource="https://ega.industry.com/ontologies/core/process/SubProcess"/>
        <rdfs:range rdf:resource="http://www.w3.org/2001/XMLSchema#integer"/>
        <rdfs:label>has sub process id</rdfs:label>
    </owl:DatatypeProperty>
    


    <!-- https://ega.industry.com/ontologies/core/process/isCurrentStep -->

    <owl:DatatypeProperty rdf:about="https://ega.industry.com/ontologies/core/process/isCurrentStep">
        <rdfs:domain rdf:resource="https://ega.industry.com/ontologies/core/process/Step"/>
        <rdfs:range rdf:resource="http://www.w3.org/2001/XMLSchema#boolean"/>
        <rdfs:comment>Indicate if a Step is Sub Process current Step, it&apos;s boolean type</rdfs:comment>
        <rdfs:label>is current step</rdfs:label>
    </owl:DatatypeProperty>
    


    <!-- https://ega.industry.com/ontologies/core/process/isCurrentSubProcess -->

    <owl:DatatypeProperty rdf:about="https://ega.industry.com/ontologies/core/process/isCurrentSubProcess">
        <rdfs:domain rdf:resource="https://ega.industry.com/ontologies/core/process/SubProcess"/>
        <rdfs:range rdf:resource="http://www.w3.org/2001/XMLSchema#boolean"/>
        <rdfs:label>is current subprocess</rdfs:label>
    </owl:DatatypeProperty>
    


    <!-- https://ega.industry.com/ontologies/core/process/isIterationCompleted -->

    <owl:DatatypeProperty rdf:about="https://ega.industry.com/ontologies/core/process/isIterationCompleted">
        <rdfs:domain rdf:resource="https://ega.industry.com/ontologies/core/process/IterativeStep"/>
        <rdfs:range rdf:resource="http://www.w3.org/2001/XMLSchema#boolean"/>
        <rdfs:comment>Links IterativeStep to loop condition true or false, if it&apos;s true the Step loop</rdfs:comment>
        <rdfs:label>is iteration completed</rdfs:label>
    </owl:DatatypeProperty>
    


    <!-- https://ega.industry.com/ontologies/core/process/isRunning -->

    <owl:DatatypeProperty rdf:about="https://ega.industry.com/ontologies/core/process/isRunning">
        <rdfs:domain rdf:resource="https://ega.industry.com/ontologies/core/process/Process"/>
        <rdfs:range rdf:resource="http://www.w3.org/2001/XMLSchema#boolean"/>
        <rdfs:label>is running</rdfs:label>
    </owl:DatatypeProperty>
    


    <!-- https://ega.industry.com/ontologies/core/process/iterationCount -->

    <owl:DatatypeProperty rdf:about="https://ega.industry.com/ontologies/core/process/iterationCount">
        <rdf:type rdf:resource="http://www.w3.org/2002/07/owl#FunctionalProperty"/>
        <rdfs:domain rdf:resource="https://ega.industry.com/ontologies/core/process/IterativeStep"/>
        <rdfs:range rdf:resource="http://www.w3.org/2001/XMLSchema#integer"/>
        <rdfs:comment xml:lang="en">It&apos;s IterativeStep loop counter</rdfs:comment>
        <rdfs:label xml:lang="en">has iteration counter</rdfs:label>
    </owl:DatatypeProperty>
    


    <!-- https://saref.etsi.org/core/hasManufacturer -->

    <owl:DatatypeProperty rdf:about="https://saref.etsi.org/core/hasManufacturer">
        <rdfs:domain>
            <owl:Class>
                <owl:unionOf rdf:parseType="Collection">
                    <rdf:Description rdf:about="https://saref.etsi.org/core/FeatureKind"/>
                    <rdf:Description rdf:about="https://saref.etsi.org/core/FeatureOfInterest"/>
                </owl:unionOf>
            </owl:Class>
        </rdfs:domain>
        <rdfs:comment xml:lang="en">A relationship identifying the manufacturer of an entity (e.g., device). The value is expected to be a string or a string with language tag.</rdfs:comment>
        <rdfs:label xml:lang="en">has manufacturer</rdfs:label>
        <skos:historyNote xml:lang="en">V3.2.1: Defined domain of saref:hasManufacturer to union of feature kind and feature of interest.</skos:historyNote>
    </owl:DatatypeProperty>
    


    <!-- https://saref.etsi.org/core/hasModel -->

    <owl:DatatypeProperty rdf:about="https://saref.etsi.org/core/hasModel">
        <rdfs:domain>
            <owl:Class>
                <owl:unionOf rdf:parseType="Collection">
                    <rdf:Description rdf:about="https://saref.etsi.org/core/FeatureKind"/>
                    <rdf:Description rdf:about="https://saref.etsi.org/core/FeatureOfInterest"/>
                </owl:unionOf>
            </owl:Class>
        </rdfs:domain>
        <rdfs:comment xml:lang="en">A relationship identifying the model of an entity (e.g., device). The value is expected to be a string or a string with language tag.</rdfs:comment>
        <rdfs:label xml:lang="en">has model</rdfs:label>
        <skos:historyNote xml:lang="en">V3.2.1: Defined domain of saref:hasModel to union of feature kind and feature of interest.</skos:historyNote>
    </owl:DatatypeProperty>
    


    <!-- https://saref.etsi.org/core/hasResultTime -->

    <owl:DatatypeProperty rdf:about="https://saref.etsi.org/core/hasResultTime">
        <rdfs:domain rdf:resource="https://saref.etsi.org/core/ProcedureExecution"/>
        <rdfs:range rdf:resource="http://www.w3.org/2001/XMLSchema#dateTime"/>
        <rdfs:comment xml:lang="en">Links a procedure execution to the instant of time when the activity was completed, expressed as an xsd:dateTime literal.</rdfs:comment>
        <rdfs:label xml:lang="en">has result time</rdfs:label>
        <skos:historyNote xml:lang="en">V3.2.1: Introduced saref:hasResultTime as part of general will to make SAREF and SOSA/SSN converge.</skos:historyNote>
    </owl:DatatypeProperty>
    


    <!-- https://saref.etsi.org/core/hasRevisionNumber -->

    <owl:DatatypeProperty rdf:about="https://saref.etsi.org/core/hasRevisionNumber">
        <rdfs:range rdf:resource="http://www.w3.org/2001/XMLSchema#string"/>
        <rdfs:comment xml:lang="en">Links some entity (e.g., a device) to its revision number.</rdfs:comment>
        <rdfs:label xml:lang="en">has revision number</rdfs:label>
        <rdfs:seeAlso rdf:resource="https://labs.etsi.org/rep/saref/saref-core/-/issues/53"/>
    </owl:DatatypeProperty>
    


    <!-- https://saref.etsi.org/core/hasTimestamp -->

    <owl:DatatypeProperty rdf:about="https://saref.etsi.org/core/hasTimestamp">
        <rdfs:range rdf:resource="http://www.w3.org/2001/XMLSchema#dateTime"/>
        <terms:description></terms:description>
        <rdfs:comment xml:lang="en">Links a procedure execution or a profile to an instant.</rdfs:comment>
        <rdfs:label xml:lang="en">has timestamp</rdfs:label>
        <skos:historyNote xml:lang="en">V3.2.1: Tried to clarify definition of saref:hasTimestamp. Still unclear.</skos:historyNote>
        <skos:note xml:lang="en">Applied on a profile, it describes the applicable instant of that profile</skos:note>
        <skos:note xml:lang="en">When the execution time and the phenomenon time are the same time instants, then DP saref:hasTimestamp can be used to simply link a procedure execution to the time of these instants, expressed as an xsd:dateTime literal.</skos:note>
    </owl:DatatypeProperty>
    


    <!-- https://saref.etsi.org/core/hasValue -->

    <owl:DatatypeProperty rdf:about="https://saref.etsi.org/core/hasValue">
        <rdfs:range rdf:resource="http://www.w3.org/2001/XMLSchema#float"/>
        <rdfs:comment xml:lang="en">Value of a property value expressed as an RDF literal. Note that, even if decimal values are expected, values could use other datatypes.</rdfs:comment>
        <rdfs:label xml:lang="en">has value</rdfs:label>
        <skos:historyNote xml:lang="en">V3.2.1: Clarified definition of saref:hasValue.</skos:historyNote>
    </owl:DatatypeProperty>
    


    <!-- https://saref.etsi.org/core/hasVersion -->

    <owl:DatatypeProperty rdf:about="https://saref.etsi.org/core/hasVersion">
        <rdfs:range rdf:resource="http://www.w3.org/2001/XMLSchema#string"/>
        <rdfs:comment xml:lang="en">Links some entity (e.g., a device) to its version.</rdfs:comment>
        <rdfs:label xml:lang="en">has version</rdfs:label>
        <rdfs:seeAlso rdf:resource="https://labs.etsi.org/rep/saref/saref-core/-/issues/53"/>
    </owl:DatatypeProperty>
    


    <!-- https://saref.etsi.org/saref4inma/hasCertificate -->

    <owl:DatatypeProperty rdf:about="https://saref.etsi.org/saref4inma/hasCertificate">
        <rdfs:range rdf:resource="http://www.w3.org/2001/XMLSchema#string"/>
        <rdfs:comment>The MaterialBatch can contain material quality certificates, for example a NEN 10204:2004 3.1 steel certificate.</rdfs:comment>
        <rdfs:label xml:lang="en">has certificate</rdfs:label>
    </owl:DatatypeProperty>
    


    <!-- https://saref.etsi.org/saref4inma/hasGTIN12IDValue -->

    <owl:DatatypeProperty rdf:about="https://saref.etsi.org/saref4inma/hasGTIN12IDValue">
        <rdfs:subPropertyOf rdf:resource="https://saref.etsi.org/saref4inma/hasIDValue"/>
        <rdfs:range rdf:resource="http://www.w3.org/2001/XMLSchema#string"/>
        <rdfs:comment>A relation to express the value of an GTIN12 as a string</rdfs:comment>
        <rdfs:label xml:lang="en">has GTIN12ID value</rdfs:label>
    </owl:DatatypeProperty>
    


    <!-- https://saref.etsi.org/saref4inma/hasGTIN13IDValue -->

    <owl:DatatypeProperty rdf:about="https://saref.etsi.org/saref4inma/hasGTIN13IDValue">
        <rdfs:subPropertyOf rdf:resource="https://saref.etsi.org/saref4inma/hasIDValue"/>
        <rdfs:range rdf:resource="http://www.w3.org/2001/XMLSchema#string"/>
        <rdfs:comment>A relation to express the value of an GTIN13 as a string</rdfs:comment>
        <rdfs:label xml:lang="en">has GTIN13ID value</rdfs:label>
    </owl:DatatypeProperty>
    


    <!-- https://saref.etsi.org/saref4inma/hasGTIN14IDValue -->

    <owl:DatatypeProperty rdf:about="https://saref.etsi.org/saref4inma/hasGTIN14IDValue">
        <rdfs:subPropertyOf rdf:resource="https://saref.etsi.org/saref4inma/hasIDValue"/>
        <rdfs:range rdf:resource="http://www.w3.org/2001/XMLSchema#string"/>
        <rdfs:comment>A relation to express the value of an GTIN14 as a string</rdfs:comment>
        <rdfs:label xml:lang="en">has GTIN14ID value</rdfs:label>
    </owl:DatatypeProperty>
    


    <!-- https://saref.etsi.org/saref4inma/hasGTIN8IDValue -->

    <owl:DatatypeProperty rdf:about="https://saref.etsi.org/saref4inma/hasGTIN8IDValue">
        <rdfs:subPropertyOf rdf:resource="https://saref.etsi.org/saref4inma/hasIDValue"/>
        <rdfs:range rdf:resource="http://www.w3.org/2001/XMLSchema#string"/>
        <rdfs:comment>A relation to express the value of an GTIN8 as a string</rdfs:comment>
        <rdfs:label xml:lang="en">has GTIN8ID value</rdfs:label>
    </owl:DatatypeProperty>
    


    <!-- https://saref.etsi.org/saref4inma/hasIDValue -->

    <owl:DatatypeProperty rdf:about="https://saref.etsi.org/saref4inma/hasIDValue">
        <rdfs:range rdf:resource="http://www.w3.org/2001/XMLSchema#string"/>
        <rdfs:comment>A relation to express the value of an indentifier as a string (it can be used as alternative to or in combination with the s4inma:hasIdentifier object property</rdfs:comment>
        <rdfs:label xml:lang="en">has identifier value</rdfs:label>
    </owl:DatatypeProperty>
    


    <!-- https://saref.etsi.org/saref4inma/hasIRDIValue -->

    <owl:DatatypeProperty rdf:about="https://saref.etsi.org/saref4inma/hasIRDIValue">
        <rdfs:subPropertyOf rdf:resource="https://saref.etsi.org/saref4inma/hasIDValue"/>
        <rdfs:range rdf:resource="http://www.w3.org/2001/XMLSchema#string"/>
        <rdfs:comment>A relation to express the value of an IRDI as a string</rdfs:comment>
        <rdfs:label xml:lang="en">has IRDI value</rdfs:label>
    </owl:DatatypeProperty>
    


    <!-- https://saref.etsi.org/saref4inma/hasModelNumber -->

    <owl:DatatypeProperty rdf:about="https://saref.etsi.org/saref4inma/hasModelNumber">
        <rdfs:range rdf:resource="http://www.w3.org/2001/XMLSchema#string"/>
        <rdfs:comment>A relation to express the model number of a certain object (item, product, equipment, etc.) </rdfs:comment>
        <rdfs:label xml:lang="en">has model number</rdfs:label>
    </owl:DatatypeProperty>
    


    <!-- https://saref.etsi.org/saref4inma/hasSerialNumber -->

    <owl:DatatypeProperty rdf:about="https://saref.etsi.org/saref4inma/hasSerialNumber">
        <rdfs:range rdf:resource="http://www.w3.org/2001/XMLSchema#string"/>
        <rdfs:comment>A relation to describe the serial number of a certain Item, which is unique per Item.</rdfs:comment>
        <rdfs:label xml:lang="en">has serial number</rdfs:label>
    </owl:DatatypeProperty>
    


    <!-- https://saref.etsi.org/saref4inma/hasUUIDValue -->

    <owl:DatatypeProperty rdf:about="https://saref.etsi.org/saref4inma/hasUUIDValue">
        <rdfs:subPropertyOf rdf:resource="https://saref.etsi.org/saref4inma/hasIDValue"/>
        <rdfs:range rdf:resource="http://www.w3.org/2001/XMLSchema#string"/>
        <rdfs:comment>A relation to express the value of an UUID as a string</rdfs:comment>
        <rdfs:label xml:lang="en">has UUID value</rdfs:label>
    </owl:DatatypeProperty>
    


    <!-- https://saref.etsi.org/saref4inma/hasVersion -->

    <owl:DatatypeProperty rdf:about="https://saref.etsi.org/saref4inma/hasVersion">
        <rdfs:comment>An item has a certain revision or version number, whereas a higher number indicates a newer version.</rdfs:comment>
        <rdfs:label xml:lang="en">has version</rdfs:label>
    </owl:DatatypeProperty>
    


    <!-- 
    ///////////////////////////////////////////////////////////////////////////////////////
    //
    // Classes
    //
    ///////////////////////////////////////////////////////////////////////////////////////
     -->

    


    <!-- http://www.w3.org/2004/02/skos/core#ConceptScheme -->

    <owl:Class rdf:about="http://www.w3.org/2004/02/skos/core#ConceptScheme">
        <rdfs:comment>SKOS concept scheme can be viewed as an aggregation of one or more SKOS concepts.</rdfs:comment>
        <rdfs:label xml:lang="en">Concept Scheme</rdfs:label>
    </owl:Class>
    


    <!-- http://www.w3.org/2006/time#TemporalEntity -->

    <owl:Class rdf:about="http://www.w3.org/2006/time#TemporalEntity"/>
    


    <!-- http://www.w3.org/2006/time#TemporalPosition -->

    <owl:Class rdf:about="http://www.w3.org/2006/time#TemporalPosition"/>
    


    <!-- https://ega.industry.com/ontologies/core/asset/ActuatingFunction -->

    <owl:Class rdf:about="https://ega.industry.com/ontologies/core/asset/ActuatingFunction">
        <rdfs:subClassOf rdf:resource="https://saref.etsi.org/core/Function"/>
        <rdfs:comment>A function that allows to transmit data to device, binary switching (e.g., open/close, on/off), etc.</rdfs:comment>
        <rdfs:label>Actuating Function</rdfs:label>
    </owl:Class>
    


    <!-- https://ega.industry.com/ontologies/core/asset/AirFlowSensor -->

    <owl:Class rdf:about="https://ega.industry.com/ontologies/core/asset/AirFlowSensor">
        <rdfs:subClassOf rdf:resource="https://saref.etsi.org/core/Sensor"/>
        <rdfs:comment xml:lang="en">Measurement device for Air flow</rdfs:comment>
        <rdfs:label>Air Flow Sensor</rdfs:label>
    </owl:Class>
    


    <!-- https://ega.industry.com/ontologies/core/asset/AirSupply -->

    <owl:Class rdf:about="https://ega.industry.com/ontologies/core/asset/AirSupply">
        <rdfs:subClassOf rdf:resource="https://saref.etsi.org/core/Device"/>
        <rdfs:subClassOf>
            <owl:Restriction>
                <owl:onProperty rdf:resource="https://saref.etsi.org/core/consistsOf"/>
                <owl:someValuesFrom rdf:resource="https://ega.industry.com/ontologies/core/asset/AirFlowSensor"/>
            </owl:Restriction>
        </rdfs:subClassOf>
        <rdfs:subClassOf>
            <owl:Restriction>
                <owl:onProperty rdf:resource="https://saref.etsi.org/core/consistsOf"/>
                <owl:someValuesFrom rdf:resource="https://ega.industry.com/ontologies/core/asset/OxygenSensor"/>
            </owl:Restriction>
        </rdfs:subClassOf>
        <rdfs:comment xml:lang="en">Device that provides regulated Air flow to achieve optimal combustion ratio with gas</rdfs:comment>
        <rdfs:label>Air Supply</rdfs:label>
    </owl:Class>
    


    <!-- https://ega.industry.com/ontologies/core/asset/Aluminium -->

    <owl:Class rdf:about="https://ega.industry.com/ontologies/core/asset/Aluminium">
        <rdfs:subClassOf rdf:resource="https://saref.etsi.org/saref4inma/MaterialBatch"/>
        <rdfs:comment xml:lang="en">Primary raw material processed in Furnance</rdfs:comment>
    </owl:Class>
    


    <!-- https://ega.industry.com/ontologies/core/asset/Burner -->

    <owl:Class rdf:about="https://ega.industry.com/ontologies/core/asset/Burner">
        <rdfs:subClassOf rdf:resource="https://saref.etsi.org/core/Device"/>
        <rdfs:subClassOf>
            <owl:Restriction>
                <owl:onProperty rdf:resource="https://saref.etsi.org/core/consistsOf"/>
                <owl:someValuesFrom rdf:resource="https://ega.industry.com/ontologies/core/asset/AirSupply"/>
            </owl:Restriction>
        </rdfs:subClassOf>
        <rdfs:subClassOf>
            <owl:Restriction>
                <owl:onProperty rdf:resource="https://saref.etsi.org/core/consistsOf"/>
                <owl:someValuesFrom rdf:resource="https://ega.industry.com/ontologies/core/asset/GasSupply"/>
            </owl:Restriction>
        </rdfs:subClassOf>
        <rdfs:comment>Heating device that combusts gas and air mixtures to generate and control heat within the furnace</rdfs:comment>
    </owl:Class>
    


    <!-- https://ega.industry.com/ontologies/core/asset/CastingStatusSensor -->

    <owl:Class rdf:about="https://ega.industry.com/ontologies/core/asset/CastingStatusSensor">
        <rdfs:subClassOf rdf:resource="https://saref.etsi.org/core/Sensor"/>
        <rdfs:label>Casting Status Sensor</rdfs:label>
    </owl:Class>
    


    <!-- https://ega.industry.com/ontologies/core/asset/CastingSystem -->

    <owl:Class rdf:about="https://ega.industry.com/ontologies/core/asset/CastingSystem">
        <rdfs:subClassOf rdf:resource="https://ega.industry.com/ontologies/core/asset/IndustrySystem"/>
        <rdfs:comment>Downstream component that receives processed aluminium to form final products (billets, sheets, ingots)</rdfs:comment>
        <rdfs:label>Casting System</rdfs:label>
    </owl:Class>
    


    <!-- https://ega.industry.com/ontologies/core/asset/CloseCommand -->

    <owl:Class rdf:about="https://ega.industry.com/ontologies/core/asset/CloseCommand">
        <rdfs:subClassOf rdf:resource="https://saref.etsi.org/core/Command"/>
        <rdfs:comment xml:lang="en">Represents a command to close a device</rdfs:comment>
        <rdfs:label>Close Command</rdfs:label>
    </owl:Class>
    


    <!-- https://ega.industry.com/ontologies/core/asset/CoolingSystem -->

    <owl:Class rdf:about="https://ega.industry.com/ontologies/core/asset/CoolingSystem">
        <rdfs:subClassOf rdf:resource="https://ega.industry.com/ontologies/core/asset/IndustrySystem"/>
        <rdfs:comment>Heat management infrastructure that prevents overheating of furnace components</rdfs:comment>
        <rdfs:label>Cooling System</rdfs:label>
    </owl:Class>
    


    <!-- https://ega.industry.com/ontologies/core/asset/Door -->

    <owl:Class rdf:about="https://ega.industry.com/ontologies/core/asset/Door">
        <rdfs:subClassOf rdf:resource="https://saref.etsi.org/core/Device"/>
        <rdfs:subClassOf>
            <owl:Restriction>
                <owl:onProperty rdf:resource="https://saref.etsi.org/core/hasFunction"/>
                <owl:someValuesFrom rdf:resource="https://ega.industry.com/ontologies/core/asset/OpenCloseFunction"/>
            </owl:Restriction>
        </rdfs:subClassOf>
        <rdfs:subClassOf>
            <owl:Restriction>
                <owl:onProperty rdf:resource="https://saref.etsi.org/core/hasState"/>
                <owl:someValuesFrom rdf:resource="https://ega.industry.com/ontologies/core/asset/OpenCloseState"/>
            </owl:Restriction>
        </rdfs:subClassOf>
        <rdfs:comment xml:lang="en">Access portal for material loading and sampling operations</rdfs:comment>
    </owl:Class>
    


    <!-- https://ega.industry.com/ontologies/core/asset/Furnace -->

    <owl:Class rdf:about="https://ega.industry.com/ontologies/core/asset/Furnace">
        <rdfs:subClassOf rdf:resource="https://saref.etsi.org/core/Device"/>
        <rdfs:subClassOf>
            <owl:Restriction>
                <owl:onProperty rdf:resource="https://ega.industry.com/ontologies/core/asset/feeds"/>
                <owl:someValuesFrom rdf:resource="https://ega.industry.com/ontologies/core/asset/CastingSystem"/>
            </owl:Restriction>
        </rdfs:subClassOf>
        <rdfs:subClassOf>
            <owl:Restriction>
                <owl:onProperty rdf:resource="https://ega.industry.com/ontologies/core/asset/hasProcess"/>
                <owl:someValuesFrom rdf:resource="https://ega.industry.com/ontologies/core/process/Process"/>
            </owl:Restriction>
        </rdfs:subClassOf>
        <rdfs:subClassOf>
            <owl:Restriction>
                <owl:onProperty rdf:resource="https://ega.industry.com/ontologies/core/asset/isFedBy"/>
                <owl:someValuesFrom rdf:resource="https://ega.industry.com/ontologies/core/asset/RawMaterialFeederSystem"/>
            </owl:Restriction>
        </rdfs:subClassOf>
        <rdfs:subClassOf>
            <owl:Restriction>
                <owl:onProperty rdf:resource="https://saref.etsi.org/core/consistsOf"/>
                <owl:someValuesFrom rdf:resource="https://ega.industry.com/ontologies/core/asset/Burner"/>
            </owl:Restriction>
        </rdfs:subClassOf>
        <rdfs:subClassOf>
            <owl:Restriction>
                <owl:onProperty rdf:resource="https://saref.etsi.org/core/consistsOf"/>
                <owl:someValuesFrom rdf:resource="https://ega.industry.com/ontologies/core/asset/CastingStatusSensor"/>
            </owl:Restriction>
        </rdfs:subClassOf>
        <rdfs:subClassOf>
            <owl:Restriction>
                <owl:onProperty rdf:resource="https://saref.etsi.org/core/consistsOf"/>
                <owl:someValuesFrom rdf:resource="https://ega.industry.com/ontologies/core/asset/Door"/>
            </owl:Restriction>
        </rdfs:subClassOf>
        <rdfs:subClassOf>
            <owl:Restriction>
                <owl:onProperty rdf:resource="https://saref.etsi.org/core/consistsOf"/>
                <owl:someValuesFrom rdf:resource="https://ega.industry.com/ontologies/core/asset/PressureSensor"/>
            </owl:Restriction>
        </rdfs:subClassOf>
        <rdfs:subClassOf>
            <owl:Restriction>
                <owl:onProperty rdf:resource="https://saref.etsi.org/core/consistsOf"/>
                <owl:someValuesFrom rdf:resource="https://ega.industry.com/ontologies/core/asset/Tank"/>
            </owl:Restriction>
        </rdfs:subClassOf>
        <rdfs:subClassOf>
            <owl:Restriction>
                <owl:onProperty rdf:resource="https://saref.etsi.org/core/consistsOf"/>
                <owl:someValuesFrom rdf:resource="https://ega.industry.com/ontologies/core/asset/TemperatureSensor"/>
            </owl:Restriction>
        </rdfs:subClassOf>
        <rdfs:comment xml:lang="en">Primary aluminium processing unit that maintains and controls metal temperature and composition</rdfs:comment>
    </owl:Class>
    


    <!-- https://ega.industry.com/ontologies/core/asset/GasFlowSensor -->

    <owl:Class rdf:about="https://ega.industry.com/ontologies/core/asset/GasFlowSensor">
        <rdfs:subClassOf rdf:resource="https://saref.etsi.org/core/Sensor"/>
        <rdfs:comment xml:lang="en">Measurement Sensor device for Gas flow</rdfs:comment>
        <rdfs:label>Gas Flow Sensor</rdfs:label>
    </owl:Class>
    


    <!-- https://ega.industry.com/ontologies/core/asset/GasSupply -->

    <owl:Class rdf:about="https://ega.industry.com/ontologies/core/asset/GasSupply">
        <rdfs:subClassOf rdf:resource="https://saref.etsi.org/core/Device"/>
        <rdfs:subClassOf>
            <owl:Restriction>
                <owl:onProperty rdf:resource="https://saref.etsi.org/core/consistsOf"/>
                <owl:someValuesFrom rdf:resource="https://ega.industry.com/ontologies/core/asset/GasFlowSensor"/>
            </owl:Restriction>
        </rdfs:subClassOf>
        <rdfs:comment xml:lang="en">Device that delivers regulated gas to the burner for combustion</rdfs:comment>
        <rdfs:label>Gas Supply</rdfs:label>
    </owl:Class>
    


    <!-- https://ega.industry.com/ontologies/core/asset/IndustrySystem -->

    <owl:Class rdf:about="https://ega.industry.com/ontologies/core/asset/IndustrySystem">
        <rdfs:subClassOf rdf:resource="https://saref.etsi.org/saref4syst/System"/>
        <rdfs:comment>It&apos;s designed a group of Device of Feature of Interest which has an objective or functional around the activity of furnance</rdfs:comment>
    </owl:Class>
    


    <!-- https://ega.industry.com/ontologies/core/asset/Lining -->

    <owl:Class rdf:about="https://ega.industry.com/ontologies/core/asset/Lining">
        <rdfs:subClassOf rdf:resource="https://saref.etsi.org/core/Device"/>
        <rdfs:subClassOf>
            <owl:Restriction>
                <owl:onProperty rdf:resource="https://saref.etsi.org/core/consistsOf"/>
                <owl:someValuesFrom rdf:resource="https://ega.industry.com/ontologies/core/asset/CoolingSystem"/>
            </owl:Restriction>
        </rdfs:subClassOf>
        <rdfs:comment xml:lang="en">Refractory brick assembly that insulates the tank, protecting the structure and maintaining thermal efficiency</rdfs:comment>
    </owl:Class>
    


    <!-- https://ega.industry.com/ontologies/core/asset/Metals -->

    <owl:Class rdf:about="https://ega.industry.com/ontologies/core/asset/Metals">
        <rdfs:subClassOf rdf:resource="https://saref.etsi.org/saref4inma/MaterialBatch"/>
        <rdfs:comment xml:lang="en">Alloying elements added to aluminum to achieve specific chemical composition and physical properties in the final product</rdfs:comment>
    </owl:Class>
    


    <!-- https://ega.industry.com/ontologies/core/asset/OpenCloseFunction -->

    <owl:Class rdf:about="https://ega.industry.com/ontologies/core/asset/OpenCloseFunction">
        <rdfs:subClassOf rdf:resource="https://ega.industry.com/ontologies/core/asset/ActuatingFunction"/>
        <rdfs:subClassOf>
            <owl:Restriction>
                <owl:onProperty rdf:resource="https://saref.etsi.org/core/hasCommand"/>
                <owl:someValuesFrom rdf:resource="https://ega.industry.com/ontologies/core/asset/CloseCommand"/>
            </owl:Restriction>
        </rdfs:subClassOf>
        <rdfs:subClassOf>
            <owl:Restriction>
                <owl:onProperty rdf:resource="https://saref.etsi.org/core/hasCommand"/>
                <owl:someValuesFrom rdf:resource="https://ega.industry.com/ontologies/core/asset/OpenCommand"/>
            </owl:Restriction>
        </rdfs:subClassOf>
        <rdfs:comment>An actuating function that allows to open and close a device</rdfs:comment>
        <rdfs:label>Open Close Function</rdfs:label>
    </owl:Class>
    


    <!-- https://ega.industry.com/ontologies/core/asset/OpenCloseState -->

    <owl:Class rdf:about="https://ega.industry.com/ontologies/core/asset/OpenCloseState">
        <rdfs:subClassOf rdf:resource="https://saref.etsi.org/core/State"/>
        <rdfs:subClassOf>
            <owl:Restriction>
                <owl:onProperty rdf:resource="https://ega.industry.com/ontologies/core/asset/hasOpenReason"/>
                <owl:someValuesFrom rdf:resource="https://ega.industry.com/ontologies/core/asset/OpenReason"/>
            </owl:Restriction>
        </rdfs:subClassOf>
        <rdfs:subClassOf>
            <owl:Restriction>
                <owl:onProperty rdf:resource="https://saref.etsi.org/core/hasStateValue"/>
                <owl:someValuesFrom>
                    <owl:Class>
                        <owl:oneOf rdf:parseType="Collection">
                            <rdf:Description rdf:about="https://ega.industry.com/ontologies/core/asset/CLOSE"/>
                            <rdf:Description rdf:about="https://ega.industry.com/ontologies/core/asset/OPEN"/>
                        </owl:oneOf>
                    </owl:Class>
                </owl:someValuesFrom>
            </owl:Restriction>
        </rdfs:subClassOf>
    </owl:Class>
    


    <!-- https://ega.industry.com/ontologies/core/asset/OpenCloseStateValue -->

    <owl:Class rdf:about="https://ega.industry.com/ontologies/core/asset/OpenCloseStateValue">
        <owl:equivalentClass>
            <owl:Class>
                <owl:oneOf rdf:parseType="Collection">
                    <rdf:Description rdf:about="https://ega.industry.com/ontologies/core/asset/CLOSE"/>
                    <rdf:Description rdf:about="https://ega.industry.com/ontologies/core/asset/OPEN"/>
                </owl:oneOf>
            </owl:Class>
        </owl:equivalentClass>
        <rdfs:subClassOf rdf:resource="https://saref.etsi.org/core/StateValue"/>
        <rdfs:comment xml:lang="en">A controlled vocabulary representing the possible states of an open/close mechanism. Typical values include: OPEN and CLOSE.</rdfs:comment>
        <rdfs:label>Open Close State Value</rdfs:label>
    </owl:Class>
    


    <!-- https://ega.industry.com/ontologies/core/asset/OpenCommand -->

    <owl:Class rdf:about="https://ega.industry.com/ontologies/core/asset/OpenCommand">
        <rdfs:subClassOf rdf:resource="https://saref.etsi.org/core/Command"/>
        <rdfs:comment xml:lang="en">Represents a command to open a device</rdfs:comment>
        <rdfs:label>Open Command</rdfs:label>
    </owl:Class>
    


    <!-- https://ega.industry.com/ontologies/core/asset/OpenReason -->

    <owl:Class rdf:about="https://ega.industry.com/ontologies/core/asset/OpenReason">
        <owl:equivalentClass>
            <owl:Class>
                <owl:oneOf rdf:parseType="Collection">
                    <rdf:Description rdf:about="https://ega.industry.com/ontologies/core/asset/AlloyAddition"/>
                    <rdf:Description rdf:about="https://ega.industry.com/ontologies/core/asset/AluminiumCharging"/>
                    <rdf:Description rdf:about="https://ega.industry.com/ontologies/core/asset/Sampling"/>
                    <rdf:Description rdf:about="https://ega.industry.com/ontologies/core/asset/ScrapCharging"/>
                    <rdf:Description rdf:about="https://ega.industry.com/ontologies/core/asset/Skimming"/>
                    <rdf:Description rdf:about="https://ega.industry.com/ontologies/core/asset/Stirring"/>
                    <rdf:Description rdf:about="https://ega.industry.com/ontologies/core/asset/Unknown"/>
                </owl:oneOf>
            </owl:Class>
        </owl:equivalentClass>
        <rdfs:subClassOf rdf:resource="https://ega.industry.com/ontologies/core/asset/Reason"/>
        <rdfs:subClassOf>
            <owl:Restriction>
                <owl:onProperty rdf:resource="https://ega.industry.com/ontologies/core/data/hasTag"/>
                <owl:someValuesFrom rdf:resource="http://www.w3.org/2001/XMLSchema#string"/>
            </owl:Restriction>
        </rdfs:subClassOf>
        <rdfs:comment xml:lang="en">A subclass of &apos;Reason&apos; that specifies the causes for  openings. This includes enumerated reasons such as: Casting, Skimming, Sampling, Unknow, etc.. These reasons may relate to technical interventions, events, or manual actions.&quot; It&apos;s a controlled vocabulary representing opening reasons</rdfs:comment>
        <rdfs:label>Open Reason</rdfs:label>
    </owl:Class>
    


    <!-- https://ega.industry.com/ontologies/core/asset/OxygenSensor -->

    <owl:Class rdf:about="https://ega.industry.com/ontologies/core/asset/OxygenSensor">
        <rdfs:subClassOf rdf:resource="https://saref.etsi.org/core/Sensor"/>
        <rdfs:comment xml:lang="en">Measurement device for Oxygen</rdfs:comment>
        <rdfs:label>Oxygen Sensor</rdfs:label>
    </owl:Class>
    


    <!-- https://ega.industry.com/ontologies/core/asset/PowerSensor -->

    <owl:Class rdf:about="https://ega.industry.com/ontologies/core/asset/PowerSensor">
        <rdfs:subClassOf rdf:resource="https://saref.etsi.org/core/Sensor"/>
        <rdfs:comment xml:lang="en">Measurement device for Power</rdfs:comment>
        <rdfs:label>Power Sensor</rdfs:label>
    </owl:Class>
    


    <!-- https://ega.industry.com/ontologies/core/asset/PressureSensor -->

    <owl:Class rdf:about="https://ega.industry.com/ontologies/core/asset/PressureSensor">
        <rdfs:subClassOf rdf:resource="https://saref.etsi.org/core/Sensor"/>
        <rdfs:comment xml:lang="en">Measurement device for Pressure</rdfs:comment>
        <rdfs:label>Pressure Sensor</rdfs:label>
    </owl:Class>
    


    <!-- https://ega.industry.com/ontologies/core/asset/RawMaterialBatch -->

    <owl:Class rdf:about="https://ega.industry.com/ontologies/core/asset/RawMaterialBatch">
        <rdfs:subClassOf rdf:resource="https://saref.etsi.org/saref4inma/MaterialBatch"/>
        <rdfs:subClassOf>
            <owl:Restriction>
                <owl:onProperty rdf:resource="https://saref.etsi.org/saref4inma/consistsOfBatch"/>
                <owl:someValuesFrom rdf:resource="https://ega.industry.com/ontologies/core/asset/Aluminium"/>
            </owl:Restriction>
        </rdfs:subClassOf>
        <rdfs:subClassOf>
            <owl:Restriction>
                <owl:onProperty rdf:resource="https://saref.etsi.org/saref4inma/consistsOfBatch"/>
                <owl:someValuesFrom rdf:resource="https://ega.industry.com/ontologies/core/asset/Metals"/>
            </owl:Restriction>
        </rdfs:subClassOf>
        <rdfs:subClassOf>
            <owl:Restriction>
                <owl:onProperty rdf:resource="https://saref.etsi.org/saref4inma/consistsOfBatch"/>
                <owl:someValuesFrom rdf:resource="https://ega.industry.com/ontologies/core/asset/Scrap"/>
            </owl:Restriction>
        </rdfs:subClassOf>
        <rdfs:comment xml:lang="en">Specific raw material or elements used in creating a batch</rdfs:comment>
        <rdfs:label>Raw Material Batch</rdfs:label>
    </owl:Class>
    


    <!-- https://ega.industry.com/ontologies/core/asset/RawMaterialFeederSystem -->

    <owl:Class rdf:about="https://ega.industry.com/ontologies/core/asset/RawMaterialFeederSystem">
        <rdfs:subClassOf rdf:resource="https://ega.industry.com/ontologies/core/asset/IndustrySystem"/>
        <rdfs:comment>Delivery system for introducing aluminium and alloying elements into the furnace</rdfs:comment>
        <rdfs:label>Raw Material Feeder System</rdfs:label>
    </owl:Class>
    


    <!-- https://ega.industry.com/ontologies/core/asset/Reason -->

    <owl:Class rdf:about="https://ega.industry.com/ontologies/core/asset/Reason">
        <rdfs:subClassOf rdf:resource="http://www.w3.org/2004/02/skos/core#ConceptScheme"/>
        <rdfs:comment xml:lang="en">A general category representing various reasons related to actions or states within the system, such as door openings or security alerts.</rdfs:comment>
    </owl:Class>
    


    <!-- https://ega.industry.com/ontologies/core/asset/Scrap -->

    <owl:Class rdf:about="https://ega.industry.com/ontologies/core/asset/Scrap">
        <rdfs:subClassOf rdf:resource="https://saref.etsi.org/saref4inma/MaterialBatch"/>
        <rdfs:comment xml:lang="en">Recycled aluminium material reintroduced into the production process</rdfs:comment>
    </owl:Class>
    


    <!-- https://ega.industry.com/ontologies/core/asset/StartStopFunction -->

    <owl:Class rdf:about="https://ega.industry.com/ontologies/core/asset/StartStopFunction">
        <rdfs:subClassOf rdf:resource="https://ega.industry.com/ontologies/core/asset/ActuatingFunction"/>
        <rdfs:comment>An actuating function that allows to start and stop a device</rdfs:comment>
        <rdfs:label>Start Stop Function</rdfs:label>
    </owl:Class>
    


    <!-- https://ega.industry.com/ontologies/core/asset/Tank -->

    <owl:Class rdf:about="https://ega.industry.com/ontologies/core/asset/Tank">
        <rdfs:subClassOf rdf:resource="https://saref.etsi.org/core/Device"/>
        <rdfs:subClassOf>
            <owl:Restriction>
                <owl:onProperty rdf:resource="https://ega.industry.com/ontologies/core/asset/contains"/>
                <owl:someValuesFrom rdf:resource="https://ega.industry.com/ontologies/core/asset/RawMaterialBatch"/>
            </owl:Restriction>
        </rdfs:subClassOf>
        <rdfs:subClassOf>
            <owl:Restriction>
                <owl:onProperty rdf:resource="https://saref.etsi.org/core/consistsOf"/>
                <owl:someValuesFrom rdf:resource="https://ega.industry.com/ontologies/core/asset/Lining"/>
            </owl:Restriction>
        </rdfs:subClassOf>
        <rdfs:subClassOf>
            <owl:Restriction>
                <owl:onProperty rdf:resource="https://saref.etsi.org/core/consistsOf"/>
                <owl:someValuesFrom rdf:resource="https://ega.industry.com/ontologies/core/asset/TemperatureSensor"/>
            </owl:Restriction>
        </rdfs:subClassOf>
        <rdfs:comment xml:lang="en">Main vessel component that contains the molten aluminum during processing</rdfs:comment>
    </owl:Class>
    


    <!-- https://ega.industry.com/ontologies/core/asset/TemperatureSensor -->

    <owl:Class rdf:about="https://ega.industry.com/ontologies/core/asset/TemperatureSensor">
        <rdfs:subClassOf rdf:resource="https://saref.etsi.org/core/Sensor"/>
        <rdfs:comment xml:lang="en">Measurement device for temperature</rdfs:comment>
        <rdfs:label>Temperature Sensor</rdfs:label>
    </owl:Class>
    


    <!-- https://ega.industry.com/ontologies/core/data/DimensionlessProperty -->

    <owl:Class rdf:about="https://ega.industry.com/ontologies/core/data/DimensionlessProperty">
        <rdfs:subClassOf rdf:resource="https://saref.etsi.org/core/Property"/>
        <owl:disjointWith rdf:resource="https://ega.industry.com/ontologies/core/data/NumberUnit"/>
        <owl:disjointWith rdf:resource="https://ega.industry.com/ontologies/core/data/PercentUnit"/>
        <owl:disjointWith rdf:resource="https://ega.industry.com/ontologies/core/data/PowerUnit"/>
        <owl:disjointWith rdf:resource="https://ega.industry.com/ontologies/core/data/PressureUnit"/>
        <owl:disjointWith rdf:resource="https://ega.industry.com/ontologies/core/data/TemperatureUnit"/>
        <owl:disjointWith rdf:resource="https://ega.industry.com/ontologies/core/data/VolumeFlowRateUnit"/>
        <owl:disjointWith rdf:resource="https://saref.etsi.org/core/UnitOfMeasure"/>
        <rdfs:label>Dimensionless Property</rdfs:label>
    </owl:Class>
    


    <!-- https://ega.industry.com/ontologies/core/data/DimensionlessRatioProperty -->

    <owl:Class rdf:about="https://ega.industry.com/ontologies/core/data/DimensionlessRatioProperty">
        <rdfs:subClassOf rdf:resource="https://saref.etsi.org/core/Property"/>
        <owl:disjointWith rdf:resource="https://ega.industry.com/ontologies/core/data/NumberUnit"/>
        <owl:disjointWith rdf:resource="https://ega.industry.com/ontologies/core/data/PercentUnit"/>
        <owl:disjointWith rdf:resource="https://ega.industry.com/ontologies/core/data/PowerUnit"/>
        <owl:disjointWith rdf:resource="https://ega.industry.com/ontologies/core/data/PressureUnit"/>
        <owl:disjointWith rdf:resource="https://ega.industry.com/ontologies/core/data/TemperatureUnit"/>
        <owl:disjointWith rdf:resource="https://ega.industry.com/ontologies/core/data/VolumeFlowRateUnit"/>
        <owl:disjointWith rdf:resource="https://saref.etsi.org/core/UnitOfMeasure"/>
        <rdfs:label>Dimensionless Ratio Property</rdfs:label>
    </owl:Class>
    


    <!-- https://ega.industry.com/ontologies/core/data/ElectricCurrentProperty -->

    <owl:Class rdf:about="https://ega.industry.com/ontologies/core/data/ElectricCurrentProperty">
        <rdfs:subClassOf rdf:resource="https://saref.etsi.org/core/Property"/>
        <owl:disjointWith rdf:resource="https://ega.industry.com/ontologies/core/data/NumberUnit"/>
        <owl:disjointWith rdf:resource="https://ega.industry.com/ontologies/core/data/PercentUnit"/>
        <owl:disjointWith rdf:resource="https://ega.industry.com/ontologies/core/data/PowerUnit"/>
        <owl:disjointWith rdf:resource="https://ega.industry.com/ontologies/core/data/PressureUnit"/>
        <owl:disjointWith rdf:resource="https://ega.industry.com/ontologies/core/data/TemperatureUnit"/>
        <owl:disjointWith rdf:resource="https://ega.industry.com/ontologies/core/data/VolumeFlowRateUnit"/>
        <owl:disjointWith rdf:resource="https://saref.etsi.org/core/UnitOfMeasure"/>
        <rdfs:label>ElectricCurrent Property</rdfs:label>
    </owl:Class>
    


    <!-- https://ega.industry.com/ontologies/core/data/EventFunction -->

    <owl:Class rdf:about="https://ega.industry.com/ontologies/core/data/EventFunction">
        <rdfs:subClassOf rdf:resource="https://saref.etsi.org/core/Function"/>
        <rdfs:subClassOf>
            <owl:Restriction>
                <owl:onProperty rdf:resource="https://ega.industry.com/ontologies/core/data/hasSpecificState"/>
                <owl:minQualifiedCardinality rdf:datatype="http://www.w3.org/2001/XMLSchema#nonNegativeInteger">1</owl:minQualifiedCardinality>
                <owl:onClass rdf:resource="https://saref.etsi.org/core/State"/>
            </owl:Restriction>
        </rdfs:subClassOf>
        <rdfs:subClassOf>
            <owl:Restriction>
                <owl:onProperty rdf:resource="https://ega.industry.com/ontologies/core/data/hasThresholdPropertyValue"/>
                <owl:minQualifiedCardinality rdf:datatype="http://www.w3.org/2001/XMLSchema#nonNegativeInteger">1</owl:minQualifiedCardinality>
                <owl:onClass rdf:resource="https://saref.etsi.org/core/PropertyValue"/>
            </owl:Restriction>
        </rdfs:subClassOf>
        <rdfs:comment>A function that allows to notify about some relevant activity; e.g., that a certain threshold value has been exceeded, that some object has moved or the state of Object is changed</rdfs:comment>
    </owl:Class>
    


    <!-- https://ega.industry.com/ontologies/core/data/NumberUnit -->

    <owl:Class rdf:about="https://ega.industry.com/ontologies/core/data/NumberUnit">
        <rdfs:subClassOf rdf:resource="https://saref.etsi.org/core/UnitOfMeasure"/>
        <owl:disjointWith rdf:resource="https://ega.industry.com/ontologies/core/data/OxygenProperty"/>
        <owl:disjointWith rdf:resource="https://ega.industry.com/ontologies/core/data/PowerProperty"/>
        <owl:disjointWith rdf:resource="https://ega.industry.com/ontologies/core/data/PressureProperty"/>
        <owl:disjointWith rdf:resource="https://ega.industry.com/ontologies/core/data/SpeedProperty"/>
        <owl:disjointWith rdf:resource="https://ega.industry.com/ontologies/core/data/TemperatureProperty"/>
        <owl:disjointWith rdf:resource="https://ega.industry.com/ontologies/core/data/VolumeFlowRateProperty"/>
        <owl:disjointWith rdf:resource="https://saref.etsi.org/core/Property"/>
        <owl:disjointWith rdf:resource="https://saref.etsi.org/saref4inma/Size"/>
        <rdfs:label>Number Unit</rdfs:label>
    </owl:Class>
    


    <!-- https://ega.industry.com/ontologies/core/data/OxygenProperty -->

    <owl:Class rdf:about="https://ega.industry.com/ontologies/core/data/OxygenProperty">
        <rdfs:subClassOf rdf:resource="https://saref.etsi.org/core/Property"/>
        <owl:disjointWith rdf:resource="https://ega.industry.com/ontologies/core/data/PercentUnit"/>
        <owl:disjointWith rdf:resource="https://ega.industry.com/ontologies/core/data/PowerUnit"/>
        <owl:disjointWith rdf:resource="https://ega.industry.com/ontologies/core/data/PressureUnit"/>
        <owl:disjointWith rdf:resource="https://ega.industry.com/ontologies/core/data/TemperatureUnit"/>
        <owl:disjointWith rdf:resource="https://ega.industry.com/ontologies/core/data/VolumeFlowRateUnit"/>
        <owl:disjointWith rdf:resource="https://saref.etsi.org/core/UnitOfMeasure"/>
        <rdfs:label>Oxygen Property</rdfs:label>
    </owl:Class>
    


    <!-- https://ega.industry.com/ontologies/core/data/PercentUnit -->

    <owl:Class rdf:about="https://ega.industry.com/ontologies/core/data/PercentUnit">
        <rdfs:subClassOf rdf:resource="https://saref.etsi.org/core/UnitOfMeasure"/>
        <owl:disjointWith rdf:resource="https://ega.industry.com/ontologies/core/data/PowerProperty"/>
        <owl:disjointWith rdf:resource="https://ega.industry.com/ontologies/core/data/PressureProperty"/>
        <owl:disjointWith rdf:resource="https://ega.industry.com/ontologies/core/data/SpeedProperty"/>
        <owl:disjointWith rdf:resource="https://ega.industry.com/ontologies/core/data/TemperatureProperty"/>
        <owl:disjointWith rdf:resource="https://ega.industry.com/ontologies/core/data/VolumeFlowRateProperty"/>
        <owl:disjointWith rdf:resource="https://saref.etsi.org/core/Property"/>
        <owl:disjointWith rdf:resource="https://saref.etsi.org/saref4inma/Size"/>
        <rdfs:label>Percent Unit</rdfs:label>
    </owl:Class>
    


    <!-- https://ega.industry.com/ontologies/core/data/PowerProperty -->

    <owl:Class rdf:about="https://ega.industry.com/ontologies/core/data/PowerProperty">
        <rdfs:subClassOf rdf:resource="https://saref.etsi.org/core/Property"/>
        <owl:disjointWith rdf:resource="https://ega.industry.com/ontologies/core/data/PowerUnit"/>
        <owl:disjointWith rdf:resource="https://ega.industry.com/ontologies/core/data/PressureUnit"/>
        <owl:disjointWith rdf:resource="https://ega.industry.com/ontologies/core/data/TemperatureUnit"/>
        <owl:disjointWith rdf:resource="https://ega.industry.com/ontologies/core/data/VolumeFlowRateUnit"/>
        <owl:disjointWith rdf:resource="https://saref.etsi.org/core/UnitOfMeasure"/>
        <rdfs:label>Power Property</rdfs:label>
    </owl:Class>
    


    <!-- https://ega.industry.com/ontologies/core/data/PowerUnit -->

    <owl:Class rdf:about="https://ega.industry.com/ontologies/core/data/PowerUnit">
        <rdfs:subClassOf rdf:resource="https://saref.etsi.org/core/UnitOfMeasure"/>
        <owl:disjointWith rdf:resource="https://ega.industry.com/ontologies/core/data/PressureProperty"/>
        <owl:disjointWith rdf:resource="https://ega.industry.com/ontologies/core/data/SpeedProperty"/>
        <owl:disjointWith rdf:resource="https://ega.industry.com/ontologies/core/data/TemperatureProperty"/>
        <owl:disjointWith rdf:resource="https://ega.industry.com/ontologies/core/data/VolumeFlowRateProperty"/>
        <owl:disjointWith rdf:resource="https://saref.etsi.org/core/Property"/>
        <owl:disjointWith rdf:resource="https://saref.etsi.org/saref4inma/Size"/>
        <rdfs:label>Power Unit</rdfs:label>
    </owl:Class>
    


    <!-- https://ega.industry.com/ontologies/core/data/PressureProperty -->

    <owl:Class rdf:about="https://ega.industry.com/ontologies/core/data/PressureProperty">
        <rdfs:subClassOf rdf:resource="https://saref.etsi.org/core/Property"/>
        <owl:disjointWith rdf:resource="https://ega.industry.com/ontologies/core/data/PressureUnit"/>
        <owl:disjointWith rdf:resource="https://ega.industry.com/ontologies/core/data/TemperatureUnit"/>
        <owl:disjointWith rdf:resource="https://ega.industry.com/ontologies/core/data/VolumeFlowRateUnit"/>
        <owl:disjointWith rdf:resource="https://saref.etsi.org/core/UnitOfMeasure"/>
        <rdfs:label>Pressure Property</rdfs:label>
    </owl:Class>
    


    <!-- https://ega.industry.com/ontologies/core/data/PressureUnit -->

    <owl:Class rdf:about="https://ega.industry.com/ontologies/core/data/PressureUnit">
        <rdfs:subClassOf rdf:resource="https://saref.etsi.org/core/UnitOfMeasure"/>
        <owl:disjointWith rdf:resource="https://ega.industry.com/ontologies/core/data/SpeedProperty"/>
        <owl:disjointWith rdf:resource="https://ega.industry.com/ontologies/core/data/TemperatureProperty"/>
        <owl:disjointWith rdf:resource="https://ega.industry.com/ontologies/core/data/VolumeFlowRateProperty"/>
        <owl:disjointWith rdf:resource="https://saref.etsi.org/core/Property"/>
        <owl:disjointWith rdf:resource="https://saref.etsi.org/saref4inma/Size"/>
        <rdfs:label>Pressure Unit</rdfs:label>
    </owl:Class>
    


    <!-- https://ega.industry.com/ontologies/core/data/SpeedProperty -->

    <owl:Class rdf:about="https://ega.industry.com/ontologies/core/data/SpeedProperty">
        <rdfs:subClassOf rdf:resource="https://saref.etsi.org/core/Property"/>
        <owl:disjointWith rdf:resource="https://ega.industry.com/ontologies/core/data/TemperatureUnit"/>
        <owl:disjointWith rdf:resource="https://ega.industry.com/ontologies/core/data/VolumeFlowRateUnit"/>
        <owl:disjointWith rdf:resource="https://saref.etsi.org/core/UnitOfMeasure"/>
        <rdfs:label>Speed Property</rdfs:label>
    </owl:Class>
    


    <!-- https://ega.industry.com/ontologies/core/data/TemperatureProperty -->

    <owl:Class rdf:about="https://ega.industry.com/ontologies/core/data/TemperatureProperty">
        <rdfs:subClassOf rdf:resource="https://saref.etsi.org/core/Property"/>
        <owl:disjointWith rdf:resource="https://ega.industry.com/ontologies/core/data/TemperatureUnit"/>
        <owl:disjointWith rdf:resource="https://ega.industry.com/ontologies/core/data/VolumeFlowRateUnit"/>
        <owl:disjointWith rdf:resource="https://saref.etsi.org/core/UnitOfMeasure"/>
        <rdfs:label>Temperature Property</rdfs:label>
    </owl:Class>
    


    <!-- https://ega.industry.com/ontologies/core/data/TemperatureUnit -->

    <owl:Class rdf:about="https://ega.industry.com/ontologies/core/data/TemperatureUnit">
        <rdfs:subClassOf rdf:resource="https://saref.etsi.org/core/UnitOfMeasure"/>
        <owl:disjointWith rdf:resource="https://ega.industry.com/ontologies/core/data/VolumeFlowRateProperty"/>
        <owl:disjointWith rdf:resource="https://saref.etsi.org/core/Property"/>
        <owl:disjointWith rdf:resource="https://saref.etsi.org/saref4inma/Size"/>
        <rdfs:label>Temperature Unit</rdfs:label>
    </owl:Class>
    


    <!-- https://ega.industry.com/ontologies/core/data/VolumeFlowRateProperty -->

    <owl:Class rdf:about="https://ega.industry.com/ontologies/core/data/VolumeFlowRateProperty">
        <rdfs:subClassOf rdf:resource="https://saref.etsi.org/core/Property"/>
        <owl:disjointWith rdf:resource="https://ega.industry.com/ontologies/core/data/VolumeFlowRateUnit"/>
        <owl:disjointWith rdf:resource="https://saref.etsi.org/core/UnitOfMeasure"/>
        <terms:description>Volumetric Flow Rate, (also known as volume flow rate, rate of fluid flow or volume velocity) is the volume of fluid which passes through a given surface per unit time.</terms:description>
        <rdfs:label>Volume Flow Rate Property</rdfs:label>
    </owl:Class>
    


    <!-- https://ega.industry.com/ontologies/core/data/VolumeFlowRateUnit -->

    <owl:Class rdf:about="https://ega.industry.com/ontologies/core/data/VolumeFlowRateUnit">
        <rdfs:subClassOf rdf:resource="https://saref.etsi.org/core/UnitOfMeasure"/>
        <owl:disjointWith rdf:resource="https://saref.etsi.org/core/Property"/>
        <owl:disjointWith rdf:resource="https://saref.etsi.org/saref4inma/Size"/>
        <rdfs:label>Volume Flow Rate Unit</rdfs:label>
    </owl:Class>
    


    <!-- https://ega.industry.com/ontologies/core/process/Condition -->

    <owl:Class rdf:about="https://ega.industry.com/ontologies/core/process/Condition">
        <rdfs:subClassOf>
            <owl:Restriction>
                <owl:onProperty rdf:resource="https://ega.industry.com/ontologies/core/process/isTriggeredBy"/>
                <owl:someValuesFrom rdf:resource="https://ega.industry.com/ontologies/core/data/EventFunction"/>
            </owl:Restriction>
        </rdfs:subClassOf>
        <rdfs:subClassOf>
            <owl:Restriction>
                <owl:onProperty rdf:resource="https://ega.industry.com/ontologies/core/process/conditionAchieved"/>
                <owl:someValuesFrom rdf:resource="http://www.w3.org/2001/XMLSchema#boolean"/>
            </owl:Restriction>
        </rdfs:subClassOf>
        <rdfs:comment xml:lang="en">A condition holds the result of a logical expression thanks to data property conditionAchieved. This result is a boolean value. Logical expression is computed by an EventFunction individual.</rdfs:comment>
        <rdfs:label>Condition</rdfs:label>
    </owl:Class>
    


    <!-- https://ega.industry.com/ontologies/core/process/ConditionalSubProcess -->

    <owl:Class rdf:about="https://ega.industry.com/ontologies/core/process/ConditionalSubProcess">
        <rdfs:subClassOf rdf:resource="https://ega.industry.com/ontologies/core/process/SubProcess"/>
        <rdfs:subClassOf>
            <owl:Restriction>
                <owl:onProperty rdf:resource="https://ega.industry.com/ontologies/core/process/pathDependsOnStep"/>
                <owl:someValuesFrom rdf:resource="https://ega.industry.com/ontologies/core/process/IterativeStep"/>
            </owl:Restriction>
        </rdfs:subClassOf>
        <owl:disjointWith rdf:resource="https://ega.industry.com/ontologies/core/process/SequentialSubProcess"/>
    </owl:Class>
    


    <!-- https://ega.industry.com/ontologies/core/process/IterativeStep -->

    <owl:Class rdf:about="https://ega.industry.com/ontologies/core/process/IterativeStep">
        <rdfs:subClassOf rdf:resource="https://ega.industry.com/ontologies/core/process/Step"/>
        <rdfs:subClassOf>
            <owl:Restriction>
                <owl:onProperty rdf:resource="https://ega.industry.com/ontologies/core/process/isIterationCompleted"/>
                <owl:someValuesFrom rdf:resource="http://www.w3.org/2001/XMLSchema#boolean"/>
            </owl:Restriction>
        </rdfs:subClassOf>
        <rdfs:subClassOf>
            <owl:Restriction>
                <owl:onProperty rdf:resource="https://ega.industry.com/ontologies/core/process/iterationCount"/>
                <owl:qualifiedCardinality rdf:datatype="http://www.w3.org/2001/XMLSchema#nonNegativeInteger">1</owl:qualifiedCardinality>
                <owl:onDataRange rdf:resource="http://www.w3.org/2001/XMLSchema#integer"/>
            </owl:Restriction>
        </rdfs:subClassOf>
        <owl:disjointWith rdf:resource="https://ega.industry.com/ontologies/core/process/NormalStep"/>
        <rdfs:comment xml:lang="en">it is a Step that implements the notion of a condition based loop, a step that manage a loop</rdfs:comment>
    </owl:Class>
    


    <!-- https://ega.industry.com/ontologies/core/process/NormalStep -->

    <owl:Class rdf:about="https://ega.industry.com/ontologies/core/process/NormalStep">
        <rdfs:subClassOf rdf:resource="https://ega.industry.com/ontologies/core/process/Step"/>
        <rdfs:comment xml:lang="en">It&apos;s a Step without loop concept</rdfs:comment>
    </owl:Class>
    


    <!-- https://ega.industry.com/ontologies/core/process/Process -->

    <owl:Class rdf:about="https://ega.industry.com/ontologies/core/process/Process">
        <rdfs:subClassOf>
            <owl:Restriction>
                <owl:onProperty rdf:resource="https://ega.industry.com/ontologies/core/process/hasSubProcess"/>
                <owl:someValuesFrom rdf:resource="https://ega.industry.com/ontologies/core/process/SubProcess"/>
            </owl:Restriction>
        </rdfs:subClassOf>
        <rdfs:subClassOf>
            <owl:Restriction>
                <owl:onProperty rdf:resource="https://ega.industry.com/ontologies/core/process/hasAlloyCode"/>
                <owl:someValuesFrom rdf:resource="http://www.w3.org/2001/XMLSchema#integer"/>
            </owl:Restriction>
        </rdfs:subClassOf>
        <rdfs:subClassOf>
            <owl:Restriction>
                <owl:onProperty rdf:resource="https://ega.industry.com/ontologies/core/process/hasAlloyCodeId"/>
                <owl:someValuesFrom rdf:resource="http://www.w3.org/2001/XMLSchema#integer"/>
            </owl:Restriction>
        </rdfs:subClassOf>
        <rdfs:subClassOf>
            <owl:Restriction>
                <owl:onProperty rdf:resource="https://ega.industry.com/ontologies/core/process/hasBatchId"/>
                <owl:someValuesFrom rdf:resource="http://www.w3.org/2001/XMLSchema#integer"/>
            </owl:Restriction>
        </rdfs:subClassOf>
        <rdfs:subClassOf>
            <owl:Restriction>
                <owl:onProperty rdf:resource="https://ega.industry.com/ontologies/core/process/hasBatchNo"/>
                <owl:someValuesFrom rdf:resource="http://www.w3.org/2001/XMLSchema#string"/>
            </owl:Restriction>
        </rdfs:subClassOf>
        <rdfs:subClassOf>
            <owl:Restriction>
                <owl:onProperty rdf:resource="https://ega.industry.com/ontologies/core/process/hasEndTimestamp"/>
                <owl:someValuesFrom rdf:resource="http://www.w3.org/2001/XMLSchema#dateTime"/>
            </owl:Restriction>
        </rdfs:subClassOf>
        <rdfs:subClassOf>
            <owl:Restriction>
                <owl:onProperty rdf:resource="https://ega.industry.com/ontologies/core/process/hasStartTimestamp"/>
                <owl:someValuesFrom rdf:resource="http://www.w3.org/2001/XMLSchema#dateTime"/>
            </owl:Restriction>
        </rdfs:subClassOf>
        <rdfs:subClassOf>
            <owl:Restriction>
                <owl:onProperty rdf:resource="https://ega.industry.com/ontologies/core/process/isRunning"/>
                <owl:someValuesFrom rdf:resource="http://www.w3.org/2001/XMLSchema#boolean"/>
            </owl:Restriction>
        </rdfs:subClassOf>
        <rdfs:comment>Represents a complete Process.</rdfs:comment>
    </owl:Class>
    


    <!-- https://ega.industry.com/ontologies/core/process/SequentialSubProcess -->

    <owl:Class rdf:about="https://ega.industry.com/ontologies/core/process/SequentialSubProcess">
        <rdfs:subClassOf rdf:resource="https://ega.industry.com/ontologies/core/process/SubProcess"/>
    </owl:Class>
    


    <!-- https://ega.industry.com/ontologies/core/process/Step -->

    <owl:Class rdf:about="https://ega.industry.com/ontologies/core/process/Step">
        <rdfs:subClassOf>
            <owl:Restriction>
                <owl:onProperty rdf:resource="https://ega.industry.com/ontologies/core/process/hasCondition"/>
                <owl:someValuesFrom rdf:resource="https://ega.industry.com/ontologies/core/process/Condition"/>
            </owl:Restriction>
        </rdfs:subClassOf>
        <rdfs:subClassOf>
            <owl:Restriction>
                <owl:onProperty rdf:resource="https://ega.industry.com/ontologies/core/process/hasNextStep"/>
                <owl:someValuesFrom rdf:resource="https://ega.industry.com/ontologies/core/process/Step"/>
            </owl:Restriction>
        </rdfs:subClassOf>
        <rdfs:subClassOf>
            <owl:Restriction>
                <owl:onProperty rdf:resource="https://ega.industry.com/ontologies/core/process/hasStepType"/>
                <owl:someValuesFrom rdf:resource="https://ega.industry.com/ontologies/core/process/StepType"/>
            </owl:Restriction>
        </rdfs:subClassOf>
        <rdfs:subClassOf>
            <owl:Restriction>
                <owl:onProperty rdf:resource="https://ega.industry.com/ontologies/core/process/isStepOf"/>
                <owl:someValuesFrom rdf:resource="https://ega.industry.com/ontologies/core/process/SubProcess"/>
            </owl:Restriction>
        </rdfs:subClassOf>
        <rdfs:subClassOf>
            <owl:Restriction>
                <owl:onProperty rdf:resource="https://ega.industry.com/ontologies/core/process/hasEndTimestamp"/>
                <owl:someValuesFrom rdf:resource="http://www.w3.org/2001/XMLSchema#dateTime"/>
            </owl:Restriction>
        </rdfs:subClassOf>
        <rdfs:subClassOf>
            <owl:Restriction>
                <owl:onProperty rdf:resource="https://ega.industry.com/ontologies/core/process/hasStartTimestamp"/>
                <owl:someValuesFrom rdf:resource="http://www.w3.org/2001/XMLSchema#dateTime"/>
            </owl:Restriction>
        </rdfs:subClassOf>
        <rdfs:subClassOf>
            <owl:Restriction>
                <owl:onProperty rdf:resource="https://ega.industry.com/ontologies/core/process/hasStepId"/>
                <owl:someValuesFrom rdf:resource="http://www.w3.org/2001/XMLSchema#integer"/>
            </owl:Restriction>
        </rdfs:subClassOf>
        <rdfs:subClassOf>
            <owl:Restriction>
                <owl:onProperty rdf:resource="https://ega.industry.com/ontologies/core/process/isCurrentStep"/>
                <owl:someValuesFrom rdf:resource="http://www.w3.org/2001/XMLSchema#boolean"/>
            </owl:Restriction>
        </rdfs:subClassOf>
        <rdfs:comment>Atomic action unit of a process</rdfs:comment>
    </owl:Class>
    


    <!-- https://ega.industry.com/ontologies/core/process/StepType -->

    <owl:Class rdf:about="https://ega.industry.com/ontologies/core/process/StepType">
        <owl:equivalentClass>
            <owl:Class>
                <owl:oneOf rdf:parseType="Collection">
                    <rdf:Description rdf:about="https://ega.industry.com/ontologies/core/process/Machine"/>
                    <rdf:Description rdf:about="https://ega.industry.com/ontologies/core/process/Operator"/>
                </owl:oneOf>
            </owl:Class>
        </owl:equivalentClass>
        <rdfs:comment xml:lang="en">Classification of the type of action performed in a step</rdfs:comment>
    </owl:Class>
    


    <!-- https://ega.industry.com/ontologies/core/process/SubProcess -->

    <owl:Class rdf:about="https://ega.industry.com/ontologies/core/process/SubProcess">
        <rdfs:subClassOf>
            <owl:Restriction>
                <owl:onProperty rdf:resource="https://ega.industry.com/ontologies/core/process/hasEndStep"/>
                <owl:someValuesFrom rdf:resource="https://ega.industry.com/ontologies/core/process/Step"/>
            </owl:Restriction>
        </rdfs:subClassOf>
        <rdfs:subClassOf>
            <owl:Restriction>
                <owl:onProperty rdf:resource="https://ega.industry.com/ontologies/core/process/hasStartStep"/>
                <owl:someValuesFrom rdf:resource="https://ega.industry.com/ontologies/core/process/Step"/>
            </owl:Restriction>
        </rdfs:subClassOf>
        <rdfs:subClassOf>
            <owl:Restriction>
                <owl:onProperty rdf:resource="https://ega.industry.com/ontologies/core/process/hasStep"/>
                <owl:someValuesFrom rdf:resource="https://ega.industry.com/ontologies/core/process/Step"/>
            </owl:Restriction>
        </rdfs:subClassOf>
        <rdfs:subClassOf>
            <owl:Restriction>
                <owl:onProperty rdf:resource="https://ega.industry.com/ontologies/core/process/hasEndTimestamp"/>
                <owl:someValuesFrom rdf:resource="http://www.w3.org/2001/XMLSchema#dateTime"/>
            </owl:Restriction>
        </rdfs:subClassOf>
        <rdfs:subClassOf>
            <owl:Restriction>
                <owl:onProperty rdf:resource="https://ega.industry.com/ontologies/core/process/hasStartTimestamp"/>
                <owl:someValuesFrom rdf:resource="http://www.w3.org/2001/XMLSchema#dateTime"/>
            </owl:Restriction>
        </rdfs:subClassOf>
        <rdfs:subClassOf>
            <owl:Restriction>
                <owl:onProperty rdf:resource="https://ega.industry.com/ontologies/core/process/hasSubProcessId"/>
                <owl:someValuesFrom rdf:resource="http://www.w3.org/2001/XMLSchema#integer"/>
            </owl:Restriction>
        </rdfs:subClassOf>
        <rdfs:subClassOf>
            <owl:Restriction>
                <owl:onProperty rdf:resource="https://ega.industry.com/ontologies/core/process/isCurrentSubProcess"/>
                <owl:someValuesFrom rdf:resource="http://www.w3.org/2001/XMLSchema#boolean"/>
            </owl:Restriction>
        </rdfs:subClassOf>
        <rdfs:comment>a Logical grouping of related steps of process</rdfs:comment>
        <rdfs:label>SubProcess</rdfs:label>
    </owl:Class>
    


    <!-- https://saref.etsi.org/core/Actuation -->

    <owl:Class rdf:about="https://saref.etsi.org/core/Actuation">
        <rdfs:subClassOf rdf:resource="https://saref.etsi.org/core/ProcedureExecution"/>
        <rdfs:subClassOf>
            <owl:Restriction>
                <owl:onProperty rdf:resource="https://saref.etsi.org/core/madeBy"/>
                <owl:allValuesFrom rdf:resource="https://saref.etsi.org/core/Actuator"/>
            </owl:Restriction>
        </rdfs:subClassOf>
        <rdfs:subClassOf>
            <owl:Restriction>
                <owl:onProperty rdf:resource="https://saref.etsi.org/core/controls"/>
                <owl:minCardinality rdf:datatype="http://www.w3.org/2001/XMLSchema#nonNegativeInteger">1</owl:minCardinality>
            </owl:Restriction>
        </rdfs:subClassOf>
        <rdfs:comment xml:lang="en">A saref:Actuation is the act of carrying out a procedure to control the state of the world using an actuator. It links to an actuator to describe what made the actuation, and to the controlled feature, property, property of interest, state, or state of interest. Typically, its input is a property value or a state. An actuation of a state (OP saref:controls) should have a state as input (OP saref:hasInput). Respectively, an actuation of a property should have a property value as input.</rdfs:comment>
        <rdfs:label xml:lang="en">Actuation</rdfs:label>
    </owl:Class>
    


    <!-- https://saref.etsi.org/core/Actuator -->

    <owl:Class rdf:about="https://saref.etsi.org/core/Actuator">
        <rdfs:subClassOf rdf:resource="https://saref.etsi.org/core/Device"/>
        <rdfs:subClassOf>
            <owl:Restriction>
                <owl:onProperty rdf:resource="https://saref.etsi.org/core/controls"/>
                <owl:minCardinality rdf:datatype="http://www.w3.org/2001/XMLSchema#nonNegativeInteger">1</owl:minCardinality>
            </owl:Restriction>
        </rdfs:subClassOf>
        <rdfs:comment xml:lang="en">A device designed to control one or more properties or states of one or more features of interest.</rdfs:comment>
        <rdfs:label xml:lang="en">Actuator</rdfs:label>
        <skos:historyNote xml:lang="en">V3.2.1: Definition of Actuator is simplified and grounded on saref:controls. Local restriction on saref:hasFunction is deleted.</skos:historyNote>
    </owl:Class>
    


    <!-- https://saref.etsi.org/core/Appliance -->

    <owl:Class rdf:about="https://saref.etsi.org/core/Appliance">
        <rdfs:subClassOf rdf:resource="https://saref.etsi.org/core/Device"/>
        <rdfs:comment xml:lang="en">A device designed to accomplish a particular task for occupant use. It consumes, produces, or stores, some commodity.</rdfs:comment>
        <rdfs:label xml:lang="en">Appliance</rdfs:label>
        <skos:historyNote xml:lang="en">V3.2.1: Definition of saref:Appliance is grounded on tasks and commodities.</skos:historyNote>
    </owl:Class>
    


    <!-- https://saref.etsi.org/core/Command -->

    <owl:Class rdf:about="https://saref.etsi.org/core/Command">
        <rdfs:subClassOf>
            <owl:Restriction>
                <owl:onProperty rdf:resource="http://www.w3.org/2004/02/skos/core#broader"/>
                <owl:allValuesFrom rdf:resource="https://saref.etsi.org/core/Command"/>
            </owl:Restriction>
        </rdfs:subClassOf>
        <rdfs:subClassOf>
            <owl:Restriction>
                <owl:onProperty rdf:resource="http://www.w3.org/2004/02/skos/core#narrower"/>
                <owl:allValuesFrom rdf:resource="https://saref.etsi.org/core/Command"/>
            </owl:Restriction>
        </rdfs:subClassOf>
        <rdfs:comment xml:lang="en">The lowest-level directives a function exposes to some network. Commands can target (OP saref:targets and its sub-properties) features, properties, or states. An instance of saref:Command is independent of any device.</rdfs:comment>
        <rdfs:label xml:lang="en">Command</rdfs:label>
        <skos:example xml:lang="en">Observe property, control property, observe state, control state, invoke action, cancel action, turn on or off, change color, subscribe, publish, etc. are all commands.</skos:example>
        <skos:historyNote xml:lang="en">V3.2.1: Simplified definition and axiomatization of saref:Command. Added examples.</skos:historyNote>
    </owl:Class>
    


    <!-- https://saref.etsi.org/core/CommandExecution -->

    <owl:Class rdf:about="https://saref.etsi.org/core/CommandExecution">
        <rdfs:subClassOf rdf:resource="https://saref.etsi.org/core/ProcedureExecution"/>
        <rdfs:subClassOf>
            <owl:Restriction>
                <owl:onProperty rdf:resource="https://saref.etsi.org/core/isExecutionOf"/>
                <owl:allValuesFrom>
                    <owl:Class>
                        <owl:unionOf rdf:parseType="Collection">
                            <rdf:Description rdf:about="https://saref.etsi.org/core/Command"/>
                            <rdf:Description rdf:about="https://saref.etsi.org/core/CommandOfInterest"/>
                        </owl:unionOf>
                    </owl:Class>
                </owl:allValuesFrom>
            </owl:Restriction>
        </rdfs:subClassOf>
        <rdfs:comment xml:lang="en">Describes the execution of a command. Typically, its inputs and outputs are human understandable and relate to some feature of interest, such as its state (e.g., s4abcd:On), or the value of its temperature (e.g., property value 21.0 C).</rdfs:comment>
        <rdfs:label xml:lang="en">Command Execution</rdfs:label>
    </owl:Class>
    


    <!-- https://saref.etsi.org/core/CommandOfInterest -->

    <owl:Class rdf:about="https://saref.etsi.org/core/CommandOfInterest">
        <rdfs:subClassOf>
            <owl:Restriction>
                <owl:onProperty rdf:resource="https://saref.etsi.org/core/isCommandOfInterestOf"/>
                <owl:cardinality rdf:datatype="http://www.w3.org/2001/XMLSchema#nonNegativeInteger">1</owl:cardinality>
            </owl:Restriction>
        </rdfs:subClassOf>
        <rdfs:comment xml:lang="en">The lowest-level directives a device supports and exposes to some network. Commands can target (OP saref:targets and its sub-properties) features, properties, or states. A saref:CommandOfInterest is a directives actually supported by a device and exposed to some network.</rdfs:comment>
        <rdfs:label xml:lang="en">Command Of Interest</rdfs:label>
        <skos:example xml:lang="en">The corridor smart light switch supports a command of kind turn on/off, which controls the state of the outdoor light.</skos:example>
        <skos:example xml:lang="en">The smart fridge supports a command of kind observe temperature, which observes the temperature of the fridge.</skos:example>
        <skos:historyNote xml:lang="en">V3.2.1: Introduced saref:CommandOfInterest, parallel to saref:PropertyOfInterest.</skos:historyNote>
        <skos:note xml:lang="en">Commands of interest need not always be explicited. It depends on the use case. Typically, commands of interest are useful to specify the actual property of interest or state of interest that is expected as input parameter, output, or that will be targeted.</skos:note>
        <skos:note xml:lang="en">Like for commands, commands of interest may be described in terms of their input parameters, outputs, and which properties or states they target.</skos:note>
    </owl:Class>
    


    <!-- https://saref.etsi.org/core/Commodity -->

    <owl:Class rdf:about="https://saref.etsi.org/core/Commodity">
        <rdfs:subClassOf>
            <owl:Restriction>
                <owl:onProperty rdf:resource="http://www.w3.org/2004/02/skos/core#broader"/>
                <owl:allValuesFrom rdf:resource="https://saref.etsi.org/core/Commodity"/>
            </owl:Restriction>
        </rdfs:subClassOf>
        <rdfs:subClassOf>
            <owl:Restriction>
                <owl:onProperty rdf:resource="http://www.w3.org/2004/02/skos/core#narrower"/>
                <owl:allValuesFrom rdf:resource="https://saref.etsi.org/core/Commodity"/>
            </owl:Restriction>
        </rdfs:subClassOf>
        <rdfs:comment xml:lang="en">A marketable item which may be supplied without qualitative differentiation.</rdfs:comment>
        <rdfs:label xml:lang="en">Commodity</rdfs:label>
        <skos:historyNote xml:lang="en">V3.2.1: Definition of saref:Commodity is simplified.</skos:historyNote>
        <skos:historyNote xml:lang="en">V4.1.1: Removed examples of commodity categories.</skos:historyNote>
        <skos:note xml:lang="en">Concepts from existing code lists, vocabularies, and taxonomies, may be used as instances of saref:Commodity, for example from the ISDA taxonomy of commodities, the Standard International Energy product Classification (SIEC), the IRENA Energy Taxonomy or Wikidata.</skos:note>
        <skos:note xml:lang="en">SAREF refers to energy commodities such as electricity, gas, coal and oil.</skos:note>
    </owl:Class>
    


    <!-- https://saref.etsi.org/core/Device -->

    <owl:Class rdf:about="https://saref.etsi.org/core/Device">
        <rdfs:subClassOf rdf:resource="https://saref.etsi.org/core/FeatureOfInterest"/>
        <rdfs:subClassOf rdf:resource="https://saref.etsi.org/saref4syst/System"/>
        <rdfs:comment xml:lang="en">A tangible object designed to accomplish a particular task. In order to accomplish this task, the device performs one or more functions. An instance of saref:Device represents one specific real world entity.</rdfs:comment>
        <rdfs:comment>A tangible object designed to accomplish a particular task. In order to accomplish this task, the device performs one or more functions. For example, a washing machine is designed to wash (task) and to accomplish this task it performs a start and stop function.</rdfs:comment>
        <rdfs:label xml:lang="en">Device</rdfs:label>
        <skos:example xml:lang="en">Examples of devices are a light switch, a temperature sensor, an energy meter, a water flow meter, and a laundry dryer. A laundry dryer is designed to dry laundry, and to accomplish this task it has a start/stop function.</skos:example>
        <skos:example xml:lang="en">For example, a washing machine is designed to wash (task) and to accomplish this task it performs a start and stop function.</skos:example>
        <skos:historyNote xml:lang="en">V3.2.1: Most axioms on saref:Device were useless and have been deleted.</skos:historyNote>
        <skos:historyNote xml:lang="en">V3.2.1: definition of saref:Device clarifies it&apos;s a real world entity.</skos:historyNote>
        <skos:historyNote xml:lang="en">V3.2.1: saref:Device is explicitly a subclass of saref:FeatureOfInterest and s4syst:System.</skos:historyNote>
    </owl:Class>
    


    <!-- https://saref.etsi.org/core/DeviceKind -->

    <owl:Class rdf:about="https://saref.etsi.org/core/DeviceKind">
        <rdfs:subClassOf rdf:resource="https://saref.etsi.org/core/FeatureKind"/>
        <rdfs:subClassOf>
            <owl:Restriction>
                <owl:onProperty rdf:resource="http://www.w3.org/2004/02/skos/core#broader"/>
                <owl:allValuesFrom rdf:resource="https://saref.etsi.org/core/FeatureKind"/>
            </owl:Restriction>
        </rdfs:subClassOf>
        <rdfs:subClassOf>
            <owl:Restriction>
                <owl:onProperty rdf:resource="http://www.w3.org/2004/02/skos/core#narrower"/>
                <owl:allValuesFrom rdf:resource="https://saref.etsi.org/core/FeatureKind"/>
            </owl:Restriction>
        </rdfs:subClassOf>
        <rdfs:comment xml:lang="en">Device kinds allow to describe kinds of devices, with common properties and common states having the same value, targeting the same properties and states, common functions, and common services. Devices kinds may be used to describe models of devices in online catalogues.</rdfs:comment>
        <rdfs:label xml:lang="en">Device kinds</rdfs:label>
        <skos:historyNote xml:lang="en">V4.1.1: Introduced class saref:DeviceKind</skos:historyNote>
        <skos:historyNote xml:lang="en">V4.1.1: Use SKOS to organize generic classes in taxonomies.</skos:historyNote>
    </owl:Class>
    


    <!-- https://saref.etsi.org/core/FeatureKind -->

    <owl:Class rdf:about="https://saref.etsi.org/core/FeatureKind">
        <rdfs:subClassOf>
            <owl:Restriction>
                <owl:onProperty rdf:resource="http://www.w3.org/2004/02/skos/core#broader"/>
                <owl:allValuesFrom rdf:resource="https://saref.etsi.org/core/FeatureKind"/>
            </owl:Restriction>
        </rdfs:subClassOf>
        <rdfs:subClassOf>
            <owl:Restriction>
                <owl:onProperty rdf:resource="http://www.w3.org/2004/02/skos/core#narrower"/>
                <owl:allValuesFrom rdf:resource="https://saref.etsi.org/core/FeatureKind"/>
            </owl:Restriction>
        </rdfs:subClassOf>
        <rdfs:subClassOf>
            <owl:Restriction>
                <owl:onProperty rdf:resource="https://saref.etsi.org/core/consistsOf"/>
                <owl:allValuesFrom rdf:resource="https://saref.etsi.org/core/FeatureKind"/>
            </owl:Restriction>
        </rdfs:subClassOf>
        <rdfs:comment xml:lang="en">Feature kinds allow to describe kinds of features of interest, with common properties having the same value, and common states being the same. An instance of saref:FeatureKind represents an archetype of real world entities, for example to populate product catalogs.</rdfs:comment>
        <rdfs:label xml:lang="en">Feature kinds</rdfs:label>
        <skos:historyNote xml:lang="en">V3.2.1: Introduced class saref:FeatureKind</skos:historyNote>
        <skos:historyNote xml:lang="en">V3.2.1: Use SKOS to organize generic classes in taxonomies.</skos:historyNote>
    </owl:Class>
    


    <!-- https://saref.etsi.org/core/FeatureOfInterest -->

    <owl:Class rdf:about="https://saref.etsi.org/core/FeatureOfInterest">
        <rdfs:subClassOf>
            <owl:Restriction>
                <owl:onProperty rdf:resource="https://saref.etsi.org/core/consistsOf"/>
                <owl:allValuesFrom rdf:resource="https://saref.etsi.org/core/FeatureOfInterest"/>
            </owl:Restriction>
        </rdfs:subClassOf>
        <rdfs:comment>A feature of interest represents any real world entity from which a property is measured.</rdfs:comment>
        <rdfs:comment xml:lang="en">A feature of interest represents any real world entity from which a property or a state may be targeted, such as observed and controlled. An instance of saref:FeatureOfInterest represents one specific real world entity.</rdfs:comment>
        <rdfs:label xml:lang="en">Feature of interest</rdfs:label>
        <skos:historyNote xml:lang="en">V3.2.1: Definition of saref:FeatureOfInterest is clarified, not only properties are measured, but properties and states can be observed and controlled.</skos:historyNote>
        <skos:historyNote xml:lang="en">V3.2.1: Definition of saref:FeatureOfInterest: Clarify it&apos;s a specific real world entity.</skos:historyNote>
        <skos:historyNote xml:lang="en">V3.2.1: Definition of saref:FeatureOfInterest: allValuesFrom axioms are unnecessary and have been deleted.</skos:historyNote>
    </owl:Class>
    


    <!-- https://saref.etsi.org/core/Function -->

    <owl:Class rdf:about="https://saref.etsi.org/core/Function">
        <rdfs:subClassOf>
            <owl:Restriction>
                <owl:onProperty rdf:resource="http://www.w3.org/2004/02/skos/core#broader"/>
                <owl:allValuesFrom rdf:resource="https://saref.etsi.org/core/Function"/>
            </owl:Restriction>
        </rdfs:subClassOf>
        <rdfs:subClassOf>
            <owl:Restriction>
                <owl:onProperty rdf:resource="http://www.w3.org/2004/02/skos/core#narrower"/>
                <owl:allValuesFrom rdf:resource="https://saref.etsi.org/core/Function"/>
            </owl:Restriction>
        </rdfs:subClassOf>
        <rdfs:comment xml:lang="en">Logical groups of commands that devices support to accomplish their tasks. Function can target (OP saref:targets and its sub-properties) features, properties, or states. An instance of saref:Function can apply to different devices.</rdfs:comment>
        <rdfs:comment>The functionality necessary to accomplish the task for which a device is designed. A device can be designed to perform more than one function. Functions can be structured in categories (subclasses) that reflect different points of view, for example, considering the specific application area for which a function can be used (e.g., light, temperature, motion, heat, power, etc.), or the capability that a function can support (e.g., receive, reply, notify, etc.), and so forth.</rdfs:comment>
        <rdfs:label xml:lang="en">Function</rdfs:label>
        <skos:example xml:lang="en">To accomplish the task of controlling the light, a smart light switch may have a function for turning on and off the light, and another to set the luminosity of the light.</skos:example>
        <skos:example xml:lang="en">To accomplish the task of sensing the temperature, a temperature sensor should have a sensing function.</skos:example>
        <skos:example xml:lang="en">To accomplish the task of washing clothes, a washing machine should have a function for washing.</skos:example>
        <skos:historyNote xml:lang="en">V3.2.1: Simplified definition and axiomatization of saref:Function. Added examples.</skos:historyNote>
    </owl:Class>
    


    <!-- https://saref.etsi.org/core/FunctionOfInterest -->

    <owl:Class rdf:about="https://saref.etsi.org/core/FunctionOfInterest">
        <rdfs:subClassOf>
            <owl:Restriction>
                <owl:onProperty rdf:resource="https://saref.etsi.org/core/isFunctionOfInterestOf"/>
                <owl:cardinality rdf:datatype="http://www.w3.org/2001/XMLSchema#nonNegativeInteger">1</owl:cardinality>
            </owl:Restriction>
        </rdfs:subClassOf>
        <rdfs:comment xml:lang="en">Logical groups of commands that devices support to accomplish their tasks. Function can target (OP saref:targets and its sub-properties) features, properties, or states. An instance of saref:FunctionOfInterest is supported by exactly one device.</rdfs:comment>
        <rdfs:label xml:lang="en">Function of Interest</rdfs:label>
        <skos:historyNote xml:lang="en">V3.2.1: Introduced saref:FunctionOfInterest, parallel to saref:PropertyOfInterest.</skos:historyNote>
        <skos:note xml:lang="en">A function of interest is the function of (OP saref:isFunctionOfInterestOf) exactly one device.</skos:note>
        <skos:note xml:lang="en">Functions of interest need not always be explicited. It depends on the use case. Typically, functions of interest are useful to specify which command is actually exposed, and which actual property of interest or state of interest it targets.</skos:note>
    </owl:Class>
    


    <!-- https://saref.etsi.org/core/Measurement -->

    <owl:Class rdf:about="https://saref.etsi.org/core/Measurement">
        <rdfs:comment>Represents the measured value made over a property. It is also linked to the unit of measure in which the value is expressed and the timestamp of the measurement.</rdfs:comment>
        <rdfs:label xml:lang="en">Measurement</rdfs:label>
    </owl:Class>
    


    <!-- https://saref.etsi.org/core/Meter -->

    <owl:Class rdf:about="https://saref.etsi.org/core/Meter">
        <rdfs:subClassOf rdf:resource="https://saref.etsi.org/core/Device"/>
        <rdfs:subClassOf>
            <owl:Restriction>
                <owl:onProperty rdf:resource="https://saref.etsi.org/core/observes"/>
                <owl:minCardinality rdf:datatype="http://www.w3.org/2001/XMLSchema#nonNegativeInteger">1</owl:minCardinality>
            </owl:Restriction>
        </rdfs:subClassOf>
        <rdfs:comment xml:lang="en">A device designed to observe and additionally do some computation and/or display one or more properties of one or more features of interest.</rdfs:comment>
        <rdfs:label xml:lang="en">Meter</rdfs:label>
        <skos:historyNote xml:lang="en">V3.2.1: Definition of Meter is simplified and grounded on saref:observes. Local restriction on saref:hasFunction is deleted.</skos:historyNote>
        <skos:historyNote xml:lang="en">V4.1.1: Definition of Sensor and Meter are updated to better distinguish one from the other.</skos:historyNote>
    </owl:Class>
    


    <!-- https://saref.etsi.org/core/Observation -->

    <owl:Class rdf:about="https://saref.etsi.org/core/Observation">
        <rdfs:subClassOf rdf:resource="https://saref.etsi.org/core/ProcedureExecution"/>
        <rdfs:subClassOf>
            <owl:Restriction>
                <owl:onProperty rdf:resource="https://saref.etsi.org/core/madeBy"/>
                <owl:allValuesFrom rdf:resource="https://saref.etsi.org/core/Sensor"/>
            </owl:Restriction>
        </rdfs:subClassOf>
        <rdfs:subClassOf>
            <owl:Restriction>
                <owl:onProperty rdf:resource="https://saref.etsi.org/core/observes"/>
                <owl:minCardinality rdf:datatype="http://www.w3.org/2001/XMLSchema#nonNegativeInteger">1</owl:minCardinality>
            </owl:Restriction>
        </rdfs:subClassOf>
        <rdfs:comment xml:lang="en">A saref:Observation is the act of carrying out a procedure to estimate or calculate a value of a property of a feature of interest, or a state of a feature of interest. It links to a sensor to describe what made the observation, and to the observed feature, property, property of interest, state, or state of interest. Typically, its result is a property value or a state. An observation of a state (OP saref:observes) should have a state as a result (OP saref:hasResult). Respectively, an observation of a property should have a property value as a result.</rdfs:comment>
        <rdfs:label xml:lang="en">Observation</rdfs:label>
    </owl:Class>
    


    <!-- https://saref.etsi.org/core/Operation -->

    <owl:Class rdf:about="https://saref.etsi.org/core/Operation">
        <rdfs:subClassOf>
            <owl:Restriction>
                <owl:onProperty rdf:resource="https://saref.etsi.org/core/represents"/>
                <owl:allValuesFrom>
                    <owl:Class>
                        <owl:unionOf rdf:parseType="Collection">
                            <rdf:Description rdf:about="https://saref.etsi.org/core/Command"/>
                            <rdf:Description rdf:about="https://saref.etsi.org/core/CommandOfInterest"/>
                        </owl:unionOf>
                    </owl:Class>
                </owl:allValuesFrom>
            </owl:Restriction>
        </rdfs:subClassOf>
        <rdfs:subClassOf>
            <owl:Restriction>
                <owl:onProperty rdf:resource="https://saref.etsi.org/core/represents"/>
                <owl:minQualifiedCardinality rdf:datatype="http://www.w3.org/2001/XMLSchema#nonNegativeInteger">1</owl:minQualifiedCardinality>
                <owl:onClass rdf:resource="https://saref.etsi.org/core/CommandOfInterest"/>
            </owl:Restriction>
        </rdfs:subClassOf>
        <rdfs:subClassOf>
            <owl:Restriction>
                <owl:onProperty rdf:resource="https://saref.etsi.org/core/isOperationOf"/>
                <owl:cardinality rdf:datatype="http://www.w3.org/2001/XMLSchema#nonNegativeInteger">1</owl:cardinality>
            </owl:Restriction>
        </rdfs:subClassOf>
        <rdfs:comment xml:lang="en">A saref:Operation is the means of a service to communicate in a procedure-type manner over the network (i.e. transmit data to/from other devices). It is the machine interpretable exposure of a human understandable command to a network.</rdfs:comment>
        <rdfs:label xml:lang="en">Operation</rdfs:label>
        <skos:example xml:lang="en">In the set of operations exposed by a smart light bulb on a given network, one may be dedicated to turn on and off the light and expect a boolean as input. Another one may be dedicated to set the luminosity status and expect a target luminosity level (a byte) and a transition time (encoded on two bytes).</skos:example>
        <skos:example xml:lang="en">In the set of operations exposed by a smart washing machine on a given network, one may be dedicated to set the water temperature for the washing cycle, and expected as input a enumerated value. Another one may be dedicated to start, pause, or stop the washing cycle.</skos:example>
        <skos:example xml:lang="en">To turn on a light, send a CoAP PUT request with CBOR content 0xf5 (true)</skos:example>
        <skos:historyNote xml:lang="en">V3.2.1: Introduced saref:Operation and associated properties from oneM2M base ontology.</skos:historyNote>
        <skos:note xml:lang="en">An operation may be described in terms of its inputs and outputs using OP saref:hasInput and saref:hasOutput. Inputs and outputs of operations typically describe the expected schema or shape of network messages.</skos:note>
        <skos:note xml:lang="en">Typically, a device connected to a given network offers one service for each of its functions of interest, and each service has one operation per command of interest of the function of interest it represents.</skos:note>
    </owl:Class>
    


    <!-- https://saref.etsi.org/core/OperationExecution -->

    <owl:Class rdf:about="https://saref.etsi.org/core/OperationExecution">
        <rdfs:subClassOf rdf:resource="https://saref.etsi.org/core/ProcedureExecution"/>
        <rdfs:subClassOf>
            <owl:Restriction>
                <owl:onProperty rdf:resource="https://saref.etsi.org/core/isExecutionOf"/>
                <owl:allValuesFrom rdf:resource="https://saref.etsi.org/core/Operation"/>
            </owl:Restriction>
        </rdfs:subClassOf>
        <rdfs:comment xml:lang="en">Describes the execution of an operation in a network: themachine interpretable  description of a communication between devices over the network. Typically, its input and result are network messages, that conform to the input and output of the executed operation.</rdfs:comment>
        <rdfs:label xml:lang="en">Operation Execution</rdfs:label>
    </owl:Class>
    


    <!-- https://saref.etsi.org/core/ProcedureExecution -->

    <owl:Class rdf:about="https://saref.etsi.org/core/ProcedureExecution">
        <rdfs:comment xml:lang="en">Represents the act of carrying out a procedure.</rdfs:comment>
        <rdfs:label xml:lang="en">Procedure Execution</rdfs:label>
        <skos:historyNote xml:lang="en">V3.2.1: Introduced saref:ProcedureExecution.</skos:historyNote>
    </owl:Class>
    


    <!-- https://saref.etsi.org/core/Profile -->

    <owl:Class rdf:about="https://saref.etsi.org/core/Profile">
        <rdfs:comment xml:lang="en">A saref:Profile describes the money earned (negative values) or paied (positive values) for the use (production or consumption) of a commodity by a device in a certain context.</rdfs:comment>
        <rdfs:label xml:lang="en">Profile</rdfs:label>
        <skos:historyNote xml:lang="en">V3.2.1: Class saref:Profile has been re-specified, to take into account findings from SAREF4ENER V1.2.1.</skos:historyNote>
        <skos:note xml:lang="en">OP saref:hasPrice links a profile to the money earned (negative values) or paid (positive values) for the use (production or consumption) of the commodity by the device.</skos:note>
        <skos:note xml:lang="en">OP saref:hasProfile links a device to its profile. The device should be linked to a certain commodity using OP saref:consumes, saref:produces, or saref:stores, and optionally to some property or state using OP saref:targets or its sub-properties.</skos:note>
        <skos:note xml:lang="en">The applicable context can be restricted to when a feature of interest has a certain state (OPs saref:whenState).</skos:note>
        <skos:note xml:lang="en">The applicable context can be restricted to when the property of a feature of interest has some value (OPs saref:whenPropertyValue)</skos:note>
        <skos:note xml:lang="en">The applicable context of a profile can be bound temporally using DP saref:hasTimestamp or its subproperties defined by SAREF extensions, or OP saref:hasApplicableTime which links to instant or interval or other compound temporal entity expressed using OWL Time.</skos:note>
    </owl:Class>
    


    <!-- https://saref.etsi.org/core/Property -->

    <owl:Class rdf:about="https://saref.etsi.org/core/Property">
        <rdfs:subClassOf>
            <owl:Restriction>
                <owl:onProperty rdf:resource="http://www.w3.org/2004/02/skos/core#broader"/>
                <owl:allValuesFrom rdf:resource="https://saref.etsi.org/core/Property"/>
            </owl:Restriction>
        </rdfs:subClassOf>
        <rdfs:subClassOf>
            <owl:Restriction>
                <owl:onProperty rdf:resource="http://www.w3.org/2004/02/skos/core#narrower"/>
                <owl:allValuesFrom rdf:resource="https://saref.etsi.org/core/Property"/>
            </owl:Restriction>
        </rdfs:subClassOf>
        <rdfs:subClassOf>
            <owl:Restriction>
                <owl:onProperty rdf:resource="https://saref.etsi.org/core/consistsOf"/>
                <owl:allValuesFrom>
                    <owl:Class>
                        <owl:unionOf rdf:parseType="Collection">
                            <rdf:Description rdf:about="https://saref.etsi.org/core/FeatureKind"/>
                            <rdf:Description rdf:about="https://saref.etsi.org/core/Property"/>
                            <rdf:Description rdf:about="https://saref.etsi.org/core/State"/>
                        </owl:unionOf>
                    </owl:Class>
                </owl:allValuesFrom>
            </owl:Restriction>
        </rdfs:subClassOf>
        <owl:disjointWith rdf:resource="https://saref.etsi.org/core/UnitOfMeasure"/>
        <rdfs:comment>An aspect of an entity that can be observable by a sensor.</rdfs:comment>
        <rdfs:comment xml:lang="en">Identifiable qualities of features of interest that can be target of devices, such as observed or controlled. A property can apply to different features of interest.</rdfs:comment>
        <rdfs:label xml:lang="en">Property</rdfs:label>
        <skos:example xml:lang="en">Air temperature, pressure, luminance, etc. are all properties.</skos:example>
        <skos:example xml:lang="en">Two examples using the QUDT Quantity Kind vocabulary, and the British Oceanographic Data Centre Parameter Usage Vocabulary.

&lt;https://qudt.org/2.1/vocab/quantitykind/ActiveEnergy&gt; a saref:Property ;
    rdfs:label &quot;Active Energy&quot;@en ;
    rdfs:comment &quot;&quot;Active Energy&quot; is the electrical energy transformable into some other form of energy.&quot;@en .

&lt;http://vocab.nerc.ac.uk/collection/P01/current/CDTSZZ01/&gt; a saref:Property ;
    skos:prefLabel &quot;Absolute temperature standard deviation of the atmosphere by dry bulb thermometer&quot;@en .
</skos:example>
        <skos:historyNote xml:lang="en">Until SAREF V3.1.1, there was an ambiguity between whether properties should be specific or generic to features of interest. This ambiguity has been solved in SAREF V3.2.1, and the new modeling will be enforced in the next major revision of SAREF.</skos:historyNote>
        <skos:historyNote xml:lang="en">V3.2.1: The definition and scope of usage for saref:Property is clarified. Axiomatization is simplified.</skos:historyNote>
        <skos:note xml:lang="en">Concepts from existing code lists, vocabularies, and taxonomies, may be used as instances of saref:Property.</skos:note>
    </owl:Class>
    


    <!-- https://saref.etsi.org/core/PropertyOfInterest -->

    <owl:Class rdf:about="https://saref.etsi.org/core/PropertyOfInterest">
        <rdfs:subClassOf>
            <owl:Restriction>
                <owl:onProperty rdf:resource="https://saref.etsi.org/core/consistsOf"/>
                <owl:allValuesFrom>
                    <owl:Class>
                        <owl:unionOf rdf:parseType="Collection">
                            <rdf:Description rdf:about="https://saref.etsi.org/core/FeatureKind"/>
                            <rdf:Description rdf:about="https://saref.etsi.org/core/Property"/>
                            <rdf:Description rdf:about="https://saref.etsi.org/core/PropertyOfInterest"/>
                            <rdf:Description rdf:about="https://saref.etsi.org/core/State"/>
                            <rdf:Description rdf:about="https://saref.etsi.org/core/StateOfInterest"/>
                        </owl:unionOf>
                    </owl:Class>
                </owl:allValuesFrom>
            </owl:Restriction>
        </rdfs:subClassOf>
        <rdfs:subClassOf>
            <owl:Restriction>
                <owl:onProperty rdf:resource="https://saref.etsi.org/core/isPropertyOfInterestOf"/>
                <owl:cardinality rdf:datatype="http://www.w3.org/2001/XMLSchema#nonNegativeInteger">1</owl:cardinality>
            </owl:Restriction>
        </rdfs:subClassOf>
        <rdfs:comment xml:lang="en">Identifiable qualities of features of interest that can be target of devices, such as observed or controlled. An instance of saref:PropertyOfInterest is specific to a feature of interest. It is inherent to and cannot exist without that feature of interest.</rdfs:comment>
        <rdfs:label xml:lang="en">Property of Interest</rdfs:label>
        <skos:example xml:lang="en">The air temperature of the atmosphere sample at a certain location and altitude, the received signal strength indicator of an wireless IoT connection, the luminance of the ETSI ATHENA amphitheatre.

&lt;etsi_premises/athena#luminance&gt; a saref:PropertyOfInterest ;
    saref:isPropertyOfInterestOf &lt;etsi_premises/athena&gt; ;
    saref:hasPropertyKind saref:Luminance ;
    rdfs:comment &quot;The luminance of amphitheatre ATHENA&quot;@en .
</skos:example>
        <skos:historyNote xml:lang="en">V3.2.1: Introduced saref:PropertyOfInterest to solved the ambiguity between generic vs specific properties.</skos:historyNote>
        <skos:note xml:lang="en">A property of interest is the property of (OP saref:isPropertyOfInterestOf) exactly one feature of interest.</skos:note>
        <skos:note xml:lang="en">Per convention, the IRI of properties of interest should consist of the IRI of their feature of interest, suffixed with a fragment identifier #{P} where {P} refers to the name of the property.</skos:note>
        <skos:note xml:lang="en">Properties of interest need not always be explicited. It depends on the use case. Typically, properties of interest are useful in applications, where the association between a feature of interest and a property (i.e., the property of interest) needs to be identified and related to other properties of interest.</skos:note>
    </owl:Class>
    


    <!-- https://saref.etsi.org/core/PropertyValue -->

    <owl:Class rdf:about="https://saref.etsi.org/core/PropertyValue">
        <rdfs:subClassOf>
            <owl:Restriction>
                <owl:onProperty rdf:resource="https://saref.etsi.org/core/consistsOf"/>
                <owl:allValuesFrom>
                    <owl:Class>
                        <owl:unionOf rdf:parseType="Collection">
                            <rdf:Description rdf:about="https://saref.etsi.org/core/FeatureKind"/>
                            <rdf:Description rdf:about="https://saref.etsi.org/core/FeatureOfInterest"/>
                            <rdf:Description rdf:about="https://saref.etsi.org/core/Property"/>
                            <rdf:Description rdf:about="https://saref.etsi.org/core/PropertyOfInterest"/>
                            <rdf:Description rdf:about="https://saref.etsi.org/core/PropertyValue"/>
                            <rdf:Description rdf:about="https://saref.etsi.org/core/State"/>
                            <rdf:Description rdf:about="https://saref.etsi.org/core/StateOfInterest"/>
                            <rdf:Description rdf:about="https://saref.etsi.org/core/StateValue"/>
                        </owl:unionOf>
                    </owl:Class>
                </owl:allValuesFrom>
            </owl:Restriction>
        </rdfs:subClassOf>
        <rdfs:subClassOf>
            <owl:Restriction>
                <owl:onProperty rdf:resource="https://saref.etsi.org/core/isMeasuredIn"/>
                <owl:maxCardinality rdf:datatype="http://www.w3.org/2001/XMLSchema#nonNegativeInteger">1</owl:maxCardinality>
            </owl:Restriction>
        </rdfs:subClassOf>
        <rdfs:subClassOf>
            <owl:Restriction>
                <owl:onProperty rdf:resource="https://ega.industry.com/ontologies/core/data/hasTag"/>
                <owl:someValuesFrom rdf:resource="http://www.w3.org/2001/XMLSchema#string"/>
            </owl:Restriction>
        </rdfs:subClassOf>
        <rdfs:subClassOf>
            <owl:Restriction>
                <owl:onProperty rdf:resource="https://saref.etsi.org/core/hasTimestamp"/>
                <owl:someValuesFrom rdf:resource="http://www.w3.org/2001/XMLSchema#dateTime"/>
            </owl:Restriction>
        </rdfs:subClassOf>
        <rdfs:subClassOf>
            <owl:Restriction>
                <owl:onProperty rdf:resource="https://saref.etsi.org/core/hasValue"/>
                <owl:maxCardinality rdf:datatype="http://www.w3.org/2001/XMLSchema#nonNegativeInteger">1</owl:maxCardinality>
            </owl:Restriction>
        </rdfs:subClassOf>
        <rdfs:comment xml:lang="en">Describes the value for a property. The property value is optionally linked to its value expressed as an RDF literal (DP saref:hasValue), optionally to the unit of measurement (OP saref:isMeasuredIn), and optionally to the properties or properties of interest it is a value of (OP saref:isValueOfProperty).</rdfs:comment>
        <rdfs:label xml:lang="en">Property Value</rdfs:label>
        <skos:historyNote xml:lang="en">V3.2.1: Introduced saref:PropertyValue to simplify the association of a measure to a property, without always needing it to be a measurement made by a device.</skos:historyNote>
        <skos:historyNote xml:lang="en">V4.1.1: saref:hasValue is now optional on saref:PropertyValue.</skos:historyNote>
    </owl:Class>
    


    <!-- https://saref.etsi.org/core/Sensor -->

    <owl:Class rdf:about="https://saref.etsi.org/core/Sensor">
        <rdfs:subClassOf rdf:resource="https://saref.etsi.org/core/Device"/>
        <rdfs:subClassOf>
            <owl:Restriction>
                <owl:onProperty rdf:resource="https://saref.etsi.org/core/observes"/>
                <owl:minCardinality rdf:datatype="http://www.w3.org/2001/XMLSchema#nonNegativeInteger">1</owl:minCardinality>
            </owl:Restriction>
        </rdfs:subClassOf>
        <rdfs:comment xml:lang="en">A device designed to observe and measure one or more properties or states of one or more features of interest.</rdfs:comment>
        <rdfs:label xml:lang="en">Sensor</rdfs:label>
        <skos:historyNote xml:lang="en">V3.2.1: Definition of Sensor is simplified and grounded on saref:observes. Local restriction on saref:hasFunction is deleted.</skos:historyNote>
        <skos:historyNote xml:lang="en">V4.1.1: Definition of Sensor and Meter are updated to better distinguish one from the other.</skos:historyNote>
    </owl:Class>
    


    <!-- https://saref.etsi.org/core/Service -->

    <owl:Class rdf:about="https://saref.etsi.org/core/Service">
        <rdfs:subClassOf>
            <owl:Restriction>
                <owl:onProperty rdf:resource="https://saref.etsi.org/core/represents"/>
                <owl:allValuesFrom>
                    <owl:Class>
                        <owl:unionOf rdf:parseType="Collection">
                            <rdf:Description rdf:about="https://saref.etsi.org/core/Function"/>
                            <rdf:Description rdf:about="https://saref.etsi.org/core/FunctionOfInterest"/>
                        </owl:unionOf>
                    </owl:Class>
                </owl:allValuesFrom>
            </owl:Restriction>
        </rdfs:subClassOf>
        <rdfs:subClassOf>
            <owl:Restriction>
                <owl:onProperty rdf:resource="https://saref.etsi.org/core/represents"/>
                <owl:minQualifiedCardinality rdf:datatype="http://www.w3.org/2001/XMLSchema#nonNegativeInteger">1</owl:minQualifiedCardinality>
                <owl:onClass rdf:resource="https://saref.etsi.org/core/FunctionOfInterest"/>
            </owl:Restriction>
        </rdfs:subClassOf>
        <rdfs:subClassOf>
            <owl:Restriction>
                <owl:onProperty rdf:resource="https://saref.etsi.org/core/isOfferedBy"/>
                <owl:cardinality rdf:datatype="http://www.w3.org/2001/XMLSchema#nonNegativeInteger">1</owl:cardinality>
            </owl:Restriction>
        </rdfs:subClassOf>
        <rdfs:comment xml:lang="en">A saref:Service is a digital representation of a function in a network, making it discoverable, registerable and remotely controllable in the network.</rdfs:comment>
        <rdfs:label xml:lang="en">Service</rdfs:label>
        <skos:example xml:lang="en">For example, a light switch can offer the service of remotely switching the lights in a home through mobile phone devices that are connected to the local network (ex:SwitchOnService class). This &quot;remote switching&quot; service represents the ex:OnOffFunction.</skos:example>
        <skos:historyNote xml:lang="en">V3.2.1: Simplified definition of saref:Service. Added examples.</skos:historyNote>
        <skos:note xml:lang="en">Typically, a device connected to a given network offers one service for each of its functions of interest.</skos:note>
    </owl:Class>
    


    <!-- https://saref.etsi.org/core/State -->

    <owl:Class rdf:about="https://saref.etsi.org/core/State">
        <rdfs:subClassOf>
            <owl:Restriction>
                <owl:onProperty rdf:resource="http://www.w3.org/2004/02/skos/core#broader"/>
                <owl:allValuesFrom rdf:resource="https://saref.etsi.org/core/State"/>
            </owl:Restriction>
        </rdfs:subClassOf>
        <rdfs:subClassOf>
            <owl:Restriction>
                <owl:onProperty rdf:resource="http://www.w3.org/2004/02/skos/core#narrower"/>
                <owl:allValuesFrom rdf:resource="https://saref.etsi.org/core/State"/>
            </owl:Restriction>
        </rdfs:subClassOf>
        <rdfs:subClassOf>
            <owl:Restriction>
                <owl:onProperty rdf:resource="https://ega.industry.com/ontologies/core/data/hasTag"/>
                <owl:someValuesFrom rdf:resource="http://www.w3.org/2001/XMLSchema#string"/>
            </owl:Restriction>
        </rdfs:subClassOf>
        <rdfs:comment xml:lang="en">Identifiable conditions that features of interest are or may be in, and that can be target of devices, such as observed and controlled. A state can apply to different features of interest.</rdfs:comment>
        <rdfs:label xml:lang="en">State</rdfs:label>
        <skos:example xml:lang="en">A switch can be found in the saref:OnOffState.</skos:example>
        <skos:historyNote xml:lang="en">V3.2.1: Clarified and generalized definition of saref:State. Can now apply to all features of interest, not just devices.</skos:historyNote>
        <skos:note xml:lang="en">Concepts from existing code lists, vocabularies, and taxonomies, may be used as instances of saref:State.</skos:note>
        <skos:note xml:lang="en">SAREF is not restricted to binary states such as the ex:OnOffState, but allows to define also enumerated states.</skos:note>
    </owl:Class>
    


    <!-- https://saref.etsi.org/core/StateOfInterest -->

    <owl:Class rdf:about="https://saref.etsi.org/core/StateOfInterest">
        <rdfs:subClassOf>
            <owl:Restriction>
                <owl:onProperty rdf:resource="https://saref.etsi.org/core/isStateOfInterestOf"/>
                <owl:cardinality rdf:datatype="http://www.w3.org/2001/XMLSchema#nonNegativeInteger">1</owl:cardinality>
            </owl:Restriction>
        </rdfs:subClassOf>
        <rdfs:comment xml:lang="en">Identifiable conditions that features of interest are or may be in, and that can be target of devices, such as observed and controlled. An instance of saref:StateOfInterest is specific to a feature of interest. It is inherent to and cannot exist without that feature of interest.</rdfs:comment>
        <rdfs:label xml:lang="en">State of Interest</rdfs:label>
        <skos:historyNote xml:lang="en">V3.2.1: Introduced saref:StateOfInterest, parallel to saref:PropertyOfInterest.</skos:historyNote>
        <skos:note xml:lang="en">A state of interest is the state of (OP saref:isStateOfInterestOf) exactly one feature of interest.</skos:note>
        <skos:note xml:lang="en">Per convention, the IRI of states of interest should consist of the IRI of their feature of interest, suffixed with a fragment identifier #{S} where {S} refers to the name of the state.</skos:note>
        <skos:note xml:lang="en">States of interest need not always be explicited. It depends on the use case. Typically, states of interest are useful in applications, where the association between a feature of interest and a state (i.e., the state of interest) needs to be identified and related to other states of interest.</skos:note>
    </owl:Class>
    


    <!-- https://saref.etsi.org/core/StateValue -->

    <owl:Class rdf:about="https://saref.etsi.org/core/StateValue">
        <rdfs:comment xml:lang="en">Describes the value for a state. The state value is optionally linked the states or states of interest it is a value of (OP saref:isValueOfState).</rdfs:comment>
        <rdfs:label xml:lang="en">State Value</rdfs:label>
        <skos:historyNote xml:lang="en">V4.1.1: Introduced saref:StateValue.</skos:historyNote>
    </owl:Class>
    


    <!-- https://saref.etsi.org/core/Task -->

    <owl:Class rdf:about="https://saref.etsi.org/core/Task">
        <rdfs:subClassOf>
            <owl:Restriction>
                <owl:onProperty rdf:resource="http://www.w3.org/2004/02/skos/core#broader"/>
                <owl:allValuesFrom rdf:resource="https://saref.etsi.org/core/Task"/>
            </owl:Restriction>
        </rdfs:subClassOf>
        <rdfs:subClassOf>
            <owl:Restriction>
                <owl:onProperty rdf:resource="http://www.w3.org/2004/02/skos/core#narrower"/>
                <owl:allValuesFrom rdf:resource="https://saref.etsi.org/core/Task"/>
            </owl:Restriction>
        </rdfs:subClassOf>
        <rdfs:comment xml:lang="en">The goal for which a device is designed, from a user perspective.</rdfs:comment>
        <rdfs:label xml:lang="en">Task</rdfs:label>
        <skos:example xml:lang="en">For example, a washing machine is designed for the task of washing.</skos:example>
        <skos:note xml:lang="en">Tasks can be accomplished by devices (saref:isAccomplishedBy).</skos:note>
    </owl:Class>
    


    <!-- https://saref.etsi.org/core/UnitOfMeasure -->

    <owl:Class rdf:about="https://saref.etsi.org/core/UnitOfMeasure">
        <owl:disjointWith rdf:resource="https://saref.etsi.org/saref4inma/Size"/>
        <rdfs:comment xml:lang="en">The unit of measure is a standard for measurement of a quantity, such as a Property.</rdfs:comment>
        <rdfs:label xml:lang="en">Unit of measure</rdfs:label>
        <skos:example xml:lang="en">For example, consumption power is a property and Watt is a unit of power that represents a definite predetermined power: when we say 10 Watt, we actually mean 10 times the definite predetermined power &quot;Watt&quot;.</skos:example>
        <skos:note xml:lang="en">Concepts from existing code lists, vocabularies, and taxonomies, may be used as instances of saref:UnitOfMeasure. For example the QUDT Unit vocabulary</skos:note>
        <skos:note xml:lang="en">Our definition is based on the definition of unit of measure in the Ontology of units of Measure (OM).</skos:note>
    </owl:Class>
    


    <!-- https://saref.etsi.org/saref4bldg/Building -->

    <owl:Class rdf:about="https://saref.etsi.org/saref4bldg/Building">
        <rdfs:comment>A building represents a structure that provides shelter for its occupants or contents and stands in one place. The building is also used to provide a basic element within the spatial structure hierarchy for the components of a building project (together with site, storey, and space).</rdfs:comment>
        <rdfs:label xml:lang="en">Building</rdfs:label>
    </owl:Class>
    


    <!-- https://saref.etsi.org/saref4bldg/BuildingSpace -->

    <owl:Class rdf:about="https://saref.etsi.org/saref4bldg/BuildingSpace">
        <rdfs:comment>An entity used to define the physical spaces of the building. A building space contains devices or building objects.</rdfs:comment>
        <rdfs:label xml:lang="en">Building space</rdfs:label>
    </owl:Class>
    


    <!-- https://saref.etsi.org/saref4bldg/PhysicalObject -->

    <owl:Class rdf:about="https://saref.etsi.org/saref4bldg/PhysicalObject">
        <rdfs:comment>Any Object that has a proper space region.  (Definition extracted from DUL ontology)</rdfs:comment>
        <rdfs:label xml:lang="en">Physical object</rdfs:label>
    </owl:Class>
    


    <!-- https://saref.etsi.org/saref4inma/ActualMeasurement -->

    <owl:Class rdf:about="https://saref.etsi.org/saref4inma/ActualMeasurement">
        <rdfs:subClassOf rdf:resource="https://saref.etsi.org/saref4inma/Measurement"/>
        <owl:disjointWith rdf:resource="https://saref.etsi.org/saref4inma/ExpectedMeasurement"/>
        <rdfs:comment>Describes whether the measurement is actually measured during the production process. Disjoint with ExpectedMeasurement.</rdfs:comment>
        <rdfs:label xml:lang="en">Actual measurement</rdfs:label>
    </owl:Class>
    


    <!-- https://saref.etsi.org/saref4inma/Area -->

    <owl:Class rdf:about="https://saref.etsi.org/saref4inma/Area">
        <rdfs:subClassOf rdf:resource="https://saref.etsi.org/saref4bldg/BuildingSpace"/>
        <owl:disjointWith rdf:resource="https://saref.etsi.org/saref4inma/Site"/>
        <owl:disjointWith rdf:resource="https://saref.etsi.org/saref4inma/WorkCenter"/>
        <rdfs:comment>A subclass of s4bldg:BuildingSpace used to define the physical spaces of the building. According to IEC 62264, areas are physical, geographical or logical groupings of resources determined by the site. A site can be divided in areas, whereas areas contain work centers.s.</rdfs:comment>
        <rdfs:label xml:lang="en">Area</rdfs:label>
    </owl:Class>
    


    <!-- https://saref.etsi.org/saref4inma/Batch -->

    <owl:Class rdf:about="https://saref.etsi.org/saref4inma/Batch">
        <rdfs:subClassOf rdf:resource="http://www.w3.org/2002/07/owl#Thing"/>
        <rdfs:subClassOf rdf:resource="https://saref.etsi.org/core/FeatureOfInterest"/>
        <rdfs:subClassOf>
            <owl:Restriction>
                <owl:onProperty rdf:resource="https://saref.etsi.org/saref4inma/consistsOfBatch"/>
                <owl:allValuesFrom rdf:resource="https://saref.etsi.org/saref4inma/Batch"/>
            </owl:Restriction>
        </rdfs:subClassOf>
        <rdfs:subClassOf>
            <owl:Restriction>
                <owl:onProperty rdf:resource="https://saref.etsi.org/saref4inma/hasIdentifier"/>
                <owl:allValuesFrom rdf:resource="https://saref.etsi.org/saref4inma/ID"/>
            </owl:Restriction>
        </rdfs:subClassOf>
        <rdfs:subClassOf>
            <owl:Restriction>
                <owl:onProperty rdf:resource="https://saref.etsi.org/saref4inma/isFeatureOfInterestOf"/>
                <owl:allValuesFrom rdf:resource="https://saref.etsi.org/saref4inma/Measurement"/>
            </owl:Restriction>
        </rdfs:subClassOf>
        <rdfs:subClassOf>
            <owl:Restriction>
                <owl:onProperty rdf:resource="https://saref.etsi.org/saref4inma/needsEquipment"/>
                <owl:allValuesFrom rdf:resource="https://saref.etsi.org/saref4inma/ProductionEquipment"/>
            </owl:Restriction>
        </rdfs:subClassOf>
        <rdfs:subClassOf>
            <owl:Restriction>
                <owl:onProperty rdf:resource="https://saref.etsi.org/saref4inma/hasSize"/>
                <owl:maxQualifiedCardinality rdf:datatype="http://www.w3.org/2001/XMLSchema#nonNegativeInteger">1</owl:maxQualifiedCardinality>
                <owl:onClass rdf:resource="https://saref.etsi.org/saref4inma/Size"/>
            </owl:Restriction>
        </rdfs:subClassOf>
        <rdfs:comment>A uniform collection of tangible objects or Lot. This can either be a collection of produced items (i.e. the outflow of products) or a collection of raw material or required material (i.e. the inflow of products). It is assumed that the objects in a batch are similar and thus have shared attributes. Note that this definition is broader than the definition in IEC 61512, which defines a batch as the material that is being produced (whereas in SAREF4INMA a batch can be items or materials). </rdfs:comment>
        <rdfs:label xml:lang="en">Batch</rdfs:label>
    </owl:Class>
    


    <!-- https://saref.etsi.org/saref4inma/ExpectedMeasurement -->

    <owl:Class rdf:about="https://saref.etsi.org/saref4inma/ExpectedMeasurement">
        <rdfs:subClassOf rdf:resource="https://saref.etsi.org/saref4inma/Measurement"/>
        <rdfs:comment>Describes whether the measurement is expected (i.e., planned before the production process). Disjoint with ActualMeasurement.</rdfs:comment>
        <rdfs:label xml:lang="en">Expected measurement</rdfs:label>
    </owl:Class>
    


    <!-- https://saref.etsi.org/saref4inma/Factory -->

    <owl:Class rdf:about="https://saref.etsi.org/saref4inma/Factory">
        <rdfs:subClassOf rdf:resource="https://saref.etsi.org/saref4bldg/Building"/>
        <rdfs:comment>A subclass of s4bldg:Building specialized for the purpose of SAREF4INMA, a factory represents one or more organizations sharing a definit mission, goals and objectives which provides an output such as a product (definition taken from IEC 62264). A factory can be divided in one or multiple sites. </rdfs:comment>
        <rdfs:label xml:lang="en">Factory</rdfs:label>
    </owl:Class>
    


    <!-- https://saref.etsi.org/saref4inma/GTIN12ID -->

    <owl:Class rdf:about="https://saref.etsi.org/saref4inma/GTIN12ID">
        <rdfs:subClassOf rdf:resource="https://saref.etsi.org/saref4inma/ID"/>
        <rdfs:comment>GTIN-12 (UPC-A) is a 12-digit number used primarily in North America</rdfs:comment>
        <rdfs:label xml:lang="en">GTIN12ID</rdfs:label>
    </owl:Class>
    


    <!-- https://saref.etsi.org/saref4inma/GTIN13ID -->

    <owl:Class rdf:about="https://saref.etsi.org/saref4inma/GTIN13ID">
        <rdfs:subClassOf rdf:resource="https://saref.etsi.org/saref4inma/ID"/>
        <rdfs:comment>GTIN-13 (EAN/UCC-13) is a 13-digit number used predominately outside of North America</rdfs:comment>
        <rdfs:label xml:lang="en">GTIN13ID</rdfs:label>
    </owl:Class>
    


    <!-- https://saref.etsi.org/saref4inma/GTIN14ID -->

    <owl:Class rdf:about="https://saref.etsi.org/saref4inma/GTIN14ID">
        <rdfs:subClassOf rdf:resource="https://saref.etsi.org/saref4inma/ID"/>
        <rdfs:comment>GTIN-14 (EAN/UCC-14 or ITF-14 or also known as ITF Symbol, SCC-14, DUN-14, UPC Case Code, UPC Shipping Container Code, UCC Code 128, EAN Code 128) is a 14-digit number used to identify trade items at various packaging levels.</rdfs:comment>
        <rdfs:label xml:lang="en">GTIN14ID</rdfs:label>
    </owl:Class>
    


    <!-- https://saref.etsi.org/saref4inma/GTIN8ID -->

    <owl:Class rdf:about="https://saref.etsi.org/saref4inma/GTIN8ID">
        <rdfs:subClassOf rdf:resource="https://saref.etsi.org/saref4inma/ID"/>
        <rdfs:comment>GTIN-8 (EAN/UCC-8) is an 8-digit number used predominately outside of North America.</rdfs:comment>
        <rdfs:label xml:lang="en">GTIN18ID</rdfs:label>
    </owl:Class>
    


    <!-- https://saref.etsi.org/saref4inma/ID -->

    <owl:Class rdf:about="https://saref.etsi.org/saref4inma/ID">
        <rdfs:subClassOf rdf:resource="http://www.w3.org/2004/02/skos/core#ConceptScheme"/>
        <rdfs:subClassOf>
            <owl:Restriction>
                <owl:onProperty rdf:resource="https://saref.etsi.org/saref4inma/hasIDValue"/>
                <owl:someValuesFrom rdf:resource="http://www.w3.org/2001/XMLSchema#string"/>
            </owl:Restriction>
        </rdfs:subClassOf>
        <rdfs:comment>A unique identifier.</rdfs:comment>
        <rdfs:label xml:lang="en">Identifier</rdfs:label>
    </owl:Class>
    


    <!-- https://saref.etsi.org/saref4inma/IRDI -->

    <owl:Class rdf:about="https://saref.etsi.org/saref4inma/IRDI">
        <rdfs:subClassOf rdf:resource="https://saref.etsi.org/saref4inma/ID"/>
        <rdfs:comment>International Registration Data Identifier (IRDI) is based on the international standards ISO/IEC 11179-6, ISO 29002 and ISO 6532 and used in eCl@ss and the Asset Administration Shell as unique identifier.</rdfs:comment>
        <rdfs:label xml:lang="en">IRDI</rdfs:label>
    </owl:Class>
    


    <!-- https://saref.etsi.org/saref4inma/Item -->

    <owl:Class rdf:about="https://saref.etsi.org/saref4inma/Item">
        <rdfs:subClassOf rdf:resource="https://saref.etsi.org/core/FeatureOfInterest"/>
        <rdfs:subClassOf>
            <owl:Restriction>
                <owl:onProperty rdf:resource="https://saref.etsi.org/saref4inma/hasIdentifier"/>
                <owl:someValuesFrom rdf:resource="https://saref.etsi.org/saref4inma/ID"/>
            </owl:Restriction>
        </rdfs:subClassOf>
        <rdfs:subClassOf>
            <owl:Restriction>
                <owl:onProperty rdf:resource="https://saref.etsi.org/saref4inma/consistsOfItem"/>
                <owl:allValuesFrom rdf:resource="https://saref.etsi.org/saref4inma/Item"/>
            </owl:Restriction>
        </rdfs:subClassOf>
        <rdfs:subClassOf>
            <owl:Restriction>
                <owl:onProperty rdf:resource="https://saref.etsi.org/saref4inma/hasIdentifier"/>
                <owl:allValuesFrom rdf:resource="https://saref.etsi.org/saref4inma/ID"/>
            </owl:Restriction>
        </rdfs:subClassOf>
        <rdfs:subClassOf>
            <owl:Restriction>
                <owl:onProperty rdf:resource="https://saref.etsi.org/saref4inma/isCreatedIn"/>
                <owl:allValuesFrom rdf:resource="https://saref.etsi.org/saref4inma/ItemBatch"/>
            </owl:Restriction>
        </rdfs:subClassOf>
        <rdfs:subClassOf>
            <owl:Restriction>
                <owl:onProperty rdf:resource="https://saref.etsi.org/saref4inma/isFeatureOfInterestOf"/>
                <owl:allValuesFrom rdf:resource="https://saref.etsi.org/saref4inma/Measurement"/>
            </owl:Restriction>
        </rdfs:subClassOf>
        <rdfs:subClassOf>
            <owl:Restriction>
                <owl:onProperty rdf:resource="https://saref.etsi.org/saref4inma/isCreatedIn"/>
                <owl:qualifiedCardinality rdf:datatype="http://www.w3.org/2001/XMLSchema#nonNegativeInteger">1</owl:qualifiedCardinality>
                <owl:onClass rdf:resource="https://saref.etsi.org/saref4inma/ItemBatch"/>
            </owl:Restriction>
        </rdfs:subClassOf>
        <rdfs:subClassOf>
            <owl:Restriction>
                <owl:onProperty rdf:resource="https://saref.etsi.org/saref4inma/hasIDValue"/>
                <owl:allValuesFrom rdf:resource="http://www.w3.org/2001/XMLSchema#string"/>
            </owl:Restriction>
        </rdfs:subClassOf>
        <rdfs:subClassOf>
            <owl:Restriction>
                <owl:onProperty rdf:resource="https://saref.etsi.org/saref4inma/hasSerialNumber"/>
                <owl:maxQualifiedCardinality rdf:datatype="http://www.w3.org/2001/XMLSchema#nonNegativeInteger">1</owl:maxQualifiedCardinality>
                <owl:onDataRange rdf:resource="http://www.w3.org/2001/XMLSchema#string"/>
            </owl:Restriction>
        </rdfs:subClassOf>
        <rdfs:comment>A tangible object which can be unique identified, for example, with a GTIN in the form of a barcode/QR/RFID tag. An item product can be the result of the organization&apos;s production process (i.e. outflow of objects/goods) or can be uniquely identifiable material (i.e. inflow of objects/supplies). Each item is part of exactly one ItemBatch, whereas each ItemBatch contains only Items which have similar properties. An item can consists of multiple Batches and other Items (i.e. subassemblies).</rdfs:comment>
        <rdfs:label xml:lang="en">Item</rdfs:label>
    </owl:Class>
    


    <!-- https://saref.etsi.org/saref4inma/ItemBatch -->

    <owl:Class rdf:about="https://saref.etsi.org/saref4inma/ItemBatch">
        <rdfs:subClassOf rdf:resource="https://saref.etsi.org/saref4inma/Batch"/>
        <rdfs:subClassOf>
            <owl:Restriction>
                <owl:onProperty rdf:resource="https://saref.etsi.org/saref4inma/belongsToCategory"/>
                <owl:allValuesFrom rdf:resource="https://saref.etsi.org/saref4inma/ItemCategory"/>
            </owl:Restriction>
        </rdfs:subClassOf>
        <rdfs:subClassOf>
            <owl:Restriction>
                <owl:onProperty rdf:resource="https://saref.etsi.org/saref4inma/creates"/>
                <owl:allValuesFrom rdf:resource="https://saref.etsi.org/saref4inma/Item"/>
            </owl:Restriction>
        </rdfs:subClassOf>
        <rdfs:comment>A uniform collection of tangible objects which are relevant for the prodcution process. The ItemBatch consists of a set of objects with similar properties (e.g. a certain type of sensors or metal sheets). The difference between ItemBatch and MaterialBatch is that individual items can be traced in a ItemBatch, whereas this is not possible in a MaterialBatch, meaning that, for example, it is possible to trace the individual metal sheet used in a ItemBatch. This implies that the objects in an ItemBatch have an unique identifier (e.g. a GTIN code in the form of a barcode/QR-code or RFID tag).</rdfs:comment>
        <rdfs:label xml:lang="en">Item Batch</rdfs:label>
    </owl:Class>
    


    <!-- https://saref.etsi.org/saref4inma/ItemCategory -->

    <owl:Class rdf:about="https://saref.etsi.org/saref4inma/ItemCategory">
        <rdfs:subClassOf>
            <owl:Restriction>
                <owl:onProperty rdf:resource="https://saref.etsi.org/saref4inma/hasIdentifier"/>
                <owl:someValuesFrom rdf:resource="https://saref.etsi.org/saref4inma/ID"/>
            </owl:Restriction>
        </rdfs:subClassOf>
        <rdfs:subClassOf>
            <owl:Restriction>
                <owl:onProperty rdf:resource="https://saref.etsi.org/saref4inma/hasIdentifier"/>
                <owl:allValuesFrom rdf:resource="https://saref.etsi.org/saref4inma/ID"/>
            </owl:Restriction>
        </rdfs:subClassOf>
        <rdfs:subClassOf>
            <owl:Restriction>
                <owl:onProperty rdf:resource="https://saref.etsi.org/saref4inma/hasUpdate"/>
                <owl:allValuesFrom rdf:resource="https://saref.etsi.org/saref4inma/ItemCategory"/>
            </owl:Restriction>
        </rdfs:subClassOf>
        <rdfs:subClassOf>
            <owl:Restriction>
                <owl:onProperty rdf:resource="https://saref.etsi.org/saref4inma/isCategoryOf"/>
                <owl:allValuesFrom rdf:resource="https://saref.etsi.org/saref4inma/ItemBatch"/>
            </owl:Restriction>
        </rdfs:subClassOf>
        <rdfs:subClassOf>
            <owl:Restriction>
                <owl:onProperty rdf:resource="https://saref.etsi.org/saref4inma/isProducedBy"/>
                <owl:allValuesFrom rdf:resource="https://saref.etsi.org/saref4inma/ProductionEquipmentCategory"/>
            </owl:Restriction>
        </rdfs:subClassOf>
        <rdfs:subClassOf>
            <owl:Restriction>
                <owl:onProperty rdf:resource="https://saref.etsi.org/saref4inma/hasModelNumber"/>
                <owl:maxQualifiedCardinality rdf:datatype="http://www.w3.org/2001/XMLSchema#nonNegativeInteger">1</owl:maxQualifiedCardinality>
                <owl:onDataRange rdf:resource="http://www.w3.org/2001/XMLSchema#string"/>
            </owl:Restriction>
        </rdfs:subClassOf>
        <rdfs:subClassOf>
            <owl:Restriction>
                <owl:onProperty rdf:resource="https://saref.etsi.org/saref4inma/hasVersion"/>
                <owl:maxQualifiedCardinality rdf:datatype="http://www.w3.org/2001/XMLSchema#nonNegativeInteger">1</owl:maxQualifiedCardinality>
                <owl:onDataRange rdf:resource="http://www.w3.org/2001/XMLSchema#string"/>
            </owl:Restriction>
        </rdfs:subClassOf>
        <rdfs:comment>An ItemCategory describes a single type of item in terms of its static properties. Each ItemCategory can have multiple related ItemBatches, which all contain individual Items. The essential properties of each Item in all ItemBatches are the same. However, each batch might use different MaterialBatches and/or different ProductionEquipment. Therefore, small deviations between batches might occur, while the essential properties of all Items related to an ItemCategory are similar.</rdfs:comment>
        <rdfs:label xml:lang="en">Item category</rdfs:label>
    </owl:Class>
    


    <!-- https://saref.etsi.org/saref4inma/MaterialBatch -->

    <owl:Class rdf:about="https://saref.etsi.org/saref4inma/MaterialBatch">
        <rdfs:subClassOf rdf:resource="https://saref.etsi.org/saref4inma/Batch"/>
        <rdfs:subClassOf>
            <owl:Restriction>
                <owl:onProperty rdf:resource="https://saref.etsi.org/saref4inma/belongsToCategory"/>
                <owl:allValuesFrom rdf:resource="https://saref.etsi.org/saref4inma/MaterialCategory"/>
            </owl:Restriction>
        </rdfs:subClassOf>
        <rdfs:subClassOf>
            <owl:Restriction>
                <owl:onProperty rdf:resource="https://saref.etsi.org/saref4inma/hasCertificate"/>
                <owl:allValuesFrom rdf:resource="http://www.w3.org/2001/XMLSchema#string"/>
            </owl:Restriction>
        </rdfs:subClassOf>
        <rdfs:comment>A uniform collection of tangible raw material which are relevant for the prodcution process. The MaterialBatch can consists of a set of objects with similar properties (e.g. a certain type of screws) or a stock of homogeen material (e.g. oil, water). The difference between MaterialBatch and ItemBatch is that individual items cannot be traced in a MaterialBatch, whereas this is possible in an ItemBatch, meaning that, for example, it is not possible to trace the individual screw used in a MaterialBatch.</rdfs:comment>
        <rdfs:label xml:lang="en">Material Batch</rdfs:label>
    </owl:Class>
    


    <!-- https://saref.etsi.org/saref4inma/MaterialCategory -->

    <owl:Class rdf:about="https://saref.etsi.org/saref4inma/MaterialCategory">
        <rdfs:subClassOf>
            <owl:Restriction>
                <owl:onProperty rdf:resource="https://saref.etsi.org/saref4inma/isCategoryOf"/>
                <owl:allValuesFrom rdf:resource="https://saref.etsi.org/saref4inma/MaterialBatch"/>
            </owl:Restriction>
        </rdfs:subClassOf>
        <rdfs:comment>A MaterialCategory describes a category of material in terms of its static properties. Examples are: a certain category of steel or plastic. Each MaterialCategory can have multiple related MaterialBatches, which represent the physical material. The essential properties of the material in all MaterialBatches are the same. However, each batch might use different MaterialBatches and/or different ProductionEquipment. Therefore, small deviations between batches might occur, while the essential properties of the material related to an MaterialCategory are similar.</rdfs:comment>
        <rdfs:label xml:lang="en">Material category</rdfs:label>
    </owl:Class>
    


    <!-- https://saref.etsi.org/saref4inma/Measurement -->

    <owl:Class rdf:about="https://saref.etsi.org/saref4inma/Measurement">
        <rdfs:subClassOf rdf:resource="https://saref.etsi.org/core/Measurement"/>
        <rdfs:subClassOf>
            <owl:Restriction>
                <owl:onProperty rdf:resource="https://saref.etsi.org/saref4inma/hasFeatureOfInterest"/>
                <owl:allValuesFrom>
                    <owl:Class>
                        <owl:unionOf rdf:parseType="Collection">
                            <rdf:Description rdf:about="https://saref.etsi.org/saref4inma/Batch"/>
                            <rdf:Description rdf:about="https://saref.etsi.org/saref4inma/Item"/>
                        </owl:unionOf>
                    </owl:Class>
                </owl:allValuesFrom>
            </owl:Restriction>
        </rdfs:subClassOf>
        <rdfs:comment>A subclass of saref:Measurement that represents the measured value made over a property. It is also linked to the unit of measure in which the value is expressed and the timestamp of the measurement. The saref4imna:Measurement can be linked to individual Batches or Items. Moreover, the Measurement can be an ExpectedMeasurement (i.e. the value which is planned) or the ActualMeasurement (i.e. the value measured during production), which enables to check for deviations between the planned and actual values.</rdfs:comment>
        <rdfs:label xml:lang="en">Measurement</rdfs:label>
    </owl:Class>
    


    <!-- https://saref.etsi.org/saref4inma/ProductionEquipment -->

    <owl:Class rdf:about="https://saref.etsi.org/saref4inma/ProductionEquipment">
        <rdfs:subClassOf rdf:resource="https://saref.etsi.org/core/Device"/>
        <rdfs:subClassOf rdf:resource="https://saref.etsi.org/saref4bldg/PhysicalObject"/>
        <rdfs:subClassOf>
            <owl:Restriction>
                <owl:onProperty rdf:resource="https://saref.etsi.org/core/hasFunction"/>
                <owl:allValuesFrom rdf:resource="https://saref.etsi.org/saref4inma/ProductionEquipmentFunction"/>
            </owl:Restriction>
        </rdfs:subClassOf>
        <rdfs:subClassOf>
            <owl:Restriction>
                <owl:onProperty rdf:resource="https://saref.etsi.org/core/hasState"/>
                <owl:allValuesFrom rdf:resource="https://saref.etsi.org/core/State"/>
            </owl:Restriction>
        </rdfs:subClassOf>
        <rdfs:subClassOf>
            <owl:Restriction>
                <owl:onProperty rdf:resource="https://saref.etsi.org/core/makesMeasurement"/>
                <owl:allValuesFrom rdf:resource="https://saref.etsi.org/saref4inma/Measurement"/>
            </owl:Restriction>
        </rdfs:subClassOf>
        <rdfs:subClassOf>
            <owl:Restriction>
                <owl:onProperty rdf:resource="https://saref.etsi.org/core/measuresProperty"/>
                <owl:allValuesFrom rdf:resource="https://saref.etsi.org/core/Property"/>
            </owl:Restriction>
        </rdfs:subClassOf>
        <rdfs:subClassOf>
            <owl:Restriction>
                <owl:onProperty rdf:resource="https://saref.etsi.org/saref4inma/belongsToCategory"/>
                <owl:allValuesFrom rdf:resource="https://saref.etsi.org/saref4inma/ProductionEquipmentCategory"/>
            </owl:Restriction>
        </rdfs:subClassOf>
        <rdfs:subClassOf>
            <owl:Restriction>
                <owl:onProperty rdf:resource="https://saref.etsi.org/saref4inma/hasIdentifier"/>
                <owl:allValuesFrom rdf:resource="https://saref.etsi.org/saref4inma/ID"/>
            </owl:Restriction>
        </rdfs:subClassOf>
        <rdfs:subClassOf>
            <owl:Restriction>
                <owl:onProperty rdf:resource="https://saref.etsi.org/saref4inma/hasIDValue"/>
                <owl:allValuesFrom rdf:resource="http://www.w3.org/2001/XMLSchema#string"/>
            </owl:Restriction>
        </rdfs:subClassOf>
        <rdfs:comment>A production equipment is a specialization of a saref:Device and s4bldg:PhysicalObject that can produce items in a manufacturing process. This class represents an individual production equipment device and includes their specification in terms of functions, states and services. Different types of machines can be defined under this class as needed, for example, LaserCuttingMachine (i.e., a type of production equipment to cut steel material), MillingMachine (i.e., to drill holes in steel material), MouldingMachine (i.e., to mold liquid material, such as iron or plastic, and let it harden in a certain shape), WeldingMachine (i.e., join parts of material, such as steel, together), etc.</rdfs:comment>
        <rdfs:label xml:lang="en">ProductionEquipment</rdfs:label>
    </owl:Class>
    


    <!-- https://saref.etsi.org/saref4inma/ProductionEquipmentCategory -->

    <owl:Class rdf:about="https://saref.etsi.org/saref4inma/ProductionEquipmentCategory">
        <rdfs:subClassOf>
            <owl:Restriction>
                <owl:onProperty rdf:resource="https://saref.etsi.org/saref4inma/isCategoryOf"/>
                <owl:allValuesFrom rdf:resource="https://saref.etsi.org/saref4inma/ProductionEquipment"/>
            </owl:Restriction>
        </rdfs:subClassOf>
        <rdfs:subClassOf>
            <owl:Restriction>
                <owl:onProperty rdf:resource="https://saref.etsi.org/saref4inma/hasModelNumber"/>
                <owl:maxQualifiedCardinality rdf:datatype="http://www.w3.org/2001/XMLSchema#nonNegativeInteger">1</owl:maxQualifiedCardinality>
                <owl:onDataRange rdf:resource="http://www.w3.org/2001/XMLSchema#string"/>
            </owl:Restriction>
        </rdfs:subClassOf>
        <rdfs:comment>A ProductionEquipmentCategory represents a certain type of production equipment, which is generally static over time. More concretely, the ProductionEquipmentCategory represents a certain model and brand of a production equipment. Each ProductionEquipmentCategory can have multiple related ProductionEquipment, which represent the actual individual machines. Moreover, each ItemCategory can be produced by multiple ProductionEquipmentCategories.</rdfs:comment>
        <rdfs:label xml:lang="en">Production equipment category</rdfs:label>
    </owl:Class>
    


    <!-- https://saref.etsi.org/saref4inma/ProductionEquipmentFunction -->

    <owl:Class rdf:about="https://saref.etsi.org/saref4inma/ProductionEquipmentFunction">
        <rdfs:subClassOf rdf:resource="http://www.w3.org/2002/07/owl#Thing"/>
        <rdfs:subClassOf rdf:resource="https://saref.etsi.org/core/Function"/>
        <rdfs:comment>Functionallity neccessary to accomplish the task for which a production equipment is designed.</rdfs:comment>
        <rdfs:label xml:lang="en">Production equipment function</rdfs:label>
    </owl:Class>
    


    <!-- https://saref.etsi.org/saref4inma/Site -->

    <owl:Class rdf:about="https://saref.etsi.org/saref4inma/Site">
        <rdfs:subClassOf rdf:resource="https://saref.etsi.org/saref4bldg/BuildingSpace"/>
        <owl:disjointWith rdf:resource="https://saref.etsi.org/saref4inma/WorkCenter"/>
        <rdfs:comment>A subclass of s4bldg:BuildingSpace used to define the physical spaces of the building. According to IEC 62264, sites are identified physical, geographical, and/or logical component groupings of a manufacturing enterprise. A factory can be divided in sites, whereas sites can be divided areas</rdfs:comment>
        <rdfs:label xml:lang="en">Site</rdfs:label>
    </owl:Class>
    


    <!-- https://saref.etsi.org/saref4inma/Size -->

    <owl:Class rdf:about="https://saref.etsi.org/saref4inma/Size">
        <rdfs:subClassOf rdf:resource="https://saref.etsi.org/core/Property"/>
        <rdfs:comment>The amount of certain objects in a collection (e.g., size of a material batch).</rdfs:comment>
        <rdfs:label xml:lang="en">Size</rdfs:label>
    </owl:Class>
    


    <!-- https://saref.etsi.org/saref4inma/UUID -->

    <owl:Class rdf:about="https://saref.etsi.org/saref4inma/UUID">
        <rdfs:subClassOf rdf:resource="https://saref.etsi.org/saref4inma/ID"/>
        <rdfs:comment>A universally unique identifier (UUID) is a 128-bit number used to identify items and is also known as: globally unique identifier (GUID). In its canonical textual representation, the sixteen octets of a UUID are represented as 32 hexadecimal (base 16) digits, displayed in five groups separated by hyphens, in the form 8-4-4-4-12 for a total of 36 characters (32 alphanumeric characters and four hyphens). UUID are documented in ISO/IEC 11578:1996 &quot;Information technology  Open Systems Interconnection  Remote Procedure Call (RPC)&quot; and in ITU-T Rec. X.667 | ISO/IEC 9834-8:2005.</rdfs:comment>
        <rdfs:label xml:lang="en">UUID</rdfs:label>
    </owl:Class>
    


    <!-- https://saref.etsi.org/saref4inma/WorkCenter -->

    <owl:Class rdf:about="https://saref.etsi.org/saref4inma/WorkCenter">
        <rdfs:subClassOf rdf:resource="https://saref.etsi.org/saref4inma/ProductionEquipment"/>
        <rdfs:comment>A subclass of s4inma:ProductionEquipment (and therefore of s4bld:PhysicalObject). It is an equipment element under an area in a role-based equipment hierarchy that performs production, storage or material movement (definition taken from IEC 62264). An Area contains work centers.</rdfs:comment>
        <rdfs:label xml:lang="en">Work center</rdfs:label>
    </owl:Class>
    


    <!-- https://saref.etsi.org/saref4syst/System -->

    <owl:Class rdf:about="https://saref.etsi.org/saref4syst/System"/>
    


    <!-- 
    ///////////////////////////////////////////////////////////////////////////////////////
    //
    // Individuals
    //
    ///////////////////////////////////////////////////////////////////////////////////////
     -->

    


    <!-- http://qudt.org/vocab/quantitykind/Dimensionless -->

    <owl:NamedIndividual rdf:about="http://qudt.org/vocab/quantitykind/Dimensionless">
        <rdf:type rdf:resource="https://ega.industry.com/ontologies/core/data/DimensionlessProperty"/>
        <rdf:type rdf:resource="https://saref.etsi.org/core/Property"/>
        <core:isPropertyOf rdf:resource="https://ega.industry.com/ontologies/core/asset/furnace_10"/>
        <core:isPropertyOf rdf:resource="https://ega.industry.com/ontologies/core/asset/furnace_12"/>
        <terms:description rdf:datatype="http://qudt.org/schema/qudt/LatexString">In dimensional analysis, a dimensionless quantity or quantity of dimension one is a quantity without an associated physical dimension. It is thus a &quot;pure&quot; number, and as such always has a dimension of 1. Dimensionless quantities are widely used in mathematics, physics, engineering, economics, and in everyday life (such as in counting). Numerous well-known quantities, such as $\pi$, $\epsilon$, and $\psi$, are dimensionless. By contrast, non-dimensionless quantities are measured in units of length, area, time, etc. Dimensionless quantities are often defined as products or ratios of quantities that are not dimensionless, but whose dimensions cancel out when their powers are multiplied.</terms:description>
        <qudt:dbpediaMatch rdf:datatype="http://www.w3.org/2001/XMLSchema#anyURI">http://dbpedia.org/resource/Dimensionless_quantity</qudt:dbpediaMatch>
        <qudt:informativeReference rdf:datatype="http://www.w3.org/2001/XMLSchema#anyURI">http://en.wikipedia.org/wiki/Dimensionless_quantity</qudt:informativeReference>
        <qudt:symbol>U</qudt:symbol>
        <rdfs:comment>Applicable units are those of quantitykind:Dimensionless</rdfs:comment>
        <rdfs:isDefinedBy rdf:resource="http://qudt.org/3.1.1/vocab/quantitykind"/>
        <rdfs:label xml:lang="en">Dimensionless</rdfs:label>
    </owl:NamedIndividual>
    


    <!-- http://qudt.org/vocab/quantitykind/DimensionlessRatio -->

    <owl:NamedIndividual rdf:about="http://qudt.org/vocab/quantitykind/DimensionlessRatio">
        <rdf:type rdf:resource="https://ega.industry.com/ontologies/core/data/DimensionlessRatioProperty"/>
        <rdf:type rdf:resource="https://saref.etsi.org/core/Property"/>
        <core:isPropertyOf rdf:resource="https://ega.industry.com/ontologies/core/asset/airSupply_10"/>
        <core:isPropertyOf rdf:resource="https://ega.industry.com/ontologies/core/asset/airSupply_12"/>
        <core:isPropertyOf rdf:resource="https://ega.industry.com/ontologies/core/asset/tank_10"/>
        <core:isPropertyOf rdf:resource="https://ega.industry.com/ontologies/core/asset/tank_12"/>
        <rdfs:comment>Applicable units are those of quantitykind:DimensionlessRatio</rdfs:comment>
        <rdfs:isDefinedBy rdf:resource="http://qudt.org/3.1.1/vocab/quantitykind"/>
        <rdfs:label xml:lang="en">Dimensionless Ratio</rdfs:label>
    </owl:NamedIndividual>
    


    <!-- http://qudt.org/vocab/quantitykind/ElectricCurrent -->

    <owl:NamedIndividual rdf:about="http://qudt.org/vocab/quantitykind/ElectricCurrent">
        <rdf:type rdf:resource="https://ega.industry.com/ontologies/core/data/ElectricCurrentProperty"/>
        <rdf:type rdf:resource="https://saref.etsi.org/core/Property"/>
        <terms:description rdf:datatype="http://www.w3.org/1999/02/22-rdf-syntax-ns#HTML">
  The quantity kind $\textit{Electric Current}$ is the flow (movement) of electric charge. 
  The amount of electric current through some surface, for example, a section through a copper conductor,
   is defined as the amount of electric charge flowing through that surface over time. 
  Current is a scalar-valued quantity. 
  Electric current is one of the base quantities in the International System of Quantities, ISQ,
   on which the International System of Units, SI, is based.
  </terms:description>
        <qudt:dbpediaMatch rdf:datatype="http://www.w3.org/2001/XMLSchema#anyURI">http://dbpedia.org/resource/Electric_current</qudt:dbpediaMatch>
        <qudt:informativeReference rdf:datatype="http://www.w3.org/2001/XMLSchema#anyURI">http://www.iso.org/iso/home/store/catalogue_tc/catalogue_detail.htm?csnumber=31891</qudt:informativeReference>
        <qudt:informativeReference rdf:datatype="http://www.w3.org/2001/XMLSchema#anyURI">https://cdd.iec.ch/cdd/iec61987/iec61987.nsf/ListsOfUnitsAllVersions/0112-2---62720%23UAD039</qudt:informativeReference>
        <qudt:symbol>I</qudt:symbol>
        <rdfs:comment>Applicable units are those of quantitykind:ElectricCurrent</rdfs:comment>
        <rdfs:isDefinedBy rdf:resource="http://qudt.org/3.1.1/vocab/quantitykind"/>
        <rdfs:label xml:lang="en">electric current</rdfs:label>
    </owl:NamedIndividual>
    


    <!-- http://qudt.org/vocab/quantitykind/Power -->

    <owl:NamedIndividual rdf:about="http://qudt.org/vocab/quantitykind/Power">
        <rdf:type rdf:resource="https://ega.industry.com/ontologies/core/data/PowerProperty"/>
        <rdf:type rdf:resource="https://saref.etsi.org/core/Property"/>
        <terms:description rdf:datatype="http://qudt.org/schema/qudt/LatexString">Power is the rate at which work is performed or energy is transmitted, or the amount of energy required or expended for a given unit of time. As a rate of change of work done or the energy of a subsystem, power is: $P = W/t$, where $P$ is power, $W$ is work and {t} is time.</terms:description>
        <qudt:dbpediaMatch rdf:datatype="http://www.w3.org/2001/XMLSchema#anyURI">http://dbpedia.org/resource/Power</qudt:dbpediaMatch>
        <qudt:informativeReference rdf:datatype="http://www.w3.org/2001/XMLSchema#anyURI">http://en.wikipedia.org/wiki/Power</qudt:informativeReference>
        <qudt:informativeReference rdf:datatype="http://www.w3.org/2001/XMLSchema#anyURI">http://en.wikipedia.org/wiki/Power_%28physics%29</qudt:informativeReference>
        <qudt:symbol>P</qudt:symbol>
        <rdfs:comment>Applicable units are those of quantitykind:Power</rdfs:comment>
        <rdfs:isDefinedBy rdf:resource="http://qudt.org/3.1.1/vocab/quantitykind"/>
        <rdfs:label xml:lang="en">power</rdfs:label>
    </owl:NamedIndividual>
    


    <!-- http://qudt.org/vocab/quantitykind/Pressure -->

    <owl:NamedIndividual rdf:about="http://qudt.org/vocab/quantitykind/Pressure">
        <rdf:type rdf:resource="https://ega.industry.com/ontologies/core/data/PressureProperty"/>
        <rdf:type rdf:resource="https://saref.etsi.org/core/Property"/>
        <core:isPropertyOf rdf:resource="https://ega.industry.com/ontologies/core/asset/furnace_10"/>
        <core:isPropertyOf rdf:resource="https://ega.industry.com/ontologies/core/asset/furnace_12"/>
        <terms:description rdf:datatype="http://qudt.org/schema/qudt/LatexString">Pressure is an effect which occurs when a force is applied on a surface. Pressure is the amount of force acting on a unit area. Pressure is distinct from stress, as the former is the ratio of the component of force normal to a surface to the surface area. Stress is a tensor that relates the vector force to the vector area.</terms:description>
        <qudt:dbpediaMatch rdf:datatype="http://www.w3.org/2001/XMLSchema#anyURI">http://dbpedia.org/resource/Pressure</qudt:dbpediaMatch>
        <qudt:informativeReference rdf:datatype="http://www.w3.org/2001/XMLSchema#anyURI">http://en.wikipedia.org/wiki/Pressure</qudt:informativeReference>
        <qudt:informativeReference rdf:datatype="http://www.w3.org/2001/XMLSchema#anyURI">https://cdd.iec.ch/cdd/iec61987/iec61987.nsf/ListsOfUnitsAllVersions/0112-2---62720%23UAD142</qudt:informativeReference>
        <rdfs:comment>Applicable units are those of quantitykind:ForcePerArea</rdfs:comment>
        <rdfs:isDefinedBy rdf:resource="http://qudt.org/3.1.1/vocab/quantitykind"/>
        <rdfs:label xml:lang="en">pressure</rdfs:label>
    </owl:NamedIndividual>
    


    <!-- http://qudt.org/vocab/quantitykind/Speed -->

    <owl:NamedIndividual rdf:about="http://qudt.org/vocab/quantitykind/Speed">
        <rdf:type rdf:resource="https://ega.industry.com/ontologies/core/data/SpeedProperty"/>
        <rdf:type rdf:resource="https://saref.etsi.org/core/Property"/>
        <terms:description rdf:datatype="http://qudt.org/schema/qudt/LatexString">Speed is the magnitude of velocity.</terms:description>
        <qudt:dbpediaMatch rdf:datatype="http://www.w3.org/2001/XMLSchema#anyURI">http://dbpedia.org/resource/Speed</qudt:dbpediaMatch>
        <rdfs:comment>Applicable units are those of quantitykind:Speed</rdfs:comment>
        <rdfs:isDefinedBy rdf:resource="http://qudt.org/3.1.1/vocab/quantitykind"/>
        <rdfs:label xml:lang="en">Speed</rdfs:label>
    </owl:NamedIndividual>
    


    <!-- http://qudt.org/vocab/quantitykind/Temperature -->

    <owl:NamedIndividual rdf:about="http://qudt.org/vocab/quantitykind/Temperature">
        <rdf:type rdf:resource="https://ega.industry.com/ontologies/core/data/TemperatureProperty"/>
        <rdf:type rdf:resource="https://saref.etsi.org/core/Property"/>
        <core:isPropertyOf rdf:resource="https://ega.industry.com/ontologies/core/asset/furnace_10"/>
        <core:isPropertyOf rdf:resource="https://ega.industry.com/ontologies/core/asset/furnace_12"/>
        <core:isPropertyOf rdf:resource="https://ega.industry.com/ontologies/core/asset/tank_10"/>
        <core:isPropertyOf rdf:resource="https://ega.industry.com/ontologies/core/asset/tank_12"/>
        <terms:description rdf:datatype="http://qudt.org/schema/qudt/LatexString">Temperature is a physical property of matter that quantitatively expresses the common notions of hot and cold. Objects of low temperature are cold, while various degrees of higher temperatures are referred to as warm or hot. Heat spontaneously flows from bodies of a higher temperature to bodies of lower temperature, at a rate that increases with the temperature difference and the thermal conductivity.</terms:description>
        <qudt:dbpediaMatch rdf:datatype="http://www.w3.org/2001/XMLSchema#anyURI">http://dbpedia.org/resource/Temperature</qudt:dbpediaMatch>
        <qudt:informativeReference rdf:datatype="http://www.w3.org/2001/XMLSchema#anyURI">https://cdd.iec.ch/cdd/iec61987/iec61987.nsf/ListsOfUnitsAllVersions/0112-2---62720%23UAD374</qudt:informativeReference>
        <rdfs:comment>Applicable units are those of quantitykind:Temperature</rdfs:comment>
        <rdfs:isDefinedBy rdf:resource="http://qudt.org/3.1.1/vocab/quantitykind"/>
        <rdfs:label xml:lang="en">Temperature</rdfs:label>
        <rdfs:seeAlso rdf:resource="http://qudt.org/vocab/quantitykind/ThermodynamicTemperature"/>
    </owl:NamedIndividual>
    


    <!-- http://qudt.org/vocab/quantitykind/VolumeFlowRate -->

    <owl:NamedIndividual rdf:about="http://qudt.org/vocab/quantitykind/VolumeFlowRate">
        <rdf:type rdf:resource="https://ega.industry.com/ontologies/core/data/VolumeFlowRateProperty"/>
        <rdf:type rdf:resource="https://saref.etsi.org/core/Property"/>
        <core:isPropertyOf rdf:resource="https://ega.industry.com/ontologies/core/asset/gasSupply_10"/>
        <core:isPropertyOf rdf:resource="https://ega.industry.com/ontologies/core/asset/gasSupply_12"/>
        <terms:description rdf:datatype="http://qudt.org/schema/qudt/LatexString">Volumetric Flow Rate, (also known as volume flow rate, rate of fluid flow or volume velocity) is the volume of fluid which passes through a given surface per unit time.</terms:description>
        <qudt:informativeReference rdf:datatype="http://www.w3.org/2001/XMLSchema#anyURI">http://en.wikipedia.org/wiki/Volumetric_flow_rate</qudt:informativeReference>
        <qudt:informativeReference rdf:datatype="http://www.w3.org/2001/XMLSchema#anyURI">https://cdd.iec.ch/cdd/iec61987/iec61987.nsf/ListsOfUnitsAllVersions/0112-2---62720%23UAD239</qudt:informativeReference>
        <qudt:symbol>q_V</qudt:symbol>
        <rdfs:comment>Applicable units are those of quantitykind:VolumeFlowRate</rdfs:comment>
        <rdfs:isDefinedBy rdf:resource="http://qudt.org/3.1.1/vocab/quantitykind"/>
        <rdfs:label xml:lang="en">Volume Flow Rate</rdfs:label>
    </owl:NamedIndividual>
    


    <!-- http://qudt.org/vocab/unit/CentiM3-PER-HR -->

    <owl:NamedIndividual rdf:about="http://qudt.org/vocab/unit/CentiM3-PER-HR">
        <rdf:type rdf:resource="https://ega.industry.com/ontologies/core/data/VolumeFlowRateUnit"/>
        <rdf:type rdf:resource="https://saref.etsi.org/core/UnitOfMeasure"/>
        <data:hasSymbol>cm/h</data:hasSymbol>
        <terms:description rdf:datatype="http://www.w3.org/1999/02/22-rdf-syntax-ns#HTML">0,000 001-fold of the power of the SI base unit metre with the exponent 3 divided by the unit hour</terms:description>
        <qudt:informativeReference rdf:datatype="http://www.w3.org/2001/XMLSchema#anyURI">https://cdd.iec.ch/cdd/iec62720/iec62720.nsf/Units/0112-2---62720%23UAA391</qudt:informativeReference>
        <qudt:symbol>cm/h</qudt:symbol>
        <rdfs:isDefinedBy rdf:resource="http://qudt.org/3.1.1/vocab/unit"/>
        <rdfs:label xml:lang="en">Cubic Centimetre per Hour</rdfs:label>
    </owl:NamedIndividual>
    


    <!-- http://qudt.org/vocab/unit/DEG_C -->

    <owl:NamedIndividual rdf:about="http://qudt.org/vocab/unit/DEG_C">
        <rdf:type rdf:resource="https://ega.industry.com/ontologies/core/data/TemperatureUnit"/>
        <rdf:type rdf:resource="https://saref.etsi.org/core/UnitOfMeasure"/>
        <data:hasSymbol>C</data:hasSymbol>
        <terms:description rdf:datatype="http://qudt.org/schema/qudt/LatexString">
  The unit $\textit{Celsius}$, also known as centigrade, is a scale and unit of measurement for temperature. 
  It can refer to a specific temperature on the Celsius scale as well as a unit to indicate a temperature interval, 
  a difference between two temperatures or an uncertainty. 
  This definition fixes the magnitude of both the degree Celsius and the kelvin as precisely 1 part 
  in 273.16 (approximately 0.00366) of the difference between absolute zero and the triple point of water. 
  Thus, it sets the magnitude of one degree Celsius and that of one kelvin as exactly the same. 
  Additionally, it establishes the difference between the two scales&apos; null points as being precisely $273.15^{\circ}\text{C}$.
  </terms:description>
        <qudt:dbpediaMatch rdf:datatype="http://www.w3.org/2001/XMLSchema#anyURI">http://dbpedia.org/resource/Celsius</qudt:dbpediaMatch>
        <qudt:expression rdf:datatype="http://qudt.org/schema/qudt/LatexString">$degC$</qudt:expression>
        <qudt:informativeReference rdf:datatype="http://www.w3.org/2001/XMLSchema#anyURI">http://en.wikipedia.org/wiki/Celsius?oldid=494152178</qudt:informativeReference>
        <qudt:informativeReference rdf:datatype="http://www.w3.org/2001/XMLSchema#anyURI">https://cdd.iec.ch/cdd/iec62720/iec62720.nsf/Units/0112-2---62720%23UAA033</qudt:informativeReference>
        <qudt:omUnit rdf:resource="http://www.ontology-of-units-of-measure.org/resource/om-2/degreeCelsius"/>
        <qudt:symbol>C</qudt:symbol>
        <rdfs:isDefinedBy rdf:resource="http://qudt.org/3.1.1/vocab/unit"/>
        <rdfs:label xml:lang="en">degree Celsius</rdfs:label>
    </owl:NamedIndividual>
    


    <!-- http://qudt.org/vocab/unit/K -->

    <owl:NamedIndividual rdf:about="http://qudt.org/vocab/unit/K">
        <rdf:type rdf:resource="https://ega.industry.com/ontologies/core/data/TemperatureUnit"/>
        <rdf:type rdf:resource="https://saref.etsi.org/core/UnitOfMeasure"/>
        <data:hasSymbol>K</data:hasSymbol>
        <terms:description rdf:datatype="http://qudt.org/schema/qudt/LatexString">
  The unit $\textit{Kelvin}$ is the SI base unit of temperature, previously called the degree Kelvin. 
  One kelvin represents the same temperature difference as one degree Celsius. 
  In 1967 the General Conference on Weights and Measures defined the temperature of the triple point of water
   (the temperature at which water exists simultaneously in the gaseous, liquid, and solid states) to be exactly 273.16 kelvins. 
  Since this temperature is also equal to 0.01 u00b0C, the temperature in kelvins is always equal to 273.15 plus the temperature in degrees Celsius. 
  The kelvin equals exactly 1.8 degrees Fahrenheit. 
  The unit is named for the British mathematician and physicist William Thomson (1824-1907),
   later known as Lord Kelvin after he was named Baron Kelvin of Largs.
  </terms:description>
        <qudt:dbpediaMatch rdf:datatype="http://www.w3.org/2001/XMLSchema#anyURI">http://dbpedia.org/resource/Kelvin</qudt:dbpediaMatch>
        <qudt:informativeReference rdf:datatype="http://www.w3.org/2001/XMLSchema#anyURI">http://en.wikipedia.org/wiki/Kelvin?oldid=495075694</qudt:informativeReference>
        <qudt:informativeReference rdf:datatype="http://www.w3.org/2001/XMLSchema#anyURI">https://cdd.iec.ch/cdd/iec62720/iec62720.nsf/Units/0112-2---62720%23UAA185</qudt:informativeReference>
        <qudt:omUnit rdf:resource="http://www.ontology-of-units-of-measure.org/resource/om-2/kelvin"/>
        <qudt:symbol>K</qudt:symbol>
        <rdfs:isDefinedBy rdf:resource="http://qudt.org/3.1.1/vocab/unit"/>
        <rdfs:label xml:lang="en">kelvin</rdfs:label>
    </owl:NamedIndividual>
    


    <!-- http://qudt.org/vocab/unit/MilliBAR -->

    <owl:NamedIndividual rdf:about="http://qudt.org/vocab/unit/MilliBAR">
        <rdf:type rdf:resource="https://ega.industry.com/ontologies/core/data/PressureUnit"/>
        <rdf:type rdf:resource="https://saref.etsi.org/core/UnitOfMeasure"/>
        <data:hasSymbol>mbar</data:hasSymbol>
        <terms:description rdf:datatype="http://qudt.org/schema/qudt/LatexString">The bar is a non-SI unit of pressure, defined by the IUPAC as exactly equal to 100,000 Pa. It is about equal to the atmospheric pressure on Earth at sea level, and since 1982 the IUPAC has recommended that the standard for atmospheric pressure should be harmonized to $100,000 Pa = 1 bar \approx 750.0616827 Torr$. Units derived from the bar are the megabar (symbol: Mbar), kilobar (symbol: kbar), decibar (symbol: dbar), centibar (symbol: cbar), and millibar (symbol: mbar or mb). They are not SI or cgs units, but they are accepted for use with the SI.</terms:description>
        <qudt:informativeReference rdf:datatype="http://www.w3.org/2001/XMLSchema#anyURI">http://en.wikipedia.org/wiki/Bar_(unit)</qudt:informativeReference>
        <qudt:informativeReference rdf:datatype="http://www.w3.org/2001/XMLSchema#anyURI">https://cdd.iec.ch/cdd/iec62720/iec62720.nsf/Units/0112-2---62720%23UAA810</qudt:informativeReference>
        <qudt:symbol>mbar</qudt:symbol>
        <rdfs:isDefinedBy rdf:resource="http://qudt.org/3.1.1/vocab/unit"/>
        <rdfs:label xml:lang="en">Millibar</rdfs:label>
    </owl:NamedIndividual>
    


    <!-- http://qudt.org/vocab/unit/NUM -->

    <owl:NamedIndividual rdf:about="http://qudt.org/vocab/unit/NUM">
        <rdf:type rdf:resource="https://ega.industry.com/ontologies/core/data/NumberUnit"/>
        <rdf:type rdf:resource="https://saref.etsi.org/core/UnitOfMeasure"/>
        <data:hasSymbol>#</data:hasSymbol>
        <terms:description rdf:datatype="http://www.w3.org/1999/02/22-rdf-syntax-ns#HTML">&quot;Number&quot; is a unit for  &apos;Dimensionless&apos; expressed as (\#$.</terms:description>
        <qudt:symbol>#</qudt:symbol>
        <rdfs:isDefinedBy rdf:resource="http://qudt.org/3.1.1/vocab/unit"/>
        <rdfs:label xml:lang="en">Number</rdfs:label>
    </owl:NamedIndividual>
    


    <!-- http://qudt.org/vocab/unit/PERCENT -->

    <owl:NamedIndividual rdf:about="http://qudt.org/vocab/unit/PERCENT">
        <rdf:type rdf:resource="https://ega.industry.com/ontologies/core/data/PercentUnit"/>
        <rdf:type rdf:resource="https://saref.etsi.org/core/UnitOfMeasure"/>
        <data:hasSymbol>%</data:hasSymbol>
        <terms:description rdf:datatype="http://qudt.org/schema/qudt/LatexString">&quot;Percent&quot; is a unit for  &apos;Dimensionless Ratio&apos; expressed as $\%$.</terms:description>
        <qudt:dbpediaMatch rdf:datatype="http://www.w3.org/2001/XMLSchema#anyURI">http://dbpedia.org/resource/Percentage</qudt:dbpediaMatch>
        <qudt:informativeReference rdf:datatype="http://www.w3.org/2001/XMLSchema#anyURI">http://en.wikipedia.org/wiki/Percentage?oldid=495284540</qudt:informativeReference>
        <qudt:informativeReference rdf:datatype="http://www.w3.org/2001/XMLSchema#anyURI">https://cdd.iec.ch/cdd/iec62720/iec62720.nsf/Units/0112-2---62720%23UAA000</qudt:informativeReference>
        <qudt:omUnit rdf:resource="http://www.ontology-of-units-of-measure.org/resource/om-2/percent"/>
        <qudt:symbol>%</qudt:symbol>
        <rdfs:isDefinedBy rdf:resource="http://qudt.org/3.1.1/vocab/unit"/>
        <rdfs:label xml:lang="en">Percent</rdfs:label>
    </owl:NamedIndividual>
    


    <!-- http://qudt.org/vocab/unit/W -->

    <owl:NamedIndividual rdf:about="http://qudt.org/vocab/unit/W">
        <rdf:type rdf:resource="https://ega.industry.com/ontologies/core/data/PowerUnit"/>
        <rdf:type rdf:resource="https://saref.etsi.org/core/UnitOfMeasure"/>
        <data:hasSymbol>W</data:hasSymbol>
        <terms:description rdf:datatype="http://www.w3.org/1999/02/22-rdf-syntax-ns#HTML">The SI unit of power. Power is the rate at which work is done, or (equivalently) the rate at which energy is expended. One watt is equal to a power rate of one joule of work per second of time. This unit is used both in mechanics and in electricity, so it links the mechanical and electrical units to one another. In mechanical terms, one watt equals about 0.001 341 02 horsepower (hp) or 0.737 562 foot-pound per second (lbf/s). In electrical terms, one watt is the power produced by a current of one ampere flowing through an electric potential of one volt. The name of the unit honors James Watt (1736-1819), the British engineer whose improvements to the steam engine are often credited with igniting the Industrial Revolution.</terms:description>
        <qudt:dbpediaMatch rdf:datatype="http://www.w3.org/2001/XMLSchema#anyURI">http://dbpedia.org/resource/Watt</qudt:dbpediaMatch>
        <qudt:informativeReference rdf:datatype="http://www.w3.org/2001/XMLSchema#anyURI">http://en.wikipedia.org/wiki/Watt?oldid=494906356</qudt:informativeReference>
        <qudt:informativeReference rdf:datatype="http://www.w3.org/2001/XMLSchema#anyURI">https://cdd.iec.ch/cdd/iec62720/iec62720.nsf/Units/0112-2---62720%23UAA306</qudt:informativeReference>
        <qudt:omUnit rdf:resource="http://www.ontology-of-units-of-measure.org/resource/om-2/watt"/>
        <qudt:symbol>W</qudt:symbol>
        <rdfs:isDefinedBy rdf:resource="http://qudt.org/3.1.1/vocab/unit"/>
        <rdfs:label xml:lang="en">watt</rdfs:label>
    </owl:NamedIndividual>
    


    <!-- https://ega.industry.com/ontologies/core/asset/AlloyAddition -->

    <owl:NamedIndividual rdf:about="https://ega.industry.com/ontologies/core/asset/AlloyAddition">
        <rdf:type rdf:resource="http://www.w3.org/2004/02/skos/core#ConceptScheme"/>
        <rdf:type rdf:resource="https://ega.industry.com/ontologies/core/asset/OpenReason"/>
        <rdf:type rdf:resource="https://ega.industry.com/ontologies/core/asset/Reason"/>
    </owl:NamedIndividual>
    


    <!-- https://ega.industry.com/ontologies/core/asset/AluminiumCharging -->

    <owl:NamedIndividual rdf:about="https://ega.industry.com/ontologies/core/asset/AluminiumCharging">
        <rdf:type rdf:resource="http://www.w3.org/2004/02/skos/core#ConceptScheme"/>
        <rdf:type rdf:resource="https://ega.industry.com/ontologies/core/asset/OpenReason"/>
        <rdf:type rdf:resource="https://ega.industry.com/ontologies/core/asset/Reason"/>
    </owl:NamedIndividual>
    


    <!-- https://ega.industry.com/ontologies/core/asset/CLOSE -->

    <owl:NamedIndividual rdf:about="https://ega.industry.com/ontologies/core/asset/CLOSE">
        <rdf:type rdf:resource="https://ega.industry.com/ontologies/core/asset/OpenCloseStateValue"/>
        <rdf:type rdf:resource="https://saref.etsi.org/core/StateValue"/>
        <rdfs:comment xml:lang="en">Represents the state where the mechanism or object is in the close position</rdfs:comment>
    </owl:NamedIndividual>
    


    <!-- https://ega.industry.com/ontologies/core/asset/OPEN -->

    <owl:NamedIndividual rdf:about="https://ega.industry.com/ontologies/core/asset/OPEN">
        <rdf:type rdf:resource="https://ega.industry.com/ontologies/core/asset/OpenCloseStateValue"/>
        <rdf:type rdf:resource="https://saref.etsi.org/core/StateValue"/>
        <rdfs:comment xml:lang="en">Represents the state where the mechanism or object is in the open position</rdfs:comment>
    </owl:NamedIndividual>
    


    <!-- https://ega.industry.com/ontologies/core/asset/Sampling -->

    <owl:NamedIndividual rdf:about="https://ega.industry.com/ontologies/core/asset/Sampling">
        <rdf:type rdf:resource="http://www.w3.org/2004/02/skos/core#ConceptScheme"/>
        <rdf:type rdf:resource="https://ega.industry.com/ontologies/core/asset/OpenReason"/>
        <rdf:type rdf:resource="https://ega.industry.com/ontologies/core/asset/Reason"/>
    </owl:NamedIndividual>
    


    <!-- https://ega.industry.com/ontologies/core/asset/ScrapCharging -->

    <owl:NamedIndividual rdf:about="https://ega.industry.com/ontologies/core/asset/ScrapCharging">
        <rdf:type rdf:resource="http://www.w3.org/2004/02/skos/core#ConceptScheme"/>
        <rdf:type rdf:resource="https://ega.industry.com/ontologies/core/asset/OpenReason"/>
        <rdf:type rdf:resource="https://ega.industry.com/ontologies/core/asset/Reason"/>
    </owl:NamedIndividual>
    


    <!-- https://ega.industry.com/ontologies/core/asset/Skimming -->

    <owl:NamedIndividual rdf:about="https://ega.industry.com/ontologies/core/asset/Skimming">
        <rdf:type rdf:resource="http://www.w3.org/2004/02/skos/core#ConceptScheme"/>
        <rdf:type rdf:resource="https://ega.industry.com/ontologies/core/asset/OpenReason"/>
        <rdf:type rdf:resource="https://ega.industry.com/ontologies/core/asset/Reason"/>
    </owl:NamedIndividual>
    


    <!-- https://ega.industry.com/ontologies/core/asset/Stirring -->

    <owl:NamedIndividual rdf:about="https://ega.industry.com/ontologies/core/asset/Stirring">
        <rdf:type rdf:resource="http://www.w3.org/2004/02/skos/core#ConceptScheme"/>
        <rdf:type rdf:resource="https://ega.industry.com/ontologies/core/asset/OpenReason"/>
        <rdf:type rdf:resource="https://ega.industry.com/ontologies/core/asset/Reason"/>
    </owl:NamedIndividual>
    


    <!-- https://ega.industry.com/ontologies/core/asset/Unknown -->

    <owl:NamedIndividual rdf:about="https://ega.industry.com/ontologies/core/asset/Unknown">
        <rdf:type rdf:resource="http://www.w3.org/2004/02/skos/core#ConceptScheme"/>
        <rdf:type rdf:resource="https://ega.industry.com/ontologies/core/asset/OpenReason"/>
        <rdf:type rdf:resource="https://ega.industry.com/ontologies/core/asset/Reason"/>
        <asset:isOpenReasonOf rdf:resource="https://ega.industry.com/ontologies/core/asset/stateOpenCloseDoor_10"/>
        <asset:isOpenReasonOf rdf:resource="https://ega.industry.com/ontologies/core/asset/stateOpenCloseDoor_12"/>
    </owl:NamedIndividual>
    


    <!-- https://ega.industry.com/ontologies/core/asset/airSupply_10 -->

    <owl:NamedIndividual rdf:about="https://ega.industry.com/ontologies/core/asset/airSupply_10">
        <rdf:type rdf:resource="https://ega.industry.com/ontologies/core/asset/AirSupply"/>
        <rdf:type rdf:resource="https://saref.etsi.org/core/Device"/>
        <rdf:type rdf:resource="https://saref.etsi.org/core/FeatureOfInterest"/>
        <rdf:type rdf:resource="https://saref.etsi.org/saref4syst/System"/>
        <asset:isPartOf rdf:resource="https://ega.industry.com/ontologies/core/asset/burner_10"/>
        <core:consistsOf rdf:resource="https://ega.industry.com/ontologies/core/asset/sensorFlowAir_10"/>
        <core:consistsOf rdf:resource="https://ega.industry.com/ontologies/core/asset/sensorOxygen_10"/>
        <core:hasProperty rdf:resource="http://qudt.org/vocab/quantitykind/DimensionlessRatio"/>
        <core:hasPropertyOfInterest rdf:resource="https://saref.etsi.org/core/propertyOfInterestConcentrationAirBurner_10"/>
        <rdfs:comment xml:lang="en">Burner Air Supply</rdfs:comment>
    </owl:NamedIndividual>
    


    <!-- https://ega.industry.com/ontologies/core/asset/airSupply_12 -->

    <owl:NamedIndividual rdf:about="https://ega.industry.com/ontologies/core/asset/airSupply_12">
        <rdf:type rdf:resource="https://ega.industry.com/ontologies/core/asset/AirSupply"/>
        <rdf:type rdf:resource="https://saref.etsi.org/core/Device"/>
        <rdf:type rdf:resource="https://saref.etsi.org/core/FeatureOfInterest"/>
        <rdf:type rdf:resource="https://saref.etsi.org/saref4syst/System"/>
        <asset:isPartOf rdf:resource="https://ega.industry.com/ontologies/core/asset/burner_12"/>
        <core:consistsOf rdf:resource="https://ega.industry.com/ontologies/core/asset/sensorFlowAir_12"/>
        <core:consistsOf rdf:resource="https://ega.industry.com/ontologies/core/asset/sensorOxygen_12"/>
        <core:hasProperty rdf:resource="http://qudt.org/vocab/quantitykind/DimensionlessRatio"/>
        <core:hasPropertyOfInterest rdf:resource="https://saref.etsi.org/core/propertyOfInterestConcentrationAirBurner_12"/>
        <rdfs:comment xml:lang="en">Burner Air Supply</rdfs:comment>
    </owl:NamedIndividual>
    


    <!-- https://ega.industry.com/ontologies/core/asset/burner_10 -->

    <owl:NamedIndividual rdf:about="https://ega.industry.com/ontologies/core/asset/burner_10">
        <rdf:type rdf:resource="https://ega.industry.com/ontologies/core/asset/Burner"/>
        <rdf:type rdf:resource="https://saref.etsi.org/core/Device"/>
        <rdf:type rdf:resource="https://saref.etsi.org/core/FeatureOfInterest"/>
        <rdf:type rdf:resource="https://saref.etsi.org/saref4syst/System"/>
        <asset:isPartOf rdf:resource="https://ega.industry.com/ontologies/core/asset/furnace_10"/>
        <core:consistsOf rdf:resource="https://ega.industry.com/ontologies/core/asset/airSupply_10"/>
        <core:consistsOf rdf:resource="https://ega.industry.com/ontologies/core/asset/gasSupply_10"/>
    </owl:NamedIndividual>
    


    <!-- https://ega.industry.com/ontologies/core/asset/burner_12 -->

    <owl:NamedIndividual rdf:about="https://ega.industry.com/ontologies/core/asset/burner_12">
        <rdf:type rdf:resource="https://ega.industry.com/ontologies/core/asset/Burner"/>
        <rdf:type rdf:resource="https://saref.etsi.org/core/Device"/>
        <rdf:type rdf:resource="https://saref.etsi.org/core/FeatureOfInterest"/>
        <rdf:type rdf:resource="https://saref.etsi.org/saref4syst/System"/>
        <asset:isPartOf rdf:resource="https://ega.industry.com/ontologies/core/asset/furnace_12"/>
        <core:consistsOf rdf:resource="https://ega.industry.com/ontologies/core/asset/airSupply_12"/>
        <core:consistsOf rdf:resource="https://ega.industry.com/ontologies/core/asset/gasSupply_12"/>
    </owl:NamedIndividual>
    


    <!-- https://ega.industry.com/ontologies/core/asset/castingSystem_10 -->

    <owl:NamedIndividual rdf:about="https://ega.industry.com/ontologies/core/asset/castingSystem_10">
        <rdf:type rdf:resource="https://ega.industry.com/ontologies/core/asset/CastingSystem"/>
        <rdf:type rdf:resource="https://ega.industry.com/ontologies/core/asset/IndustrySystem"/>
        <rdf:type rdf:resource="https://saref.etsi.org/saref4syst/System"/>
        <asset:isFedBy rdf:resource="https://ega.industry.com/ontologies/core/asset/furnace_10"/>
    </owl:NamedIndividual>
    


    <!-- https://ega.industry.com/ontologies/core/asset/castingSystem_12 -->

    <owl:NamedIndividual rdf:about="https://ega.industry.com/ontologies/core/asset/castingSystem_12">
        <rdf:type rdf:resource="https://ega.industry.com/ontologies/core/asset/CastingSystem"/>
        <rdf:type rdf:resource="https://ega.industry.com/ontologies/core/asset/IndustrySystem"/>
        <rdf:type rdf:resource="https://saref.etsi.org/saref4syst/System"/>
        <asset:isFedBy rdf:resource="https://ega.industry.com/ontologies/core/asset/furnace_12"/>
    </owl:NamedIndividual>
    


    <!-- https://ega.industry.com/ontologies/core/asset/coolingSystem_10 -->

    <owl:NamedIndividual rdf:about="https://ega.industry.com/ontologies/core/asset/coolingSystem_10">
        <rdf:type rdf:resource="https://ega.industry.com/ontologies/core/asset/CoolingSystem"/>
        <rdf:type rdf:resource="https://ega.industry.com/ontologies/core/asset/IndustrySystem"/>
        <rdf:type rdf:resource="https://saref.etsi.org/core/FeatureOfInterest"/>
        <rdf:type rdf:resource="https://saref.etsi.org/saref4syst/System"/>
        <asset:isPartOf rdf:resource="https://ega.industry.com/ontologies/core/asset/lining_10"/>
    </owl:NamedIndividual>
    


    <!-- https://ega.industry.com/ontologies/core/asset/coolingSystem_12 -->

    <owl:NamedIndividual rdf:about="https://ega.industry.com/ontologies/core/asset/coolingSystem_12">
        <rdf:type rdf:resource="https://ega.industry.com/ontologies/core/asset/CoolingSystem"/>
        <rdf:type rdf:resource="https://ega.industry.com/ontologies/core/asset/IndustrySystem"/>
        <rdf:type rdf:resource="https://saref.etsi.org/core/FeatureOfInterest"/>
        <rdf:type rdf:resource="https://saref.etsi.org/saref4syst/System"/>
        <asset:isPartOf rdf:resource="https://ega.industry.com/ontologies/core/asset/lining_12"/>
    </owl:NamedIndividual>
    


    <!-- https://ega.industry.com/ontologies/core/asset/door_10 -->

    <owl:NamedIndividual rdf:about="https://ega.industry.com/ontologies/core/asset/door_10">
        <rdf:type rdf:resource="https://ega.industry.com/ontologies/core/asset/Door"/>
        <rdf:type rdf:resource="https://saref.etsi.org/core/Device"/>
        <rdf:type rdf:resource="https://saref.etsi.org/core/FeatureOfInterest"/>
        <rdf:type rdf:resource="https://saref.etsi.org/saref4syst/System"/>
        <asset:isPartOf rdf:resource="https://ega.industry.com/ontologies/core/asset/furnace_10"/>
        <core:hasState rdf:resource="https://ega.industry.com/ontologies/core/asset/stateOpenCloseDoor_10"/>
        <rdfs:comment xml:lang="en">it&apos;is instance of Furnace Door</rdfs:comment>
    </owl:NamedIndividual>
    


    <!-- https://ega.industry.com/ontologies/core/asset/door_12 -->

    <owl:NamedIndividual rdf:about="https://ega.industry.com/ontologies/core/asset/door_12">
        <rdf:type rdf:resource="https://ega.industry.com/ontologies/core/asset/Door"/>
        <rdf:type rdf:resource="https://saref.etsi.org/core/Device"/>
        <rdf:type rdf:resource="https://saref.etsi.org/core/FeatureOfInterest"/>
        <rdf:type rdf:resource="https://saref.etsi.org/saref4syst/System"/>
        <asset:isPartOf rdf:resource="https://ega.industry.com/ontologies/core/asset/furnace_12"/>
        <core:hasState rdf:resource="https://ega.industry.com/ontologies/core/asset/stateOpenCloseDoor_12"/>
        <rdfs:comment xml:lang="en">it&apos;is instance of Furnace Door</rdfs:comment>
    </owl:NamedIndividual>
    


    <!-- https://ega.industry.com/ontologies/core/asset/furnace_10 -->

    <owl:NamedIndividual rdf:about="https://ega.industry.com/ontologies/core/asset/furnace_10">
        <rdf:type rdf:resource="https://ega.industry.com/ontologies/core/asset/Furnace"/>
        <rdf:type rdf:resource="https://saref.etsi.org/core/Device"/>
        <rdf:type rdf:resource="https://saref.etsi.org/core/FeatureOfInterest"/>
        <rdf:type rdf:resource="https://saref.etsi.org/saref4syst/System"/>
        <asset:feeds rdf:resource="https://ega.industry.com/ontologies/core/asset/castingSystem_10"/>
        <asset:hasProcess rdf:resource="https://ega.industry.com/ontologies/core/process/processFurnace_10"/>
        <asset:isFedBy rdf:resource="https://ega.industry.com/ontologies/core/asset/rawMaterialFeederSystem_10"/>
        <core:consistsOf rdf:resource="https://ega.industry.com/ontologies/core/asset/burner_10"/>
        <core:consistsOf rdf:resource="https://ega.industry.com/ontologies/core/asset/door_10"/>
        <core:consistsOf rdf:resource="https://ega.industry.com/ontologies/core/asset/sensorCastingStatusFurnace_10"/>
        <core:consistsOf rdf:resource="https://ega.industry.com/ontologies/core/asset/sensorPressureFurnace_10"/>
        <core:consistsOf rdf:resource="https://ega.industry.com/ontologies/core/asset/sensorTemperatureExhaustFurnace_10"/>
        <core:consistsOf rdf:resource="https://ega.industry.com/ontologies/core/asset/tank_10"/>
        <core:hasProperty rdf:resource="http://qudt.org/vocab/quantitykind/Dimensionless"/>
        <core:hasProperty rdf:resource="http://qudt.org/vocab/quantitykind/Pressure"/>
        <core:hasProperty rdf:resource="http://qudt.org/vocab/quantitykind/Temperature"/>
        <core:hasPropertyOfInterest rdf:resource="https://saref.etsi.org/core/propertyOfInterestCastingStatusFurnace_10"/>
        <core:hasPropertyOfInterest rdf:resource="https://saref.etsi.org/core/propertyOfInterestPressureFurnace_10"/>
        <core:hasPropertyOfInterest rdf:resource="https://saref.etsi.org/core/propertyOfInterestTemperatureExhaustFurnace_10"/>
        <rdfs:comment xml:lang="en">it&apos;s an Instance of a Furnace </rdfs:comment>
    </owl:NamedIndividual>
    


    <!-- https://ega.industry.com/ontologies/core/asset/furnace_12 -->

    <owl:NamedIndividual rdf:about="https://ega.industry.com/ontologies/core/asset/furnace_12">
        <rdf:type rdf:resource="https://ega.industry.com/ontologies/core/asset/Furnace"/>
        <rdf:type rdf:resource="https://saref.etsi.org/core/Device"/>
        <rdf:type rdf:resource="https://saref.etsi.org/core/FeatureOfInterest"/>
        <rdf:type rdf:resource="https://saref.etsi.org/saref4syst/System"/>
        <asset:feeds rdf:resource="https://ega.industry.com/ontologies/core/asset/castingSystem_12"/>
        <asset:hasProcess rdf:resource="https://ega.industry.com/ontologies/core/process/processFurnace_12"/>
        <asset:isFedBy rdf:resource="https://ega.industry.com/ontologies/core/asset/rawMaterialFeederSystem_12"/>
        <core:consistsOf rdf:resource="https://ega.industry.com/ontologies/core/asset/burner_12"/>
        <core:consistsOf rdf:resource="https://ega.industry.com/ontologies/core/asset/door_12"/>
        <core:consistsOf rdf:resource="https://ega.industry.com/ontologies/core/asset/sensorCastingStatusFurnace_12"/>
        <core:consistsOf rdf:resource="https://ega.industry.com/ontologies/core/asset/sensorPressureFurnace_12"/>
        <core:consistsOf rdf:resource="https://ega.industry.com/ontologies/core/asset/sensorTemperatureExhaustFurnace_12"/>
        <core:consistsOf rdf:resource="https://ega.industry.com/ontologies/core/asset/tank_12"/>
        <core:hasProperty rdf:resource="http://qudt.org/vocab/quantitykind/Dimensionless"/>
        <core:hasProperty rdf:resource="http://qudt.org/vocab/quantitykind/Pressure"/>
        <core:hasProperty rdf:resource="http://qudt.org/vocab/quantitykind/Temperature"/>
        <core:hasPropertyOfInterest rdf:resource="https://saref.etsi.org/core/propertyOfInterestCastingStatusFurnace_12"/>
        <core:hasPropertyOfInterest rdf:resource="https://saref.etsi.org/core/propertyOfInterestPressureFurnace_12"/>
        <core:hasPropertyOfInterest rdf:resource="https://saref.etsi.org/core/propertyOfInterestTemperatureExhaustFurnace_12"/>
        <rdfs:comment xml:lang="en">it&apos;s an Instance of a Furnace </rdfs:comment>
    </owl:NamedIndividual>
    


    <!-- https://ega.industry.com/ontologies/core/asset/gasSupply_10 -->

    <owl:NamedIndividual rdf:about="https://ega.industry.com/ontologies/core/asset/gasSupply_10">
        <rdf:type rdf:resource="https://ega.industry.com/ontologies/core/asset/GasSupply"/>
        <rdf:type rdf:resource="https://saref.etsi.org/core/Device"/>
        <rdf:type rdf:resource="https://saref.etsi.org/core/FeatureOfInterest"/>
        <rdf:type rdf:resource="https://saref.etsi.org/saref4syst/System"/>
        <asset:isPartOf rdf:resource="https://ega.industry.com/ontologies/core/asset/burner_10"/>
        <core:consistsOf rdf:resource="https://ega.industry.com/ontologies/core/asset/sensorFlowGas_10"/>
        <core:hasProperty rdf:resource="http://qudt.org/vocab/quantitykind/VolumeFlowRate"/>
        <core:hasPropertyOfInterest rdf:resource="https://saref.etsi.org/core/propertyOfInterestFlowRateGasBurner_10"/>
        <rdfs:comment xml:lang="en">Burner Gas Supply</rdfs:comment>
    </owl:NamedIndividual>
    


    <!-- https://ega.industry.com/ontologies/core/asset/gasSupply_12 -->

    <owl:NamedIndividual rdf:about="https://ega.industry.com/ontologies/core/asset/gasSupply_12">
        <rdf:type rdf:resource="https://ega.industry.com/ontologies/core/asset/GasSupply"/>
        <rdf:type rdf:resource="https://saref.etsi.org/core/Device"/>
        <rdf:type rdf:resource="https://saref.etsi.org/core/FeatureOfInterest"/>
        <rdf:type rdf:resource="https://saref.etsi.org/saref4syst/System"/>
        <asset:isPartOf rdf:resource="https://ega.industry.com/ontologies/core/asset/burner_12"/>
        <core:consistsOf rdf:resource="https://ega.industry.com/ontologies/core/asset/sensorFlowGas_12"/>
        <core:hasProperty rdf:resource="http://qudt.org/vocab/quantitykind/VolumeFlowRate"/>
        <core:hasPropertyOfInterest rdf:resource="https://saref.etsi.org/core/propertyOfInterestFlowRateGasBurner_12"/>
        <rdfs:comment xml:lang="en">Burner Gas Supply</rdfs:comment>
    </owl:NamedIndividual>
    


    <!-- https://ega.industry.com/ontologies/core/asset/lining_10 -->

    <owl:NamedIndividual rdf:about="https://ega.industry.com/ontologies/core/asset/lining_10">
        <rdf:type rdf:resource="https://ega.industry.com/ontologies/core/asset/Lining"/>
        <rdf:type rdf:resource="https://saref.etsi.org/core/Device"/>
        <rdf:type rdf:resource="https://saref.etsi.org/core/FeatureOfInterest"/>
        <rdf:type rdf:resource="https://saref.etsi.org/saref4syst/System"/>
        <asset:isPartOf rdf:resource="https://ega.industry.com/ontologies/core/asset/tank_10"/>
        <core:consistsOf rdf:resource="https://ega.industry.com/ontologies/core/asset/coolingSystem_10"/>
    </owl:NamedIndividual>
    


    <!-- https://ega.industry.com/ontologies/core/asset/lining_12 -->

    <owl:NamedIndividual rdf:about="https://ega.industry.com/ontologies/core/asset/lining_12">
        <rdf:type rdf:resource="https://ega.industry.com/ontologies/core/asset/Lining"/>
        <rdf:type rdf:resource="https://saref.etsi.org/core/Device"/>
        <rdf:type rdf:resource="https://saref.etsi.org/core/FeatureOfInterest"/>
        <rdf:type rdf:resource="https://saref.etsi.org/saref4syst/System"/>
        <asset:isPartOf rdf:resource="https://ega.industry.com/ontologies/core/asset/tank_12"/>
        <core:consistsOf rdf:resource="https://ega.industry.com/ontologies/core/asset/coolingSystem_12"/>
    </owl:NamedIndividual>
    


    <!-- https://ega.industry.com/ontologies/core/asset/rawMaterialBatch_10 -->

    <owl:NamedIndividual rdf:about="https://ega.industry.com/ontologies/core/asset/rawMaterialBatch_10">
        <rdf:type rdf:resource="https://ega.industry.com/ontologies/core/asset/RawMaterialBatch"/>
        <rdf:type rdf:resource="https://saref.etsi.org/core/FeatureOfInterest"/>
        <rdf:type rdf:resource="https://saref.etsi.org/saref4inma/Batch"/>
        <rdf:type rdf:resource="https://saref.etsi.org/saref4inma/MaterialBatch"/>
        <rdfs:comment xml:lang="en">Raw Material in Tank</rdfs:comment>
    </owl:NamedIndividual>
    


    <!-- https://ega.industry.com/ontologies/core/asset/rawMaterialBatch_12 -->

    <owl:NamedIndividual rdf:about="https://ega.industry.com/ontologies/core/asset/rawMaterialBatch_12">
        <rdf:type rdf:resource="https://ega.industry.com/ontologies/core/asset/RawMaterialBatch"/>
        <rdf:type rdf:resource="https://saref.etsi.org/core/FeatureOfInterest"/>
        <rdf:type rdf:resource="https://saref.etsi.org/saref4inma/Batch"/>
        <rdf:type rdf:resource="https://saref.etsi.org/saref4inma/MaterialBatch"/>
        <rdfs:comment xml:lang="en">Raw Material in Tank</rdfs:comment>
    </owl:NamedIndividual>
    


    <!-- https://ega.industry.com/ontologies/core/asset/rawMaterialFeederSystem_10 -->

    <owl:NamedIndividual rdf:about="https://ega.industry.com/ontologies/core/asset/rawMaterialFeederSystem_10">
        <rdf:type rdf:resource="https://ega.industry.com/ontologies/core/asset/IndustrySystem"/>
        <rdf:type rdf:resource="https://ega.industry.com/ontologies/core/asset/RawMaterialFeederSystem"/>
        <rdf:type rdf:resource="https://saref.etsi.org/saref4syst/System"/>
        <asset:feeds rdf:resource="https://ega.industry.com/ontologies/core/asset/furnace_10"/>
    </owl:NamedIndividual>
    


    <!-- https://ega.industry.com/ontologies/core/asset/rawMaterialFeederSystem_12 -->

    <owl:NamedIndividual rdf:about="https://ega.industry.com/ontologies/core/asset/rawMaterialFeederSystem_12">
        <rdf:type rdf:resource="https://ega.industry.com/ontologies/core/asset/IndustrySystem"/>
        <rdf:type rdf:resource="https://ega.industry.com/ontologies/core/asset/RawMaterialFeederSystem"/>
        <rdf:type rdf:resource="https://saref.etsi.org/saref4syst/System"/>
        <asset:feeds rdf:resource="https://ega.industry.com/ontologies/core/asset/furnace_12"/>
    </owl:NamedIndividual>
    


    <!-- https://ega.industry.com/ontologies/core/asset/sensorCastingStatusFurnace_10 -->

    <owl:NamedIndividual rdf:about="https://ega.industry.com/ontologies/core/asset/sensorCastingStatusFurnace_10">
        <rdf:type rdf:resource="https://ega.industry.com/ontologies/core/asset/CastingStatusSensor"/>
        <rdf:type rdf:resource="https://saref.etsi.org/core/Device"/>
        <rdf:type rdf:resource="https://saref.etsi.org/core/FeatureOfInterest"/>
        <rdf:type rdf:resource="https://saref.etsi.org/core/Sensor"/>
        <rdf:type rdf:resource="https://saref.etsi.org/saref4syst/System"/>
        <asset:isPartOf rdf:resource="https://ega.industry.com/ontologies/core/asset/furnace_10"/>
        <core:observes rdf:resource="https://saref.etsi.org/core/propertyValueCastingStatusFurnace_10"/>
        <core:targets rdf:resource="https://saref.etsi.org/core/propertyValueCastingStatusFurnace_10"/>
        <rdfs:comment xml:lang="en">Sensor that Obserse Casting Status</rdfs:comment>
    </owl:NamedIndividual>
    


    <!-- https://ega.industry.com/ontologies/core/asset/sensorCastingStatusFurnace_12 -->

    <owl:NamedIndividual rdf:about="https://ega.industry.com/ontologies/core/asset/sensorCastingStatusFurnace_12">
        <rdf:type rdf:resource="https://ega.industry.com/ontologies/core/asset/CastingStatusSensor"/>
        <rdf:type rdf:resource="https://saref.etsi.org/core/Device"/>
        <rdf:type rdf:resource="https://saref.etsi.org/core/FeatureOfInterest"/>
        <rdf:type rdf:resource="https://saref.etsi.org/core/Sensor"/>
        <rdf:type rdf:resource="https://saref.etsi.org/saref4syst/System"/>
        <asset:isPartOf rdf:resource="https://ega.industry.com/ontologies/core/asset/furnace_12"/>
        <core:observes rdf:resource="https://saref.etsi.org/core/propertyValueCastingStatusFurnace_12"/>
        <core:targets rdf:resource="https://saref.etsi.org/core/propertyValueCastingStatusFurnace_12"/>
        <rdfs:comment xml:lang="en">Sensor that Obserse Casting Status</rdfs:comment>
    </owl:NamedIndividual>
    


    <!-- https://ega.industry.com/ontologies/core/asset/sensorFlowAir_10 -->

    <owl:NamedIndividual rdf:about="https://ega.industry.com/ontologies/core/asset/sensorFlowAir_10">
        <rdf:type rdf:resource="https://ega.industry.com/ontologies/core/asset/AirFlowSensor"/>
        <rdf:type rdf:resource="https://saref.etsi.org/core/Device"/>
        <rdf:type rdf:resource="https://saref.etsi.org/core/FeatureOfInterest"/>
        <rdf:type rdf:resource="https://saref.etsi.org/core/Sensor"/>
        <rdf:type rdf:resource="https://saref.etsi.org/saref4syst/System"/>
        <asset:isPartOf rdf:resource="https://ega.industry.com/ontologies/core/asset/airSupply_10"/>
        <rdfs:comment xml:lang="en">Burner Air Supply  Air Sensor</rdfs:comment>
    </owl:NamedIndividual>
    


    <!-- https://ega.industry.com/ontologies/core/asset/sensorFlowAir_12 -->

    <owl:NamedIndividual rdf:about="https://ega.industry.com/ontologies/core/asset/sensorFlowAir_12">
        <rdf:type rdf:resource="https://ega.industry.com/ontologies/core/asset/AirFlowSensor"/>
        <rdf:type rdf:resource="https://saref.etsi.org/core/Device"/>
        <rdf:type rdf:resource="https://saref.etsi.org/core/FeatureOfInterest"/>
        <rdf:type rdf:resource="https://saref.etsi.org/core/Sensor"/>
        <rdf:type rdf:resource="https://saref.etsi.org/saref4syst/System"/>
        <asset:isPartOf rdf:resource="https://ega.industry.com/ontologies/core/asset/airSupply_12"/>
        <rdfs:comment xml:lang="en">Burner Air Supply  Air Sensor</rdfs:comment>
    </owl:NamedIndividual>
    


    <!-- https://ega.industry.com/ontologies/core/asset/sensorFlowGas_10 -->

    <owl:NamedIndividual rdf:about="https://ega.industry.com/ontologies/core/asset/sensorFlowGas_10">
        <rdf:type rdf:resource="https://ega.industry.com/ontologies/core/asset/GasFlowSensor"/>
        <rdf:type rdf:resource="https://saref.etsi.org/core/Device"/>
        <rdf:type rdf:resource="https://saref.etsi.org/core/FeatureOfInterest"/>
        <rdf:type rdf:resource="https://saref.etsi.org/core/Sensor"/>
        <rdf:type rdf:resource="https://saref.etsi.org/saref4syst/System"/>
        <asset:isPartOf rdf:resource="https://ega.industry.com/ontologies/core/asset/gasSupply_10"/>
        <core:observes rdf:resource="https://saref.etsi.org/core/propertyValueFlowRateGasBurner_10"/>
        <core:targets rdf:resource="https://saref.etsi.org/core/propertyValueFlowRateGasBurner_10"/>
        <rdfs:comment xml:lang="en">Burner Gas Supply Sensor</rdfs:comment>
    </owl:NamedIndividual>
    


    <!-- https://ega.industry.com/ontologies/core/asset/sensorFlowGas_12 -->

    <owl:NamedIndividual rdf:about="https://ega.industry.com/ontologies/core/asset/sensorFlowGas_12">
        <rdf:type rdf:resource="https://ega.industry.com/ontologies/core/asset/GasFlowSensor"/>
        <rdf:type rdf:resource="https://saref.etsi.org/core/Device"/>
        <rdf:type rdf:resource="https://saref.etsi.org/core/FeatureOfInterest"/>
        <rdf:type rdf:resource="https://saref.etsi.org/core/Sensor"/>
        <rdf:type rdf:resource="https://saref.etsi.org/saref4syst/System"/>
        <asset:isPartOf rdf:resource="https://ega.industry.com/ontologies/core/asset/gasSupply_12"/>
        <core:observes rdf:resource="https://saref.etsi.org/core/propertyValueFlowRateGasBurner_12"/>
        <core:targets rdf:resource="https://saref.etsi.org/core/propertyValueFlowRateGasBurner_12"/>
        <rdfs:comment xml:lang="en">Burner Gas Supply Sensor</rdfs:comment>
    </owl:NamedIndividual>
    


    <!-- https://ega.industry.com/ontologies/core/asset/sensorOxygen_10 -->

    <owl:NamedIndividual rdf:about="https://ega.industry.com/ontologies/core/asset/sensorOxygen_10">
        <rdf:type rdf:resource="https://ega.industry.com/ontologies/core/asset/OxygenSensor"/>
        <rdf:type rdf:resource="https://saref.etsi.org/core/Device"/>
        <rdf:type rdf:resource="https://saref.etsi.org/core/FeatureOfInterest"/>
        <rdf:type rdf:resource="https://saref.etsi.org/core/Sensor"/>
        <rdf:type rdf:resource="https://saref.etsi.org/saref4syst/System"/>
        <asset:isPartOf rdf:resource="https://ega.industry.com/ontologies/core/asset/airSupply_10"/>
        <core:observes rdf:resource="https://saref.etsi.org/core/propertyValueConcentrationAirBurner_10"/>
        <core:targets rdf:resource="https://saref.etsi.org/core/propertyValueConcentrationAirBurner_10"/>
        <rdfs:comment xml:lang="en">Burner Air Supply Oxygen sensor</rdfs:comment>
    </owl:NamedIndividual>
    


    <!-- https://ega.industry.com/ontologies/core/asset/sensorOxygen_12 -->

    <owl:NamedIndividual rdf:about="https://ega.industry.com/ontologies/core/asset/sensorOxygen_12">
        <rdf:type rdf:resource="https://ega.industry.com/ontologies/core/asset/OxygenSensor"/>
        <rdf:type rdf:resource="https://saref.etsi.org/core/Device"/>
        <rdf:type rdf:resource="https://saref.etsi.org/core/FeatureOfInterest"/>
        <rdf:type rdf:resource="https://saref.etsi.org/core/Sensor"/>
        <rdf:type rdf:resource="https://saref.etsi.org/saref4syst/System"/>
        <asset:isPartOf rdf:resource="https://ega.industry.com/ontologies/core/asset/airSupply_12"/>
        <core:observes rdf:resource="https://saref.etsi.org/core/propertyValueConcentrationAirBurner_12"/>
        <core:targets rdf:resource="https://saref.etsi.org/core/propertyValueConcentrationAirBurner_12"/>
        <rdfs:comment xml:lang="en">Burner Air Supply Oxygen sensor</rdfs:comment>
    </owl:NamedIndividual>
    


    <!-- https://ega.industry.com/ontologies/core/asset/sensorPowerPercentBathTank_10 -->

    <owl:NamedIndividual rdf:about="https://ega.industry.com/ontologies/core/asset/sensorPowerPercentBathTank_10">
        <rdf:type rdf:resource="https://ega.industry.com/ontologies/core/asset/PowerSensor"/>
        <rdf:type rdf:resource="https://saref.etsi.org/core/Device"/>
        <rdf:type rdf:resource="https://saref.etsi.org/core/FeatureOfInterest"/>
        <rdf:type rdf:resource="https://saref.etsi.org/core/Sensor"/>
        <rdf:type rdf:resource="https://saref.etsi.org/saref4syst/System"/>
        <asset:isPartOf rdf:resource="https://ega.industry.com/ontologies/core/asset/tank_10"/>
        <core:observes rdf:resource="https://saref.etsi.org/core/propertyValueHeatingPowerPercentBathTank_10"/>
        <core:targets rdf:resource="https://saref.etsi.org/core/propertyValueHeatingPowerPercentBathTank_10"/>
        <rdfs:comment xml:lang="en">Sensor Power of Power Percent of Tank Bath</rdfs:comment>
    </owl:NamedIndividual>
    


    <!-- https://ega.industry.com/ontologies/core/asset/sensorPowerPercentBathTank_12 -->

    <owl:NamedIndividual rdf:about="https://ega.industry.com/ontologies/core/asset/sensorPowerPercentBathTank_12">
        <rdf:type rdf:resource="https://ega.industry.com/ontologies/core/asset/PowerSensor"/>
        <rdf:type rdf:resource="https://saref.etsi.org/core/Device"/>
        <rdf:type rdf:resource="https://saref.etsi.org/core/FeatureOfInterest"/>
        <rdf:type rdf:resource="https://saref.etsi.org/core/Sensor"/>
        <rdf:type rdf:resource="https://saref.etsi.org/saref4syst/System"/>
        <asset:isPartOf rdf:resource="https://ega.industry.com/ontologies/core/asset/tank_12"/>
        <core:observes rdf:resource="https://saref.etsi.org/core/propertyValueHeatingPowerPercentBathTank_12"/>
        <core:targets rdf:resource="https://saref.etsi.org/core/propertyValueHeatingPowerPercentBathTank_12"/>
        <rdfs:comment xml:lang="en">Sensor Power of Power Percent of Tank Bath</rdfs:comment>
    </owl:NamedIndividual>
    


    <!-- https://ega.industry.com/ontologies/core/asset/sensorPowerPercentRoofTank_10 -->

    <owl:NamedIndividual rdf:about="https://ega.industry.com/ontologies/core/asset/sensorPowerPercentRoofTank_10">
        <rdf:type rdf:resource="https://ega.industry.com/ontologies/core/asset/PowerSensor"/>
        <rdf:type rdf:resource="https://saref.etsi.org/core/Device"/>
        <rdf:type rdf:resource="https://saref.etsi.org/core/FeatureOfInterest"/>
        <rdf:type rdf:resource="https://saref.etsi.org/core/Sensor"/>
        <rdf:type rdf:resource="https://saref.etsi.org/saref4syst/System"/>
        <asset:isPartOf rdf:resource="https://ega.industry.com/ontologies/core/asset/tank_10"/>
        <core:observes rdf:resource="https://saref.etsi.org/core/propertyValueHeatingPowerPercentRoofTank_10"/>
        <core:targets rdf:resource="https://saref.etsi.org/core/propertyValueHeatingPowerPercentRoofTank_10"/>
        <rdfs:comment xml:lang="en">Sensor Power of Power Percent of Tank Roof</rdfs:comment>
    </owl:NamedIndividual>
    


    <!-- https://ega.industry.com/ontologies/core/asset/sensorPowerPercentRoofTank_12 -->

    <owl:NamedIndividual rdf:about="https://ega.industry.com/ontologies/core/asset/sensorPowerPercentRoofTank_12">
        <rdf:type rdf:resource="https://ega.industry.com/ontologies/core/asset/PowerSensor"/>
        <rdf:type rdf:resource="https://saref.etsi.org/core/Device"/>
        <rdf:type rdf:resource="https://saref.etsi.org/core/FeatureOfInterest"/>
        <rdf:type rdf:resource="https://saref.etsi.org/core/Sensor"/>
        <rdf:type rdf:resource="https://saref.etsi.org/saref4syst/System"/>
        <asset:isPartOf rdf:resource="https://ega.industry.com/ontologies/core/asset/tank_12"/>
        <core:observes rdf:resource="https://saref.etsi.org/core/propertyValueHeatingPowerPercentRoofTank_12"/>
        <core:targets rdf:resource="https://saref.etsi.org/core/propertyValueHeatingPowerPercentRoofTank_12"/>
        <rdfs:comment xml:lang="en">Sensor Power of Power Percent of Tank Roof</rdfs:comment>
    </owl:NamedIndividual>
    


    <!-- https://ega.industry.com/ontologies/core/asset/sensorPressureFurnace_10 -->

    <owl:NamedIndividual rdf:about="https://ega.industry.com/ontologies/core/asset/sensorPressureFurnace_10">
        <rdf:type rdf:resource="https://ega.industry.com/ontologies/core/asset/PressureSensor"/>
        <rdf:type rdf:resource="https://saref.etsi.org/core/Device"/>
        <rdf:type rdf:resource="https://saref.etsi.org/core/FeatureOfInterest"/>
        <rdf:type rdf:resource="https://saref.etsi.org/core/Sensor"/>
        <rdf:type rdf:resource="https://saref.etsi.org/saref4syst/System"/>
        <asset:isPartOf rdf:resource="https://ega.industry.com/ontologies/core/asset/furnace_10"/>
        <core:observes rdf:resource="https://saref.etsi.org/core/propertyValuePressureFurnace_10"/>
        <core:targets rdf:resource="https://saref.etsi.org/core/propertyValuePressureFurnace_10"/>
    </owl:NamedIndividual>
    


    <!-- https://ega.industry.com/ontologies/core/asset/sensorPressureFurnace_12 -->

    <owl:NamedIndividual rdf:about="https://ega.industry.com/ontologies/core/asset/sensorPressureFurnace_12">
        <rdf:type rdf:resource="https://ega.industry.com/ontologies/core/asset/PressureSensor"/>
        <rdf:type rdf:resource="https://saref.etsi.org/core/Device"/>
        <rdf:type rdf:resource="https://saref.etsi.org/core/FeatureOfInterest"/>
        <rdf:type rdf:resource="https://saref.etsi.org/core/Sensor"/>
        <rdf:type rdf:resource="https://saref.etsi.org/saref4syst/System"/>
        <asset:isPartOf rdf:resource="https://ega.industry.com/ontologies/core/asset/furnace_12"/>
        <core:observes rdf:resource="https://saref.etsi.org/core/propertyValuePressureFurnace_12"/>
        <core:targets rdf:resource="https://saref.etsi.org/core/propertyValuePressureFurnace_12"/>
    </owl:NamedIndividual>
    


    <!-- https://ega.industry.com/ontologies/core/asset/sensorTemperatureBathTank_10 -->

    <owl:NamedIndividual rdf:about="https://ega.industry.com/ontologies/core/asset/sensorTemperatureBathTank_10">
        <rdf:type rdf:resource="https://ega.industry.com/ontologies/core/asset/TemperatureSensor"/>
        <rdf:type rdf:resource="https://saref.etsi.org/core/Device"/>
        <rdf:type rdf:resource="https://saref.etsi.org/core/FeatureOfInterest"/>
        <rdf:type rdf:resource="https://saref.etsi.org/core/Sensor"/>
        <rdf:type rdf:resource="https://saref.etsi.org/saref4syst/System"/>
        <asset:isPartOf rdf:resource="https://ega.industry.com/ontologies/core/asset/tank_10"/>
        <core:observes rdf:resource="https://saref.etsi.org/core/propertyValueTemperatureBathTank_10"/>
        <core:targets rdf:resource="https://saref.etsi.org/core/propertyValueTemperatureBathTank_10"/>
        <rdfs:comment xml:lang="en">Sensor Tempetature of Tank Bath</rdfs:comment>
    </owl:NamedIndividual>
    


    <!-- https://ega.industry.com/ontologies/core/asset/sensorTemperatureBathTank_12 -->

    <owl:NamedIndividual rdf:about="https://ega.industry.com/ontologies/core/asset/sensorTemperatureBathTank_12">
        <rdf:type rdf:resource="https://ega.industry.com/ontologies/core/asset/TemperatureSensor"/>
        <rdf:type rdf:resource="https://saref.etsi.org/core/Device"/>
        <rdf:type rdf:resource="https://saref.etsi.org/core/FeatureOfInterest"/>
        <rdf:type rdf:resource="https://saref.etsi.org/core/Sensor"/>
        <rdf:type rdf:resource="https://saref.etsi.org/saref4syst/System"/>
        <asset:isPartOf rdf:resource="https://ega.industry.com/ontologies/core/asset/tank_12"/>
        <core:observes rdf:resource="https://saref.etsi.org/core/propertyValueTemperatureBathTank_12"/>
        <core:targets rdf:resource="https://saref.etsi.org/core/propertyValueTemperatureBathTank_12"/>
        <rdfs:comment xml:lang="en">Sensor Tempetature of Tank Bath</rdfs:comment>
    </owl:NamedIndividual>
    


    <!-- https://ega.industry.com/ontologies/core/asset/sensorTemperatureExhaustFurnace_10 -->

    <owl:NamedIndividual rdf:about="https://ega.industry.com/ontologies/core/asset/sensorTemperatureExhaustFurnace_10">
        <rdf:type rdf:resource="https://ega.industry.com/ontologies/core/asset/TemperatureSensor"/>
        <rdf:type rdf:resource="https://saref.etsi.org/core/Device"/>
        <rdf:type rdf:resource="https://saref.etsi.org/core/FeatureOfInterest"/>
        <rdf:type rdf:resource="https://saref.etsi.org/core/Sensor"/>
        <rdf:type rdf:resource="https://saref.etsi.org/saref4syst/System"/>
        <asset:isPartOf rdf:resource="https://ega.industry.com/ontologies/core/asset/furnace_10"/>
        <core:observes rdf:resource="https://saref.etsi.org/core/propertyValueTemperatureExhaustFurnace_10"/>
        <core:targets rdf:resource="https://saref.etsi.org/core/propertyValueTemperatureExhaustFurnace_10"/>
        <rdfs:comment xml:lang="en">Sensor Tempetature of Furnace</rdfs:comment>
    </owl:NamedIndividual>
    


    <!-- https://ega.industry.com/ontologies/core/asset/sensorTemperatureExhaustFurnace_12 -->

    <owl:NamedIndividual rdf:about="https://ega.industry.com/ontologies/core/asset/sensorTemperatureExhaustFurnace_12">
        <rdf:type rdf:resource="https://ega.industry.com/ontologies/core/asset/TemperatureSensor"/>
        <rdf:type rdf:resource="https://saref.etsi.org/core/Device"/>
        <rdf:type rdf:resource="https://saref.etsi.org/core/FeatureOfInterest"/>
        <rdf:type rdf:resource="https://saref.etsi.org/core/Sensor"/>
        <rdf:type rdf:resource="https://saref.etsi.org/saref4syst/System"/>
        <asset:isPartOf rdf:resource="https://ega.industry.com/ontologies/core/asset/furnace_12"/>
        <core:observes rdf:resource="https://saref.etsi.org/core/propertyValueTemperatureExhaustFurnace_12"/>
        <core:targets rdf:resource="https://saref.etsi.org/core/propertyValueTemperatureExhaustFurnace_12"/>
        <rdfs:comment xml:lang="en">Sensor Tempetature of Furnace</rdfs:comment>
    </owl:NamedIndividual>
    


    <!-- https://ega.industry.com/ontologies/core/asset/sensorTemperatureRoofTank_10 -->

    <owl:NamedIndividual rdf:about="https://ega.industry.com/ontologies/core/asset/sensorTemperatureRoofTank_10">
        <rdf:type rdf:resource="https://ega.industry.com/ontologies/core/asset/TemperatureSensor"/>
        <rdf:type rdf:resource="https://saref.etsi.org/core/Device"/>
        <rdf:type rdf:resource="https://saref.etsi.org/core/FeatureOfInterest"/>
        <rdf:type rdf:resource="https://saref.etsi.org/core/Sensor"/>
        <rdf:type rdf:resource="https://saref.etsi.org/saref4syst/System"/>
        <asset:isPartOf rdf:resource="https://ega.industry.com/ontologies/core/asset/tank_10"/>
        <core:observes rdf:resource="https://saref.etsi.org/core/propertyValueTemperatureRoofTank_10"/>
        <core:targets rdf:resource="https://saref.etsi.org/core/propertyValueTemperatureRoofTank_10"/>
        <rdfs:comment xml:lang="en">Sensor Tempetature of Tank Root</rdfs:comment>
    </owl:NamedIndividual>
    


    <!-- https://ega.industry.com/ontologies/core/asset/sensorTemperatureRoofTank_12 -->

    <owl:NamedIndividual rdf:about="https://ega.industry.com/ontologies/core/asset/sensorTemperatureRoofTank_12">
        <rdf:type rdf:resource="https://ega.industry.com/ontologies/core/asset/TemperatureSensor"/>
        <rdf:type rdf:resource="https://saref.etsi.org/core/Device"/>
        <rdf:type rdf:resource="https://saref.etsi.org/core/FeatureOfInterest"/>
        <rdf:type rdf:resource="https://saref.etsi.org/core/Sensor"/>
        <rdf:type rdf:resource="https://saref.etsi.org/saref4syst/System"/>
        <asset:isPartOf rdf:resource="https://ega.industry.com/ontologies/core/asset/tank_12"/>
        <core:observes rdf:resource="https://saref.etsi.org/core/propertyValueTemperatureRoofTank_12"/>
        <core:targets rdf:resource="https://saref.etsi.org/core/propertyValueTemperatureRoofTank_12"/>
        <rdfs:comment xml:lang="en">Sensor Tempetature of Tank Root</rdfs:comment>
    </owl:NamedIndividual>
    


    <!-- https://ega.industry.com/ontologies/core/asset/stateOpenCloseDoor_10 -->

    <owl:NamedIndividual rdf:about="https://ega.industry.com/ontologies/core/asset/stateOpenCloseDoor_10">
        <rdf:type rdf:resource="https://ega.industry.com/ontologies/core/asset/OpenCloseState"/>
        <rdf:type rdf:resource="https://saref.etsi.org/core/State"/>
        <asset:hasOpenReason rdf:resource="https://ega.industry.com/ontologies/core/asset/Unknown"/>
        <core:hasStateValue rdf:resource="https://ega.industry.com/ontologies/core/asset/CLOSE"/>
        <core:isStateOf rdf:resource="https://ega.industry.com/ontologies/core/asset/door_10"/>
        <data:hasTag>fce_door_closed</data:hasTag>
        <data:hasTag>fce_door_open_reason</data:hasTag>
        <rdfs:comment xml:lang="en">Open Close State of Furnace Door</rdfs:comment>
    </owl:NamedIndividual>
    


    <!-- https://ega.industry.com/ontologies/core/asset/stateOpenCloseDoor_12 -->

    <owl:NamedIndividual rdf:about="https://ega.industry.com/ontologies/core/asset/stateOpenCloseDoor_12">
        <rdf:type rdf:resource="https://ega.industry.com/ontologies/core/asset/OpenCloseState"/>
        <rdf:type rdf:resource="https://saref.etsi.org/core/State"/>
        <asset:hasOpenReason rdf:resource="https://ega.industry.com/ontologies/core/asset/Unknown"/>
        <core:hasStateValue rdf:resource="https://ega.industry.com/ontologies/core/asset/CLOSE"/>
        <core:isStateOf rdf:resource="https://ega.industry.com/ontologies/core/asset/door_12"/>
        <data:hasTag>fce_door_closed</data:hasTag>
        <data:hasTag>fce_door_open_reason</data:hasTag>
        <rdfs:comment xml:lang="en">Open Close State of Furnace Door</rdfs:comment>
    </owl:NamedIndividual>
    


    <!-- https://ega.industry.com/ontologies/core/asset/tank_10 -->

    <owl:NamedIndividual rdf:about="https://ega.industry.com/ontologies/core/asset/tank_10">
        <rdf:type rdf:resource="https://ega.industry.com/ontologies/core/asset/Tank"/>
        <rdf:type rdf:resource="https://saref.etsi.org/core/Device"/>
        <rdf:type rdf:resource="https://saref.etsi.org/core/FeatureOfInterest"/>
        <rdf:type rdf:resource="https://saref.etsi.org/saref4syst/System"/>
        <asset:contains rdf:resource="https://ega.industry.com/ontologies/core/asset/rawMaterialBatch_10"/>
        <asset:isPartOf rdf:resource="https://ega.industry.com/ontologies/core/asset/furnace_10"/>
        <core:consistsOf rdf:resource="https://ega.industry.com/ontologies/core/asset/lining_10"/>
        <core:consistsOf rdf:resource="https://ega.industry.com/ontologies/core/asset/sensorPowerPercentBathTank_10"/>
        <core:consistsOf rdf:resource="https://ega.industry.com/ontologies/core/asset/sensorPowerPercentRoofTank_10"/>
        <core:consistsOf rdf:resource="https://ega.industry.com/ontologies/core/asset/sensorTemperatureBathTank_10"/>
        <core:consistsOf rdf:resource="https://ega.industry.com/ontologies/core/asset/sensorTemperatureRoofTank_10"/>
        <core:hasProperty rdf:resource="http://qudt.org/vocab/quantitykind/DimensionlessRatio"/>
        <core:hasProperty rdf:resource="http://qudt.org/vocab/quantitykind/Temperature"/>
        <core:hasPropertyOfInterest rdf:resource="https://saref.etsi.org/core/propertyOfInterestHeatingPowerPercentBathTank_10"/>
        <core:hasPropertyOfInterest rdf:resource="https://saref.etsi.org/core/propertyOfInterestHeatingPowerPercentRoofTank_10"/>
        <core:hasPropertyOfInterest rdf:resource="https://saref.etsi.org/core/propertyOfInterestTemperatureBatchTank_10"/>
        <core:hasPropertyOfInterest rdf:resource="https://saref.etsi.org/core/propertyOfInterestTemperatureBathThresholdTank_10"/>
        <core:hasPropertyOfInterest rdf:resource="https://saref.etsi.org/core/propertyOfInterestTemperatureRoofTank_10"/>
        <core:hasPropertyOfInterest rdf:resource="https://saref.etsi.org/core/propertyOfInterestTemperatureRoofThresholdTank_10"/>
        <rdfs:comment xml:lang="en">it&apos;s an instance of a Furnace Tank</rdfs:comment>
    </owl:NamedIndividual>
    


    <!-- https://ega.industry.com/ontologies/core/asset/tank_12 -->

    <owl:NamedIndividual rdf:about="https://ega.industry.com/ontologies/core/asset/tank_12">
        <rdf:type rdf:resource="https://ega.industry.com/ontologies/core/asset/Tank"/>
        <rdf:type rdf:resource="https://saref.etsi.org/core/Device"/>
        <rdf:type rdf:resource="https://saref.etsi.org/core/FeatureOfInterest"/>
        <rdf:type rdf:resource="https://saref.etsi.org/saref4syst/System"/>
        <asset:contains rdf:resource="https://ega.industry.com/ontologies/core/asset/rawMaterialBatch_12"/>
        <asset:isPartOf rdf:resource="https://ega.industry.com/ontologies/core/asset/furnace_12"/>
        <core:consistsOf rdf:resource="https://ega.industry.com/ontologies/core/asset/lining_12"/>
        <core:consistsOf rdf:resource="https://ega.industry.com/ontologies/core/asset/sensorPowerPercentBathTank_12"/>
        <core:consistsOf rdf:resource="https://ega.industry.com/ontologies/core/asset/sensorPowerPercentRoofTank_12"/>
        <core:consistsOf rdf:resource="https://ega.industry.com/ontologies/core/asset/sensorTemperatureBathTank_12"/>
        <core:consistsOf rdf:resource="https://ega.industry.com/ontologies/core/asset/sensorTemperatureRoofTank_12"/>
        <core:hasProperty rdf:resource="http://qudt.org/vocab/quantitykind/DimensionlessRatio"/>
        <core:hasProperty rdf:resource="http://qudt.org/vocab/quantitykind/Temperature"/>
        <core:hasPropertyOfInterest rdf:resource="https://saref.etsi.org/core/propertyOfInterestHeatingPowerPercentBathTank_12"/>
        <core:hasPropertyOfInterest rdf:resource="https://saref.etsi.org/core/propertyOfInterestHeatingPowerPercentRoofTank_12"/>
        <core:hasPropertyOfInterest rdf:resource="https://saref.etsi.org/core/propertyOfInterestTemperatureBatchTank_12"/>
        <core:hasPropertyOfInterest rdf:resource="https://saref.etsi.org/core/propertyOfInterestTemperatureBathThresholdTank_12"/>
        <core:hasPropertyOfInterest rdf:resource="https://saref.etsi.org/core/propertyOfInterestTemperatureRoofTank_12"/>
        <core:hasPropertyOfInterest rdf:resource="https://saref.etsi.org/core/propertyOfInterestTemperatureRoofThresholdTank_12"/>
        <rdfs:comment xml:lang="en">it&apos;s an instance of a Furnace Tank</rdfs:comment>
    </owl:NamedIndividual>
    


    <!-- https://ega.industry.com/ontologies/core/data/eventFunctionCasting_10 -->

    <owl:NamedIndividual rdf:about="https://ega.industry.com/ontologies/core/data/eventFunctionCasting_10">
        <rdf:type rdf:resource="https://ega.industry.com/ontologies/core/data/EventFunction"/>
        <rdf:type rdf:resource="https://saref.etsi.org/core/Function"/>
        <data:hasThresholdPropertyValue rdf:resource="https://saref.etsi.org/core/propertyValueCastingStatusFurnace_10"/>
        <data:hasThresholdPropertyValue rdf:resource="https://saref.etsi.org/core/propertyValueTemperatureBathTank_10"/>
        <process:triggers rdf:resource="https://ega.industry.com/ontologies/core/process/conditionCasting_10"/>
    </owl:NamedIndividual>
    


    <!-- https://ega.industry.com/ontologies/core/data/eventFunctionCasting_12 -->

    <owl:NamedIndividual rdf:about="https://ega.industry.com/ontologies/core/data/eventFunctionCasting_12">
        <rdf:type rdf:resource="https://ega.industry.com/ontologies/core/data/EventFunction"/>
        <rdf:type rdf:resource="https://saref.etsi.org/core/Function"/>
        <data:hasThresholdPropertyValue rdf:resource="https://saref.etsi.org/core/propertyValueCastingStatusFurnace_12"/>
        <data:hasThresholdPropertyValue rdf:resource="https://saref.etsi.org/core/propertyValueTemperatureBathTank_12"/>
        <process:triggers rdf:resource="https://ega.industry.com/ontologies/core/process/conditionCasting_12"/>
    </owl:NamedIndividual>
    


    <!-- https://ega.industry.com/ontologies/core/data/eventFunctionHolding_10 -->

    <owl:NamedIndividual rdf:about="https://ega.industry.com/ontologies/core/data/eventFunctionHolding_10">
        <rdf:type rdf:resource="https://ega.industry.com/ontologies/core/data/EventFunction"/>
        <rdf:type rdf:resource="https://saref.etsi.org/core/Function"/>
        <data:hasSpecificState rdf:resource="https://ega.industry.com/ontologies/core/asset/stateOpenCloseDoor_10"/>
        <data:hasThresholdPropertyValue rdf:resource="https://saref.etsi.org/core/propertyValueTemperatureBathTank_10"/>
        <data:hasThresholdPropertyValue rdf:resource="https://saref.etsi.org/core/propertyValueTemperatureBathThresholdTank_10"/>
        <process:triggers rdf:resource="https://ega.industry.com/ontologies/core/process/conditionHolding_10"/>
    </owl:NamedIndividual>
    


    <!-- https://ega.industry.com/ontologies/core/data/eventFunctionHolding_12 -->

    <owl:NamedIndividual rdf:about="https://ega.industry.com/ontologies/core/data/eventFunctionHolding_12">
        <rdf:type rdf:resource="https://ega.industry.com/ontologies/core/data/EventFunction"/>
        <rdf:type rdf:resource="https://saref.etsi.org/core/Function"/>
        <data:hasSpecificState rdf:resource="https://ega.industry.com/ontologies/core/asset/stateOpenCloseDoor_12"/>
        <data:hasThresholdPropertyValue rdf:resource="https://saref.etsi.org/core/propertyValueTemperatureBathTank_12"/>
        <data:hasThresholdPropertyValue rdf:resource="https://saref.etsi.org/core/propertyValueTemperatureBathThresholdTank_12"/>
        <process:triggers rdf:resource="https://ega.industry.com/ontologies/core/process/conditionHolding_12"/>
    </owl:NamedIndividual>
    


    <!-- https://ega.industry.com/ontologies/core/data/eventFunctionLaboratoryAnalysis_10 -->

    <owl:NamedIndividual rdf:about="https://ega.industry.com/ontologies/core/data/eventFunctionLaboratoryAnalysis_10">
        <rdf:type rdf:resource="https://ega.industry.com/ontologies/core/data/EventFunction"/>
        <rdf:type rdf:resource="https://saref.etsi.org/core/Function"/>
        <data:hasThresholdPropertyValue rdf:resource="https://saref.etsi.org/core/propertyValueTemperatureExhaustFurnace_10"/>
        <process:triggers rdf:resource="https://ega.industry.com/ontologies/core/process/conditionLaboratoryAnalysis_10"/>
    </owl:NamedIndividual>
    


    <!-- https://ega.industry.com/ontologies/core/data/eventFunctionLaboratoryAnalysis_12 -->

    <owl:NamedIndividual rdf:about="https://ega.industry.com/ontologies/core/data/eventFunctionLaboratoryAnalysis_12">
        <rdf:type rdf:resource="https://ega.industry.com/ontologies/core/data/EventFunction"/>
        <rdf:type rdf:resource="https://saref.etsi.org/core/Function"/>
        <data:hasThresholdPropertyValue rdf:resource="https://saref.etsi.org/core/propertyValueTemperatureExhaustFurnace_12"/>
        <process:triggers rdf:resource="https://ega.industry.com/ontologies/core/process/conditionLaboratoryAnalysis_12"/>
    </owl:NamedIndividual>
    


    <!-- https://ega.industry.com/ontologies/core/data/eventFunctionLoadingScrapAdjustment_10 -->

    <owl:NamedIndividual rdf:about="https://ega.industry.com/ontologies/core/data/eventFunctionLoadingScrapAdjustment_10">
        <rdf:type rdf:resource="https://ega.industry.com/ontologies/core/data/EventFunction"/>
        <rdf:type rdf:resource="https://saref.etsi.org/core/Function"/>
        <data:hasSpecificState rdf:resource="https://ega.industry.com/ontologies/core/asset/stateOpenCloseDoor_10"/>
        <process:triggers rdf:resource="https://ega.industry.com/ontologies/core/process/conditionLoadingScrapAdjustment_10"/>
    </owl:NamedIndividual>
    


    <!-- https://ega.industry.com/ontologies/core/data/eventFunctionLoadingScrapAdjustment_12 -->

    <owl:NamedIndividual rdf:about="https://ega.industry.com/ontologies/core/data/eventFunctionLoadingScrapAdjustment_12">
        <rdf:type rdf:resource="https://ega.industry.com/ontologies/core/data/EventFunction"/>
        <rdf:type rdf:resource="https://saref.etsi.org/core/Function"/>
        <data:hasSpecificState rdf:resource="https://ega.industry.com/ontologies/core/asset/stateOpenCloseDoor_12"/>
        <process:triggers rdf:resource="https://ega.industry.com/ontologies/core/process/conditionLoadingScrapAdjustment_12"/>
    </owl:NamedIndividual>
    


    <!-- https://ega.industry.com/ontologies/core/data/eventFunctionLoadingScrap_10 -->

    <owl:NamedIndividual rdf:about="https://ega.industry.com/ontologies/core/data/eventFunctionLoadingScrap_10">
        <rdf:type rdf:resource="https://ega.industry.com/ontologies/core/data/EventFunction"/>
        <rdf:type rdf:resource="https://saref.etsi.org/core/Function"/>
        <data:hasSpecificState rdf:resource="https://ega.industry.com/ontologies/core/asset/stateOpenCloseDoor_10"/>
        <process:triggers rdf:resource="https://ega.industry.com/ontologies/core/process/conditionLoadingScrap_10"/>
    </owl:NamedIndividual>
    


    <!-- https://ega.industry.com/ontologies/core/data/eventFunctionLoadingScrap_12 -->

    <owl:NamedIndividual rdf:about="https://ega.industry.com/ontologies/core/data/eventFunctionLoadingScrap_12">
        <rdf:type rdf:resource="https://ega.industry.com/ontologies/core/data/EventFunction"/>
        <rdf:type rdf:resource="https://saref.etsi.org/core/Function"/>
        <data:hasSpecificState rdf:resource="https://ega.industry.com/ontologies/core/asset/stateOpenCloseDoor_12"/>
        <process:triggers rdf:resource="https://ega.industry.com/ontologies/core/process/conditionLoadingScrap_12"/>
    </owl:NamedIndividual>
    


    <!-- https://ega.industry.com/ontologies/core/data/eventFunctionPouringAluminiumAdjustment_10 -->

    <owl:NamedIndividual rdf:about="https://ega.industry.com/ontologies/core/data/eventFunctionPouringAluminiumAdjustment_10">
        <rdf:type rdf:resource="https://ega.industry.com/ontologies/core/data/EventFunction"/>
        <rdf:type rdf:resource="https://saref.etsi.org/core/Function"/>
        <data:hasSpecificState rdf:resource="https://ega.industry.com/ontologies/core/asset/stateOpenCloseDoor_10"/>
        <process:triggers rdf:resource="https://ega.industry.com/ontologies/core/process/conditionPouringAluminiumAdjustment_10"/>
    </owl:NamedIndividual>
    


    <!-- https://ega.industry.com/ontologies/core/data/eventFunctionPouringAluminiumAdjustment_12 -->

    <owl:NamedIndividual rdf:about="https://ega.industry.com/ontologies/core/data/eventFunctionPouringAluminiumAdjustment_12">
        <rdf:type rdf:resource="https://ega.industry.com/ontologies/core/data/EventFunction"/>
        <rdf:type rdf:resource="https://saref.etsi.org/core/Function"/>
        <data:hasSpecificState rdf:resource="https://ega.industry.com/ontologies/core/asset/stateOpenCloseDoor_12"/>
        <process:triggers rdf:resource="https://ega.industry.com/ontologies/core/process/conditionPouringAluminiumAdjustment_12"/>
    </owl:NamedIndividual>
    


    <!-- https://ega.industry.com/ontologies/core/data/eventFunctionPouringAluminium_10 -->

    <owl:NamedIndividual rdf:about="https://ega.industry.com/ontologies/core/data/eventFunctionPouringAluminium_10">
        <rdf:type rdf:resource="https://ega.industry.com/ontologies/core/data/EventFunction"/>
        <rdf:type rdf:resource="https://saref.etsi.org/core/Function"/>
        <data:hasSpecificState rdf:resource="https://ega.industry.com/ontologies/core/asset/stateOpenCloseDoor_10"/>
        <process:triggers rdf:resource="https://ega.industry.com/ontologies/core/process/conditionPouringAluminium_10"/>
    </owl:NamedIndividual>
    


    <!-- https://ega.industry.com/ontologies/core/data/eventFunctionPouringAluminium_12 -->

    <owl:NamedIndividual rdf:about="https://ega.industry.com/ontologies/core/data/eventFunctionPouringAluminium_12">
        <rdf:type rdf:resource="https://ega.industry.com/ontologies/core/data/EventFunction"/>
        <rdf:type rdf:resource="https://saref.etsi.org/core/Function"/>
        <data:hasSpecificState rdf:resource="https://ega.industry.com/ontologies/core/asset/stateOpenCloseDoor_12"/>
        <process:triggers rdf:resource="https://ega.industry.com/ontologies/core/process/conditionPouringAluminium_12"/>
    </owl:NamedIndividual>
    


    <!-- https://ega.industry.com/ontologies/core/data/eventFunctionPouringMetalsAdjustment_10 -->

    <owl:NamedIndividual rdf:about="https://ega.industry.com/ontologies/core/data/eventFunctionPouringMetalsAdjustment_10">
        <rdf:type rdf:resource="https://ega.industry.com/ontologies/core/data/EventFunction"/>
        <rdf:type rdf:resource="https://saref.etsi.org/core/Function"/>
        <data:hasSpecificState rdf:resource="https://ega.industry.com/ontologies/core/asset/stateOpenCloseDoor_10"/>
        <process:triggers rdf:resource="https://ega.industry.com/ontologies/core/process/conditionPouringMetalsAdjustment_10"/>
    </owl:NamedIndividual>
    


    <!-- https://ega.industry.com/ontologies/core/data/eventFunctionPouringMetalsAdjustment_12 -->

    <owl:NamedIndividual rdf:about="https://ega.industry.com/ontologies/core/data/eventFunctionPouringMetalsAdjustment_12">
        <rdf:type rdf:resource="https://ega.industry.com/ontologies/core/data/EventFunction"/>
        <rdf:type rdf:resource="https://saref.etsi.org/core/Function"/>
        <data:hasSpecificState rdf:resource="https://ega.industry.com/ontologies/core/asset/stateOpenCloseDoor_12"/>
        <process:triggers rdf:resource="https://ega.industry.com/ontologies/core/process/conditionPouringMetalsAdjustment_12"/>
    </owl:NamedIndividual>
    


    <!-- https://ega.industry.com/ontologies/core/data/eventFunctionPouringMetals_10 -->

    <owl:NamedIndividual rdf:about="https://ega.industry.com/ontologies/core/data/eventFunctionPouringMetals_10">
        <rdf:type rdf:resource="https://ega.industry.com/ontologies/core/data/EventFunction"/>
        <rdf:type rdf:resource="https://saref.etsi.org/core/Function"/>
        <data:hasSpecificState rdf:resource="https://ega.industry.com/ontologies/core/asset/stateOpenCloseDoor_10"/>
        <process:triggers rdf:resource="https://ega.industry.com/ontologies/core/process/conditionPouringMetals_10"/>
    </owl:NamedIndividual>
    


    <!-- https://ega.industry.com/ontologies/core/data/eventFunctionPouringMetals_12 -->

    <owl:NamedIndividual rdf:about="https://ega.industry.com/ontologies/core/data/eventFunctionPouringMetals_12">
        <rdf:type rdf:resource="https://ega.industry.com/ontologies/core/data/EventFunction"/>
        <rdf:type rdf:resource="https://saref.etsi.org/core/Function"/>
        <data:hasSpecificState rdf:resource="https://ega.industry.com/ontologies/core/asset/stateOpenCloseDoor_12"/>
        <process:triggers rdf:resource="https://ega.industry.com/ontologies/core/process/conditionPouringMetals_12"/>
    </owl:NamedIndividual>
    


    <!-- https://ega.industry.com/ontologies/core/data/eventFunctionPreheating_10 -->

    <owl:NamedIndividual rdf:about="https://ega.industry.com/ontologies/core/data/eventFunctionPreheating_10">
        <rdf:type rdf:resource="https://ega.industry.com/ontologies/core/data/EventFunction"/>
        <rdf:type rdf:resource="https://saref.etsi.org/core/Function"/>
        <data:hasSpecificState rdf:resource="https://ega.industry.com/ontologies/core/asset/stateOpenCloseDoor_10"/>
        <data:hasThresholdPropertyValue rdf:resource="https://saref.etsi.org/core/propertyValueFlowRateGasBurner_10"/>
        <data:hasThresholdPropertyValue rdf:resource="https://saref.etsi.org/core/propertyValueTemperatureBathTank_10"/>
        <data:hasThresholdPropertyValue rdf:resource="https://saref.etsi.org/core/propertyValueTemperatureBathThresholdTank_10"/>
        <process:triggers rdf:resource="https://ega.industry.com/ontologies/core/process/conditionPreheating_10"/>
    </owl:NamedIndividual>
    


    <!-- https://ega.industry.com/ontologies/core/data/eventFunctionPreheating_12 -->

    <owl:NamedIndividual rdf:about="https://ega.industry.com/ontologies/core/data/eventFunctionPreheating_12">
        <rdf:type rdf:resource="https://ega.industry.com/ontologies/core/data/EventFunction"/>
        <rdf:type rdf:resource="https://saref.etsi.org/core/Function"/>
        <data:hasSpecificState rdf:resource="https://ega.industry.com/ontologies/core/asset/stateOpenCloseDoor_12"/>
        <data:hasThresholdPropertyValue rdf:resource="https://saref.etsi.org/core/propertyValueFlowRateGasBurner_12"/>
        <data:hasThresholdPropertyValue rdf:resource="https://saref.etsi.org/core/propertyValueTemperatureBathTank_12"/>
        <data:hasThresholdPropertyValue rdf:resource="https://saref.etsi.org/core/propertyValueTemperatureBathThresholdTank_12"/>
        <process:triggers rdf:resource="https://ega.industry.com/ontologies/core/process/conditionPreheating_12"/>
    </owl:NamedIndividual>
    


    <!-- https://ega.industry.com/ontologies/core/data/eventFunctionSampling_10 -->

    <owl:NamedIndividual rdf:about="https://ega.industry.com/ontologies/core/data/eventFunctionSampling_10">
        <rdf:type rdf:resource="https://ega.industry.com/ontologies/core/data/EventFunction"/>
        <rdf:type rdf:resource="https://saref.etsi.org/core/Function"/>
        <data:hasSpecificState rdf:resource="https://ega.industry.com/ontologies/core/asset/stateOpenCloseDoor_10"/>
        <process:triggers rdf:resource="https://ega.industry.com/ontologies/core/process/conditionSampling_10"/>
    </owl:NamedIndividual>
    


    <!-- https://ega.industry.com/ontologies/core/data/eventFunctionSampling_12 -->

    <owl:NamedIndividual rdf:about="https://ega.industry.com/ontologies/core/data/eventFunctionSampling_12">
        <rdf:type rdf:resource="https://ega.industry.com/ontologies/core/data/EventFunction"/>
        <rdf:type rdf:resource="https://saref.etsi.org/core/Function"/>
        <data:hasSpecificState rdf:resource="https://ega.industry.com/ontologies/core/asset/stateOpenCloseDoor_12"/>
        <process:triggers rdf:resource="https://ega.industry.com/ontologies/core/process/conditionSampling_12"/>
    </owl:NamedIndividual>
    


    <!-- https://ega.industry.com/ontologies/core/data/eventFunctionSkimming_10 -->

    <owl:NamedIndividual rdf:about="https://ega.industry.com/ontologies/core/data/eventFunctionSkimming_10">
        <rdf:type rdf:resource="https://ega.industry.com/ontologies/core/data/EventFunction"/>
        <rdf:type rdf:resource="https://saref.etsi.org/core/Function"/>
        <data:hasSpecificState rdf:resource="https://ega.industry.com/ontologies/core/asset/stateOpenCloseDoor_10"/>
        <process:triggers rdf:resource="https://ega.industry.com/ontologies/core/process/conditionSkimming_10"/>
    </owl:NamedIndividual>
    


    <!-- https://ega.industry.com/ontologies/core/data/eventFunctionSkimming_12 -->

    <owl:NamedIndividual rdf:about="https://ega.industry.com/ontologies/core/data/eventFunctionSkimming_12">
        <rdf:type rdf:resource="https://ega.industry.com/ontologies/core/data/EventFunction"/>
        <rdf:type rdf:resource="https://saref.etsi.org/core/Function"/>
        <data:hasSpecificState rdf:resource="https://ega.industry.com/ontologies/core/asset/stateOpenCloseDoor_12"/>
        <process:triggers rdf:resource="https://ega.industry.com/ontologies/core/process/conditionSkimming_12"/>
    </owl:NamedIndividual>
    


    <!-- https://ega.industry.com/ontologies/core/data/eventFunctionStirring_10 -->

    <owl:NamedIndividual rdf:about="https://ega.industry.com/ontologies/core/data/eventFunctionStirring_10">
        <rdf:type rdf:resource="https://ega.industry.com/ontologies/core/data/EventFunction"/>
        <rdf:type rdf:resource="https://saref.etsi.org/core/Function"/>
        <data:hasSpecificState rdf:resource="https://ega.industry.com/ontologies/core/asset/stateOpenCloseDoor_10"/>
        <process:triggers rdf:resource="https://ega.industry.com/ontologies/core/process/conditionStirring_10"/>
    </owl:NamedIndividual>
    


    <!-- https://ega.industry.com/ontologies/core/data/eventFunctionStirring_12 -->

    <owl:NamedIndividual rdf:about="https://ega.industry.com/ontologies/core/data/eventFunctionStirring_12">
        <rdf:type rdf:resource="https://ega.industry.com/ontologies/core/data/EventFunction"/>
        <rdf:type rdf:resource="https://saref.etsi.org/core/Function"/>
        <data:hasSpecificState rdf:resource="https://ega.industry.com/ontologies/core/asset/stateOpenCloseDoor_12"/>
        <process:triggers rdf:resource="https://ega.industry.com/ontologies/core/process/conditionStirring_12"/>
    </owl:NamedIndividual>
    


    <!-- https://ega.industry.com/ontologies/core/process/Machine -->

    <owl:NamedIndividual rdf:about="https://ega.industry.com/ontologies/core/process/Machine">
        <rdf:type rdf:resource="https://ega.industry.com/ontologies/core/process/StepType"/>
    </owl:NamedIndividual>
    


    <!-- https://ega.industry.com/ontologies/core/process/Operator -->

    <owl:NamedIndividual rdf:about="https://ega.industry.com/ontologies/core/process/Operator">
        <rdf:type rdf:resource="https://ega.industry.com/ontologies/core/process/StepType"/>
    </owl:NamedIndividual>
    


    <!-- https://ega.industry.com/ontologies/core/process/SubProcessCasting_10 -->

    <owl:NamedIndividual rdf:about="https://ega.industry.com/ontologies/core/process/SubProcessCasting_10">
        <rdf:type rdf:resource="https://ega.industry.com/ontologies/core/process/SequentialSubProcess"/>
        <rdf:type rdf:resource="https://ega.industry.com/ontologies/core/process/SubProcess"/>
        <process:hasEndStep rdf:resource="https://ega.industry.com/ontologies/core/process/stepCastingStep_10"/>
        <process:hasStartStep rdf:resource="https://ega.industry.com/ontologies/core/process/stepCastingStep_10"/>
        <process:hasStep rdf:resource="https://ega.industry.com/ontologies/core/process/stepCastingStep_10"/>
        <process:hasEndTimestamp rdf:datatype="http://www.w3.org/2001/XMLSchema#dateTime">2025-06-03T09:59:07.456561</process:hasEndTimestamp>
        <process:hasStartTimestamp rdf:datatype="http://www.w3.org/2001/XMLSchema#dateTime">2025-06-03T09:59:07.456561</process:hasStartTimestamp>
        <process:hasSubProcessId rdf:datatype="http://www.w3.org/2001/XMLSchema#integer">6</process:hasSubProcessId>
        <process:isCurrentSubProcess rdf:datatype="http://www.w3.org/2001/XMLSchema#boolean">false</process:isCurrentSubProcess>
        <rdfs:comment xml:lang="en">Transfer of final metal to casting system</rdfs:comment>
    </owl:NamedIndividual>
    


    <!-- https://ega.industry.com/ontologies/core/process/SubProcessCasting_12 -->

    <owl:NamedIndividual rdf:about="https://ega.industry.com/ontologies/core/process/SubProcessCasting_12">
        <rdf:type rdf:resource="https://ega.industry.com/ontologies/core/process/SequentialSubProcess"/>
        <rdf:type rdf:resource="https://ega.industry.com/ontologies/core/process/SubProcess"/>
        <process:hasEndStep rdf:resource="https://ega.industry.com/ontologies/core/process/stepCastingStep_12"/>
        <process:hasStartStep rdf:resource="https://ega.industry.com/ontologies/core/process/stepCastingStep_12"/>
        <process:hasStep rdf:resource="https://ega.industry.com/ontologies/core/process/stepCastingStep_12"/>
        <process:hasEndTimestamp rdf:datatype="http://www.w3.org/2001/XMLSchema#dateTime">2025-06-03T09:59:08.322482</process:hasEndTimestamp>
        <process:hasStartTimestamp rdf:datatype="http://www.w3.org/2001/XMLSchema#dateTime">2025-06-03T09:59:08.322482</process:hasStartTimestamp>
        <process:hasSubProcessId rdf:datatype="http://www.w3.org/2001/XMLSchema#integer">6</process:hasSubProcessId>
        <process:isCurrentSubProcess rdf:datatype="http://www.w3.org/2001/XMLSchema#boolean">false</process:isCurrentSubProcess>
        <rdfs:comment xml:lang="en">Transfer of final metal to casting system</rdfs:comment>
    </owl:NamedIndividual>
    


    <!-- https://ega.industry.com/ontologies/core/process/conditionCasting_10 -->

    <owl:NamedIndividual rdf:about="https://ega.industry.com/ontologies/core/process/conditionCasting_10">
        <rdf:type rdf:resource="https://ega.industry.com/ontologies/core/process/Condition"/>
        <process:isTriggeredBy rdf:resource="https://ega.industry.com/ontologies/core/data/eventFunctionCasting_10"/>
        <process:conditionAchieved rdf:datatype="http://www.w3.org/2001/XMLSchema#boolean">false</process:conditionAchieved>
        <rdfs:comment xml:lang="en">Condition of Step</rdfs:comment>
    </owl:NamedIndividual>
    


    <!-- https://ega.industry.com/ontologies/core/process/conditionCasting_12 -->

    <owl:NamedIndividual rdf:about="https://ega.industry.com/ontologies/core/process/conditionCasting_12">
        <rdf:type rdf:resource="https://ega.industry.com/ontologies/core/process/Condition"/>
        <process:isTriggeredBy rdf:resource="https://ega.industry.com/ontologies/core/data/eventFunctionCasting_12"/>
        <process:conditionAchieved rdf:datatype="http://www.w3.org/2001/XMLSchema#boolean">false</process:conditionAchieved>
        <rdfs:comment xml:lang="en">Condition of Step</rdfs:comment>
    </owl:NamedIndividual>
    


    <!-- https://ega.industry.com/ontologies/core/process/conditionHolding_10 -->

    <owl:NamedIndividual rdf:about="https://ega.industry.com/ontologies/core/process/conditionHolding_10">
        <rdf:type rdf:resource="https://ega.industry.com/ontologies/core/process/Condition"/>
        <process:isTriggeredBy rdf:resource="https://ega.industry.com/ontologies/core/data/eventFunctionHolding_10"/>
        <process:conditionAchieved rdf:datatype="http://www.w3.org/2001/XMLSchema#boolean">false</process:conditionAchieved>
        <rdfs:comment xml:lang="en">Condition of Step</rdfs:comment>
    </owl:NamedIndividual>
    


    <!-- https://ega.industry.com/ontologies/core/process/conditionHolding_12 -->

    <owl:NamedIndividual rdf:about="https://ega.industry.com/ontologies/core/process/conditionHolding_12">
        <rdf:type rdf:resource="https://ega.industry.com/ontologies/core/process/Condition"/>
        <process:isTriggeredBy rdf:resource="https://ega.industry.com/ontologies/core/data/eventFunctionHolding_12"/>
        <process:conditionAchieved rdf:datatype="http://www.w3.org/2001/XMLSchema#boolean">false</process:conditionAchieved>
        <rdfs:comment xml:lang="en">Condition of Step</rdfs:comment>
    </owl:NamedIndividual>
    


    <!-- https://ega.industry.com/ontologies/core/process/conditionLaboratoryAnalysis_10 -->

    <owl:NamedIndividual rdf:about="https://ega.industry.com/ontologies/core/process/conditionLaboratoryAnalysis_10">
        <rdf:type rdf:resource="https://ega.industry.com/ontologies/core/process/Condition"/>
        <process:isTriggeredBy rdf:resource="https://ega.industry.com/ontologies/core/data/eventFunctionLaboratoryAnalysis_10"/>
        <process:conditionAchieved rdf:datatype="http://www.w3.org/2001/XMLSchema#boolean">false</process:conditionAchieved>
        <rdfs:comment xml:lang="en">Condition of Step</rdfs:comment>
    </owl:NamedIndividual>
    


    <!-- https://ega.industry.com/ontologies/core/process/conditionLaboratoryAnalysis_12 -->

    <owl:NamedIndividual rdf:about="https://ega.industry.com/ontologies/core/process/conditionLaboratoryAnalysis_12">
        <rdf:type rdf:resource="https://ega.industry.com/ontologies/core/process/Condition"/>
        <process:isTriggeredBy rdf:resource="https://ega.industry.com/ontologies/core/data/eventFunctionLaboratoryAnalysis_12"/>
        <process:conditionAchieved rdf:datatype="http://www.w3.org/2001/XMLSchema#boolean">false</process:conditionAchieved>
        <rdfs:comment xml:lang="en">Condition of Step</rdfs:comment>
    </owl:NamedIndividual>
    


    <!-- https://ega.industry.com/ontologies/core/process/conditionLoadingScrapAdjustment_10 -->

    <owl:NamedIndividual rdf:about="https://ega.industry.com/ontologies/core/process/conditionLoadingScrapAdjustment_10">
        <rdf:type rdf:resource="https://ega.industry.com/ontologies/core/process/Condition"/>
        <process:isTriggeredBy rdf:resource="https://ega.industry.com/ontologies/core/data/eventFunctionLoadingScrapAdjustment_10"/>
        <process:conditionAchieved rdf:datatype="http://www.w3.org/2001/XMLSchema#boolean">false</process:conditionAchieved>
        <rdfs:comment xml:lang="en">Condition of Step</rdfs:comment>
    </owl:NamedIndividual>
    


    <!-- https://ega.industry.com/ontologies/core/process/conditionLoadingScrapAdjustment_12 -->

    <owl:NamedIndividual rdf:about="https://ega.industry.com/ontologies/core/process/conditionLoadingScrapAdjustment_12">
        <rdf:type rdf:resource="https://ega.industry.com/ontologies/core/process/Condition"/>
        <process:isTriggeredBy rdf:resource="https://ega.industry.com/ontologies/core/data/eventFunctionLoadingScrapAdjustment_12"/>
        <process:conditionAchieved rdf:datatype="http://www.w3.org/2001/XMLSchema#boolean">false</process:conditionAchieved>
        <rdfs:comment xml:lang="en">Condition of Step</rdfs:comment>
    </owl:NamedIndividual>
    


    <!-- https://ega.industry.com/ontologies/core/process/conditionLoadingScrap_10 -->

    <owl:NamedIndividual rdf:about="https://ega.industry.com/ontologies/core/process/conditionLoadingScrap_10">
        <rdf:type rdf:resource="https://ega.industry.com/ontologies/core/process/Condition"/>
        <process:isTriggeredBy rdf:resource="https://ega.industry.com/ontologies/core/data/eventFunctionLoadingScrap_10"/>
        <process:conditionAchieved rdf:datatype="http://www.w3.org/2001/XMLSchema#boolean">false</process:conditionAchieved>
        <rdfs:comment xml:lang="en">Condition of Step</rdfs:comment>
    </owl:NamedIndividual>
    


    <!-- https://ega.industry.com/ontologies/core/process/conditionLoadingScrap_12 -->

    <owl:NamedIndividual rdf:about="https://ega.industry.com/ontologies/core/process/conditionLoadingScrap_12">
        <rdf:type rdf:resource="https://ega.industry.com/ontologies/core/process/Condition"/>
        <process:isTriggeredBy rdf:resource="https://ega.industry.com/ontologies/core/data/eventFunctionLoadingScrap_12"/>
        <process:conditionAchieved rdf:datatype="http://www.w3.org/2001/XMLSchema#boolean">false</process:conditionAchieved>
        <rdfs:comment xml:lang="en">Condition of Step</rdfs:comment>
    </owl:NamedIndividual>
    


    <!-- https://ega.industry.com/ontologies/core/process/conditionPouringAluminiumAdjustment_10 -->

    <owl:NamedIndividual rdf:about="https://ega.industry.com/ontologies/core/process/conditionPouringAluminiumAdjustment_10">
        <rdf:type rdf:resource="https://ega.industry.com/ontologies/core/process/Condition"/>
        <process:isTriggeredBy rdf:resource="https://ega.industry.com/ontologies/core/data/eventFunctionPouringAluminiumAdjustment_10"/>
        <process:conditionAchieved rdf:datatype="http://www.w3.org/2001/XMLSchema#boolean">false</process:conditionAchieved>
        <rdfs:comment xml:lang="en">Condition of Step</rdfs:comment>
    </owl:NamedIndividual>
    


    <!-- https://ega.industry.com/ontologies/core/process/conditionPouringAluminiumAdjustment_12 -->

    <owl:NamedIndividual rdf:about="https://ega.industry.com/ontologies/core/process/conditionPouringAluminiumAdjustment_12">
        <rdf:type rdf:resource="https://ega.industry.com/ontologies/core/process/Condition"/>
        <process:isTriggeredBy rdf:resource="https://ega.industry.com/ontologies/core/data/eventFunctionPouringAluminiumAdjustment_12"/>
        <process:conditionAchieved rdf:datatype="http://www.w3.org/2001/XMLSchema#boolean">false</process:conditionAchieved>
        <rdfs:comment xml:lang="en">Condition of Step</rdfs:comment>
    </owl:NamedIndividual>
    


    <!-- https://ega.industry.com/ontologies/core/process/conditionPouringAluminium_10 -->

    <owl:NamedIndividual rdf:about="https://ega.industry.com/ontologies/core/process/conditionPouringAluminium_10">
        <rdf:type rdf:resource="https://ega.industry.com/ontologies/core/process/Condition"/>
        <process:isTriggeredBy rdf:resource="https://ega.industry.com/ontologies/core/data/eventFunctionPouringAluminium_10"/>
        <process:conditionAchieved rdf:datatype="http://www.w3.org/2001/XMLSchema#boolean">false</process:conditionAchieved>
        <rdfs:comment xml:lang="en">Condition of Step</rdfs:comment>
    </owl:NamedIndividual>
    


    <!-- https://ega.industry.com/ontologies/core/process/conditionPouringAluminium_12 -->

    <owl:NamedIndividual rdf:about="https://ega.industry.com/ontologies/core/process/conditionPouringAluminium_12">
        <rdf:type rdf:resource="https://ega.industry.com/ontologies/core/process/Condition"/>
        <process:isTriggeredBy rdf:resource="https://ega.industry.com/ontologies/core/data/eventFunctionPouringAluminium_12"/>
        <process:conditionAchieved rdf:datatype="http://www.w3.org/2001/XMLSchema#boolean">false</process:conditionAchieved>
        <rdfs:comment xml:lang="en">Condition of Step</rdfs:comment>
    </owl:NamedIndividual>
    


    <!-- https://ega.industry.com/ontologies/core/process/conditionPouringMetalsAdjustment_10 -->

    <owl:NamedIndividual rdf:about="https://ega.industry.com/ontologies/core/process/conditionPouringMetalsAdjustment_10">
        <rdf:type rdf:resource="https://ega.industry.com/ontologies/core/process/Condition"/>
        <process:isTriggeredBy rdf:resource="https://ega.industry.com/ontologies/core/data/eventFunctionPouringMetalsAdjustment_10"/>
        <process:conditionAchieved rdf:datatype="http://www.w3.org/2001/XMLSchema#boolean">false</process:conditionAchieved>
        <rdfs:comment xml:lang="en">Condition of Step</rdfs:comment>
    </owl:NamedIndividual>
    


    <!-- https://ega.industry.com/ontologies/core/process/conditionPouringMetalsAdjustment_12 -->

    <owl:NamedIndividual rdf:about="https://ega.industry.com/ontologies/core/process/conditionPouringMetalsAdjustment_12">
        <rdf:type rdf:resource="https://ega.industry.com/ontologies/core/process/Condition"/>
        <process:isTriggeredBy rdf:resource="https://ega.industry.com/ontologies/core/data/eventFunctionPouringMetalsAdjustment_12"/>
        <process:conditionAchieved rdf:datatype="http://www.w3.org/2001/XMLSchema#boolean">false</process:conditionAchieved>
        <rdfs:comment xml:lang="en">Condition of Step</rdfs:comment>
    </owl:NamedIndividual>
    


    <!-- https://ega.industry.com/ontologies/core/process/conditionPouringMetals_10 -->

    <owl:NamedIndividual rdf:about="https://ega.industry.com/ontologies/core/process/conditionPouringMetals_10">
        <rdf:type rdf:resource="https://ega.industry.com/ontologies/core/process/Condition"/>
        <process:isTriggeredBy rdf:resource="https://ega.industry.com/ontologies/core/data/eventFunctionPouringMetals_10"/>
        <process:conditionAchieved rdf:datatype="http://www.w3.org/2001/XMLSchema#boolean">false</process:conditionAchieved>
        <rdfs:comment xml:lang="en">Condition of Step</rdfs:comment>
    </owl:NamedIndividual>
    


    <!-- https://ega.industry.com/ontologies/core/process/conditionPouringMetals_12 -->

    <owl:NamedIndividual rdf:about="https://ega.industry.com/ontologies/core/process/conditionPouringMetals_12">
        <rdf:type rdf:resource="https://ega.industry.com/ontologies/core/process/Condition"/>
        <process:isTriggeredBy rdf:resource="https://ega.industry.com/ontologies/core/data/eventFunctionPouringMetals_12"/>
        <process:conditionAchieved rdf:datatype="http://www.w3.org/2001/XMLSchema#boolean">false</process:conditionAchieved>
        <rdfs:comment xml:lang="en">Condition of Step</rdfs:comment>
    </owl:NamedIndividual>
    


    <!-- https://ega.industry.com/ontologies/core/process/conditionPreheating_10 -->

    <owl:NamedIndividual rdf:about="https://ega.industry.com/ontologies/core/process/conditionPreheating_10">
        <rdf:type rdf:resource="https://ega.industry.com/ontologies/core/process/Condition"/>
        <process:isTriggeredBy rdf:resource="https://ega.industry.com/ontologies/core/data/eventFunctionPreheating_10"/>
        <process:conditionAchieved rdf:datatype="http://www.w3.org/2001/XMLSchema#boolean">false</process:conditionAchieved>
        <rdfs:comment xml:lang="en">Condition of Step</rdfs:comment>
    </owl:NamedIndividual>
    


    <!-- https://ega.industry.com/ontologies/core/process/conditionPreheating_12 -->

    <owl:NamedIndividual rdf:about="https://ega.industry.com/ontologies/core/process/conditionPreheating_12">
        <rdf:type rdf:resource="https://ega.industry.com/ontologies/core/process/Condition"/>
        <process:isTriggeredBy rdf:resource="https://ega.industry.com/ontologies/core/data/eventFunctionPreheating_12"/>
        <process:conditionAchieved rdf:datatype="http://www.w3.org/2001/XMLSchema#boolean">false</process:conditionAchieved>
        <rdfs:comment xml:lang="en">Condition of Step</rdfs:comment>
    </owl:NamedIndividual>
    


    <!-- https://ega.industry.com/ontologies/core/process/conditionSampling_10 -->

    <owl:NamedIndividual rdf:about="https://ega.industry.com/ontologies/core/process/conditionSampling_10">
        <rdf:type rdf:resource="https://ega.industry.com/ontologies/core/process/Condition"/>
        <process:isTriggeredBy rdf:resource="https://ega.industry.com/ontologies/core/data/eventFunctionSampling_10"/>
        <process:conditionAchieved rdf:datatype="http://www.w3.org/2001/XMLSchema#boolean">false</process:conditionAchieved>
        <rdfs:comment xml:lang="en">Condition of Step</rdfs:comment>
    </owl:NamedIndividual>
    


    <!-- https://ega.industry.com/ontologies/core/process/conditionSampling_12 -->

    <owl:NamedIndividual rdf:about="https://ega.industry.com/ontologies/core/process/conditionSampling_12">
        <rdf:type rdf:resource="https://ega.industry.com/ontologies/core/process/Condition"/>
        <process:isTriggeredBy rdf:resource="https://ega.industry.com/ontologies/core/data/eventFunctionSampling_12"/>
        <process:conditionAchieved rdf:datatype="http://www.w3.org/2001/XMLSchema#boolean">false</process:conditionAchieved>
        <rdfs:comment xml:lang="en">Condition of Step</rdfs:comment>
    </owl:NamedIndividual>
    


    <!-- https://ega.industry.com/ontologies/core/process/conditionSkimming_10 -->

    <owl:NamedIndividual rdf:about="https://ega.industry.com/ontologies/core/process/conditionSkimming_10">
        <rdf:type rdf:resource="https://ega.industry.com/ontologies/core/process/Condition"/>
        <process:isTriggeredBy rdf:resource="https://ega.industry.com/ontologies/core/data/eventFunctionSkimming_10"/>
        <process:conditionAchieved rdf:datatype="http://www.w3.org/2001/XMLSchema#boolean">false</process:conditionAchieved>
        <rdfs:comment xml:lang="en">Condition of Step</rdfs:comment>
    </owl:NamedIndividual>
    


    <!-- https://ega.industry.com/ontologies/core/process/conditionSkimming_12 -->

    <owl:NamedIndividual rdf:about="https://ega.industry.com/ontologies/core/process/conditionSkimming_12">
        <rdf:type rdf:resource="https://ega.industry.com/ontologies/core/process/Condition"/>
        <process:isTriggeredBy rdf:resource="https://ega.industry.com/ontologies/core/data/eventFunctionSkimming_12"/>
        <process:conditionAchieved rdf:datatype="http://www.w3.org/2001/XMLSchema#boolean">false</process:conditionAchieved>
        <rdfs:comment xml:lang="en">Condition of Step</rdfs:comment>
    </owl:NamedIndividual>
    


    <!-- https://ega.industry.com/ontologies/core/process/conditionStirring_10 -->

    <owl:NamedIndividual rdf:about="https://ega.industry.com/ontologies/core/process/conditionStirring_10">
        <rdf:type rdf:resource="https://ega.industry.com/ontologies/core/process/Condition"/>
        <process:isTriggeredBy rdf:resource="https://ega.industry.com/ontologies/core/data/eventFunctionStirring_10"/>
        <process:conditionAchieved rdf:datatype="http://www.w3.org/2001/XMLSchema#boolean">false</process:conditionAchieved>
        <rdfs:comment xml:lang="en">Condition of Step</rdfs:comment>
    </owl:NamedIndividual>
    


    <!-- https://ega.industry.com/ontologies/core/process/conditionStirring_12 -->

    <owl:NamedIndividual rdf:about="https://ega.industry.com/ontologies/core/process/conditionStirring_12">
        <rdf:type rdf:resource="https://ega.industry.com/ontologies/core/process/Condition"/>
        <process:isTriggeredBy rdf:resource="https://ega.industry.com/ontologies/core/data/eventFunctionStirring_12"/>
        <process:conditionAchieved rdf:datatype="http://www.w3.org/2001/XMLSchema#boolean">false</process:conditionAchieved>
        <rdfs:comment xml:lang="en">Condition of Step</rdfs:comment>
    </owl:NamedIndividual>
    


    <!-- https://ega.industry.com/ontologies/core/process/processFurnace_10 -->

    <owl:NamedIndividual rdf:about="https://ega.industry.com/ontologies/core/process/processFurnace_10">
        <rdf:type rdf:resource="https://ega.industry.com/ontologies/core/process/Process"/>
        <process:hasSubProcess rdf:resource="https://ega.industry.com/ontologies/core/process/SubProcessCasting_10"/>
        <process:hasSubProcess rdf:resource="https://ega.industry.com/ontologies/core/process/subProcessAdjustment_10"/>
        <process:hasSubProcess rdf:resource="https://ega.industry.com/ontologies/core/process/subProcessMaterialLoading_10"/>
        <process:hasSubProcess rdf:resource="https://ega.industry.com/ontologies/core/process/subProcessMelting_10"/>
        <process:hasSubProcess rdf:resource="https://ega.industry.com/ontologies/core/process/subProcessPreparation_10"/>
        <process:hasSubProcess rdf:resource="https://ega.industry.com/ontologies/core/process/subProcessSampleCheck_10"/>
        <process:hasAlloyCode rdf:datatype="http://www.w3.org/2001/XMLSchema#integer">0</process:hasAlloyCode>
        <process:hasAlloyCodeId rdf:datatype="http://www.w3.org/2001/XMLSchema#integer">0</process:hasAlloyCodeId>
        <process:hasBatchId rdf:datatype="http://www.w3.org/2001/XMLSchema#integer">0</process:hasBatchId>
        <process:hasBatchNo></process:hasBatchNo>
        <process:hasEndTimestamp rdf:datatype="http://www.w3.org/2001/XMLSchema#dateTime">2025-06-03T09:59:07.456561</process:hasEndTimestamp>
        <process:hasStartTimestamp rdf:datatype="http://www.w3.org/2001/XMLSchema#dateTime">2025-06-03T09:59:07.456561</process:hasStartTimestamp>
        <process:isRunning rdf:datatype="http://www.w3.org/2001/XMLSchema#boolean">false</process:isRunning>
        <rdfs:comment xml:lang="en">Overall aluminum furnace process managing the complete material processing cycle</rdfs:comment>
    </owl:NamedIndividual>
    


    <!-- https://ega.industry.com/ontologies/core/process/processFurnace_12 -->

    <owl:NamedIndividual rdf:about="https://ega.industry.com/ontologies/core/process/processFurnace_12">
        <rdf:type rdf:resource="https://ega.industry.com/ontologies/core/process/Process"/>
        <process:hasSubProcess rdf:resource="https://ega.industry.com/ontologies/core/process/SubProcessCasting_12"/>
        <process:hasSubProcess rdf:resource="https://ega.industry.com/ontologies/core/process/subProcessAdjustment_12"/>
        <process:hasSubProcess rdf:resource="https://ega.industry.com/ontologies/core/process/subProcessMaterialLoading_12"/>
        <process:hasSubProcess rdf:resource="https://ega.industry.com/ontologies/core/process/subProcessMelting_12"/>
        <process:hasSubProcess rdf:resource="https://ega.industry.com/ontologies/core/process/subProcessPreparation_12"/>
        <process:hasSubProcess rdf:resource="https://ega.industry.com/ontologies/core/process/subProcessSampleCheck_12"/>
        <process:hasAlloyCode rdf:datatype="http://www.w3.org/2001/XMLSchema#integer">0</process:hasAlloyCode>
        <process:hasAlloyCodeId rdf:datatype="http://www.w3.org/2001/XMLSchema#integer">0</process:hasAlloyCodeId>
        <process:hasBatchId rdf:datatype="http://www.w3.org/2001/XMLSchema#integer">0</process:hasBatchId>
        <process:hasBatchNo></process:hasBatchNo>
        <process:hasEndTimestamp rdf:datatype="http://www.w3.org/2001/XMLSchema#dateTime">2025-06-03T09:59:08.322482</process:hasEndTimestamp>
        <process:hasStartTimestamp rdf:datatype="http://www.w3.org/2001/XMLSchema#dateTime">2025-06-03T09:59:08.322482</process:hasStartTimestamp>
        <process:isRunning rdf:datatype="http://www.w3.org/2001/XMLSchema#boolean">false</process:isRunning>
        <rdfs:comment xml:lang="en">Overall aluminum furnace process managing the complete material processing cycle</rdfs:comment>
    </owl:NamedIndividual>
    


    <!-- https://ega.industry.com/ontologies/core/process/stepCastingStep_10 -->

    <owl:NamedIndividual rdf:about="https://ega.industry.com/ontologies/core/process/stepCastingStep_10">
        <rdf:type rdf:resource="https://ega.industry.com/ontologies/core/process/NormalStep"/>
        <rdf:type rdf:resource="https://ega.industry.com/ontologies/core/process/Step"/>
        <process:hasCondition rdf:resource="https://ega.industry.com/ontologies/core/process/conditionCasting_10"/>
        <process:hasStepType rdf:resource="https://ega.industry.com/ontologies/core/process/Machine"/>
        <process:isStepOf rdf:resource="https://ega.industry.com/ontologies/core/process/SubProcessCasting_10"/>
        <process:useAsset rdf:resource="https://ega.industry.com/ontologies/core/asset/castingSystem_10"/>
        <process:hasEndTimestamp rdf:datatype="http://www.w3.org/2001/XMLSchema#dateTime">2025-06-03T09:59:07.456561</process:hasEndTimestamp>
        <process:hasStartTimestamp rdf:datatype="http://www.w3.org/2001/XMLSchema#dateTime">2025-06-03T09:59:07.456561</process:hasStartTimestamp>
        <process:hasStepId rdf:datatype="http://www.w3.org/2001/XMLSchema#integer">13</process:hasStepId>
        <process:isCurrentStep rdf:datatype="http://www.w3.org/2001/XMLSchema#boolean">false</process:isCurrentStep>
        <rdfs:comment xml:lang="en">Step of transfer of final metal to casting system</rdfs:comment>
    </owl:NamedIndividual>
    


    <!-- https://ega.industry.com/ontologies/core/process/stepCastingStep_12 -->

    <owl:NamedIndividual rdf:about="https://ega.industry.com/ontologies/core/process/stepCastingStep_12">
        <rdf:type rdf:resource="https://ega.industry.com/ontologies/core/process/NormalStep"/>
        <rdf:type rdf:resource="https://ega.industry.com/ontologies/core/process/Step"/>
        <process:hasCondition rdf:resource="https://ega.industry.com/ontologies/core/process/conditionCasting_12"/>
        <process:hasStepType rdf:resource="https://ega.industry.com/ontologies/core/process/Machine"/>
        <process:isStepOf rdf:resource="https://ega.industry.com/ontologies/core/process/SubProcessCasting_12"/>
        <process:useAsset rdf:resource="https://ega.industry.com/ontologies/core/asset/castingSystem_12"/>
        <process:hasEndTimestamp rdf:datatype="http://www.w3.org/2001/XMLSchema#dateTime">2025-06-03T09:59:08.322482</process:hasEndTimestamp>
        <process:hasStartTimestamp rdf:datatype="http://www.w3.org/2001/XMLSchema#dateTime">2025-06-03T09:59:08.322482</process:hasStartTimestamp>
        <process:hasStepId rdf:datatype="http://www.w3.org/2001/XMLSchema#integer">13</process:hasStepId>
        <process:isCurrentStep rdf:datatype="http://www.w3.org/2001/XMLSchema#boolean">false</process:isCurrentStep>
        <rdfs:comment xml:lang="en">Step of transfer of final metal to casting system</rdfs:comment>
    </owl:NamedIndividual>
    


    <!-- https://ega.industry.com/ontologies/core/process/stepHolding_10 -->

    <owl:NamedIndividual rdf:about="https://ega.industry.com/ontologies/core/process/stepHolding_10">
        <rdf:type rdf:resource="https://ega.industry.com/ontologies/core/process/NormalStep"/>
        <rdf:type rdf:resource="https://ega.industry.com/ontologies/core/process/Step"/>
        <process:hasCondition rdf:resource="https://ega.industry.com/ontologies/core/process/conditionHolding_10"/>
        <process:hasPreviousStep rdf:resource="https://ega.industry.com/ontologies/core/process/stepStirring_10"/>
        <process:hasStepType rdf:resource="https://ega.industry.com/ontologies/core/process/Machine"/>
        <process:isStepOf rdf:resource="https://ega.industry.com/ontologies/core/process/subProcessMelting_10"/>
        <process:useAsset rdf:resource="https://ega.industry.com/ontologies/core/asset/tank_10"/>
        <process:hasEndTimestamp rdf:datatype="http://www.w3.org/2001/XMLSchema#dateTime">2025-06-03T09:59:07.456561</process:hasEndTimestamp>
        <process:hasStartTimestamp rdf:datatype="http://www.w3.org/2001/XMLSchema#dateTime">2025-06-03T09:59:07.456561</process:hasStartTimestamp>
        <process:hasStepId rdf:datatype="http://www.w3.org/2001/XMLSchema#integer">7</process:hasStepId>
        <process:isCurrentStep rdf:datatype="http://www.w3.org/2001/XMLSchema#boolean">false</process:isCurrentStep>
        <rdfs:comment xml:lang="en">Maintaining stable temperature for homogenization</rdfs:comment>
    </owl:NamedIndividual>
    


    <!-- https://ega.industry.com/ontologies/core/process/stepHolding_12 -->

    <owl:NamedIndividual rdf:about="https://ega.industry.com/ontologies/core/process/stepHolding_12">
        <rdf:type rdf:resource="https://ega.industry.com/ontologies/core/process/NormalStep"/>
        <rdf:type rdf:resource="https://ega.industry.com/ontologies/core/process/Step"/>
        <process:hasCondition rdf:resource="https://ega.industry.com/ontologies/core/process/conditionHolding_12"/>
        <process:hasPreviousStep rdf:resource="https://ega.industry.com/ontologies/core/process/stepStirring_12"/>
        <process:hasStepType rdf:resource="https://ega.industry.com/ontologies/core/process/Machine"/>
        <process:isStepOf rdf:resource="https://ega.industry.com/ontologies/core/process/subProcessMelting_12"/>
        <process:useAsset rdf:resource="https://ega.industry.com/ontologies/core/asset/tank_12"/>
        <process:hasEndTimestamp rdf:datatype="http://www.w3.org/2001/XMLSchema#dateTime">2025-06-03T09:59:08.322482</process:hasEndTimestamp>
        <process:hasStartTimestamp rdf:datatype="http://www.w3.org/2001/XMLSchema#dateTime">2025-06-03T09:59:08.322482</process:hasStartTimestamp>
        <process:hasStepId rdf:datatype="http://www.w3.org/2001/XMLSchema#integer">7</process:hasStepId>
        <process:isCurrentStep rdf:datatype="http://www.w3.org/2001/XMLSchema#boolean">false</process:isCurrentStep>
        <rdfs:comment xml:lang="en">Maintaining stable temperature for homogenization</rdfs:comment>
    </owl:NamedIndividual>
    


    <!-- https://ega.industry.com/ontologies/core/process/stepLaboratoryAnalysis_10 -->

    <owl:NamedIndividual rdf:about="https://ega.industry.com/ontologies/core/process/stepLaboratoryAnalysis_10">
        <rdf:type rdf:resource="https://ega.industry.com/ontologies/core/process/IterativeStep"/>
        <rdf:type rdf:resource="https://ega.industry.com/ontologies/core/process/Step"/>
        <process:hasCondition rdf:resource="https://ega.industry.com/ontologies/core/process/conditionLaboratoryAnalysis_10"/>
        <process:hasPreviousStep rdf:resource="https://ega.industry.com/ontologies/core/process/stepSampling_10"/>
        <process:hasStepType rdf:resource="https://ega.industry.com/ontologies/core/process/Machine"/>
        <process:isStepOf rdf:resource="https://ega.industry.com/ontologies/core/process/subProcessSampleCheck_10"/>
        <process:useAsset rdf:resource="https://ega.industry.com/ontologies/core/asset/tank_10"/>
        <process:hasEndTimestamp rdf:datatype="http://www.w3.org/2001/XMLSchema#dateTime">2025-06-03T09:59:07.456561</process:hasEndTimestamp>
        <process:hasStartTimestamp rdf:datatype="http://www.w3.org/2001/XMLSchema#dateTime">2025-06-03T09:59:07.456561</process:hasStartTimestamp>
        <process:hasStepId rdf:datatype="http://www.w3.org/2001/XMLSchema#integer">9</process:hasStepId>
        <process:isCurrentStep rdf:datatype="http://www.w3.org/2001/XMLSchema#boolean">false</process:isCurrentStep>
        <process:isIterationCompleted rdf:datatype="http://www.w3.org/2001/XMLSchema#boolean">false</process:isIterationCompleted>
        <process:iterationCount rdf:datatype="http://www.w3.org/2001/XMLSchema#integer">0</process:iterationCount>
        <rdfs:comment xml:lang="en">Chemical and physical testing of samples</rdfs:comment>
    </owl:NamedIndividual>
    


    <!-- https://ega.industry.com/ontologies/core/process/stepLaboratoryAnalysis_12 -->

    <owl:NamedIndividual rdf:about="https://ega.industry.com/ontologies/core/process/stepLaboratoryAnalysis_12">
        <rdf:type rdf:resource="https://ega.industry.com/ontologies/core/process/IterativeStep"/>
        <rdf:type rdf:resource="https://ega.industry.com/ontologies/core/process/Step"/>
        <process:hasCondition rdf:resource="https://ega.industry.com/ontologies/core/process/conditionLaboratoryAnalysis_12"/>
        <process:hasPreviousStep rdf:resource="https://ega.industry.com/ontologies/core/process/stepSampling_12"/>
        <process:hasStepType rdf:resource="https://ega.industry.com/ontologies/core/process/Machine"/>
        <process:isStepOf rdf:resource="https://ega.industry.com/ontologies/core/process/subProcessSampleCheck_12"/>
        <process:useAsset rdf:resource="https://ega.industry.com/ontologies/core/asset/tank_12"/>
        <process:hasEndTimestamp rdf:datatype="http://www.w3.org/2001/XMLSchema#dateTime">2025-06-03T09:59:08.322482</process:hasEndTimestamp>
        <process:hasStartTimestamp rdf:datatype="http://www.w3.org/2001/XMLSchema#dateTime">2025-06-03T09:59:08.322482</process:hasStartTimestamp>
        <process:hasStepId rdf:datatype="http://www.w3.org/2001/XMLSchema#integer">9</process:hasStepId>
        <process:isCurrentStep rdf:datatype="http://www.w3.org/2001/XMLSchema#boolean">false</process:isCurrentStep>
        <process:isIterationCompleted rdf:datatype="http://www.w3.org/2001/XMLSchema#boolean">false</process:isIterationCompleted>
        <process:iterationCount rdf:datatype="http://www.w3.org/2001/XMLSchema#integer">0</process:iterationCount>
        <rdfs:comment xml:lang="en">Chemical and physical testing of samples</rdfs:comment>
    </owl:NamedIndividual>
    


    <!-- https://ega.industry.com/ontologies/core/process/stepLoadingScrapAdjustment_10 -->

    <owl:NamedIndividual rdf:about="https://ega.industry.com/ontologies/core/process/stepLoadingScrapAdjustment_10">
        <rdf:type rdf:resource="https://ega.industry.com/ontologies/core/process/NormalStep"/>
        <rdf:type rdf:resource="https://ega.industry.com/ontologies/core/process/Step"/>
        <process:hasCondition rdf:resource="https://ega.industry.com/ontologies/core/process/conditionLoadingScrapAdjustment_10"/>
        <process:hasNextStep rdf:resource="https://ega.industry.com/ontologies/core/process/stepPouringAluminiumAdjustment_10"/>
        <process:hasStepType rdf:resource="https://ega.industry.com/ontologies/core/process/Operator"/>
        <process:isStepOf rdf:resource="https://ega.industry.com/ontologies/core/process/subProcessAdjustment_10"/>
        <process:useAsset rdf:resource="https://ega.industry.com/ontologies/core/asset/tank_10"/>
        <process:hasEndTimestamp rdf:datatype="http://www.w3.org/2001/XMLSchema#dateTime">2025-06-03T09:59:07.456561</process:hasEndTimestamp>
        <process:hasStartTimestamp rdf:datatype="http://www.w3.org/2001/XMLSchema#dateTime">2025-06-03T09:59:07.456561</process:hasStartTimestamp>
        <process:hasStepId rdf:datatype="http://www.w3.org/2001/XMLSchema#integer">10</process:hasStepId>
        <process:isCurrentStep rdf:datatype="http://www.w3.org/2001/XMLSchema#boolean">false</process:isCurrentStep>
        <rdfs:comment xml:lang="en">Introduction of recycled aluminium after a laboratory analysis</rdfs:comment>
    </owl:NamedIndividual>
    


    <!-- https://ega.industry.com/ontologies/core/process/stepLoadingScrapAdjustment_12 -->

    <owl:NamedIndividual rdf:about="https://ega.industry.com/ontologies/core/process/stepLoadingScrapAdjustment_12">
        <rdf:type rdf:resource="https://ega.industry.com/ontologies/core/process/NormalStep"/>
        <rdf:type rdf:resource="https://ega.industry.com/ontologies/core/process/Step"/>
        <process:hasCondition rdf:resource="https://ega.industry.com/ontologies/core/process/conditionLoadingScrapAdjustment_12"/>
        <process:hasNextStep rdf:resource="https://ega.industry.com/ontologies/core/process/stepPouringAluminiumAdjustment_12"/>
        <process:hasStepType rdf:resource="https://ega.industry.com/ontologies/core/process/Operator"/>
        <process:isStepOf rdf:resource="https://ega.industry.com/ontologies/core/process/subProcessAdjustment_12"/>
        <process:useAsset rdf:resource="https://ega.industry.com/ontologies/core/asset/tank_12"/>
        <process:hasEndTimestamp rdf:datatype="http://www.w3.org/2001/XMLSchema#dateTime">2025-06-03T09:59:08.322482</process:hasEndTimestamp>
        <process:hasStartTimestamp rdf:datatype="http://www.w3.org/2001/XMLSchema#dateTime">2025-06-03T09:59:08.322482</process:hasStartTimestamp>
        <process:hasStepId rdf:datatype="http://www.w3.org/2001/XMLSchema#integer">10</process:hasStepId>
        <process:isCurrentStep rdf:datatype="http://www.w3.org/2001/XMLSchema#boolean">false</process:isCurrentStep>
        <rdfs:comment xml:lang="en">Introduction of recycled aluminium after a laboratory analysis</rdfs:comment>
    </owl:NamedIndividual>
    


    <!-- https://ega.industry.com/ontologies/core/process/stepLoadingScrap_10 -->

    <owl:NamedIndividual rdf:about="https://ega.industry.com/ontologies/core/process/stepLoadingScrap_10">
        <rdf:type rdf:resource="https://ega.industry.com/ontologies/core/process/NormalStep"/>
        <rdf:type rdf:resource="https://ega.industry.com/ontologies/core/process/Step"/>
        <process:hasCondition rdf:resource="https://ega.industry.com/ontologies/core/process/conditionLoadingScrap_10"/>
        <process:hasNextStep rdf:resource="https://ega.industry.com/ontologies/core/process/stepPouringAluminium_10"/>
        <process:hasStepType rdf:resource="https://ega.industry.com/ontologies/core/process/Machine"/>
        <process:isStepOf rdf:resource="https://ega.industry.com/ontologies/core/process/subProcessMaterialLoading_10"/>
        <process:useAsset rdf:resource="https://ega.industry.com/ontologies/core/asset/tank_10"/>
        <process:hasEndTimestamp rdf:datatype="http://www.w3.org/2001/XMLSchema#dateTime">2025-06-03T09:59:07.456561</process:hasEndTimestamp>
        <process:hasStartTimestamp rdf:datatype="http://www.w3.org/2001/XMLSchema#dateTime">2025-06-03T09:59:07.456561</process:hasStartTimestamp>
        <process:hasStepId rdf:datatype="http://www.w3.org/2001/XMLSchema#integer">3</process:hasStepId>
        <process:isCurrentStep rdf:datatype="http://www.w3.org/2001/XMLSchema#boolean">false</process:isCurrentStep>
        <rdfs:comment xml:lang="en">Introduction of recycled aluminium</rdfs:comment>
    </owl:NamedIndividual>
    


    <!-- https://ega.industry.com/ontologies/core/process/stepLoadingScrap_12 -->

    <owl:NamedIndividual rdf:about="https://ega.industry.com/ontologies/core/process/stepLoadingScrap_12">
        <rdf:type rdf:resource="https://ega.industry.com/ontologies/core/process/NormalStep"/>
        <rdf:type rdf:resource="https://ega.industry.com/ontologies/core/process/Step"/>
        <process:hasCondition rdf:resource="https://ega.industry.com/ontologies/core/process/conditionLoadingScrap_12"/>
        <process:hasNextStep rdf:resource="https://ega.industry.com/ontologies/core/process/stepPouringAluminium_12"/>
        <process:hasStepType rdf:resource="https://ega.industry.com/ontologies/core/process/Machine"/>
        <process:isStepOf rdf:resource="https://ega.industry.com/ontologies/core/process/subProcessMaterialLoading_12"/>
        <process:useAsset rdf:resource="https://ega.industry.com/ontologies/core/asset/tank_12"/>
        <process:hasEndTimestamp rdf:datatype="http://www.w3.org/2001/XMLSchema#dateTime">2025-06-03T09:59:08.322482</process:hasEndTimestamp>
        <process:hasStartTimestamp rdf:datatype="http://www.w3.org/2001/XMLSchema#dateTime">2025-06-03T09:59:08.322482</process:hasStartTimestamp>
        <process:hasStepId rdf:datatype="http://www.w3.org/2001/XMLSchema#integer">3</process:hasStepId>
        <process:isCurrentStep rdf:datatype="http://www.w3.org/2001/XMLSchema#boolean">false</process:isCurrentStep>
        <rdfs:comment xml:lang="en">Introduction of recycled aluminium</rdfs:comment>
    </owl:NamedIndividual>
    


    <!-- https://ega.industry.com/ontologies/core/process/stepPouringAluminiumAdjustment_10 -->

    <owl:NamedIndividual rdf:about="https://ega.industry.com/ontologies/core/process/stepPouringAluminiumAdjustment_10">
        <rdf:type rdf:resource="https://ega.industry.com/ontologies/core/process/NormalStep"/>
        <rdf:type rdf:resource="https://ega.industry.com/ontologies/core/process/Step"/>
        <process:hasCondition rdf:resource="https://ega.industry.com/ontologies/core/process/conditionPouringAluminiumAdjustment_10"/>
        <process:hasNextStep rdf:resource="https://ega.industry.com/ontologies/core/process/stepPouringMetalsAdjustment_10"/>
        <process:hasPreviousStep rdf:resource="https://ega.industry.com/ontologies/core/process/stepLoadingScrapAdjustment_10"/>
        <process:hasStepType rdf:resource="https://ega.industry.com/ontologies/core/process/Machine"/>
        <process:isStepOf rdf:resource="https://ega.industry.com/ontologies/core/process/subProcessAdjustment_10"/>
        <process:useAsset rdf:resource="https://ega.industry.com/ontologies/core/asset/tank_10"/>
        <process:hasEndTimestamp rdf:datatype="http://www.w3.org/2001/XMLSchema#dateTime">2025-06-03T09:59:07.456561</process:hasEndTimestamp>
        <process:hasStartTimestamp rdf:datatype="http://www.w3.org/2001/XMLSchema#dateTime">2025-06-03T09:59:07.456561</process:hasStartTimestamp>
        <process:hasStepId rdf:datatype="http://www.w3.org/2001/XMLSchema#integer">11</process:hasStepId>
        <process:isCurrentStep rdf:datatype="http://www.w3.org/2001/XMLSchema#boolean">false</process:isCurrentStep>
        <rdfs:comment xml:lang="en">Addition of primary liquid aluminium after a laboratory analysis</rdfs:comment>
    </owl:NamedIndividual>
    


    <!-- https://ega.industry.com/ontologies/core/process/stepPouringAluminiumAdjustment_12 -->

    <owl:NamedIndividual rdf:about="https://ega.industry.com/ontologies/core/process/stepPouringAluminiumAdjustment_12">
        <rdf:type rdf:resource="https://ega.industry.com/ontologies/core/process/NormalStep"/>
        <rdf:type rdf:resource="https://ega.industry.com/ontologies/core/process/Step"/>
        <process:hasCondition rdf:resource="https://ega.industry.com/ontologies/core/process/conditionPouringAluminiumAdjustment_12"/>
        <process:hasNextStep rdf:resource="https://ega.industry.com/ontologies/core/process/stepPouringMetalsAdjustment_12"/>
        <process:hasPreviousStep rdf:resource="https://ega.industry.com/ontologies/core/process/stepLoadingScrapAdjustment_12"/>
        <process:hasStepType rdf:resource="https://ega.industry.com/ontologies/core/process/Machine"/>
        <process:isStepOf rdf:resource="https://ega.industry.com/ontologies/core/process/subProcessAdjustment_12"/>
        <process:useAsset rdf:resource="https://ega.industry.com/ontologies/core/asset/tank_12"/>
        <process:hasEndTimestamp rdf:datatype="http://www.w3.org/2001/XMLSchema#dateTime">2025-06-03T09:59:08.322482</process:hasEndTimestamp>
        <process:hasStartTimestamp rdf:datatype="http://www.w3.org/2001/XMLSchema#dateTime">2025-06-03T09:59:08.322482</process:hasStartTimestamp>
        <process:hasStepId rdf:datatype="http://www.w3.org/2001/XMLSchema#integer">11</process:hasStepId>
        <process:isCurrentStep rdf:datatype="http://www.w3.org/2001/XMLSchema#boolean">false</process:isCurrentStep>
        <rdfs:comment xml:lang="en">Addition of primary liquid aluminium after a laboratory analysis</rdfs:comment>
    </owl:NamedIndividual>
    


    <!-- https://ega.industry.com/ontologies/core/process/stepPouringAluminium_10 -->

    <owl:NamedIndividual rdf:about="https://ega.industry.com/ontologies/core/process/stepPouringAluminium_10">
        <rdf:type rdf:resource="https://ega.industry.com/ontologies/core/process/NormalStep"/>
        <rdf:type rdf:resource="https://ega.industry.com/ontologies/core/process/Step"/>
        <process:hasCondition rdf:resource="https://ega.industry.com/ontologies/core/process/conditionPouringAluminium_10"/>
        <process:hasNextStep rdf:resource="https://ega.industry.com/ontologies/core/process/stepPouringMetals_10"/>
        <process:hasPreviousStep rdf:resource="https://ega.industry.com/ontologies/core/process/stepLoadingScrap_10"/>
        <process:hasStepType rdf:resource="https://ega.industry.com/ontologies/core/process/Operator"/>
        <process:isStepOf rdf:resource="https://ega.industry.com/ontologies/core/process/subProcessMaterialLoading_10"/>
        <process:useAsset rdf:resource="https://ega.industry.com/ontologies/core/asset/tank_10"/>
        <process:hasEndTimestamp rdf:datatype="http://www.w3.org/2001/XMLSchema#dateTime">2025-06-03T09:59:07.456561</process:hasEndTimestamp>
        <process:hasStartTimestamp rdf:datatype="http://www.w3.org/2001/XMLSchema#dateTime">2025-06-03T09:59:07.456561</process:hasStartTimestamp>
        <process:hasStepId rdf:datatype="http://www.w3.org/2001/XMLSchema#integer">4</process:hasStepId>
        <process:isCurrentStep rdf:datatype="http://www.w3.org/2001/XMLSchema#boolean">false</process:isCurrentStep>
        <rdfs:comment xml:lang="en">Addition of primary liquid aluminium</rdfs:comment>
    </owl:NamedIndividual>
    


    <!-- https://ega.industry.com/ontologies/core/process/stepPouringAluminium_12 -->

    <owl:NamedIndividual rdf:about="https://ega.industry.com/ontologies/core/process/stepPouringAluminium_12">
        <rdf:type rdf:resource="https://ega.industry.com/ontologies/core/process/NormalStep"/>
        <rdf:type rdf:resource="https://ega.industry.com/ontologies/core/process/Step"/>
        <process:hasCondition rdf:resource="https://ega.industry.com/ontologies/core/process/conditionPouringAluminium_12"/>
        <process:hasNextStep rdf:resource="https://ega.industry.com/ontologies/core/process/stepPouringMetals_12"/>
        <process:hasPreviousStep rdf:resource="https://ega.industry.com/ontologies/core/process/stepLoadingScrap_12"/>
        <process:hasStepType rdf:resource="https://ega.industry.com/ontologies/core/process/Operator"/>
        <process:isStepOf rdf:resource="https://ega.industry.com/ontologies/core/process/subProcessMaterialLoading_12"/>
        <process:useAsset rdf:resource="https://ega.industry.com/ontologies/core/asset/tank_12"/>
        <process:hasEndTimestamp rdf:datatype="http://www.w3.org/2001/XMLSchema#dateTime">2025-06-03T09:59:08.322482</process:hasEndTimestamp>
        <process:hasStartTimestamp rdf:datatype="http://www.w3.org/2001/XMLSchema#dateTime">2025-06-03T09:59:08.322482</process:hasStartTimestamp>
        <process:hasStepId rdf:datatype="http://www.w3.org/2001/XMLSchema#integer">4</process:hasStepId>
        <process:isCurrentStep rdf:datatype="http://www.w3.org/2001/XMLSchema#boolean">false</process:isCurrentStep>
        <rdfs:comment xml:lang="en">Addition of primary liquid aluminium</rdfs:comment>
    </owl:NamedIndividual>
    


    <!-- https://ega.industry.com/ontologies/core/process/stepPouringMetalsAdjustment_10 -->

    <owl:NamedIndividual rdf:about="https://ega.industry.com/ontologies/core/process/stepPouringMetalsAdjustment_10">
        <rdf:type rdf:resource="https://ega.industry.com/ontologies/core/process/NormalStep"/>
        <rdf:type rdf:resource="https://ega.industry.com/ontologies/core/process/Step"/>
        <process:hasCondition rdf:resource="https://ega.industry.com/ontologies/core/process/conditionPouringMetalsAdjustment_10"/>
        <process:hasPreviousStep rdf:resource="https://ega.industry.com/ontologies/core/process/stepPouringAluminiumAdjustment_10"/>
        <process:hasStepType rdf:resource="https://ega.industry.com/ontologies/core/process/Operator"/>
        <process:isStepOf rdf:resource="https://ega.industry.com/ontologies/core/process/subProcessAdjustment_10"/>
        <process:useAsset rdf:resource="https://ega.industry.com/ontologies/core/asset/tank_10"/>
        <process:hasEndTimestamp rdf:datatype="http://www.w3.org/2001/XMLSchema#dateTime">2025-06-03T09:59:07.456561</process:hasEndTimestamp>
        <process:hasStartTimestamp rdf:datatype="http://www.w3.org/2001/XMLSchema#dateTime">2025-06-03T09:59:07.456561</process:hasStartTimestamp>
        <process:hasStepId rdf:datatype="http://www.w3.org/2001/XMLSchema#integer">12</process:hasStepId>
        <process:isCurrentStep rdf:datatype="http://www.w3.org/2001/XMLSchema#boolean">false</process:isCurrentStep>
        <rdfs:comment xml:lang="en">Addition of alloying elements after a laboratory analysis</rdfs:comment>
    </owl:NamedIndividual>
    


    <!-- https://ega.industry.com/ontologies/core/process/stepPouringMetalsAdjustment_12 -->

    <owl:NamedIndividual rdf:about="https://ega.industry.com/ontologies/core/process/stepPouringMetalsAdjustment_12">
        <rdf:type rdf:resource="https://ega.industry.com/ontologies/core/process/NormalStep"/>
        <rdf:type rdf:resource="https://ega.industry.com/ontologies/core/process/Step"/>
        <process:hasCondition rdf:resource="https://ega.industry.com/ontologies/core/process/conditionPouringMetalsAdjustment_12"/>
        <process:hasPreviousStep rdf:resource="https://ega.industry.com/ontologies/core/process/stepPouringAluminiumAdjustment_12"/>
        <process:hasStepType rdf:resource="https://ega.industry.com/ontologies/core/process/Operator"/>
        <process:isStepOf rdf:resource="https://ega.industry.com/ontologies/core/process/subProcessAdjustment_12"/>
        <process:useAsset rdf:resource="https://ega.industry.com/ontologies/core/asset/tank_12"/>
        <process:hasEndTimestamp rdf:datatype="http://www.w3.org/2001/XMLSchema#dateTime">2025-06-03T09:59:08.322482</process:hasEndTimestamp>
        <process:hasStartTimestamp rdf:datatype="http://www.w3.org/2001/XMLSchema#dateTime">2025-06-03T09:59:08.322482</process:hasStartTimestamp>
        <process:hasStepId rdf:datatype="http://www.w3.org/2001/XMLSchema#integer">12</process:hasStepId>
        <process:isCurrentStep rdf:datatype="http://www.w3.org/2001/XMLSchema#boolean">false</process:isCurrentStep>
        <rdfs:comment xml:lang="en">Addition of alloying elements after a laboratory analysis</rdfs:comment>
    </owl:NamedIndividual>
    


    <!-- https://ega.industry.com/ontologies/core/process/stepPouringMetals_10 -->

    <owl:NamedIndividual rdf:about="https://ega.industry.com/ontologies/core/process/stepPouringMetals_10">
        <rdf:type rdf:resource="https://ega.industry.com/ontologies/core/process/NormalStep"/>
        <rdf:type rdf:resource="https://ega.industry.com/ontologies/core/process/Step"/>
        <process:hasCondition rdf:resource="https://ega.industry.com/ontologies/core/process/conditionPouringMetals_10"/>
        <process:hasPreviousStep rdf:resource="https://ega.industry.com/ontologies/core/process/stepPouringAluminium_10"/>
        <process:hasStepType rdf:resource="https://ega.industry.com/ontologies/core/process/Machine"/>
        <process:isStepOf rdf:resource="https://ega.industry.com/ontologies/core/process/subProcessMaterialLoading_10"/>
        <process:useAsset rdf:resource="https://ega.industry.com/ontologies/core/asset/tank_10"/>
        <process:hasEndTimestamp rdf:datatype="http://www.w3.org/2001/XMLSchema#dateTime">2025-06-03T09:59:07.456561</process:hasEndTimestamp>
        <process:hasStartTimestamp rdf:datatype="http://www.w3.org/2001/XMLSchema#dateTime">2025-06-03T09:59:07.456561</process:hasStartTimestamp>
        <process:hasStepId rdf:datatype="http://www.w3.org/2001/XMLSchema#integer">5</process:hasStepId>
        <process:isCurrentStep rdf:datatype="http://www.w3.org/2001/XMLSchema#boolean">false</process:isCurrentStep>
        <rdfs:comment xml:lang="en">Addition of alloying elements</rdfs:comment>
    </owl:NamedIndividual>
    


    <!-- https://ega.industry.com/ontologies/core/process/stepPouringMetals_12 -->

    <owl:NamedIndividual rdf:about="https://ega.industry.com/ontologies/core/process/stepPouringMetals_12">
        <rdf:type rdf:resource="https://ega.industry.com/ontologies/core/process/NormalStep"/>
        <rdf:type rdf:resource="https://ega.industry.com/ontologies/core/process/Step"/>
        <process:hasCondition rdf:resource="https://ega.industry.com/ontologies/core/process/conditionPouringMetals_12"/>
        <process:hasPreviousStep rdf:resource="https://ega.industry.com/ontologies/core/process/stepPouringAluminium_12"/>
        <process:hasStepType rdf:resource="https://ega.industry.com/ontologies/core/process/Machine"/>
        <process:isStepOf rdf:resource="https://ega.industry.com/ontologies/core/process/subProcessMaterialLoading_12"/>
        <process:useAsset rdf:resource="https://ega.industry.com/ontologies/core/asset/tank_12"/>
        <process:hasEndTimestamp rdf:datatype="http://www.w3.org/2001/XMLSchema#dateTime">2025-06-03T09:59:08.322482</process:hasEndTimestamp>
        <process:hasStartTimestamp rdf:datatype="http://www.w3.org/2001/XMLSchema#dateTime">2025-06-03T09:59:08.322482</process:hasStartTimestamp>
        <process:hasStepId rdf:datatype="http://www.w3.org/2001/XMLSchema#integer">5</process:hasStepId>
        <process:isCurrentStep rdf:datatype="http://www.w3.org/2001/XMLSchema#boolean">false</process:isCurrentStep>
        <rdfs:comment xml:lang="en">Addition of alloying elements</rdfs:comment>
    </owl:NamedIndividual>
    


    <!-- https://ega.industry.com/ontologies/core/process/stepPreheating_10 -->

    <owl:NamedIndividual rdf:about="https://ega.industry.com/ontologies/core/process/stepPreheating_10">
        <rdf:type rdf:resource="https://ega.industry.com/ontologies/core/process/NormalStep"/>
        <rdf:type rdf:resource="https://ega.industry.com/ontologies/core/process/Step"/>
        <process:hasCondition rdf:resource="https://ega.industry.com/ontologies/core/process/conditionPreheating_10"/>
        <process:hasNextStep rdf:resource="https://ega.industry.com/ontologies/core/process/stepSkimming_10"/>
        <process:hasStepType rdf:resource="https://ega.industry.com/ontologies/core/process/Operator"/>
        <process:isStepOf rdf:resource="https://ega.industry.com/ontologies/core/process/subProcessPreparation_10"/>
        <process:useAsset rdf:resource="https://ega.industry.com/ontologies/core/asset/burner_10"/>
        <process:hasEndTimestamp rdf:datatype="http://www.w3.org/2001/XMLSchema#dateTime">2025-06-03T09:59:07.456561</process:hasEndTimestamp>
        <process:hasStartTimestamp rdf:datatype="http://www.w3.org/2001/XMLSchema#dateTime">2025-06-03T09:59:07.456561</process:hasStartTimestamp>
        <process:hasStepId rdf:datatype="http://www.w3.org/2001/XMLSchema#integer">1</process:hasStepId>
        <process:isCurrentStep rdf:datatype="http://www.w3.org/2001/XMLSchema#boolean">false</process:isCurrentStep>
        <rdfs:comment xml:lang="en">Bringing furnace to operational temperature</rdfs:comment>
    </owl:NamedIndividual>
    


    <!-- https://ega.industry.com/ontologies/core/process/stepPreheating_12 -->

    <owl:NamedIndividual rdf:about="https://ega.industry.com/ontologies/core/process/stepPreheating_12">
        <rdf:type rdf:resource="https://ega.industry.com/ontologies/core/process/NormalStep"/>
        <rdf:type rdf:resource="https://ega.industry.com/ontologies/core/process/Step"/>
        <process:hasCondition rdf:resource="https://ega.industry.com/ontologies/core/process/conditionPreheating_12"/>
        <process:hasNextStep rdf:resource="https://ega.industry.com/ontologies/core/process/stepSkimming_12"/>
        <process:hasStepType rdf:resource="https://ega.industry.com/ontologies/core/process/Operator"/>
        <process:isStepOf rdf:resource="https://ega.industry.com/ontologies/core/process/subProcessPreparation_12"/>
        <process:useAsset rdf:resource="https://ega.industry.com/ontologies/core/asset/burner_12"/>
        <process:hasEndTimestamp rdf:datatype="http://www.w3.org/2001/XMLSchema#dateTime">2025-06-03T09:59:08.322482</process:hasEndTimestamp>
        <process:hasStartTimestamp rdf:datatype="http://www.w3.org/2001/XMLSchema#dateTime">2025-06-03T09:59:08.322482</process:hasStartTimestamp>
        <process:hasStepId rdf:datatype="http://www.w3.org/2001/XMLSchema#integer">1</process:hasStepId>
        <process:isCurrentStep rdf:datatype="http://www.w3.org/2001/XMLSchema#boolean">false</process:isCurrentStep>
        <rdfs:comment xml:lang="en">Bringing furnace to operational temperature</rdfs:comment>
    </owl:NamedIndividual>
    


    <!-- https://ega.industry.com/ontologies/core/process/stepSampling_10 -->

    <owl:NamedIndividual rdf:about="https://ega.industry.com/ontologies/core/process/stepSampling_10">
        <rdf:type rdf:resource="https://ega.industry.com/ontologies/core/process/NormalStep"/>
        <rdf:type rdf:resource="https://ega.industry.com/ontologies/core/process/Step"/>
        <process:hasCondition rdf:resource="https://ega.industry.com/ontologies/core/process/conditionSampling_10"/>
        <process:hasNextStep rdf:resource="https://ega.industry.com/ontologies/core/process/stepLaboratoryAnalysis_10"/>
        <process:hasStepType rdf:resource="https://ega.industry.com/ontologies/core/process/Operator"/>
        <process:isStepOf rdf:resource="https://ega.industry.com/ontologies/core/process/subProcessSampleCheck_10"/>
        <process:useAsset rdf:resource="https://ega.industry.com/ontologies/core/asset/tank_10"/>
        <process:hasEndTimestamp rdf:datatype="http://www.w3.org/2001/XMLSchema#dateTime">2025-06-03T09:59:07.456561</process:hasEndTimestamp>
        <process:hasStartTimestamp rdf:datatype="http://www.w3.org/2001/XMLSchema#dateTime">2025-06-03T09:59:07.456561</process:hasStartTimestamp>
        <process:hasStepId rdf:datatype="http://www.w3.org/2001/XMLSchema#integer">8</process:hasStepId>
        <process:isCurrentStep rdf:datatype="http://www.w3.org/2001/XMLSchema#boolean">false</process:isCurrentStep>
        <rdfs:comment xml:lang="en">Collection of material samples</rdfs:comment>
    </owl:NamedIndividual>
    


    <!-- https://ega.industry.com/ontologies/core/process/stepSampling_12 -->

    <owl:NamedIndividual rdf:about="https://ega.industry.com/ontologies/core/process/stepSampling_12">
        <rdf:type rdf:resource="https://ega.industry.com/ontologies/core/process/NormalStep"/>
        <rdf:type rdf:resource="https://ega.industry.com/ontologies/core/process/Step"/>
        <process:hasCondition rdf:resource="https://ega.industry.com/ontologies/core/process/conditionSampling_12"/>
        <process:hasNextStep rdf:resource="https://ega.industry.com/ontologies/core/process/stepLaboratoryAnalysis_12"/>
        <process:hasStepType rdf:resource="https://ega.industry.com/ontologies/core/process/Operator"/>
        <process:isStepOf rdf:resource="https://ega.industry.com/ontologies/core/process/subProcessSampleCheck_12"/>
        <process:useAsset rdf:resource="https://ega.industry.com/ontologies/core/asset/tank_12"/>
        <process:hasEndTimestamp rdf:datatype="http://www.w3.org/2001/XMLSchema#dateTime">2025-06-03T09:59:08.322482</process:hasEndTimestamp>
        <process:hasStartTimestamp rdf:datatype="http://www.w3.org/2001/XMLSchema#dateTime">2025-06-03T09:59:08.322482</process:hasStartTimestamp>
        <process:hasStepId rdf:datatype="http://www.w3.org/2001/XMLSchema#integer">8</process:hasStepId>
        <process:isCurrentStep rdf:datatype="http://www.w3.org/2001/XMLSchema#boolean">false</process:isCurrentStep>
        <rdfs:comment xml:lang="en">Collection of material samples</rdfs:comment>
    </owl:NamedIndividual>
    


    <!-- https://ega.industry.com/ontologies/core/process/stepSkimming_10 -->

    <owl:NamedIndividual rdf:about="https://ega.industry.com/ontologies/core/process/stepSkimming_10">
        <rdf:type rdf:resource="https://ega.industry.com/ontologies/core/process/NormalStep"/>
        <rdf:type rdf:resource="https://ega.industry.com/ontologies/core/process/Step"/>
        <process:hasCondition rdf:resource="https://ega.industry.com/ontologies/core/process/conditionSkimming_10"/>
        <process:hasPreviousStep rdf:resource="https://ega.industry.com/ontologies/core/process/stepPreheating_10"/>
        <process:hasStepType rdf:resource="https://ega.industry.com/ontologies/core/process/Operator"/>
        <process:isStepOf rdf:resource="https://ega.industry.com/ontologies/core/process/subProcessPreparation_10"/>
        <process:useAsset rdf:resource="https://ega.industry.com/ontologies/core/asset/tank_10"/>
        <process:hasEndTimestamp rdf:datatype="http://www.w3.org/2001/XMLSchema#dateTime">2025-06-03T09:59:07.456561</process:hasEndTimestamp>
        <process:hasStartTimestamp rdf:datatype="http://www.w3.org/2001/XMLSchema#dateTime">2025-06-03T09:59:07.456561</process:hasStartTimestamp>
        <process:hasStepId rdf:datatype="http://www.w3.org/2001/XMLSchema#integer">2</process:hasStepId>
        <process:isCurrentStep rdf:datatype="http://www.w3.org/2001/XMLSchema#boolean">false</process:isCurrentStep>
        <rdfs:comment xml:lang="en">Removal of oxidized material (dross) from surface</rdfs:comment>
    </owl:NamedIndividual>
    


    <!-- https://ega.industry.com/ontologies/core/process/stepSkimming_12 -->

    <owl:NamedIndividual rdf:about="https://ega.industry.com/ontologies/core/process/stepSkimming_12">
        <rdf:type rdf:resource="https://ega.industry.com/ontologies/core/process/NormalStep"/>
        <rdf:type rdf:resource="https://ega.industry.com/ontologies/core/process/Step"/>
        <process:hasCondition rdf:resource="https://ega.industry.com/ontologies/core/process/conditionSkimming_12"/>
        <process:hasPreviousStep rdf:resource="https://ega.industry.com/ontologies/core/process/stepPreheating_12"/>
        <process:hasStepType rdf:resource="https://ega.industry.com/ontologies/core/process/Operator"/>
        <process:isStepOf rdf:resource="https://ega.industry.com/ontologies/core/process/subProcessPreparation_12"/>
        <process:useAsset rdf:resource="https://ega.industry.com/ontologies/core/asset/tank_12"/>
        <process:hasEndTimestamp rdf:datatype="http://www.w3.org/2001/XMLSchema#dateTime">2025-06-03T09:59:08.322482</process:hasEndTimestamp>
        <process:hasStartTimestamp rdf:datatype="http://www.w3.org/2001/XMLSchema#dateTime">2025-06-03T09:59:08.322482</process:hasStartTimestamp>
        <process:hasStepId rdf:datatype="http://www.w3.org/2001/XMLSchema#integer">2</process:hasStepId>
        <process:isCurrentStep rdf:datatype="http://www.w3.org/2001/XMLSchema#boolean">false</process:isCurrentStep>
        <rdfs:comment xml:lang="en">Removal of oxidized material (dross) from surface</rdfs:comment>
    </owl:NamedIndividual>
    


    <!-- https://ega.industry.com/ontologies/core/process/stepStirring_10 -->

    <owl:NamedIndividual rdf:about="https://ega.industry.com/ontologies/core/process/stepStirring_10">
        <rdf:type rdf:resource="https://ega.industry.com/ontologies/core/process/NormalStep"/>
        <rdf:type rdf:resource="https://ega.industry.com/ontologies/core/process/Step"/>
        <process:hasCondition rdf:resource="https://ega.industry.com/ontologies/core/process/conditionStirring_10"/>
        <process:hasNextStep rdf:resource="https://ega.industry.com/ontologies/core/process/stepHolding_10"/>
        <process:hasStepType rdf:resource="https://ega.industry.com/ontologies/core/process/Operator"/>
        <process:isStepOf rdf:resource="https://ega.industry.com/ontologies/core/process/subProcessMelting_10"/>
        <process:useAsset rdf:resource="https://ega.industry.com/ontologies/core/asset/tank_10"/>
        <process:hasEndTimestamp rdf:datatype="http://www.w3.org/2001/XMLSchema#dateTime">2025-06-03T09:59:07.456561</process:hasEndTimestamp>
        <process:hasStartTimestamp rdf:datatype="http://www.w3.org/2001/XMLSchema#dateTime">2025-06-03T09:59:07.456561</process:hasStartTimestamp>
        <process:hasStepId rdf:datatype="http://www.w3.org/2001/XMLSchema#integer">6</process:hasStepId>
        <process:isCurrentStep rdf:datatype="http://www.w3.org/2001/XMLSchema#boolean">false</process:isCurrentStep>
        <rdfs:comment xml:lang="en">Mechanical mixing to ensure uniform composition</rdfs:comment>
    </owl:NamedIndividual>
    


    <!-- https://ega.industry.com/ontologies/core/process/stepStirring_12 -->

    <owl:NamedIndividual rdf:about="https://ega.industry.com/ontologies/core/process/stepStirring_12">
        <rdf:type rdf:resource="https://ega.industry.com/ontologies/core/process/NormalStep"/>
        <rdf:type rdf:resource="https://ega.industry.com/ontologies/core/process/Step"/>
        <process:hasCondition rdf:resource="https://ega.industry.com/ontologies/core/process/conditionStirring_12"/>
        <process:hasNextStep rdf:resource="https://ega.industry.com/ontologies/core/process/stepHolding_12"/>
        <process:hasStepType rdf:resource="https://ega.industry.com/ontologies/core/process/Operator"/>
        <process:isStepOf rdf:resource="https://ega.industry.com/ontologies/core/process/subProcessMelting_12"/>
        <process:useAsset rdf:resource="https://ega.industry.com/ontologies/core/asset/tank_12"/>
        <process:hasEndTimestamp rdf:datatype="http://www.w3.org/2001/XMLSchema#dateTime">2025-06-03T09:59:08.322482</process:hasEndTimestamp>
        <process:hasStartTimestamp rdf:datatype="http://www.w3.org/2001/XMLSchema#dateTime">2025-06-03T09:59:08.322482</process:hasStartTimestamp>
        <process:hasStepId rdf:datatype="http://www.w3.org/2001/XMLSchema#integer">6</process:hasStepId>
        <process:isCurrentStep rdf:datatype="http://www.w3.org/2001/XMLSchema#boolean">false</process:isCurrentStep>
        <rdfs:comment xml:lang="en">Mechanical mixing to ensure uniform composition</rdfs:comment>
    </owl:NamedIndividual>
    


    <!-- https://ega.industry.com/ontologies/core/process/subProcessAdjustment_10 -->

    <owl:NamedIndividual rdf:about="https://ega.industry.com/ontologies/core/process/subProcessAdjustment_10">
        <rdf:type rdf:resource="https://ega.industry.com/ontologies/core/process/SequentialSubProcess"/>
        <rdf:type rdf:resource="https://ega.industry.com/ontologies/core/process/SubProcess"/>
        <process:hasEndStep rdf:resource="https://ega.industry.com/ontologies/core/process/stepPouringMetalsAdjustment_10"/>
        <process:hasNextSubProcess rdf:resource="https://ega.industry.com/ontologies/core/process/subProcessSampleCheck_10"/>
        <process:hasPreviousSubProcess rdf:resource="https://ega.industry.com/ontologies/core/process/subProcessSampleCheck_10"/>
        <process:hasStartStep rdf:resource="https://ega.industry.com/ontologies/core/process/stepLoadingScrapAdjustment_10"/>
        <process:hasStep rdf:resource="https://ega.industry.com/ontologies/core/process/stepLoadingScrapAdjustment_10"/>
        <process:hasStep rdf:resource="https://ega.industry.com/ontologies/core/process/stepPouringAluminiumAdjustment_10"/>
        <process:hasStep rdf:resource="https://ega.industry.com/ontologies/core/process/stepPouringMetalsAdjustment_10"/>
        <process:hasEndTimestamp rdf:datatype="http://www.w3.org/2001/XMLSchema#dateTime">2025-06-03T09:59:07.456561</process:hasEndTimestamp>
        <process:hasStartTimestamp rdf:datatype="http://www.w3.org/2001/XMLSchema#dateTime">2025-06-03T09:59:07.456561</process:hasStartTimestamp>
        <process:hasSubProcessId rdf:datatype="http://www.w3.org/2001/XMLSchema#integer">5</process:hasSubProcessId>
        <process:isCurrentSubProcess rdf:datatype="http://www.w3.org/2001/XMLSchema#boolean">false</process:isCurrentSubProcess>
        <rdfs:comment xml:lang="en">Correction of alloy composition based on test results</rdfs:comment>
    </owl:NamedIndividual>
    


    <!-- https://ega.industry.com/ontologies/core/process/subProcessAdjustment_12 -->

    <owl:NamedIndividual rdf:about="https://ega.industry.com/ontologies/core/process/subProcessAdjustment_12">
        <rdf:type rdf:resource="https://ega.industry.com/ontologies/core/process/SequentialSubProcess"/>
        <rdf:type rdf:resource="https://ega.industry.com/ontologies/core/process/SubProcess"/>
        <process:hasEndStep rdf:resource="https://ega.industry.com/ontologies/core/process/stepPouringMetalsAdjustment_12"/>
        <process:hasNextSubProcess rdf:resource="https://ega.industry.com/ontologies/core/process/subProcessSampleCheck_12"/>
        <process:hasPreviousSubProcess rdf:resource="https://ega.industry.com/ontologies/core/process/subProcessSampleCheck_12"/>
        <process:hasStartStep rdf:resource="https://ega.industry.com/ontologies/core/process/stepLoadingScrapAdjustment_12"/>
        <process:hasStep rdf:resource="https://ega.industry.com/ontologies/core/process/stepLoadingScrapAdjustment_12"/>
        <process:hasStep rdf:resource="https://ega.industry.com/ontologies/core/process/stepPouringAluminiumAdjustment_12"/>
        <process:hasStep rdf:resource="https://ega.industry.com/ontologies/core/process/stepPouringMetalsAdjustment_12"/>
        <process:hasEndTimestamp rdf:datatype="http://www.w3.org/2001/XMLSchema#dateTime">2025-06-03T09:59:08.322482</process:hasEndTimestamp>
        <process:hasStartTimestamp rdf:datatype="http://www.w3.org/2001/XMLSchema#dateTime">2025-06-03T09:59:08.322482</process:hasStartTimestamp>
        <process:hasSubProcessId rdf:datatype="http://www.w3.org/2001/XMLSchema#integer">5</process:hasSubProcessId>
        <process:isCurrentSubProcess rdf:datatype="http://www.w3.org/2001/XMLSchema#boolean">false</process:isCurrentSubProcess>
        <rdfs:comment xml:lang="en">Correction of alloy composition based on test results</rdfs:comment>
    </owl:NamedIndividual>
    


    <!-- https://ega.industry.com/ontologies/core/process/subProcessMaterialLoading_10 -->

    <owl:NamedIndividual rdf:about="https://ega.industry.com/ontologies/core/process/subProcessMaterialLoading_10">
        <rdf:type rdf:resource="https://ega.industry.com/ontologies/core/process/SequentialSubProcess"/>
        <rdf:type rdf:resource="https://ega.industry.com/ontologies/core/process/SubProcess"/>
        <process:hasEndStep rdf:resource="https://ega.industry.com/ontologies/core/process/stepPouringMetals_10"/>
        <process:hasNextSubProcess rdf:resource="https://ega.industry.com/ontologies/core/process/subProcessMelting_10"/>
        <process:hasPreviousSubProcess rdf:resource="https://ega.industry.com/ontologies/core/process/subProcessPreparation_10"/>
        <process:hasStartStep rdf:resource="https://ega.industry.com/ontologies/core/process/stepLoadingScrap_10"/>
        <process:hasStep rdf:resource="https://ega.industry.com/ontologies/core/process/stepLoadingScrap_10"/>
        <process:hasStep rdf:resource="https://ega.industry.com/ontologies/core/process/stepPouringAluminium_10"/>
        <process:hasStep rdf:resource="https://ega.industry.com/ontologies/core/process/stepPouringMetals_10"/>
        <process:hasEndTimestamp rdf:datatype="http://www.w3.org/2001/XMLSchema#dateTime">2025-06-03T09:59:07.456561</process:hasEndTimestamp>
        <process:hasStartTimestamp rdf:datatype="http://www.w3.org/2001/XMLSchema#dateTime">2025-06-03T09:59:07.456561</process:hasStartTimestamp>
        <process:hasSubProcessId rdf:datatype="http://www.w3.org/2001/XMLSchema#integer">2</process:hasSubProcessId>
        <process:isCurrentSubProcess rdf:datatype="http://www.w3.org/2001/XMLSchema#boolean">false</process:isCurrentSubProcess>
        <rdfs:comment xml:lang="en">Process of loading various materials into the furnace</rdfs:comment>
    </owl:NamedIndividual>
    


    <!-- https://ega.industry.com/ontologies/core/process/subProcessMaterialLoading_12 -->

    <owl:NamedIndividual rdf:about="https://ega.industry.com/ontologies/core/process/subProcessMaterialLoading_12">
        <rdf:type rdf:resource="https://ega.industry.com/ontologies/core/process/SequentialSubProcess"/>
        <rdf:type rdf:resource="https://ega.industry.com/ontologies/core/process/SubProcess"/>
        <process:hasEndStep rdf:resource="https://ega.industry.com/ontologies/core/process/stepPouringMetals_12"/>
        <process:hasNextSubProcess rdf:resource="https://ega.industry.com/ontologies/core/process/subProcessMelting_12"/>
        <process:hasPreviousSubProcess rdf:resource="https://ega.industry.com/ontologies/core/process/subProcessPreparation_12"/>
        <process:hasStartStep rdf:resource="https://ega.industry.com/ontologies/core/process/stepLoadingScrap_12"/>
        <process:hasStep rdf:resource="https://ega.industry.com/ontologies/core/process/stepLoadingScrap_12"/>
        <process:hasStep rdf:resource="https://ega.industry.com/ontologies/core/process/stepPouringAluminium_12"/>
        <process:hasStep rdf:resource="https://ega.industry.com/ontologies/core/process/stepPouringMetals_12"/>
        <process:hasEndTimestamp rdf:datatype="http://www.w3.org/2001/XMLSchema#dateTime">2025-06-03T09:59:08.322482</process:hasEndTimestamp>
        <process:hasStartTimestamp rdf:datatype="http://www.w3.org/2001/XMLSchema#dateTime">2025-06-03T09:59:08.322482</process:hasStartTimestamp>
        <process:hasSubProcessId rdf:datatype="http://www.w3.org/2001/XMLSchema#integer">2</process:hasSubProcessId>
        <process:isCurrentSubProcess rdf:datatype="http://www.w3.org/2001/XMLSchema#boolean">false</process:isCurrentSubProcess>
        <rdfs:comment xml:lang="en">Process of loading various materials into the furnace</rdfs:comment>
    </owl:NamedIndividual>
    


    <!-- https://ega.industry.com/ontologies/core/process/subProcessMelting_10 -->

    <owl:NamedIndividual rdf:about="https://ega.industry.com/ontologies/core/process/subProcessMelting_10">
        <rdf:type rdf:resource="https://ega.industry.com/ontologies/core/process/SequentialSubProcess"/>
        <rdf:type rdf:resource="https://ega.industry.com/ontologies/core/process/SubProcess"/>
        <process:hasEndStep rdf:resource="https://ega.industry.com/ontologies/core/process/stepHolding_10"/>
        <process:hasNextSubProcess rdf:resource="https://ega.industry.com/ontologies/core/process/subProcessSampleCheck_10"/>
        <process:hasPreviousSubProcess rdf:resource="https://ega.industry.com/ontologies/core/process/subProcessMaterialLoading_10"/>
        <process:hasStartStep rdf:resource="https://ega.industry.com/ontologies/core/process/stepStirring_10"/>
        <process:hasStep rdf:resource="https://ega.industry.com/ontologies/core/process/stepHolding_10"/>
        <process:hasStep rdf:resource="https://ega.industry.com/ontologies/core/process/stepStirring_10"/>
        <process:hasEndTimestamp rdf:datatype="http://www.w3.org/2001/XMLSchema#dateTime">2025-06-03T09:59:07.456561</process:hasEndTimestamp>
        <process:hasStartTimestamp rdf:datatype="http://www.w3.org/2001/XMLSchema#dateTime">2025-06-03T09:59:07.456561</process:hasStartTimestamp>
        <process:hasSubProcessId rdf:datatype="http://www.w3.org/2001/XMLSchema#integer">3</process:hasSubProcessId>
        <process:isCurrentSubProcess rdf:datatype="http://www.w3.org/2001/XMLSchema#boolean">false</process:isCurrentSubProcess>
        <rdfs:comment xml:lang="en">Process of transforming solid materials to liquid</rdfs:comment>
    </owl:NamedIndividual>
    


    <!-- https://ega.industry.com/ontologies/core/process/subProcessMelting_12 -->

    <owl:NamedIndividual rdf:about="https://ega.industry.com/ontologies/core/process/subProcessMelting_12">
        <rdf:type rdf:resource="https://ega.industry.com/ontologies/core/process/SequentialSubProcess"/>
        <rdf:type rdf:resource="https://ega.industry.com/ontologies/core/process/SubProcess"/>
        <process:hasEndStep rdf:resource="https://ega.industry.com/ontologies/core/process/stepHolding_12"/>
        <process:hasNextSubProcess rdf:resource="https://ega.industry.com/ontologies/core/process/subProcessSampleCheck_12"/>
        <process:hasPreviousSubProcess rdf:resource="https://ega.industry.com/ontologies/core/process/subProcessMaterialLoading_12"/>
        <process:hasStartStep rdf:resource="https://ega.industry.com/ontologies/core/process/stepStirring_12"/>
        <process:hasStep rdf:resource="https://ega.industry.com/ontologies/core/process/stepHolding_12"/>
        <process:hasStep rdf:resource="https://ega.industry.com/ontologies/core/process/stepStirring_12"/>
        <process:hasEndTimestamp rdf:datatype="http://www.w3.org/2001/XMLSchema#dateTime">2025-06-03T09:59:08.322482</process:hasEndTimestamp>
        <process:hasStartTimestamp rdf:datatype="http://www.w3.org/2001/XMLSchema#dateTime">2025-06-03T09:59:08.322482</process:hasStartTimestamp>
        <process:hasSubProcessId rdf:datatype="http://www.w3.org/2001/XMLSchema#integer">3</process:hasSubProcessId>
        <process:isCurrentSubProcess rdf:datatype="http://www.w3.org/2001/XMLSchema#boolean">false</process:isCurrentSubProcess>
        <rdfs:comment xml:lang="en">Process of transforming solid materials to liquid</rdfs:comment>
    </owl:NamedIndividual>
    


    <!-- https://ega.industry.com/ontologies/core/process/subProcessPreparation_10 -->

    <owl:NamedIndividual rdf:about="https://ega.industry.com/ontologies/core/process/subProcessPreparation_10">
        <rdf:type rdf:resource="https://ega.industry.com/ontologies/core/process/SequentialSubProcess"/>
        <rdf:type rdf:resource="https://ega.industry.com/ontologies/core/process/SubProcess"/>
        <process:hasEndStep rdf:resource="https://ega.industry.com/ontologies/core/process/stepSkimming_10"/>
        <process:hasNextSubProcess rdf:resource="https://ega.industry.com/ontologies/core/process/subProcessMaterialLoading_10"/>
        <process:hasStartStep rdf:resource="https://ega.industry.com/ontologies/core/process/stepPreheating_10"/>
        <process:hasStep rdf:resource="https://ega.industry.com/ontologies/core/process/stepPreheating_10"/>
        <process:hasStep rdf:resource="https://ega.industry.com/ontologies/core/process/stepSkimming_10"/>
        <process:hasEndTimestamp rdf:datatype="http://www.w3.org/2001/XMLSchema#dateTime">2025-06-03T09:59:07.456561</process:hasEndTimestamp>
        <process:hasStartTimestamp rdf:datatype="http://www.w3.org/2001/XMLSchema#dateTime">2025-06-03T09:59:07.456561</process:hasStartTimestamp>
        <process:hasSubProcessId rdf:datatype="http://www.w3.org/2001/XMLSchema#integer">1</process:hasSubProcessId>
        <process:isCurrentSubProcess rdf:datatype="http://www.w3.org/2001/XMLSchema#boolean">false</process:isCurrentSubProcess>
        <rdfs:comment xml:lang="en">Initial setup of furnace for a new batch</rdfs:comment>
    </owl:NamedIndividual>
    


    <!-- https://ega.industry.com/ontologies/core/process/subProcessPreparation_12 -->

    <owl:NamedIndividual rdf:about="https://ega.industry.com/ontologies/core/process/subProcessPreparation_12">
        <rdf:type rdf:resource="https://ega.industry.com/ontologies/core/process/SequentialSubProcess"/>
        <rdf:type rdf:resource="https://ega.industry.com/ontologies/core/process/SubProcess"/>
        <process:hasEndStep rdf:resource="https://ega.industry.com/ontologies/core/process/stepSkimming_12"/>
        <process:hasNextSubProcess rdf:resource="https://ega.industry.com/ontologies/core/process/subProcessMaterialLoading_12"/>
        <process:hasStartStep rdf:resource="https://ega.industry.com/ontologies/core/process/stepPreheating_12"/>
        <process:hasStep rdf:resource="https://ega.industry.com/ontologies/core/process/stepPreheating_12"/>
        <process:hasStep rdf:resource="https://ega.industry.com/ontologies/core/process/stepSkimming_12"/>
        <process:hasEndTimestamp rdf:datatype="http://www.w3.org/2001/XMLSchema#dateTime">2025-06-03T09:59:08.322482</process:hasEndTimestamp>
        <process:hasStartTimestamp rdf:datatype="http://www.w3.org/2001/XMLSchema#dateTime">2025-06-03T09:59:08.322482</process:hasStartTimestamp>
        <process:hasSubProcessId rdf:datatype="http://www.w3.org/2001/XMLSchema#integer">1</process:hasSubProcessId>
        <process:isCurrentSubProcess rdf:datatype="http://www.w3.org/2001/XMLSchema#boolean">false</process:isCurrentSubProcess>
        <rdfs:comment xml:lang="en">Initial setup of furnace for a new batch</rdfs:comment>
    </owl:NamedIndividual>
    


    <!-- https://ega.industry.com/ontologies/core/process/subProcessSampleCheck_10 -->

    <owl:NamedIndividual rdf:about="https://ega.industry.com/ontologies/core/process/subProcessSampleCheck_10">
        <rdf:type rdf:resource="https://ega.industry.com/ontologies/core/process/ConditionalSubProcess"/>
        <rdf:type rdf:resource="https://ega.industry.com/ontologies/core/process/SubProcess"/>
        <process:hasEndStep rdf:resource="https://ega.industry.com/ontologies/core/process/stepLaboratoryAnalysis_10"/>
        <process:hasNextSubProcess rdf:resource="https://ega.industry.com/ontologies/core/process/subProcessAdjustment_10"/>
        <process:hasNextSubProcessOnFailure rdf:resource="https://ega.industry.com/ontologies/core/process/subProcessAdjustment_10"/>
        <process:hasNextSubProcessOnSuccess rdf:resource="https://ega.industry.com/ontologies/core/process/SubProcessCasting_10"/>
        <process:hasPreviousSubProcess rdf:resource="https://ega.industry.com/ontologies/core/process/subProcessAdjustment_10"/>
        <process:hasPreviousSubProcess rdf:resource="https://ega.industry.com/ontologies/core/process/subProcessMelting_10"/>
        <process:hasStartStep rdf:resource="https://ega.industry.com/ontologies/core/process/stepSampling_10"/>
        <process:hasStep rdf:resource="https://ega.industry.com/ontologies/core/process/stepLaboratoryAnalysis_10"/>
        <process:hasStep rdf:resource="https://ega.industry.com/ontologies/core/process/stepSampling_10"/>
        <process:pathDependsOnStep rdf:resource="https://ega.industry.com/ontologies/core/process/stepLaboratoryAnalysis_10"/>
        <process:hasEndTimestamp rdf:datatype="http://www.w3.org/2001/XMLSchema#dateTime">2025-06-03T09:59:07.456561</process:hasEndTimestamp>
        <process:hasStartTimestamp rdf:datatype="http://www.w3.org/2001/XMLSchema#dateTime">2025-06-03T09:59:07.456561</process:hasStartTimestamp>
        <process:hasSubProcessId rdf:datatype="http://www.w3.org/2001/XMLSchema#integer">4</process:hasSubProcessId>
        <process:isCurrentSubProcess rdf:datatype="http://www.w3.org/2001/XMLSchema#boolean">false</process:isCurrentSubProcess>
        <rdfs:comment xml:lang="en">Process of sample collection and testing</rdfs:comment>
    </owl:NamedIndividual>
    


    <!-- https://ega.industry.com/ontologies/core/process/subProcessSampleCheck_12 -->

    <owl:NamedIndividual rdf:about="https://ega.industry.com/ontologies/core/process/subProcessSampleCheck_12">
        <rdf:type rdf:resource="https://ega.industry.com/ontologies/core/process/ConditionalSubProcess"/>
        <rdf:type rdf:resource="https://ega.industry.com/ontologies/core/process/SubProcess"/>
        <process:hasEndStep rdf:resource="https://ega.industry.com/ontologies/core/process/stepLaboratoryAnalysis_12"/>
        <process:hasNextSubProcess rdf:resource="https://ega.industry.com/ontologies/core/process/subProcessAdjustment_12"/>
        <process:hasNextSubProcessOnFailure rdf:resource="https://ega.industry.com/ontologies/core/process/subProcessAdjustment_12"/>
        <process:hasNextSubProcessOnSuccess rdf:resource="https://ega.industry.com/ontologies/core/process/SubProcessCasting_12"/>
        <process:hasPreviousSubProcess rdf:resource="https://ega.industry.com/ontologies/core/process/subProcessAdjustment_12"/>
        <process:hasPreviousSubProcess rdf:resource="https://ega.industry.com/ontologies/core/process/subProcessMelting_12"/>
        <process:hasStartStep rdf:resource="https://ega.industry.com/ontologies/core/process/stepSampling_12"/>
        <process:hasStep rdf:resource="https://ega.industry.com/ontologies/core/process/stepLaboratoryAnalysis_12"/>
        <process:hasStep rdf:resource="https://ega.industry.com/ontologies/core/process/stepSampling_12"/>
        <process:pathDependsOnStep rdf:resource="https://ega.industry.com/ontologies/core/process/stepLaboratoryAnalysis_12"/>
        <process:hasEndTimestamp rdf:datatype="http://www.w3.org/2001/XMLSchema#dateTime">2025-06-03T09:59:08.322482</process:hasEndTimestamp>
        <process:hasStartTimestamp rdf:datatype="http://www.w3.org/2001/XMLSchema#dateTime">2025-06-03T09:59:08.322482</process:hasStartTimestamp>
        <process:hasSubProcessId rdf:datatype="http://www.w3.org/2001/XMLSchema#integer">4</process:hasSubProcessId>
        <process:isCurrentSubProcess rdf:datatype="http://www.w3.org/2001/XMLSchema#boolean">false</process:isCurrentSubProcess>
        <rdfs:comment xml:lang="en">Process of sample collection and testing</rdfs:comment>
    </owl:NamedIndividual>
    


    <!-- https://saref.etsi.org/core/propertyOfInterestCastingStatusFurnace_10 -->

    <owl:NamedIndividual rdf:about="https://saref.etsi.org/core/propertyOfInterestCastingStatusFurnace_10">
        <rdf:type rdf:resource="https://saref.etsi.org/core/PropertyOfInterest"/>
        <core:hasPropertyKind rdf:resource="http://qudt.org/vocab/quantitykind/Dimensionless"/>
        <core:isPropertyOfInterestOf rdf:resource="https://ega.industry.com/ontologies/core/asset/furnace_10"/>
        <rdfs:comment xml:lang="en">Furnace Casting  Property of Interset</rdfs:comment>
    </owl:NamedIndividual>
    


    <!-- https://saref.etsi.org/core/propertyOfInterestCastingStatusFurnace_12 -->

    <owl:NamedIndividual rdf:about="https://saref.etsi.org/core/propertyOfInterestCastingStatusFurnace_12">
        <rdf:type rdf:resource="https://saref.etsi.org/core/PropertyOfInterest"/>
        <core:hasPropertyKind rdf:resource="http://qudt.org/vocab/quantitykind/Dimensionless"/>
        <core:isPropertyOfInterestOf rdf:resource="https://ega.industry.com/ontologies/core/asset/furnace_12"/>
        <rdfs:comment xml:lang="en">Furnace Casting  Property of Interset</rdfs:comment>
    </owl:NamedIndividual>
    


    <!-- https://saref.etsi.org/core/propertyOfInterestConcentrationAirBurner_10 -->

    <owl:NamedIndividual rdf:about="https://saref.etsi.org/core/propertyOfInterestConcentrationAirBurner_10">
        <rdf:type rdf:resource="https://saref.etsi.org/core/PropertyOfInterest"/>
        <core:hasPropertyKind rdf:resource="http://qudt.org/vocab/quantitykind/DimensionlessRatio"/>
        <core:isPropertyOfInterestOf rdf:resource="https://ega.industry.com/ontologies/core/asset/airSupply_10"/>
        <rdfs:comment xml:lang="en">Oxygen content in air mixture</rdfs:comment>
    </owl:NamedIndividual>
    


    <!-- https://saref.etsi.org/core/propertyOfInterestConcentrationAirBurner_12 -->

    <owl:NamedIndividual rdf:about="https://saref.etsi.org/core/propertyOfInterestConcentrationAirBurner_12">
        <rdf:type rdf:resource="https://saref.etsi.org/core/PropertyOfInterest"/>
        <core:hasPropertyKind rdf:resource="http://qudt.org/vocab/quantitykind/DimensionlessRatio"/>
        <core:isPropertyOfInterestOf rdf:resource="https://ega.industry.com/ontologies/core/asset/airSupply_12"/>
        <rdfs:comment xml:lang="en">Oxygen content in air mixture</rdfs:comment>
    </owl:NamedIndividual>
    


    <!-- https://saref.etsi.org/core/propertyOfInterestFlowRateGasBurner_10 -->

    <owl:NamedIndividual rdf:about="https://saref.etsi.org/core/propertyOfInterestFlowRateGasBurner_10">
        <rdf:type rdf:resource="https://saref.etsi.org/core/PropertyOfInterest"/>
        <core:hasPropertyKind rdf:resource="http://qudt.org/vocab/quantitykind/VolumeFlowRate"/>
        <core:isPropertyOfInterestOf rdf:resource="https://ega.industry.com/ontologies/core/asset/gasSupply_10"/>
        <rdfs:comment xml:lang="en">Gas volume delivery rate through burner</rdfs:comment>
    </owl:NamedIndividual>
    


    <!-- https://saref.etsi.org/core/propertyOfInterestFlowRateGasBurner_12 -->

    <owl:NamedIndividual rdf:about="https://saref.etsi.org/core/propertyOfInterestFlowRateGasBurner_12">
        <rdf:type rdf:resource="https://saref.etsi.org/core/PropertyOfInterest"/>
        <core:hasPropertyKind rdf:resource="http://qudt.org/vocab/quantitykind/VolumeFlowRate"/>
        <core:isPropertyOfInterestOf rdf:resource="https://ega.industry.com/ontologies/core/asset/gasSupply_12"/>
        <rdfs:comment xml:lang="en">Gas volume delivery rate through burner</rdfs:comment>
    </owl:NamedIndividual>
    


    <!-- https://saref.etsi.org/core/propertyOfInterestHeatingPowerPercentBathTank_10 -->

    <owl:NamedIndividual rdf:about="https://saref.etsi.org/core/propertyOfInterestHeatingPowerPercentBathTank_10">
        <rdf:type rdf:resource="https://saref.etsi.org/core/PropertyOfInterest"/>
        <core:hasPropertyKind rdf:resource="http://qudt.org/vocab/quantitykind/DimensionlessRatio"/>
        <core:isPropertyOfInterestOf rdf:resource="https://ega.industry.com/ontologies/core/asset/tank_10"/>
        <rdfs:comment xml:lang="en">Thermal energy input for bath</rdfs:comment>
    </owl:NamedIndividual>
    


    <!-- https://saref.etsi.org/core/propertyOfInterestHeatingPowerPercentBathTank_12 -->

    <owl:NamedIndividual rdf:about="https://saref.etsi.org/core/propertyOfInterestHeatingPowerPercentBathTank_12">
        <rdf:type rdf:resource="https://saref.etsi.org/core/PropertyOfInterest"/>
        <core:hasPropertyKind rdf:resource="http://qudt.org/vocab/quantitykind/DimensionlessRatio"/>
        <core:isPropertyOfInterestOf rdf:resource="https://ega.industry.com/ontologies/core/asset/tank_12"/>
        <rdfs:comment xml:lang="en">Thermal energy input for bath</rdfs:comment>
    </owl:NamedIndividual>
    


    <!-- https://saref.etsi.org/core/propertyOfInterestHeatingPowerPercentRoofTank_10 -->

    <owl:NamedIndividual rdf:about="https://saref.etsi.org/core/propertyOfInterestHeatingPowerPercentRoofTank_10">
        <rdf:type rdf:resource="https://saref.etsi.org/core/PropertyOfInterest"/>
        <core:hasPropertyKind rdf:resource="http://qudt.org/vocab/quantitykind/DimensionlessRatio"/>
        <core:isPropertyOfInterestOf rdf:resource="https://ega.industry.com/ontologies/core/asset/tank_10"/>
        <rdfs:comment xml:lang="en">Thermal energy input for roof</rdfs:comment>
    </owl:NamedIndividual>
    


    <!-- https://saref.etsi.org/core/propertyOfInterestHeatingPowerPercentRoofTank_12 -->

    <owl:NamedIndividual rdf:about="https://saref.etsi.org/core/propertyOfInterestHeatingPowerPercentRoofTank_12">
        <rdf:type rdf:resource="https://saref.etsi.org/core/PropertyOfInterest"/>
        <core:hasPropertyKind rdf:resource="http://qudt.org/vocab/quantitykind/DimensionlessRatio"/>
        <core:isPropertyOfInterestOf rdf:resource="https://ega.industry.com/ontologies/core/asset/tank_12"/>
        <rdfs:comment xml:lang="en">Thermal energy input for roof</rdfs:comment>
    </owl:NamedIndividual>
    


    <!-- https://saref.etsi.org/core/propertyOfInterestPressureFurnace_10 -->

    <owl:NamedIndividual rdf:about="https://saref.etsi.org/core/propertyOfInterestPressureFurnace_10">
        <rdf:type rdf:resource="https://saref.etsi.org/core/PropertyOfInterest"/>
        <core:hasPropertyKind rdf:resource="http://qudt.org/vocab/quantitykind/Pressure"/>
        <core:isPropertyOfInterestOf rdf:resource="https://ega.industry.com/ontologies/core/asset/furnace_10"/>
        <rdfs:comment xml:lang="en">Operating pressure at furnace combustion interface</rdfs:comment>
    </owl:NamedIndividual>
    


    <!-- https://saref.etsi.org/core/propertyOfInterestPressureFurnace_12 -->

    <owl:NamedIndividual rdf:about="https://saref.etsi.org/core/propertyOfInterestPressureFurnace_12">
        <rdf:type rdf:resource="https://saref.etsi.org/core/PropertyOfInterest"/>
        <core:hasPropertyKind rdf:resource="http://qudt.org/vocab/quantitykind/Pressure"/>
        <core:isPropertyOfInterestOf rdf:resource="https://ega.industry.com/ontologies/core/asset/furnace_12"/>
        <rdfs:comment xml:lang="en">Operating pressure at furnace combustion interface</rdfs:comment>
    </owl:NamedIndividual>
    


    <!-- https://saref.etsi.org/core/propertyOfInterestTemperatureBatchTank_10 -->

    <owl:NamedIndividual rdf:about="https://saref.etsi.org/core/propertyOfInterestTemperatureBatchTank_10">
        <rdf:type rdf:resource="https://saref.etsi.org/core/PropertyOfInterest"/>
        <core:hasPropertyKind rdf:resource="http://qudt.org/vocab/quantitykind/Temperature"/>
        <core:isPropertyOfInterestOf rdf:resource="https://ega.industry.com/ontologies/core/asset/tank_10"/>
        <rdfs:comment xml:lang="en">Specific temperature mesurement at bath level</rdfs:comment>
    </owl:NamedIndividual>
    


    <!-- https://saref.etsi.org/core/propertyOfInterestTemperatureBatchTank_12 -->

    <owl:NamedIndividual rdf:about="https://saref.etsi.org/core/propertyOfInterestTemperatureBatchTank_12">
        <rdf:type rdf:resource="https://saref.etsi.org/core/PropertyOfInterest"/>
        <core:hasPropertyKind rdf:resource="http://qudt.org/vocab/quantitykind/Temperature"/>
        <core:isPropertyOfInterestOf rdf:resource="https://ega.industry.com/ontologies/core/asset/tank_12"/>
        <rdfs:comment xml:lang="en">Specific temperature mesurement at bath level</rdfs:comment>
    </owl:NamedIndividual>
    


    <!-- https://saref.etsi.org/core/propertyOfInterestTemperatureBathThresholdTank_10 -->

    <owl:NamedIndividual rdf:about="https://saref.etsi.org/core/propertyOfInterestTemperatureBathThresholdTank_10">
        <rdf:type rdf:resource="https://saref.etsi.org/core/PropertyOfInterest"/>
        <core:hasPropertyKind rdf:resource="http://qudt.org/vocab/quantitykind/Temperature"/>
        <core:isPropertyOfInterestOf rdf:resource="https://ega.industry.com/ontologies/core/asset/tank_10"/>
        <rdfs:comment xml:lang="en">Specific temperature Set Point at bath  level in Tank</rdfs:comment>
    </owl:NamedIndividual>
    


    <!-- https://saref.etsi.org/core/propertyOfInterestTemperatureBathThresholdTank_12 -->

    <owl:NamedIndividual rdf:about="https://saref.etsi.org/core/propertyOfInterestTemperatureBathThresholdTank_12">
        <rdf:type rdf:resource="https://saref.etsi.org/core/PropertyOfInterest"/>
        <core:hasPropertyKind rdf:resource="http://qudt.org/vocab/quantitykind/Temperature"/>
        <core:isPropertyOfInterestOf rdf:resource="https://ega.industry.com/ontologies/core/asset/tank_12"/>
        <rdfs:comment xml:lang="en">Specific temperature Set Point at bath  level in Tank</rdfs:comment>
    </owl:NamedIndividual>
    


    <!-- https://saref.etsi.org/core/propertyOfInterestTemperatureExhaustFurnace_10 -->

    <owl:NamedIndividual rdf:about="https://saref.etsi.org/core/propertyOfInterestTemperatureExhaustFurnace_10">
        <rdf:type rdf:resource="https://saref.etsi.org/core/PropertyOfInterest"/>
        <core:hasPropertyKind rdf:resource="http://qudt.org/vocab/quantitykind/Temperature"/>
        <core:isPropertyOfInterestOf rdf:resource="https://ega.industry.com/ontologies/core/asset/furnace_10"/>
        <rdfs:comment xml:lang="en">Exit temperature of combustion gases from furnace system</rdfs:comment>
    </owl:NamedIndividual>
    


    <!-- https://saref.etsi.org/core/propertyOfInterestTemperatureExhaustFurnace_12 -->

    <owl:NamedIndividual rdf:about="https://saref.etsi.org/core/propertyOfInterestTemperatureExhaustFurnace_12">
        <rdf:type rdf:resource="https://saref.etsi.org/core/PropertyOfInterest"/>
        <core:hasPropertyKind rdf:resource="http://qudt.org/vocab/quantitykind/Temperature"/>
        <core:isPropertyOfInterestOf rdf:resource="https://ega.industry.com/ontologies/core/asset/furnace_12"/>
        <rdfs:comment xml:lang="en">Exit temperature of combustion gases from furnace system</rdfs:comment>
    </owl:NamedIndividual>
    


    <!-- https://saref.etsi.org/core/propertyOfInterestTemperatureRoofTank_10 -->

    <owl:NamedIndividual rdf:about="https://saref.etsi.org/core/propertyOfInterestTemperatureRoofTank_10">
        <rdf:type rdf:resource="https://saref.etsi.org/core/PropertyOfInterest"/>
        <core:hasPropertyKind rdf:resource="http://qudt.org/vocab/quantitykind/Temperature"/>
        <core:isPropertyOfInterestOf rdf:resource="https://ega.industry.com/ontologies/core/asset/tank_10"/>
        <rdfs:comment xml:lang="en">Specific temperature mesurement at roof level</rdfs:comment>
    </owl:NamedIndividual>
    


    <!-- https://saref.etsi.org/core/propertyOfInterestTemperatureRoofTank_12 -->

    <owl:NamedIndividual rdf:about="https://saref.etsi.org/core/propertyOfInterestTemperatureRoofTank_12">
        <rdf:type rdf:resource="https://saref.etsi.org/core/PropertyOfInterest"/>
        <core:hasPropertyKind rdf:resource="http://qudt.org/vocab/quantitykind/Temperature"/>
        <core:isPropertyOfInterestOf rdf:resource="https://ega.industry.com/ontologies/core/asset/tank_12"/>
        <rdfs:comment xml:lang="en">Specific temperature mesurement at roof level</rdfs:comment>
    </owl:NamedIndividual>
    


    <!-- https://saref.etsi.org/core/propertyOfInterestTemperatureRoofThresholdTank_10 -->

    <owl:NamedIndividual rdf:about="https://saref.etsi.org/core/propertyOfInterestTemperatureRoofThresholdTank_10">
        <rdf:type rdf:resource="https://saref.etsi.org/core/PropertyOfInterest"/>
        <core:hasPropertyKind rdf:resource="http://qudt.org/vocab/quantitykind/Temperature"/>
        <core:isPropertyOfInterestOf rdf:resource="https://ega.industry.com/ontologies/core/asset/tank_10"/>
        <rdfs:comment xml:lang="en">Specific temperature Set Point at Roof  level in Tank</rdfs:comment>
    </owl:NamedIndividual>
    


    <!-- https://saref.etsi.org/core/propertyOfInterestTemperatureRoofThresholdTank_12 -->

    <owl:NamedIndividual rdf:about="https://saref.etsi.org/core/propertyOfInterestTemperatureRoofThresholdTank_12">
        <rdf:type rdf:resource="https://saref.etsi.org/core/PropertyOfInterest"/>
        <core:hasPropertyKind rdf:resource="http://qudt.org/vocab/quantitykind/Temperature"/>
        <core:isPropertyOfInterestOf rdf:resource="https://ega.industry.com/ontologies/core/asset/tank_12"/>
        <rdfs:comment xml:lang="en">Specific temperature Set Point at Roof  level in Tank</rdfs:comment>
    </owl:NamedIndividual>
    


    <!-- https://saref.etsi.org/core/propertyValueCastingStatusFurnace_10 -->

    <owl:NamedIndividual rdf:about="https://saref.etsi.org/core/propertyValueCastingStatusFurnace_10">
        <rdf:type rdf:resource="https://saref.etsi.org/core/PropertyValue"/>
        <core:isMeasuredIn rdf:resource="http://qudt.org/vocab/unit/NUM"/>
        <core:isObservedBy rdf:resource="https://ega.industry.com/ontologies/core/asset/sensorCastingStatusFurnace_10"/>
        <core:isTargetOf rdf:resource="https://ega.industry.com/ontologies/core/asset/sensorCastingStatusFurnace_10"/>
        <core:isValueOfProperty rdf:resource="http://qudt.org/vocab/quantitykind/Dimensionless"/>
        <core:isValueOfProperty rdf:resource="https://saref.etsi.org/core/propertyOfInterestCastingStatusFurnace_10"/>
        <data:hasTag>casting_status</data:hasTag>
        <core:hasTimestamp rdf:datatype="http://www.w3.org/2001/XMLSchema#dateTime">2025-06-03T09:59:07.352815</core:hasTimestamp>
        <core:hasValue rdf:datatype="http://www.w3.org/2001/XMLSchema#float">0.0</core:hasValue>
        <rdfs:comment xml:lang="en">Furnace Casting status value</rdfs:comment>
    </owl:NamedIndividual>
    


    <!-- https://saref.etsi.org/core/propertyValueCastingStatusFurnace_12 -->

    <owl:NamedIndividual rdf:about="https://saref.etsi.org/core/propertyValueCastingStatusFurnace_12">
        <rdf:type rdf:resource="https://saref.etsi.org/core/PropertyValue"/>
        <core:isMeasuredIn rdf:resource="http://qudt.org/vocab/unit/NUM"/>
        <core:isObservedBy rdf:resource="https://ega.industry.com/ontologies/core/asset/sensorCastingStatusFurnace_12"/>
        <core:isTargetOf rdf:resource="https://ega.industry.com/ontologies/core/asset/sensorCastingStatusFurnace_12"/>
        <core:isValueOfProperty rdf:resource="http://qudt.org/vocab/quantitykind/Dimensionless"/>
        <core:isValueOfProperty rdf:resource="https://saref.etsi.org/core/propertyOfInterestCastingStatusFurnace_12"/>
        <data:hasTag>casting_status</data:hasTag>
        <core:hasTimestamp rdf:datatype="http://www.w3.org/2001/XMLSchema#dateTime">2025-06-03T09:59:08.262183</core:hasTimestamp>
        <core:hasValue rdf:datatype="http://www.w3.org/2001/XMLSchema#float">0.0</core:hasValue>
        <rdfs:comment xml:lang="en">Furnace Casting status value</rdfs:comment>
    </owl:NamedIndividual>
    


    <!-- https://saref.etsi.org/core/propertyValueConcentrationAirBurner_10 -->

    <owl:NamedIndividual rdf:about="https://saref.etsi.org/core/propertyValueConcentrationAirBurner_10">
        <rdf:type rdf:resource="https://saref.etsi.org/core/PropertyValue"/>
        <core:isMeasuredIn rdf:resource="http://qudt.org/vocab/unit/PERCENT"/>
        <core:isObservedBy rdf:resource="https://ega.industry.com/ontologies/core/asset/sensorOxygen_10"/>
        <core:isTargetOf rdf:resource="https://ega.industry.com/ontologies/core/asset/sensorOxygen_10"/>
        <core:isValueOfProperty rdf:resource="http://qudt.org/vocab/quantitykind/DimensionlessRatio"/>
        <core:isValueOfProperty rdf:resource="https://saref.etsi.org/core/propertyOfInterestConcentrationAirBurner_10"/>
        <data:hasTag>fce_oxygen_pv</data:hasTag>
        <core:hasTimestamp rdf:datatype="http://www.w3.org/2001/XMLSchema#dateTime">2025-06-03T09:59:07.352815</core:hasTimestamp>
        <core:hasValue rdf:datatype="http://www.w3.org/2001/XMLSchema#float">0.0</core:hasValue>
        <rdfs:comment xml:lang="en">Numerical reading of oxygen concentration at burner</rdfs:comment>
    </owl:NamedIndividual>
    


    <!-- https://saref.etsi.org/core/propertyValueConcentrationAirBurner_12 -->

    <owl:NamedIndividual rdf:about="https://saref.etsi.org/core/propertyValueConcentrationAirBurner_12">
        <rdf:type rdf:resource="https://saref.etsi.org/core/PropertyValue"/>
        <core:isMeasuredIn rdf:resource="http://qudt.org/vocab/unit/PERCENT"/>
        <core:isObservedBy rdf:resource="https://ega.industry.com/ontologies/core/asset/sensorOxygen_12"/>
        <core:isTargetOf rdf:resource="https://ega.industry.com/ontologies/core/asset/sensorOxygen_12"/>
        <core:isValueOfProperty rdf:resource="http://qudt.org/vocab/quantitykind/DimensionlessRatio"/>
        <core:isValueOfProperty rdf:resource="https://saref.etsi.org/core/propertyOfInterestConcentrationAirBurner_12"/>
        <data:hasTag>fce_oxygen_pv</data:hasTag>
        <core:hasTimestamp rdf:datatype="http://www.w3.org/2001/XMLSchema#dateTime">2025-06-03T09:59:08.262183</core:hasTimestamp>
        <core:hasValue rdf:datatype="http://www.w3.org/2001/XMLSchema#float">0.0</core:hasValue>
        <rdfs:comment xml:lang="en">Numerical reading of oxygen concentration at burner</rdfs:comment>
    </owl:NamedIndividual>
    


    <!-- https://saref.etsi.org/core/propertyValueFlowRateGasBurner_10 -->

    <owl:NamedIndividual rdf:about="https://saref.etsi.org/core/propertyValueFlowRateGasBurner_10">
        <rdf:type rdf:resource="https://saref.etsi.org/core/PropertyValue"/>
        <core:isMeasuredIn rdf:resource="http://qudt.org/vocab/unit/CentiM3-PER-HR"/>
        <core:isObservedBy rdf:resource="https://ega.industry.com/ontologies/core/asset/sensorFlowGas_10"/>
        <core:isTargetOf rdf:resource="https://ega.industry.com/ontologies/core/asset/sensorFlowGas_10"/>
        <core:isValueOfProperty rdf:resource="http://qudt.org/vocab/quantitykind/VolumeFlowRate"/>
        <core:isValueOfProperty rdf:resource="https://saref.etsi.org/core/propertyOfInterestFlowRateGasBurner_10"/>
        <data:hasTag>fce_gas_flow_burner_pv</data:hasTag>
        <core:hasTimestamp rdf:datatype="http://www.w3.org/2001/XMLSchema#dateTime">2025-06-03T09:59:07.352815</core:hasTimestamp>
        <core:hasValue rdf:datatype="http://www.w3.org/2001/XMLSchema#float">0.0</core:hasValue>
        <rdfs:comment xml:lang="en">Numerical reading of gas flow through burner</rdfs:comment>
    </owl:NamedIndividual>
    


    <!-- https://saref.etsi.org/core/propertyValueFlowRateGasBurner_12 -->

    <owl:NamedIndividual rdf:about="https://saref.etsi.org/core/propertyValueFlowRateGasBurner_12">
        <rdf:type rdf:resource="https://saref.etsi.org/core/PropertyValue"/>
        <core:isMeasuredIn rdf:resource="http://qudt.org/vocab/unit/CentiM3-PER-HR"/>
        <core:isObservedBy rdf:resource="https://ega.industry.com/ontologies/core/asset/sensorFlowGas_12"/>
        <core:isTargetOf rdf:resource="https://ega.industry.com/ontologies/core/asset/sensorFlowGas_12"/>
        <core:isValueOfProperty rdf:resource="http://qudt.org/vocab/quantitykind/VolumeFlowRate"/>
        <core:isValueOfProperty rdf:resource="https://saref.etsi.org/core/propertyOfInterestFlowRateGasBurner_12"/>
        <data:hasTag>fce_gas_flow_burner_pv</data:hasTag>
        <core:hasTimestamp rdf:datatype="http://www.w3.org/2001/XMLSchema#dateTime">2025-06-03T09:59:08.262183</core:hasTimestamp>
        <core:hasValue rdf:datatype="http://www.w3.org/2001/XMLSchema#float">0.0</core:hasValue>
        <rdfs:comment xml:lang="en">Numerical reading of gas flow through burner</rdfs:comment>
    </owl:NamedIndividual>
    


    <!-- https://saref.etsi.org/core/propertyValueHeatingPowerPercentBathTank_10 -->

    <owl:NamedIndividual rdf:about="https://saref.etsi.org/core/propertyValueHeatingPowerPercentBathTank_10">
        <rdf:type rdf:resource="https://saref.etsi.org/core/PropertyValue"/>
        <core:isMeasuredIn rdf:resource="http://qudt.org/vocab/unit/PERCENT"/>
        <core:isObservedBy rdf:resource="https://ega.industry.com/ontologies/core/asset/sensorPowerPercentBathTank_10"/>
        <core:isTargetOf rdf:resource="https://ega.industry.com/ontologies/core/asset/sensorPowerPercentBathTank_10"/>
        <core:isValueOfProperty rdf:resource="http://qudt.org/vocab/quantitykind/DimensionlessRatio"/>
        <core:isValueOfProperty rdf:resource="https://saref.etsi.org/core/propertyOfInterestHeatingPowerPercentBathTank_10"/>
        <data:hasTag>fce_bath_temp_cv</data:hasTag>
        <core:hasTimestamp rdf:datatype="http://www.w3.org/2001/XMLSchema#dateTime">2025-06-03T09:59:07.352815</core:hasTimestamp>
        <core:hasValue rdf:datatype="http://www.w3.org/2001/XMLSchema#float">0.0</core:hasValue>
        <rdfs:comment xml:lang="en">Numerical reading of bath heating power</rdfs:comment>
    </owl:NamedIndividual>
    


    <!-- https://saref.etsi.org/core/propertyValueHeatingPowerPercentBathTank_12 -->

    <owl:NamedIndividual rdf:about="https://saref.etsi.org/core/propertyValueHeatingPowerPercentBathTank_12">
        <rdf:type rdf:resource="https://saref.etsi.org/core/PropertyValue"/>
        <core:isMeasuredIn rdf:resource="http://qudt.org/vocab/unit/PERCENT"/>
        <core:isObservedBy rdf:resource="https://ega.industry.com/ontologies/core/asset/sensorPowerPercentBathTank_12"/>
        <core:isTargetOf rdf:resource="https://ega.industry.com/ontologies/core/asset/sensorPowerPercentBathTank_12"/>
        <core:isValueOfProperty rdf:resource="http://qudt.org/vocab/quantitykind/DimensionlessRatio"/>
        <core:isValueOfProperty rdf:resource="https://saref.etsi.org/core/propertyOfInterestHeatingPowerPercentBathTank_12"/>
        <data:hasTag>fce_bath_temp_cv</data:hasTag>
        <core:hasTimestamp rdf:datatype="http://www.w3.org/2001/XMLSchema#dateTime">2025-06-03T09:59:08.262183</core:hasTimestamp>
        <core:hasValue rdf:datatype="http://www.w3.org/2001/XMLSchema#float">0.0</core:hasValue>
        <rdfs:comment xml:lang="en">Numerical reading of bath heating power</rdfs:comment>
    </owl:NamedIndividual>
    


    <!-- https://saref.etsi.org/core/propertyValueHeatingPowerPercentRoofTank_10 -->

    <owl:NamedIndividual rdf:about="https://saref.etsi.org/core/propertyValueHeatingPowerPercentRoofTank_10">
        <rdf:type rdf:resource="https://saref.etsi.org/core/PropertyValue"/>
        <core:isMeasuredIn rdf:resource="http://qudt.org/vocab/unit/PERCENT"/>
        <core:isObservedBy rdf:resource="https://ega.industry.com/ontologies/core/asset/sensorPowerPercentRoofTank_10"/>
        <core:isTargetOf rdf:resource="https://ega.industry.com/ontologies/core/asset/sensorPowerPercentRoofTank_10"/>
        <core:isValueOfProperty rdf:resource="http://qudt.org/vocab/quantitykind/DimensionlessRatio"/>
        <core:isValueOfProperty rdf:resource="https://saref.etsi.org/core/propertyOfInterestHeatingPowerPercentRoofTank_10"/>
        <data:hasTag>fce_roof_temp_cv</data:hasTag>
        <core:hasTimestamp rdf:datatype="http://www.w3.org/2001/XMLSchema#dateTime">2025-06-03T09:59:07.352815</core:hasTimestamp>
        <core:hasValue rdf:datatype="http://www.w3.org/2001/XMLSchema#float">0.0</core:hasValue>
        <rdfs:comment xml:lang="en">Numerical reading of roof heating power</rdfs:comment>
    </owl:NamedIndividual>
    


    <!-- https://saref.etsi.org/core/propertyValueHeatingPowerPercentRoofTank_12 -->

    <owl:NamedIndividual rdf:about="https://saref.etsi.org/core/propertyValueHeatingPowerPercentRoofTank_12">
        <rdf:type rdf:resource="https://saref.etsi.org/core/PropertyValue"/>
        <core:isMeasuredIn rdf:resource="http://qudt.org/vocab/unit/PERCENT"/>
        <core:isObservedBy rdf:resource="https://ega.industry.com/ontologies/core/asset/sensorPowerPercentRoofTank_12"/>
        <core:isTargetOf rdf:resource="https://ega.industry.com/ontologies/core/asset/sensorPowerPercentRoofTank_12"/>
        <core:isValueOfProperty rdf:resource="http://qudt.org/vocab/quantitykind/DimensionlessRatio"/>
        <core:isValueOfProperty rdf:resource="https://saref.etsi.org/core/propertyOfInterestHeatingPowerPercentRoofTank_12"/>
        <data:hasTag>fce_roof_temp_cv</data:hasTag>
        <core:hasTimestamp rdf:datatype="http://www.w3.org/2001/XMLSchema#dateTime">2025-06-03T09:59:08.262183</core:hasTimestamp>
        <core:hasValue rdf:datatype="http://www.w3.org/2001/XMLSchema#float">0.0</core:hasValue>
        <rdfs:comment xml:lang="en">Numerical reading of roof heating power</rdfs:comment>
    </owl:NamedIndividual>
    


    <!-- https://saref.etsi.org/core/propertyValuePressureFurnace_10 -->

    <owl:NamedIndividual rdf:about="https://saref.etsi.org/core/propertyValuePressureFurnace_10">
        <rdf:type rdf:resource="https://saref.etsi.org/core/PropertyValue"/>
        <core:isMeasuredIn rdf:resource="http://qudt.org/vocab/unit/MilliBAR"/>
        <core:isObservedBy rdf:resource="https://ega.industry.com/ontologies/core/asset/sensorPressureFurnace_10"/>
        <core:isTargetOf rdf:resource="https://ega.industry.com/ontologies/core/asset/sensorPressureFurnace_10"/>
        <core:isValueOfProperty rdf:resource="http://qudt.org/vocab/quantitykind/Pressure"/>
        <core:isValueOfProperty rdf:resource="https://saref.etsi.org/core/propertyOfInterestPressureFurnace_10"/>
        <data:hasTag>fce_pressure_pv</data:hasTag>
        <core:hasTimestamp rdf:datatype="http://www.w3.org/2001/XMLSchema#dateTime">2025-06-03T09:59:07.352815</core:hasTimestamp>
        <core:hasValue rdf:datatype="http://www.w3.org/2001/XMLSchema#float">0.0</core:hasValue>
        <rdfs:comment xml:lang="en">Numerical reading of furnace pressure</rdfs:comment>
    </owl:NamedIndividual>
    


    <!-- https://saref.etsi.org/core/propertyValuePressureFurnace_12 -->

    <owl:NamedIndividual rdf:about="https://saref.etsi.org/core/propertyValuePressureFurnace_12">
        <rdf:type rdf:resource="https://saref.etsi.org/core/PropertyValue"/>
        <core:isMeasuredIn rdf:resource="http://qudt.org/vocab/unit/MilliBAR"/>
        <core:isObservedBy rdf:resource="https://ega.industry.com/ontologies/core/asset/sensorPressureFurnace_12"/>
        <core:isTargetOf rdf:resource="https://ega.industry.com/ontologies/core/asset/sensorPressureFurnace_12"/>
        <core:isValueOfProperty rdf:resource="http://qudt.org/vocab/quantitykind/Pressure"/>
        <core:isValueOfProperty rdf:resource="https://saref.etsi.org/core/propertyOfInterestPressureFurnace_12"/>
        <data:hasTag>fce_pressure_pv</data:hasTag>
        <core:hasTimestamp rdf:datatype="http://www.w3.org/2001/XMLSchema#dateTime">2025-06-03T09:59:08.262183</core:hasTimestamp>
        <core:hasValue rdf:datatype="http://www.w3.org/2001/XMLSchema#float">0.0</core:hasValue>
        <rdfs:comment xml:lang="en">Numerical reading of furnace pressure</rdfs:comment>
    </owl:NamedIndividual>
    


    <!-- https://saref.etsi.org/core/propertyValueTemperatureBathTank_10 -->

    <owl:NamedIndividual rdf:about="https://saref.etsi.org/core/propertyValueTemperatureBathTank_10">
        <rdf:type rdf:resource="https://saref.etsi.org/core/PropertyValue"/>
        <core:isMeasuredIn rdf:resource="http://qudt.org/vocab/unit/DEG_C"/>
        <core:isObservedBy rdf:resource="https://ega.industry.com/ontologies/core/asset/sensorTemperatureBathTank_10"/>
        <core:isTargetOf rdf:resource="https://ega.industry.com/ontologies/core/asset/sensorTemperatureBathTank_10"/>
        <core:isValueOfProperty rdf:resource="http://qudt.org/vocab/quantitykind/Temperature"/>
        <core:isValueOfProperty rdf:resource="https://saref.etsi.org/core/propertyOfInterestTemperatureBatchTank_10"/>
        <data:hasTag>fce_bath_temp_pv</data:hasTag>
        <core:hasTimestamp rdf:datatype="http://www.w3.org/2001/XMLSchema#dateTime">2025-06-03T09:59:07.352815</core:hasTimestamp>
        <core:hasValue rdf:datatype="http://www.w3.org/2001/XMLSchema#float">0.0</core:hasValue>
        <rdfs:comment xml:lang="en">Numerical reading of bath temperature</rdfs:comment>
    </owl:NamedIndividual>
    


    <!-- https://saref.etsi.org/core/propertyValueTemperatureBathTank_12 -->

    <owl:NamedIndividual rdf:about="https://saref.etsi.org/core/propertyValueTemperatureBathTank_12">
        <rdf:type rdf:resource="https://saref.etsi.org/core/PropertyValue"/>
        <core:isMeasuredIn rdf:resource="http://qudt.org/vocab/unit/DEG_C"/>
        <core:isObservedBy rdf:resource="https://ega.industry.com/ontologies/core/asset/sensorTemperatureBathTank_12"/>
        <core:isTargetOf rdf:resource="https://ega.industry.com/ontologies/core/asset/sensorTemperatureBathTank_12"/>
        <core:isValueOfProperty rdf:resource="http://qudt.org/vocab/quantitykind/Temperature"/>
        <core:isValueOfProperty rdf:resource="https://saref.etsi.org/core/propertyOfInterestTemperatureBatchTank_12"/>
        <data:hasTag>fce_bath_temp_pv</data:hasTag>
        <core:hasTimestamp rdf:datatype="http://www.w3.org/2001/XMLSchema#dateTime">2025-06-03T09:59:08.262183</core:hasTimestamp>
        <core:hasValue rdf:datatype="http://www.w3.org/2001/XMLSchema#float">0.0</core:hasValue>
        <rdfs:comment xml:lang="en">Numerical reading of bath temperature</rdfs:comment>
    </owl:NamedIndividual>
    


    <!-- https://saref.etsi.org/core/propertyValueTemperatureBathThresholdTank_10 -->

    <owl:NamedIndividual rdf:about="https://saref.etsi.org/core/propertyValueTemperatureBathThresholdTank_10">
        <rdf:type rdf:resource="https://saref.etsi.org/core/PropertyValue"/>
        <core:isMeasuredIn rdf:resource="http://qudt.org/vocab/unit/DEG_C"/>
        <core:isValueOfProperty rdf:resource="http://qudt.org/vocab/quantitykind/Temperature"/>
        <core:isValueOfProperty rdf:resource="https://saref.etsi.org/core/propertyOfInterestTemperatureBathThresholdTank_10"/>
        <data:hasTag>fce_bath_temp_sp</data:hasTag>
        <core:hasTimestamp rdf:datatype="http://www.w3.org/2001/XMLSchema#dateTime">2025-06-03T09:59:07.352815</core:hasTimestamp>
        <core:hasValue rdf:datatype="http://www.w3.org/2001/XMLSchema#float">0.0</core:hasValue>
        <rdfs:comment xml:lang="en">Numerical reading of bath temperature Set Point</rdfs:comment>
    </owl:NamedIndividual>
    


    <!-- https://saref.etsi.org/core/propertyValueTemperatureBathThresholdTank_12 -->

    <owl:NamedIndividual rdf:about="https://saref.etsi.org/core/propertyValueTemperatureBathThresholdTank_12">
        <rdf:type rdf:resource="https://saref.etsi.org/core/PropertyValue"/>
        <core:isMeasuredIn rdf:resource="http://qudt.org/vocab/unit/DEG_C"/>
        <core:isValueOfProperty rdf:resource="http://qudt.org/vocab/quantitykind/Temperature"/>
        <core:isValueOfProperty rdf:resource="https://saref.etsi.org/core/propertyOfInterestTemperatureBathThresholdTank_12"/>
        <data:hasTag>fce_bath_temp_sp</data:hasTag>
        <core:hasTimestamp rdf:datatype="http://www.w3.org/2001/XMLSchema#dateTime">2025-06-03T09:59:08.262183</core:hasTimestamp>
        <core:hasValue rdf:datatype="http://www.w3.org/2001/XMLSchema#float">0.0</core:hasValue>
        <rdfs:comment xml:lang="en">Numerical reading of bath temperature Set Point</rdfs:comment>
    </owl:NamedIndividual>
    


    <!-- https://saref.etsi.org/core/propertyValueTemperatureExhaustFurnace_10 -->

    <owl:NamedIndividual rdf:about="https://saref.etsi.org/core/propertyValueTemperatureExhaustFurnace_10">
        <rdf:type rdf:resource="https://saref.etsi.org/core/PropertyValue"/>
        <core:isMeasuredIn rdf:resource="http://qudt.org/vocab/unit/DEG_C"/>
        <core:isObservedBy rdf:resource="https://ega.industry.com/ontologies/core/asset/sensorTemperatureExhaustFurnace_10"/>
        <core:isTargetOf rdf:resource="https://ega.industry.com/ontologies/core/asset/sensorTemperatureExhaustFurnace_10"/>
        <core:isValueOfProperty rdf:resource="http://qudt.org/vocab/quantitykind/Temperature"/>
        <core:isValueOfProperty rdf:resource="https://saref.etsi.org/core/propertyOfInterestTemperatureExhaustFurnace_10"/>
        <data:hasTag>fce_exhaust_temp_pv</data:hasTag>
        <core:hasTimestamp rdf:datatype="http://www.w3.org/2001/XMLSchema#dateTime">2025-06-03T09:59:07.352815</core:hasTimestamp>
        <core:hasValue rdf:datatype="http://www.w3.org/2001/XMLSchema#float">0.0</core:hasValue>
        <rdfs:comment xml:lang="en">Numerical reading of exhaust gas temperature</rdfs:comment>
    </owl:NamedIndividual>
    


    <!-- https://saref.etsi.org/core/propertyValueTemperatureExhaustFurnace_12 -->

    <owl:NamedIndividual rdf:about="https://saref.etsi.org/core/propertyValueTemperatureExhaustFurnace_12">
        <rdf:type rdf:resource="https://saref.etsi.org/core/PropertyValue"/>
        <core:isMeasuredIn rdf:resource="http://qudt.org/vocab/unit/DEG_C"/>
        <core:isObservedBy rdf:resource="https://ega.industry.com/ontologies/core/asset/sensorTemperatureExhaustFurnace_12"/>
        <core:isTargetOf rdf:resource="https://ega.industry.com/ontologies/core/asset/sensorTemperatureExhaustFurnace_12"/>
        <core:isValueOfProperty rdf:resource="http://qudt.org/vocab/quantitykind/Temperature"/>
        <core:isValueOfProperty rdf:resource="https://saref.etsi.org/core/propertyOfInterestTemperatureExhaustFurnace_12"/>
        <data:hasTag>fce_exhaust_temp_pv</data:hasTag>
        <core:hasTimestamp rdf:datatype="http://www.w3.org/2001/XMLSchema#dateTime">2025-06-03T09:59:08.262183</core:hasTimestamp>
        <core:hasValue rdf:datatype="http://www.w3.org/2001/XMLSchema#float">0.0</core:hasValue>
        <rdfs:comment xml:lang="en">Numerical reading of exhaust gas temperature</rdfs:comment>
    </owl:NamedIndividual>
    


    <!-- https://saref.etsi.org/core/propertyValueTemperatureRoofTank_10 -->

    <owl:NamedIndividual rdf:about="https://saref.etsi.org/core/propertyValueTemperatureRoofTank_10">
        <rdf:type rdf:resource="https://saref.etsi.org/core/PropertyValue"/>
        <core:isMeasuredIn rdf:resource="http://qudt.org/vocab/unit/DEG_C"/>
        <core:isObservedBy rdf:resource="https://ega.industry.com/ontologies/core/asset/sensorTemperatureRoofTank_10"/>
        <core:isTargetOf rdf:resource="https://ega.industry.com/ontologies/core/asset/sensorTemperatureRoofTank_10"/>
        <core:isValueOfProperty rdf:resource="http://qudt.org/vocab/quantitykind/Temperature"/>
        <core:isValueOfProperty rdf:resource="https://saref.etsi.org/core/propertyOfInterestTemperatureRoofTank_10"/>
        <data:hasTag>fce_roof_temp_pv</data:hasTag>
        <core:hasTimestamp rdf:datatype="http://www.w3.org/2001/XMLSchema#dateTime">2025-06-03T09:59:07.352815</core:hasTimestamp>
        <core:hasValue rdf:datatype="http://www.w3.org/2001/XMLSchema#float">0.0</core:hasValue>
        <rdfs:comment xml:lang="en">Numerical reading of roof temperature</rdfs:comment>
    </owl:NamedIndividual>
    


    <!-- https://saref.etsi.org/core/propertyValueTemperatureRoofTank_12 -->

    <owl:NamedIndividual rdf:about="https://saref.etsi.org/core/propertyValueTemperatureRoofTank_12">
        <rdf:type rdf:resource="https://saref.etsi.org/core/PropertyValue"/>
        <core:isMeasuredIn rdf:resource="http://qudt.org/vocab/unit/DEG_C"/>
        <core:isObservedBy rdf:resource="https://ega.industry.com/ontologies/core/asset/sensorTemperatureRoofTank_12"/>
        <core:isTargetOf rdf:resource="https://ega.industry.com/ontologies/core/asset/sensorTemperatureRoofTank_12"/>
        <core:isValueOfProperty rdf:resource="http://qudt.org/vocab/quantitykind/Temperature"/>
        <core:isValueOfProperty rdf:resource="https://saref.etsi.org/core/propertyOfInterestTemperatureRoofTank_12"/>
        <data:hasTag>fce_roof_temp_pv</data:hasTag>
        <core:hasTimestamp rdf:datatype="http://www.w3.org/2001/XMLSchema#dateTime">2025-06-03T09:59:08.262183</core:hasTimestamp>
        <core:hasValue rdf:datatype="http://www.w3.org/2001/XMLSchema#float">0.0</core:hasValue>
        <rdfs:comment xml:lang="en">Numerical reading of roof temperature</rdfs:comment>
    </owl:NamedIndividual>
    


    <!-- https://saref.etsi.org/core/propertyValueTemperatureRoofThresholdTank_10 -->

    <owl:NamedIndividual rdf:about="https://saref.etsi.org/core/propertyValueTemperatureRoofThresholdTank_10">
        <rdf:type rdf:resource="https://saref.etsi.org/core/PropertyValue"/>
        <core:isMeasuredIn rdf:resource="http://qudt.org/vocab/unit/DEG_C"/>
        <core:isValueOfProperty rdf:resource="http://qudt.org/vocab/quantitykind/Temperature"/>
        <core:isValueOfProperty rdf:resource="https://saref.etsi.org/core/propertyOfInterestTemperatureRoofThresholdTank_10"/>
        <data:hasTag>fce_roof_temp_sp</data:hasTag>
        <core:hasTimestamp rdf:datatype="http://www.w3.org/2001/XMLSchema#dateTime">2025-06-03T09:59:07.352815</core:hasTimestamp>
        <core:hasValue rdf:datatype="http://www.w3.org/2001/XMLSchema#float">0.0</core:hasValue>
        <rdfs:comment xml:lang="en">Numerical reading of Roof temperature Set Point</rdfs:comment>
    </owl:NamedIndividual>
    


    <!-- https://saref.etsi.org/core/propertyValueTemperatureRoofThresholdTank_12 -->

    <owl:NamedIndividual rdf:about="https://saref.etsi.org/core/propertyValueTemperatureRoofThresholdTank_12">
        <rdf:type rdf:resource="https://saref.etsi.org/core/PropertyValue"/>
        <core:isMeasuredIn rdf:resource="http://qudt.org/vocab/unit/DEG_C"/>
        <core:isValueOfProperty rdf:resource="http://qudt.org/vocab/quantitykind/Temperature"/>
        <core:isValueOfProperty rdf:resource="https://saref.etsi.org/core/propertyOfInterestTemperatureRoofThresholdTank_12"/>
        <data:hasTag>fce_roof_temp_sp</data:hasTag>
        <core:hasTimestamp rdf:datatype="http://www.w3.org/2001/XMLSchema#dateTime">2025-06-03T09:59:08.262183</core:hasTimestamp>
        <core:hasValue rdf:datatype="http://www.w3.org/2001/XMLSchema#float">0.0</core:hasValue>
        <rdfs:comment xml:lang="en">Numerical reading of Roof temperature Set Point</rdfs:comment>
    </owl:NamedIndividual>
    <rdf:Description>
        <owl:minQualifiedCardinality rdf:datatype="http://www.w3.org/2001/XMLSchema#nonNegativeInteger">1</owl:minQualifiedCardinality>
    </rdf:Description>
    


    <!-- 
    ///////////////////////////////////////////////////////////////////////////////////////
    //
    // Annotations
    //
    ///////////////////////////////////////////////////////////////////////////////////////
     -->

    <rdf:Description rdf:about="https://ega.industry.com/ontologies/core/process/hasPreviousSubProcessOnFailure">
        <rdfs:label>has previous subprocess onfailure</rdfs:label>
    </rdf:Description>
    <rdf:Description rdf:about="https://ega.industry.com/ontologies/core/process/hasPreviousSubProcessOnSuccess">
        <rdfs:label>has previous subprocess onsuccess</rdfs:label>
    </rdf:Description>
    <rdf:Description rdf:about="https://saref.etsi.org/core/hasIdentifier">
        <rdfs:comment xml:lang="en">Links some entity to its identifier. Extensions of SAREF may define sub-properties such as s4abcd:hasUUID, s4abcd:hasGTIN12, etc.</rdfs:comment>
        <rdfs:label xml:lang="en">has identifier</rdfs:label>
        <rdfs:seeAlso rdf:resource="https://labs.etsi.org/rep/saref/saref-portal/-/issues/2"/>
    </rdf:Description>
    


    <!-- 
    ///////////////////////////////////////////////////////////////////////////////////////
    //
    // General axioms
    //
    ///////////////////////////////////////////////////////////////////////////////////////
     -->

    <rdf:Description>
        <rdf:type rdf:resource="http://www.w3.org/2002/07/owl#AllDisjointClasses"/>
        <owl:members rdf:parseType="Collection">
            <rdf:Description rdf:about="https://saref.etsi.org/saref4inma/Area"/>
            <rdf:Description rdf:about="https://saref.etsi.org/saref4inma/Site"/>
            <rdf:Description rdf:about="https://saref.etsi.org/saref4inma/WorkCenter"/>
        </owl:members>
    </rdf:Description>
</rdf:RDF>



<!-- Generated by the OWL API (version 4.5.29.2024-05-13T12:11:03Z) https://github.com/owlcs/owlapi -->

